<?xml version="1.0"?>
<rdf:RDF xmlns="http://purl.org/stc/ontology#"
     xml:base="http://purl.org/stc/ontology"
     xmlns:dc="http://purl.org/dc/elements/1.1/"
     xmlns:owl="http://www.w3.org/2002/07/owl#"
     xmlns:rdf="http://www.w3.org/1999/02/22-rdf-syntax-ns#"
     xmlns:stc="http://purl.org/stc/ontology#"
     xmlns:xml="http://www.w3.org/XML/1998/namespace"
     xmlns:xsd="http://www.w3.org/2001/XMLSchema#"
     xmlns:rdfs="http://www.w3.org/2000/01/rdf-schema#"
     xmlns:skos="http://www.w3.org/2004/02/skos/core#"
     xmlns:vann="http://purl.org/vocab/vann/"
     xmlns:terms="http://purl.org/stc/terms#"
     xmlns:dcterms="http://purl.org/dc/terms/">
    <owl:Ontology rdf:about="http://purl.org/stc/ontology#">
        <owl:versionIRI rdf:resource="http://purl.org/stc/ontology#/1.0.0"/>
        <owl:imports rdf:resource="http://purl.org/nemo/gufo#/1.0.0"/>
        <dc:title xml:lang="en">stc - The Software Testing Concepts Ontology</dc:title>
        <dcterms:bibliographicCitation xml:lang="en">Schieferdecker, I.K.: &quot;stc: The software testing concepts ontology&quot;, 2025, http://purl.org/stc</dcterms:bibliographicCitation>
        <dcterms:license>http://creativecommons.org/licenses/by/4.0/legalcode.en</dcterms:license>
		<dcterms:description xml:lang="en"> The Software Testing Concepts (stc) Ontology provides a formal, structured vocabulary for the domain of software testing. It is based on the ISTQB glossary, the SEVOCAB, and standard
  software testing principles, designed to facilitate interoperability and shared understanding among software testing tools, practitioners, and researchers.</dcterms:description>
        <preferredNamespacePrefix xml:lang="en">stc:</preferredNamespacePrefix>
        <preferredNamespaceURI>http://purl.org/stc/ontology#</preferredNamespaceURI>
        <rdfs:comment xml:lang="en">ISTQB test process mind map.pdf reflected, but 
- collaboration-based approach not contained (as it is too general)
- acceptance test-driven development being a test-first approach represented as a software development model (and not as a test approach)

ISTQB static &amp; dynamic testing mind map.pdf reflected, but 
- with a lot more detailed reflection of test types, test approaches, and test techniques

Top software testing concepts like testing, test activity, etc. put in relation to each other and/or to software engineering conceps

ISTQB test techniques mind map.pdf reflected</rdfs:comment>
        <owl:versionInfo rdf:datatype="http://www.w3.org/2001/XMLSchema#decimal">1</owl:versionInfo>
        <skos:prefLabel xml:lang="en">stc</skos:prefLabel>
    </owl:Ontology>
    


    <!-- 
    ///////////////////////////////////////////////////////////////////////////////////////
    //
    // Annotation properties
    //
    ///////////////////////////////////////////////////////////////////////////////////////
     -->

    


    <!-- http://purl.org/dc/elements/1.1/title -->

    <owl:AnnotationProperty rdf:about="http://purl.org/dc/elements/1.1/title"/>
    


    <!-- http://purl.org/dc/terms/bibliographicCitation -->

    <owl:AnnotationProperty rdf:about="http://purl.org/dc/terms/bibliographicCitation"/>
    


    <!-- http://purl.org/dc/terms/license -->

    <owl:AnnotationProperty rdf:about="http://purl.org/dc/terms/license"/>
    


    <!-- http://purl.org/stc/ontology#isInISTQBGlossary -->

    <owl:AnnotationProperty rdf:about="http://purl.org/stc/ontology#isInISTQBGlossary">
        <rdfs:comment>A flag indicating if this concept is defined by the ISTQB glossary</rdfs:comment>
        <rdfs:label>is in ISTQB glossary</rdfs:label>
        <skos:prefLabel xml:lang="en">is in ISTQB glossary</skos:prefLabel>
        <rdfs:range rdf:resource="http://www.w3.org/2001/XMLSchema#boolean"/>
    </owl:AnnotationProperty>
    


    <!-- http://purl.org/stc/ontology#preferredNamespacePrefix -->

    <owl:AnnotationProperty rdf:about="http://purl.org/stc/ontology#preferredNamespacePrefix"/>
    


    <!-- http://purl.org/stc/ontology#preferredNamespaceURI -->

    <owl:AnnotationProperty rdf:about="http://purl.org/stc/ontology#preferredNamespaceURI"/>
    


    <!-- http://www.w3.org/2004/02/skos/core#altLabel -->

    <owl:AnnotationProperty rdf:about="http://www.w3.org/2004/02/skos/core#altLabel"/>
    


    <!-- http://www.w3.org/2004/02/skos/core#prefLabel -->

    <owl:AnnotationProperty rdf:about="http://www.w3.org/2004/02/skos/core#prefLabel"/>
    


    <!-- 
    ///////////////////////////////////////////////////////////////////////////////////////
    //
    // Object Properties
    //
    ///////////////////////////////////////////////////////////////////////////////////////
     -->

    


    <!-- http://purl.org/stc/ontology#creates -->

    <owl:ObjectProperty rdf:about="http://purl.org/stc/ontology#creates">
        <rdfs:domain rdf:resource="http://purl.org/stc/ontology#software_engineering_activity"/>
        <rdfs:range rdf:resource="http://purl.org/stc/ontology#software"/>
        <rdfs:comment xml:lang="en">Indicates that the subject concept creates instances of the object concept.</rdfs:comment>
        <rdfs:label>creates</rdfs:label>
        <skos:prefLabel xml:lang="en">creates</skos:prefLabel>
    </owl:ObjectProperty>
    


    <!-- http://purl.org/stc/ontology#createsTestCompletionReport -->

    <owl:ObjectProperty rdf:about="http://purl.org/stc/ontology#createsTestCompletionReport">
        <rdfs:subPropertyOf rdf:resource="http://purl.org/stc/ontology#creates"/>
        <rdfs:domain rdf:resource="http://purl.org/stc/ontology#test_completion"/>
        <rdfs:range rdf:resource="http://purl.org/stc/ontology#test_completion_report"/>
        <rdfs:comment xml:lang="en">Indicates that a test completion report is created by the test completion activity.</rdfs:comment>
        <skos:prefLabel xml:lang="en">createsTestCompletionReport</skos:prefLabel>
    </owl:ObjectProperty>
    


    <!-- http://purl.org/stc/ontology#createsTestCondition -->

    <owl:ObjectProperty rdf:about="http://purl.org/stc/ontology#createsTestCondition">
        <rdfs:subPropertyOf rdf:resource="http://purl.org/stc/ontology#creates"/>
        <rdfs:domain rdf:resource="http://purl.org/stc/ontology#test_analysis"/>
        <rdfs:range rdf:resource="http://purl.org/stc/ontology#test_condition"/>
        <rdfs:comment xml:lang="en">Indicates that a test condition is created by the test analysis activity.</rdfs:comment>
        <skos:prefLabel xml:lang="en">createsTestCondition</skos:prefLabel>
    </owl:ObjectProperty>
    


    <!-- http://purl.org/stc/ontology#createsTestPlan -->

    <owl:ObjectProperty rdf:about="http://purl.org/stc/ontology#createsTestPlan">
        <rdfs:subPropertyOf rdf:resource="http://purl.org/stc/ontology#creates"/>
        <rdfs:domain rdf:resource="http://purl.org/stc/ontology#test_planning"/>
        <rdfs:range rdf:resource="http://purl.org/stc/ontology#test_plan"/>
        <rdfs:comment xml:lang="en">Indicates that a test plan is created by the test planning activity.</rdfs:comment>
        <skos:prefLabel xml:lang="en">createsTestPlan</skos:prefLabel>
    </owl:ObjectProperty>
    


    <!-- http://purl.org/stc/ontology#createsTestProgressReport -->

    <owl:ObjectProperty rdf:about="http://purl.org/stc/ontology#createsTestProgressReport">
        <rdfs:subPropertyOf rdf:resource="http://purl.org/stc/ontology#creates"/>
        <rdfs:domain rdf:resource="http://purl.org/stc/ontology#test_monitoring"/>
        <rdfs:range rdf:resource="http://purl.org/stc/ontology#test_progress_report"/>
        <rdfs:comment xml:lang="en">Indicates that a test progress report  is created by the test monitoring activity.</rdfs:comment>
        <skos:prefLabel xml:lang="en">createsTestProgressReport</skos:prefLabel>
    </owl:ObjectProperty>
    


    <!-- http://purl.org/stc/ontology#createsTests -->

    <owl:ObjectProperty rdf:about="http://purl.org/stc/ontology#createsTests">
        <rdfs:subPropertyOf rdf:resource="http://purl.org/stc/ontology#creates"/>
        <rdfs:domain rdf:resource="http://purl.org/stc/ontology#test_design"/>
        <rdfs:range rdf:resource="http://purl.org/stc/ontology#test_case"/>
        <rdfs:range rdf:resource="http://purl.org/stc/ontology#test_data"/>
        <rdfs:comment xml:lang="en">Indicates that a test case and/or test data are created by the test design activity.</rdfs:comment>
        <skos:prefLabel xml:lang="en">createsTests</skos:prefLabel>
    </owl:ObjectProperty>
    


    <!-- http://purl.org/stc/ontology#isPartOf -->

    <owl:ObjectProperty rdf:about="http://purl.org/stc/ontology#isPartOf">
        <rdfs:comment xml:lang="en">Indicates that the subject concept is part of the object concept.</rdfs:comment>
        <rdfs:label>isPartOf</rdfs:label>
        <skos:prefLabel xml:lang="en">is part of</skos:prefLabel>
    </owl:ObjectProperty>
    


    <!-- http://purl.org/stc/ontology#isPartOfTestObject -->

    <owl:ObjectProperty rdf:about="http://purl.org/stc/ontology#isPartOfTestObject">
        <rdfs:subPropertyOf rdf:resource="http://purl.org/stc/ontology#isPartOf"/>
        <rdfs:domain rdf:resource="http://purl.org/stc/ontology#test_item"/>
        <rdfs:range rdf:resource="http://purl.org/stc/ontology#test_object"/>
        <rdfs:comment xml:lang="en">Indicates that test items are part of a test object.</rdfs:comment>
        <skos:prefLabel xml:lang="en">isPartOfTestObject</skos:prefLabel>
    </owl:ObjectProperty>
    


    <!-- http://purl.org/stc/ontology#useInGreyBoxTesting -->

    <owl:ObjectProperty rdf:about="http://purl.org/stc/ontology#useInGreyBoxTesting">
        <rdfs:subPropertyOf rdf:resource="http://purl.org/stc/ontology#uses"/>
        <rdfs:domain rdf:resource="http://purl.org/stc/ontology#grey_box_test_technique"/>
        <rdfs:range rdf:resource="http://purl.org/stc/ontology#black_box_test_technique"/>
        <rdfs:range rdf:resource="http://purl.org/stc/ontology#white_box_test_technique"/>
        <rdfs:comment xml:lang="en">Indicates that a grey-box test technique utilizes principles, knowledge, or aspects from black-box and  white-box test techniques.</rdfs:comment>
        <skos:prefLabel xml:lang="en">useInGreyBoxTesting</skos:prefLabel>
    </owl:ObjectProperty>
    


    <!-- http://purl.org/stc/ontology#useInTestActivity -->

    <owl:ObjectProperty rdf:about="http://purl.org/stc/ontology#useInTestActivity">
        <rdfs:subPropertyOf rdf:resource="http://purl.org/stc/ontology#uses"/>
        <rdfs:domain rdf:resource="http://purl.org/stc/ontology#test_activity"/>
        <rdfs:range rdf:resource="http://purl.org/stc/ontology#Testware"/>
        <rdfs:range rdf:resource="http://purl.org/stc/ontology#software"/>
        <rdfs:label>Indicates that a test activity uses testware and software (of the test object).</rdfs:label>
        <rdfs:label>useInTestActivity</rdfs:label>
        <skos:prefLabel xml:lang="en">useInTestActivity</skos:prefLabel>
    </owl:ObjectProperty>
    


    <!-- http://purl.org/stc/ontology#useInTestAnalysis -->

    <owl:ObjectProperty rdf:about="http://purl.org/stc/ontology#useInTestAnalysis">
        <rdfs:subPropertyOf rdf:resource="http://purl.org/stc/ontology#uses"/>
        <rdfs:domain rdf:resource="http://purl.org/stc/ontology#test_analysis"/>
        <rdfs:range rdf:resource="http://purl.org/stc/ontology#test_basis"/>
        <rdfs:comment xml:lang="en">Indicates that a test analysis utilizes the test basis.</rdfs:comment>
        <skos:prefLabel xml:lang="en">useInTestAnalysis</skos:prefLabel>
    </owl:ObjectProperty>
    


    <!-- http://purl.org/stc/ontology#useInTestCase -->

    <owl:ObjectProperty rdf:about="http://purl.org/stc/ontology#useInTestCase">
        <rdfs:subPropertyOf rdf:resource="http://purl.org/stc/ontology#uses"/>
        <rdfs:domain rdf:resource="http://purl.org/stc/ontology#test_case"/>
        <rdfs:range rdf:resource="http://purl.org/stc/ontology#test_data"/>
        <rdfs:range rdf:resource="http://purl.org/stc/ontology#test_step"/>
        <rdfs:comment xml:lang="en">Indicates that a test case may utilizes test steps and/or test data.</rdfs:comment>
        <skos:prefLabel xml:lang="en">useInTestCase</skos:prefLabel>
    </owl:ObjectProperty>
    


    <!-- http://purl.org/stc/ontology#useInTestCondition -->

    <owl:ObjectProperty rdf:about="http://purl.org/stc/ontology#useInTestCondition">
        <rdfs:subPropertyOf rdf:resource="http://purl.org/stc/ontology#uses"/>
        <rdfs:domain rdf:resource="http://purl.org/stc/ontology#test_condition"/>
        <rdfs:range rdf:resource="http://purl.org/stc/ontology#acceptance_criteria"/>
        <rdfs:range rdf:resource="http://purl.org/stc/ontology#coverage_item"/>
        <rdfs:comment xml:lang="en">Indicates that a test condition utilizes acceptance criteria and coverage items.</rdfs:comment>
        <skos:prefLabel xml:lang="en">useInTestCondition</skos:prefLabel>
    </owl:ObjectProperty>
    


    <!-- http://purl.org/stc/ontology#useInTestDesign -->

    <owl:ObjectProperty rdf:about="http://purl.org/stc/ontology#useInTestDesign">
        <rdfs:subPropertyOf rdf:resource="http://purl.org/stc/ontology#uses"/>
        <rdfs:domain rdf:resource="http://purl.org/stc/ontology#test_design"/>
        <rdfs:range rdf:resource="http://purl.org/stc/ontology#test_condition"/>
        <rdfs:range rdf:resource="http://purl.org/stc/ontology#test_technique"/>
        <rdfs:comment xml:lang="en">Indicates that a test design utilizes test techniques and test conditions.</rdfs:comment>
        <skos:prefLabel xml:lang="en">useInTestDesign</skos:prefLabel>
    </owl:ObjectProperty>
    


    <!-- http://purl.org/stc/ontology#useInTestExecution -->

    <owl:ObjectProperty rdf:about="http://purl.org/stc/ontology#useInTestExecution">
        <rdfs:subPropertyOf rdf:resource="http://purl.org/stc/ontology#uses"/>
        <rdfs:domain rdf:resource="http://purl.org/stc/ontology#test_execution"/>
        <rdfs:range rdf:resource="http://purl.org/stc/ontology#test_object"/>
        <rdfs:range rdf:resource="http://purl.org/stc/ontology#test_suite"/>
        <rdfs:comment xml:lang="en">Indicates that a test execution utilizes test objects and test suites.</rdfs:comment>
        <skos:prefLabel xml:lang="en">useInTestExecution</skos:prefLabel>
    </owl:ObjectProperty>
    


    <!-- http://purl.org/stc/ontology#useInTestPlan -->

    <owl:ObjectProperty rdf:about="http://purl.org/stc/ontology#useInTestPlan">
        <rdfs:subPropertyOf rdf:resource="http://purl.org/stc/ontology#uses"/>
        <rdfs:domain rdf:resource="http://purl.org/stc/ontology#test_plan"/>
        <rdfs:range rdf:resource="http://purl.org/stc/ontology#entry_criteria"/>
        <rdfs:range rdf:resource="http://purl.org/stc/ontology#exit_criteria"/>
        <rdfs:range rdf:resource="http://purl.org/stc/ontology#test_approach"/>
        <rdfs:range rdf:resource="http://purl.org/stc/ontology#test_objective"/>
        <rdfs:comment xml:lang="en">Indicates that a test plan utilizes test approaches, test objectives, and entry and exit criteria.</rdfs:comment>
        <skos:prefLabel xml:lang="en">useInTestPlan</skos:prefLabel>
    </owl:ObjectProperty>
    


    <!-- http://purl.org/stc/ontology#useInTestProcess -->

    <owl:ObjectProperty rdf:about="http://purl.org/stc/ontology#useInTestProcess">
        <rdfs:subPropertyOf rdf:resource="http://purl.org/stc/ontology#uses"/>
        <rdfs:domain rdf:resource="http://purl.org/stc/ontology#test_process"/>
        <rdfs:range rdf:resource="http://purl.org/stc/ontology#Testware"/>
        <rdfs:range rdf:resource="http://purl.org/stc/ontology#test_activity"/>
        <rdfs:range rdf:resource="http://purl.org/stc/ontology#test_approach"/>
        <rdfs:range rdf:resource="http://purl.org/stc/ontology#test_level"/>
        <rdfs:range rdf:resource="http://purl.org/stc/ontology#test_metric"/>
        <rdfs:range rdf:resource="http://purl.org/stc/ontology#test_type"/>
        <rdfs:comment xml:lang="en">Indicates that a test process utilizes test activities, testware, test metrics, test levels, test approaches and test types.</rdfs:comment>
        <skos:prefLabel xml:lang="en">useInTestProcess</skos:prefLabel>
    </owl:ObjectProperty>
    


    <!-- http://purl.org/stc/ontology#useInTestQuadrants -->

    <owl:ObjectProperty rdf:about="http://purl.org/stc/ontology#useInTestQuadrants">
        <rdfs:subPropertyOf rdf:resource="http://purl.org/stc/ontology#uses"/>
        <rdfs:domain rdf:resource="http://purl.org/stc/ontology#testing_quadrants"/>
        <rdfs:range rdf:resource="http://purl.org/stc/ontology#test_approach"/>
        <rdfs:range rdf:resource="http://purl.org/stc/ontology#test_level"/>
        <rdfs:range rdf:resource="http://purl.org/stc/ontology#test_type"/>
        <rdfs:comment xml:lang="en">Indicates that a test quadrant utilizes test levels and test types/test approaches.</rdfs:comment>
        <skos:prefLabel xml:lang="en">useInTestQuadrants</skos:prefLabel>
    </owl:ObjectProperty>
    


    <!-- http://purl.org/stc/ontology#useInTesting -->

    <owl:ObjectProperty rdf:about="http://purl.org/stc/ontology#useInTesting">
        <rdfs:subPropertyOf rdf:resource="http://purl.org/stc/ontology#uses"/>
        <rdfs:domain rdf:resource="http://purl.org/stc/ontology#testing"/>
        <rdfs:range rdf:resource="http://purl.org/stc/ontology#test_management"/>
        <rdfs:range rdf:resource="http://purl.org/stc/ontology#test_process"/>
        <rdfs:range rdf:resource="http://purl.org/stc/ontology#test_work_force"/>
        <rdfs:comment xml:lang="en">Indicates that testing is done by a test work force along a test process that is to be managed.</rdfs:comment>
        <rdfs:label>useInTesting</rdfs:label>
        <skos:prefLabel xml:lang="en">useInTesting</skos:prefLabel>
    </owl:ObjectProperty>
    


    <!-- http://purl.org/stc/ontology#uses -->

    <owl:ObjectProperty rdf:about="http://purl.org/stc/ontology#uses">
        <rdfs:comment xml:lang="en">Indicates that the subject concept utilizes principles, knowledge, or aspects commonly associated with the object concept.</rdfs:comment>
        <rdfs:label>uses</rdfs:label>
        <skos:prefLabel xml:lang="en">uses</skos:prefLabel>
    </owl:ObjectProperty>
    


    <!-- http://purl.org/stc/terms#hasParent -->

    <owl:ObjectProperty rdf:about="http://purl.org/stc/terms#hasParent"/>
    


    <!-- 
    ///////////////////////////////////////////////////////////////////////////////////////
    //
    // Classes
    //
    ///////////////////////////////////////////////////////////////////////////////////////
     -->

    


    <!-- http://purl.org/stc/ontology#AI_testing -->

    <owl:Class rdf:about="http://purl.org/stc/ontology#AI_testing">
        <rdfs:subClassOf rdf:resource="http://purl.org/stc/ontology#domain-specific_test_types"/>
        <isInISTQBGlossary rdf:datatype="http://www.w3.org/2001/XMLSchema#boolean">true</isInISTQBGlossary>
        <rdfs:label>AI testing</rdfs:label>
        <skos:prefLabel xml:lang="en">ai testing</skos:prefLabel>
    </owl:Class>
    


    <!-- http://purl.org/stc/ontology#API_testing -->

    <owl:Class rdf:about="http://purl.org/stc/ontology#API_testing">
        <rdfs:subClassOf rdf:resource="http://purl.org/stc/ontology#interface_testing"/>
        <isInISTQBGlossary rdf:datatype="http://www.w3.org/2001/XMLSchema#boolean">true</isInISTQBGlossary>
        <rdfs:label>API testing</rdfs:label>
        <skos:prefLabel xml:lang="en">api testing</skos:prefLabel>
    </owl:Class>
    


    <!-- http://purl.org/stc/ontology#GUI_testing -->

    <owl:Class rdf:about="http://purl.org/stc/ontology#GUI_testing">
        <rdfs:subClassOf rdf:resource="http://purl.org/stc/ontology#interface_testing"/>
        <isInISTQBGlossary rdf:datatype="http://www.w3.org/2001/XMLSchema#boolean">true</isInISTQBGlossary>
        <rdfs:label>GUI testing</rdfs:label>
        <skos:altLabel xml:lang="en">graphical user interface testing</skos:altLabel>
        <skos:prefLabel xml:lang="en">GUI testing</skos:prefLabel>
    </owl:Class>
    


    <!-- http://purl.org/stc/ontology#LLM_structural_coverage -->

    <owl:Class rdf:about="http://purl.org/stc/ontology#LLM_structural_coverage">
        <rdfs:subClassOf rdf:resource="http://purl.org/stc/ontology#structural_coverage"/>
        <isInISTQBGlossary rdf:datatype="http://www.w3.org/2001/XMLSchema#boolean">false</isInISTQBGlossary>
        <rdfs:comment xml:lang="en">Coverage measures based on the internal structure of an LLM. (own))</rdfs:comment>
        <rdfs:label>LLM structural coverage</rdfs:label>
        <skos:prefLabel xml:lang="en">llm structural coverage</skos:prefLabel>
    </owl:Class>
    


    <!-- http://purl.org/stc/ontology#MBT_modeller -->

    <owl:Class rdf:about="http://purl.org/stc/ontology#MBT_modeller">
        <rdfs:subClassOf rdf:resource="http://purl.org/stc/ontology#related_to_role"/>
        <isInISTQBGlossary rdf:datatype="http://www.w3.org/2001/XMLSchema#boolean">false</isInISTQBGlossary>
        <rdfs:comment xml:lang="en">Develops formal test specifications in the form of models used to generate test cases as part of model-based testing. (ISO/IEC/IEEE 29119-1:2022)</rdfs:comment>
        <rdfs:label>MBT modeller</rdfs:label>
        <rdfs:seeAlso>ISO/IEC/IEEE 29119-1:2022 (Software and systems engineering — Software testing — Part 1: Concepts and definitions)</rdfs:seeAlso>
        <skos:prefLabel xml:lang="en">MBT modeller</skos:prefLabel>
    </owl:Class>
    


    <!-- http://purl.org/stc/ontology#N-switch_coverage -->

    <owl:Class rdf:about="http://purl.org/stc/ontology#N-switch_coverage">
        <rdfs:subClassOf rdf:resource="http://purl.org/stc/ontology#structural_coverage"/>
        <isInISTQBGlossary rdf:datatype="http://www.w3.org/2001/XMLSchema#boolean">true</isInISTQBGlossary>
        <rdfs:comment xml:lang="en">The coverage of sequences of N+1 transitions. (ISTQB Glossary v4.5)</rdfs:comment>
        <rdfs:label>N-switch coverage</rdfs:label>
        <rdfs:seeAlso></rdfs:seeAlso>
        <skos:altLabel xml:lang="en">chow&apos;s coverage metric</skos:altLabel>
        <skos:prefLabel xml:lang="en">n-switch coverage
N-switch coverage</skos:prefLabel>
    </owl:Class>
    


    <!-- http://purl.org/stc/ontology#Testware -->

    <owl:Class rdf:about="http://purl.org/stc/ontology#Testware">
        <rdfs:subClassOf rdf:resource="http://purl.org/stc/ontology#software_testing_concepts"/>
        <isInISTQBGlossary rdf:datatype="http://www.w3.org/2001/XMLSchema#boolean">true</isInISTQBGlossary>
        <rdfs:comment xml:lang="en">Work products produced during the test process for use in planning, designing, executing, evaluating and reporting on testing. (ISTQB Glossary v4.5)

Artefacts produced during the test process required to plan, design, and execute tests. (ISO/IEC/IEEE 29119-1:2022)</rdfs:comment>
        <rdfs:label>testware</rdfs:label>
        <rdfs:seeAlso>ISO/IEC/IEEE 29119-1 (2022) Software and systems engineering -- Software testing -- Part 1: Concepts and definitions

Foundation - v4.0
Advanced Test Manager - 2012
Advanced Test Management - v3.0
Advanced Test Analyst - v3.1
Advanced Test Analyst - v4.0
Advanced Test Automation Engineering - v2.0
Specialist - Automotive Software Tester - v1.1
Specialist - Game Testing - v1.0.1
Specialist - Model-Based Testing - v1.1
Specialist - Performance Testing - 2018
Specialist - Test Automation Engineer - 2016
Specialist - Test Automation Strategy - v1.0</rdfs:seeAlso>
        <skos:altLabel>test artefact
test artifact</skos:altLabel>
        <skos:prefLabel xml:lang="en">testware</skos:prefLabel>
    </owl:Class>
    


    <!-- http://purl.org/stc/ontology#a_b_testing -->

    <owl:Class rdf:about="http://purl.org/stc/ontology#a_b_testing">
        <rdfs:subClassOf rdf:resource="http://purl.org/stc/ontology#oracle_orientation_in_test_approach"/>
        <isInISTQBGlossary rdf:datatype="http://www.w3.org/2001/XMLSchema#boolean">true</isInISTQBGlossary>
        <rdfs:comment xml:lang="en">A test approach in which two components or systems are statistically evaluated to determine which performs better for specified criteria. (ISTQB Glossary v4.5) 

Statistical testing approach that allows testers to determine which of two systems or components performs better. (ISO/IEC/IEEE 29119-1:2022)</rdfs:comment>
        <rdfs:label>a/b testing</rdfs:label>
        <skos:prefLabel xml:lang="en">a/b testing</skos:prefLabel>
    </owl:Class>
    


    <!-- http://purl.org/stc/ontology#acceptance -->

    <owl:Class rdf:about="http://purl.org/stc/ontology#acceptance">
        <rdfs:subClassOf rdf:resource="http://purl.org/stc/ontology#software_engineering_activity"/>
    </owl:Class>
    


    <!-- http://purl.org/stc/ontology#acceptance_criteria -->

    <owl:Class rdf:about="http://purl.org/stc/ontology#acceptance_criteria">
        <rdfs:subClassOf rdf:resource="http://purl.org/stc/ontology#Testware"/>
        <isInISTQBGlossary rdf:datatype="http://www.w3.org/2001/XMLSchema#boolean">true</isInISTQBGlossary>
        <rdfs:comment xml:lang="en">The criteria that a work product must satisfy to be accepted by the stakeholders. (ISTQB Glossary v4.5, after IREB Glossary)

Criteria that a system or system component must satisfy to be accepted by a user, customer, or other authorized entity.(ISO/IEC/IEEE 29148:2018)</rdfs:comment>
        <rdfs:label>acceptance criteria</rdfs:label>
        <rdfs:seeAlso>ISO/IEC/IEEE 29148:2018 (Systems and software engineering — Life cycle processes — Requirements engineering)</rdfs:seeAlso>
        <skos:prefLabel xml:lang="en">acceptance criteria</skos:prefLabel>
    </owl:Class>
    


    <!-- http://purl.org/stc/ontology#acceptance_test-driven_development -->

    <owl:Class rdf:about="http://purl.org/stc/ontology#acceptance_test-driven_development">
        <rdfs:subClassOf rdf:resource="http://purl.org/stc/ontology#test_first_approach"/>
        <isInISTQBGlossary rdf:datatype="http://www.w3.org/2001/XMLSchema#boolean">true</isInISTQBGlossary>
        <rdfs:label>acceptance test-driven development</rdfs:label>
        <skos:prefLabel xml:lang="en">acceptance test-driven development</skos:prefLabel>
    </owl:Class>
    


    <!-- http://purl.org/stc/ontology#acceptance_testing -->

    <owl:Class rdf:about="http://purl.org/stc/ontology#acceptance_testing">
        <rdfs:subClassOf rdf:resource="http://purl.org/stc/ontology#test_level"/>
        <owl:disjointWith rdf:resource="http://purl.org/stc/ontology#component_testing"/>
        <owl:disjointWith rdf:resource="http://purl.org/stc/ontology#integration_testing"/>
        <owl:disjointWith rdf:resource="http://purl.org/stc/ontology#system_testing"/>
        <isInISTQBGlossary rdf:datatype="http://www.w3.org/2001/XMLSchema#boolean">true</isInISTQBGlossary>
        <rdfs:label>acceptance testing</rdfs:label>
        <skos:prefLabel xml:lang="en">acceptance testing</skos:prefLabel>
    </owl:Class>
    


    <!-- http://purl.org/stc/ontology#accessibility_testing -->

    <owl:Class rdf:about="http://purl.org/stc/ontology#accessibility_testing">
        <rdfs:subClassOf rdf:resource="http://purl.org/stc/ontology#system_testing"/>
        <isInISTQBGlossary rdf:datatype="http://www.w3.org/2001/XMLSchema#boolean">false</isInISTQBGlossary>
        <rdfs:label>accessibility testing</rdfs:label>
        <skos:prefLabel xml:lang="en">accessibility testing</skos:prefLabel>
    </owl:Class>
    


    <!-- http://purl.org/stc/ontology#ad_hoc_testing -->

    <owl:Class rdf:about="http://purl.org/stc/ontology#ad_hoc_testing">
        <rdfs:subClassOf rdf:resource="http://purl.org/stc/ontology#method_orientation_in_test_approach"/>
        <isInISTQBGlossary rdf:datatype="http://www.w3.org/2001/XMLSchema#boolean">true</isInISTQBGlossary>
        <rdfs:comment xml:lang="en">Informal testing performed without test analysis and test design.</rdfs:comment>
        <rdfs:label>ad hoc testing</rdfs:label>
        <rdfs:seeAlso>Specialist - Game Testing - v1.0.1</rdfs:seeAlso>
        <skos:altLabel xml:lang="en">adhoc testing
ad hoc-testing</skos:altLabel>
        <skos:prefLabel xml:lang="en">ad hoc testing</skos:prefLabel>
    </owl:Class>
    


    <!-- http://purl.org/stc/ontology#adversarial_testing -->

    <owl:Class rdf:about="http://purl.org/stc/ontology#adversarial_testing">
        <rdfs:subClassOf rdf:resource="http://purl.org/stc/ontology#AI_testing"/>
        <isInISTQBGlossary rdf:datatype="http://www.w3.org/2001/XMLSchema#boolean">true</isInISTQBGlossary>
        <rdfs:label>adversarial testing</rdfs:label>
        <skos:prefLabel xml:lang="en">adversarial testing</skos:prefLabel>
    </owl:Class>
    


    <!-- http://purl.org/stc/ontology#agile_software_development -->

    <owl:Class rdf:about="http://purl.org/stc/ontology#agile_software_development">
        <rdfs:subClassOf rdf:resource="http://purl.org/stc/ontology#process_orientation_in_software_development"/>
        <isInISTQBGlossary rdf:datatype="http://www.w3.org/2001/XMLSchema#boolean">true</isInISTQBGlossary>
        <rdfs:label>agile</rdfs:label>
        <skos:prefLabel xml:lang="en">agile software development</skos:prefLabel>
    </owl:Class>
    


    <!-- http://purl.org/stc/ontology#agile_test_leader -->

    <owl:Class rdf:about="http://purl.org/stc/ontology#agile_test_leader">
        <rdfs:subClassOf rdf:resource="http://purl.org/stc/ontology#test_leader"/>
        <isInISTQBGlossary rdf:datatype="http://www.w3.org/2001/XMLSchema#boolean">true</isInISTQBGlossary>
        <rdfs:comment xml:lang="en">A leadership role that serves agile teams, championing testing and quality at the organizational level. (ISTQB Glossary v4.5)</rdfs:comment>
        <rdfs:label>agile test leader</rdfs:label>
        <rdfs:seeAlso>Agile Test Leadership at Scale - v1.0
Specialist - Agile Test Leadership at Scale - v2.0</rdfs:seeAlso>
        <skos:altLabel xml:lang="en">quality coach
agile test manager
quality leader</skos:altLabel>
        <skos:prefLabel xml:lang="en">agile test leader</skos:prefLabel>
    </owl:Class>
    


    <!-- http://purl.org/stc/ontology#agile_test_team_leader -->

    <owl:Class rdf:about="http://purl.org/stc/ontology#agile_test_team_leader">
        <rdfs:subClassOf rdf:resource="http://purl.org/stc/ontology#test_manager"/>
        <isInISTQBGlossary rdf:datatype="http://www.w3.org/2001/XMLSchema#boolean">true</isInISTQBGlossary>
        <rdfs:comment xml:lang="en">A role that is responsible for maintaining solution quality within an agile delivery team. (ISTQB Glossary v4.5)</rdfs:comment>
        <rdfs:label>agile test team leader</rdfs:label>
        <rdfs:seeAlso>Agile Test Leadership at Scale - v1.0
Specialist - Agile Test Leadership at Scale - v2.0</rdfs:seeAlso>
        <skos:prefLabel xml:lang="en">agile test team leader</skos:prefLabel>
    </owl:Class>
    


    <!-- http://purl.org/stc/ontology#alpha_testing -->

    <owl:Class rdf:about="http://purl.org/stc/ontology#alpha_testing">
        <rdfs:subClassOf rdf:resource="http://purl.org/stc/ontology#acceptance_testing"/>
        <isInISTQBGlossary rdf:datatype="http://www.w3.org/2001/XMLSchema#boolean">true</isInISTQBGlossary>
        <rdfs:label>alpha testing</rdfs:label>
        <skos:prefLabel xml:lang="en">alpha testing</skos:prefLabel>
    </owl:Class>
    


    <!-- http://purl.org/stc/ontology#architectural_design -->

    <owl:Class rdf:about="http://purl.org/stc/ontology#architectural_design">
        <rdfs:subClassOf rdf:resource="http://purl.org/stc/ontology#software_engineering_activity"/>
    </owl:Class>
    


    <!-- http://purl.org/stc/ontology#automated_testing -->

    <owl:Class rdf:about="http://purl.org/stc/ontology#automated_testing">
        <rdfs:subClassOf rdf:resource="http://purl.org/stc/ontology#test_execution"/>
        <isInISTQBGlossary rdf:datatype="http://www.w3.org/2001/XMLSchema#boolean">false</isInISTQBGlossary>
        <rdfs:label>automated testing</rdfs:label>
        <skos:prefLabel xml:lang="en">automated testing</skos:prefLabel>
    </owl:Class>
    


    <!-- http://purl.org/stc/ontology#back-to-back_testing -->

    <owl:Class rdf:about="http://purl.org/stc/ontology#back-to-back_testing">
        <rdfs:subClassOf rdf:resource="http://purl.org/stc/ontology#oracle_orientation_in_test_approach"/>
        <isInISTQBGlossary rdf:datatype="http://www.w3.org/2001/XMLSchema#boolean">true</isInISTQBGlossary>
        <rdfs:label>back-to-back testing</rdfs:label>
        <skos:altLabel xml:lang="en">back to back testing</skos:altLabel>
        <skos:prefLabel xml:lang="en">back-to-back testing</skos:prefLabel>
    </owl:Class>
    


    <!-- http://purl.org/stc/ontology#base_choice_coverage -->

    <owl:Class rdf:about="http://purl.org/stc/ontology#base_choice_coverage">
        <rdfs:subClassOf rdf:resource="http://purl.org/stc/ontology#specification_coverage"/>
        <isInISTQBGlossary rdf:datatype="http://www.w3.org/2001/XMLSchema#boolean">true</isInISTQBGlossary>
        <rdfs:comment xml:lang="en">The coverage of parameter-value combinations in which each value of a parameter is combined with the base values of all other parameters, for a chosen base value per parameter. (ISTQB Glossary v4.5)

Coverage for base choice testing. (ISO/IEC/IEEE 29119-4)</rdfs:comment>
        <rdfs:label>base choice coverage</rdfs:label>
        <rdfs:seeAlso>ISO/IEC/IEEE 29119-4 (Software and systems engineering — Software testing — Part 4: Test techniques)</rdfs:seeAlso>
        <skos:altLabel xml:lang="en">p-v pair coverage</skos:altLabel>
        <skos:prefLabel xml:lang="en">base choice coverage</skos:prefLabel>
    </owl:Class>
    


    <!-- http://purl.org/stc/ontology#basic_concepts -->

    <owl:Class rdf:about="http://purl.org/stc/ontology#basic_concepts">
        <rdfs:subClassOf rdf:resource="http://purl.org/stc/ontology#software_engineering_concepts"/>
        <isInISTQBGlossary rdf:datatype="http://www.w3.org/2001/XMLSchema#boolean">false</isInISTQBGlossary>
        <rdfs:label>basic concepts</rdfs:label>
        <skos:prefLabel xml:lang="en">basic concepts</skos:prefLabel>
    </owl:Class>
    


    <!-- http://purl.org/stc/ontology#behavior-driven_development -->

    <owl:Class rdf:about="http://purl.org/stc/ontology#behavior-driven_development">
        <rdfs:subClassOf rdf:resource="http://purl.org/stc/ontology#target_orientation_in_software_development"/>
        <isInISTQBGlossary rdf:datatype="http://www.w3.org/2001/XMLSchema#boolean">true</isInISTQBGlossary>
        <rdfs:label>behavior-driven</rdfs:label>
        <skos:altLabel xml:lang="en">behavior driven development
bdd
BDD</skos:altLabel>
        <skos:prefLabel xml:lang="en">behavior-driven development</skos:prefLabel>
    </owl:Class>
    


    <!-- http://purl.org/stc/ontology#beta_testing -->

    <owl:Class rdf:about="http://purl.org/stc/ontology#beta_testing">
        <rdfs:subClassOf rdf:resource="http://purl.org/stc/ontology#acceptance_testing"/>
        <isInISTQBGlossary rdf:datatype="http://www.w3.org/2001/XMLSchema#boolean">true</isInISTQBGlossary>
        <rdfs:label>beta testing</rdfs:label>
        <skos:prefLabel xml:lang="en">beta testing</skos:prefLabel>
    </owl:Class>
    


    <!-- http://purl.org/stc/ontology#black_box_test_technique -->

    <owl:Class rdf:about="http://purl.org/stc/ontology#black_box_test_technique">
        <rdfs:subClassOf rdf:resource="http://purl.org/stc/ontology#test_technique"/>
        <owl:disjointWith rdf:resource="http://purl.org/stc/ontology#experience-based_testing"/>
        <owl:disjointWith rdf:resource="http://purl.org/stc/ontology#grey_box_test_technique"/>
        <owl:disjointWith rdf:resource="http://purl.org/stc/ontology#white_box_test_technique"/>
        <isInISTQBGlossary rdf:datatype="http://www.w3.org/2001/XMLSchema#boolean">true</isInISTQBGlossary>
        <rdfs:comment xml:lang="en">(ISTQB Glossary v4.5)</rdfs:comment>
        <rdfs:label>black box test technique</rdfs:label>
        <skos:altLabel xml:lang="en">specification-based testing
specification based testing
closed box testing
black-box test technique</skos:altLabel>
        <skos:prefLabel xml:lang="en">black box test technique</skos:prefLabel>
    </owl:Class>
    


    <!-- http://purl.org/stc/ontology#boundary_value_analysis -->

    <owl:Class rdf:about="http://purl.org/stc/ontology#boundary_value_analysis">
        <rdfs:subClassOf rdf:resource="http://purl.org/stc/ontology#black_box_test_technique"/>
        <isInISTQBGlossary rdf:datatype="http://www.w3.org/2001/XMLSchema#boolean">true</isInISTQBGlossary>
        <rdfs:label>boundary value analysis</rdfs:label>
        <skos:prefLabel xml:lang="en">boundary value analysis</skos:prefLabel>
    </owl:Class>
    


    <!-- http://purl.org/stc/ontology#branch_coverage -->

    <owl:Class rdf:about="http://purl.org/stc/ontology#branch_coverage">
        <rdfs:subClassOf rdf:resource="http://purl.org/stc/ontology#structural_coverage"/>
        <isInISTQBGlossary rdf:datatype="http://www.w3.org/2001/XMLSchema#boolean">true</isInISTQBGlossary>
        <rdfs:comment xml:lang="en">The coverage of branches in a control flow graph.  (ISTQB Glossary v4.5)</rdfs:comment>
        <rdfs:label>branch coverage</rdfs:label>
        <rdfs:seeAlso>Foundation - v4.0</rdfs:seeAlso>
        <skos:prefLabel xml:lang="en">branch coverage</skos:prefLabel>
    </owl:Class>
    


    <!-- http://purl.org/stc/ontology#branch_testing -->

    <owl:Class rdf:about="http://purl.org/stc/ontology#branch_testing">
        <rdfs:subClassOf rdf:resource="http://purl.org/stc/ontology#white_box_test_technique"/>
        <isInISTQBGlossary rdf:datatype="http://www.w3.org/2001/XMLSchema#boolean">true</isInISTQBGlossary>
        <rdfs:label>branch testing</rdfs:label>
        <skos:prefLabel xml:lang="en">branch testing</skos:prefLabel>
    </owl:Class>
    


    <!-- http://purl.org/stc/ontology#change_orientation_in_test_approach -->

    <owl:Class rdf:about="http://purl.org/stc/ontology#change_orientation_in_test_approach">
        <rdfs:subClassOf rdf:resource="http://purl.org/stc/ontology#test_approach"/>
        <isInISTQBGlossary rdf:datatype="http://www.w3.org/2001/XMLSchema#boolean">false</isInISTQBGlossary>
        <rdfs:label>change orientation</rdfs:label>
        <skos:prefLabel xml:lang="en">change orientation in test approach</skos:prefLabel>
    </owl:Class>
    


    <!-- http://purl.org/stc/ontology#checklist_based_testing -->

    <owl:Class rdf:about="http://purl.org/stc/ontology#checklist_based_testing">
        <rdfs:subClassOf rdf:resource="http://purl.org/stc/ontology#experience-based_testing"/>
        <isInISTQBGlossary rdf:datatype="http://www.w3.org/2001/XMLSchema#boolean">true</isInISTQBGlossary>
        <rdfs:label>checklist based testing</rdfs:label>
        <skos:prefLabel xml:lang="en">checklist based testing</skos:prefLabel>
    </owl:Class>
    


    <!-- http://purl.org/stc/ontology#code -->

    <owl:Class rdf:about="http://purl.org/stc/ontology#code">
        <rdfs:subClassOf rdf:resource="http://purl.org/stc/ontology#basic_concepts"/>
    </owl:Class>
    


    <!-- http://purl.org/stc/ontology#coding -->

    <owl:Class rdf:about="http://purl.org/stc/ontology#coding">
        <rdfs:subClassOf rdf:resource="http://purl.org/stc/ontology#software_engineering_activity"/>
    </owl:Class>
    


    <!-- http://purl.org/stc/ontology#compliance_testing -->

    <owl:Class rdf:about="http://purl.org/stc/ontology#compliance_testing">
        <rdfs:subClassOf rdf:resource="http://purl.org/stc/ontology#functional_testing"/>
        <isInISTQBGlossary rdf:datatype="http://www.w3.org/2001/XMLSchema#boolean">true</isInISTQBGlossary>
        <rdfs:comment xml:lang="en">The term conformance testing (defined by ISTQB to be a synonym for compliance testing) is used differently in telecommunication/protocol testing - see also protocol testing.</rdfs:comment>
        <rdfs:label>compliance testing</rdfs:label>
        <rdfs:seeAlso>Specialist - Gambling Industry Tester - 2018</rdfs:seeAlso>
        <skos:altLabel>conformance testing
regulation testing
standards testing</skos:altLabel>
        <skos:prefLabel xml:lang="en">compliance testing</skos:prefLabel>
    </owl:Class>
    


    <!-- http://purl.org/stc/ontology#component_integration_testing -->

    <owl:Class rdf:about="http://purl.org/stc/ontology#component_integration_testing">
        <rdfs:subClassOf rdf:resource="http://purl.org/stc/ontology#integration_testing"/>
        <isInISTQBGlossary rdf:datatype="http://www.w3.org/2001/XMLSchema#boolean">true</isInISTQBGlossary>
        <rdfs:comment xml:lang="en">The integration testing of components. (ISTQB Glossary v4.5)</rdfs:comment>
        <rdfs:label>component integration testing</rdfs:label>
        <rdfs:seeAlso>Foundation - v4.0</rdfs:seeAlso>
        <skos:altLabel xml:lang="en">module integration testing
unit integration testing</skos:altLabel>
        <skos:prefLabel xml:lang="en">component integration testing</skos:prefLabel>
    </owl:Class>
    


    <!-- http://purl.org/stc/ontology#component_testing -->

    <owl:Class rdf:about="http://purl.org/stc/ontology#component_testing">
        <rdfs:subClassOf rdf:resource="http://purl.org/stc/ontology#test_level"/>
        <owl:disjointWith rdf:resource="http://purl.org/stc/ontology#integration_testing"/>
        <owl:disjointWith rdf:resource="http://purl.org/stc/ontology#system_testing"/>
        <isInISTQBGlossary rdf:datatype="http://www.w3.org/2001/XMLSchema#boolean">true</isInISTQBGlossary>
        <rdfs:label>component testing</rdfs:label>
        <skos:prefLabel xml:lang="en">component testing</skos:prefLabel>
    </owl:Class>
    


    <!-- http://purl.org/stc/ontology#condition_coverage -->

    <owl:Class rdf:about="http://purl.org/stc/ontology#condition_coverage">
        <rdfs:subClassOf rdf:resource="http://purl.org/stc/ontology#structural_coverage"/>
        <isInISTQBGlossary rdf:datatype="http://www.w3.org/2001/XMLSchema#boolean">true</isInISTQBGlossary>
        <rdfs:comment xml:lang="en">The coverage of condition outcomes. (ISTQB Glossary v4.5)

Coverage for branch condition testing. (ISO/IEC/IEEE 29119-4)</rdfs:comment>
        <rdfs:label>condition coverage</rdfs:label>
        <rdfs:seeAlso>ISO/IEC/IEEE 29119-4 (Software and systems engineering — Software testing — Part 4: Test techniques)</rdfs:seeAlso>
        <skos:altLabel xml:lang="en">branch condition coverage</skos:altLabel>
        <skos:prefLabel xml:lang="en">condition coverage</skos:prefLabel>
    </owl:Class>
    


    <!-- http://purl.org/stc/ontology#configuration_management -->

    <owl:Class rdf:about="http://purl.org/stc/ontology#configuration_management">
        <rdfs:subClassOf rdf:resource="http://purl.org/stc/ontology#support_processes"/>
    </owl:Class>
    


    <!-- http://purl.org/stc/ontology#confirmation_testing -->

    <owl:Class rdf:about="http://purl.org/stc/ontology#confirmation_testing">
        <rdfs:subClassOf rdf:resource="http://purl.org/stc/ontology#defect_orientation_in_test_approach"/>
        <isInISTQBGlossary rdf:datatype="http://www.w3.org/2001/XMLSchema#boolean">true</isInISTQBGlossary>
        <rdfs:comment xml:lang="en">A type of change-related testing performed after fixing a defect to confirm that a failure caused by that defect does not reoccur. (ISTQB Glossary v4.5)

Testing performed to check that modifications made to correct a fault have successfully removed the fault. (ISO/IEC/IEEE 29119-1:2022)</rdfs:comment>
        <rdfs:label>confirmation testing</rdfs:label>
        <rdfs:seeAlso>ISO/IEC/IEEE 29119-1:2022 (Software and systems engineering — Software testing — Part 1: Concepts and definitions)

Foundation - v4.0
Specialist - Test Automation Engineer - 2016
Specialist - Test Automation Strategy - v1.0</rdfs:seeAlso>
        <skos:altLabel xml:lang="en">retesting</skos:altLabel>
        <skos:prefLabel xml:lang="en">confirmation testing</skos:prefLabel>
    </owl:Class>
    


    <!-- http://purl.org/stc/ontology#conformance_testing -->

    <owl:Class rdf:about="http://purl.org/stc/ontology#conformance_testing">
        <rdfs:subClassOf rdf:resource="http://purl.org/stc/ontology#protocol_or_service_testing"/>
        <isInISTQBGlossary rdf:datatype="http://www.w3.org/2001/XMLSchema#boolean">false</isInISTQBGlossary>
        <rdfs:comment xml:lang="en">The process of verifying that a system or component meets the requirements of a specified standard. (ISO/IEC 9646-1:1994)</rdfs:comment>
        <rdfs:label>conformance testing</rdfs:label>
        <rdfs:seeAlso>ISO/IEC 9646-1:1994 (Information technology — Open Systems Interconnection — Conformance testing methodology and framework. Part 1: General concepts)</rdfs:seeAlso>
        <skos:prefLabel xml:lang="en">conformance testing</skos:prefLabel>
    </owl:Class>
    


    <!-- http://purl.org/stc/ontology#continuous_testing -->

    <owl:Class rdf:about="http://purl.org/stc/ontology#continuous_testing">
        <rdfs:subClassOf rdf:resource="http://purl.org/stc/ontology#process_orientation_in_test_approach"/>
        <isInISTQBGlossary rdf:datatype="http://www.w3.org/2001/XMLSchema#boolean">true</isInISTQBGlossary>
        <rdfs:label>continuous testing</rdfs:label>
        <skos:prefLabel xml:lang="en">continuous testing</skos:prefLabel>
    </owl:Class>
    


    <!-- http://purl.org/stc/ontology#contract_testing -->

    <owl:Class rdf:about="http://purl.org/stc/ontology#contract_testing">
        <rdfs:subClassOf rdf:resource="http://purl.org/stc/ontology#target_orientation_in_test_approach"/>
        <isInISTQBGlossary rdf:datatype="http://www.w3.org/2001/XMLSchema#boolean">true</isInISTQBGlossary>
        <rdfs:label>contract testing</rdfs:label>
        <skos:prefLabel xml:lang="en">contract testing</skos:prefLabel>
    </owl:Class>
    


    <!-- http://purl.org/stc/ontology#coverage -->

    <owl:Class rdf:about="http://purl.org/stc/ontology#coverage">
        <rdfs:subClassOf rdf:resource="http://purl.org/stc/ontology#test_metric"/>
        <isInISTQBGlossary rdf:datatype="http://www.w3.org/2001/XMLSchema#boolean">true</isInISTQBGlossary>
        <rdfs:comment xml:lang="en">The degree to which specified coverage items are exercised by a test suite, expressed as a percentage. (ISTQB Glossary v4.5)</rdfs:comment>
        <rdfs:label>coverage</rdfs:label>
        <skos:altLabel xml:lang="en">coverage metric
test coverage
coverage-oriented metric</skos:altLabel>
        <skos:prefLabel xml:lang="en">coverage</skos:prefLabel>
    </owl:Class>
    


    <!-- http://purl.org/stc/ontology#coverage_item -->

    <owl:Class rdf:about="http://purl.org/stc/ontology#coverage_item">
        <rdfs:subClassOf rdf:resource="http://purl.org/stc/ontology#Testware"/>
        <isInISTQBGlossary rdf:datatype="http://www.w3.org/2001/XMLSchema#boolean">true</isInISTQBGlossary>
        <rdfs:comment xml:lang="en">An attribute or combination of attributes derived from one or more test conditions by using a test technique. (ISTQB Glossary v4.5)

Measurable attribute of a test item that is the focus of testing (ISO/IEC/IEEE 29119-1:2022, defined as test (coverage) item)</rdfs:comment>
        <rdfs:label>coverage item</rdfs:label>
        <rdfs:seeAlso>ISO/IEC/IEEE 29119-1:2022 (Software and systems engineering — Software testing — Part 1: Concepts and definitions)

Foundation - v4.0
Specialist - Model-Based Testing - v1.1</rdfs:seeAlso>
        <skos:altLabel xml:lang="en">test coverage item</skos:altLabel>
        <skos:prefLabel xml:lang="en">coverage item</skos:prefLabel>
    </owl:Class>
    


    <!-- http://purl.org/stc/ontology#crowd_testing -->

    <owl:Class rdf:about="http://purl.org/stc/ontology#crowd_testing">
        <rdfs:subClassOf rdf:resource="http://purl.org/stc/ontology#tester_orientation_in_test_approach"/>
        <isInISTQBGlossary rdf:datatype="http://www.w3.org/2001/XMLSchema#boolean">true</isInISTQBGlossary>
        <rdfs:label>crowd testing</rdfs:label>
        <skos:prefLabel xml:lang="en">crowd testing</skos:prefLabel>
    </owl:Class>
    


    <!-- http://purl.org/stc/ontology#data -->

    <owl:Class rdf:about="http://purl.org/stc/ontology#data">
        <rdfs:subClassOf rdf:resource="http://purl.org/stc/ontology#basic_concepts"/>
    </owl:Class>
    


    <!-- http://purl.org/stc/ontology#decision_coverage -->

    <owl:Class rdf:about="http://purl.org/stc/ontology#decision_coverage">
        <rdfs:subClassOf rdf:resource="http://purl.org/stc/ontology#structural_coverage"/>
        <isInISTQBGlossary rdf:datatype="http://www.w3.org/2001/XMLSchema#boolean">true</isInISTQBGlossary>
        <rdfs:comment xml:lang="en">The coverage of decision outcomes. (ISTQB Glossary v4.5)

Coverage for decision testing. (ISO/IEC/IEEE 29119-4)</rdfs:comment>
        <rdfs:label>decision coverage</rdfs:label>
        <rdfs:seeAlso>ISO/IEC/IEEE 29119-4 (Software and systems engineering — Software testing — Part 4: Test techniques)</rdfs:seeAlso>
        <skos:prefLabel xml:lang="en">decision coverage</skos:prefLabel>
    </owl:Class>
    


    <!-- http://purl.org/stc/ontology#decision_table_testing -->

    <owl:Class rdf:about="http://purl.org/stc/ontology#decision_table_testing">
        <rdfs:subClassOf rdf:resource="http://purl.org/stc/ontology#black_box_test_technique"/>
        <isInISTQBGlossary rdf:datatype="http://www.w3.org/2001/XMLSchema#boolean">true</isInISTQBGlossary>
        <rdfs:label>decision table testing</rdfs:label>
        <skos:prefLabel xml:lang="en">decision table testing</skos:prefLabel>
    </owl:Class>
    


    <!-- http://purl.org/stc/ontology#defect -->

    <owl:Class rdf:about="http://purl.org/stc/ontology#defect">
        <rdfs:subClassOf rdf:resource="http://purl.org/stc/ontology#basic_concepts"/>
    </owl:Class>
    


    <!-- http://purl.org/stc/ontology#defect_orientation_in_test_approach -->

    <owl:Class rdf:about="http://purl.org/stc/ontology#defect_orientation_in_test_approach">
        <rdfs:subClassOf rdf:resource="http://purl.org/stc/ontology#change_orientation_in_test_approach"/>
        <isInISTQBGlossary rdf:datatype="http://www.w3.org/2001/XMLSchema#boolean">false</isInISTQBGlossary>
        <rdfs:label>defect orientation</rdfs:label>
        <skos:prefLabel xml:lang="en">defect orientation in test approach</skos:prefLabel>
    </owl:Class>
    


    <!-- http://purl.org/stc/ontology#defect_oriented_metric -->

    <owl:Class rdf:about="http://purl.org/stc/ontology#defect_oriented_metric">
        <rdfs:subClassOf rdf:resource="http://purl.org/stc/ontology#test_metric"/>
        <isInISTQBGlossary rdf:datatype="http://www.w3.org/2001/XMLSchema#boolean">false</isInISTQBGlossary>
        <rdfs:label>defect oriented metric</rdfs:label>
        <skos:altLabel xml:lang="en">defect-oriented metric
defect metric</skos:altLabel>
        <skos:prefLabel xml:lang="en">defect oriented metric</skos:prefLabel>
    </owl:Class>
    


    <!-- http://purl.org/stc/ontology#destructive_testing -->

    <owl:Class rdf:about="http://purl.org/stc/ontology#destructive_testing">
        <rdfs:subClassOf rdf:resource="http://purl.org/stc/ontology#security_testing"/>
        <isInISTQBGlossary rdf:datatype="http://www.w3.org/2001/XMLSchema#boolean">true</isInISTQBGlossary>
        <rdfs:label>destructive testing</rdfs:label>
        <skos:prefLabel xml:lang="en">destructive testing</skos:prefLabel>
    </owl:Class>
    


    <!-- http://purl.org/stc/ontology#detailed_design -->

    <owl:Class rdf:about="http://purl.org/stc/ontology#detailed_design">
        <rdfs:subClassOf rdf:resource="http://purl.org/stc/ontology#software_engineering_activity"/>
    </owl:Class>
    


    <!-- http://purl.org/stc/ontology#development -->

    <owl:Class rdf:about="http://purl.org/stc/ontology#development">
        <rdfs:subClassOf rdf:resource="http://purl.org/stc/ontology#software_lifecycle"/>
    </owl:Class>
    


    <!-- http://purl.org/stc/ontology#device-based_testing -->

    <owl:Class rdf:about="http://purl.org/stc/ontology#device-based_testing">
        <rdfs:subClassOf rdf:resource="http://purl.org/stc/ontology#mobile_app_testing"/>
        <isInISTQBGlossary rdf:datatype="http://www.w3.org/2001/XMLSchema#boolean">true</isInISTQBGlossary>
        <rdfs:label>device-based testing</rdfs:label>
        <skos:prefLabel xml:lang="en">device-based testing</skos:prefLabel>
    </owl:Class>
    


    <!-- http://purl.org/stc/ontology#domain-specific_test_types -->

    <owl:Class rdf:about="http://purl.org/stc/ontology#domain-specific_test_types">
        <rdfs:subClassOf rdf:resource="http://purl.org/stc/ontology#test_type"/>
        <isInISTQBGlossary rdf:datatype="http://www.w3.org/2001/XMLSchema#boolean">false</isInISTQBGlossary>
        <rdfs:label>domain-specific test types</rdfs:label>
        <skos:prefLabel xml:lang="en">domain-specific test types</skos:prefLabel>
    </owl:Class>
    


    <!-- http://purl.org/stc/ontology#dynamic_application_security_testing -->

    <owl:Class rdf:about="http://purl.org/stc/ontology#dynamic_application_security_testing">
        <rdfs:subClassOf rdf:resource="http://purl.org/stc/ontology#security_testing"/>
        <isInISTQBGlossary rdf:datatype="http://www.w3.org/2001/XMLSchema#boolean">true</isInISTQBGlossary>
        <rdfs:label>dynamic application security testing</rdfs:label>
        <skos:prefLabel xml:lang="en">dynamic application security testing</skos:prefLabel>
    </owl:Class>
    


    <!-- http://purl.org/stc/ontology#dynamic_testing -->

    <owl:Class rdf:about="http://purl.org/stc/ontology#dynamic_testing">
        <rdfs:subClassOf rdf:resource="http://purl.org/stc/ontology#testing"/>
        <owl:disjointWith rdf:resource="http://purl.org/stc/ontology#static_testing"/>
        <isInISTQBGlossary rdf:datatype="http://www.w3.org/2001/XMLSchema#boolean">true</isInISTQBGlossary>
        <rdfs:comment xml:lang="en">Testing that involves the execution of the test item. (ISTQB Glossary v4.5)

Testing in which a test item is evaluated by executing it. (ISO/IEC/IEEE 29119-1)</rdfs:comment>
        <rdfs:label>dynamic testing</rdfs:label>
        <rdfs:seeAlso>ISO/IEC/IEEE 29119-1:2022 (Software and systems engineering — Software testing — Part 1: Concepts and definitions)

Foundation - v4.0</rdfs:seeAlso>
        <skos:prefLabel xml:lang="en">dynamic testing</skos:prefLabel>
    </owl:Class>
    


    <!-- http://purl.org/stc/ontology#each_choice_coverage -->

    <owl:Class rdf:about="http://purl.org/stc/ontology#each_choice_coverage">
        <rdfs:subClassOf rdf:resource="http://purl.org/stc/ontology#specification_coverage"/>
        <isInISTQBGlossary rdf:datatype="http://www.w3.org/2001/XMLSchema#boolean">true</isInISTQBGlossary>
        <rdfs:comment xml:lang="en">The coverage of equivalence partitions in multiple sets of partitions. (ISTQB Glossary v4.5)

Coverage for each choice testing. (ISO/IEC/IEEE 29119-4:2015)</rdfs:comment>
        <rdfs:label>each choice coverage</rdfs:label>
        <rdfs:seeAlso>ISO/IEC/IEEE 29119-4 (Software and systems engineering — Software testing — Part 4: Test techniques)</rdfs:seeAlso>
        <skos:altLabel xml:lang="en">ecc
ECC</skos:altLabel>
        <skos:prefLabel xml:lang="en">each choice coverage</skos:prefLabel>
    </owl:Class>
    


    <!-- http://purl.org/stc/ontology#end-to-end_testing -->

    <owl:Class rdf:about="http://purl.org/stc/ontology#end-to-end_testing">
        <rdfs:subClassOf rdf:resource="http://purl.org/stc/ontology#system_testing"/>
        <isInISTQBGlossary rdf:datatype="http://www.w3.org/2001/XMLSchema#boolean">true</isInISTQBGlossary>
        <rdfs:label>end-to-end testing</rdfs:label>
        <skos:altLabel xml:lang="en">e2e testing
E2E testing</skos:altLabel>
        <skos:prefLabel xml:lang="en">end-to-end testing</skos:prefLabel>
    </owl:Class>
    


    <!-- http://purl.org/stc/ontology#entry_criteria -->

    <owl:Class rdf:about="http://purl.org/stc/ontology#entry_criteria">
        <rdfs:subClassOf rdf:resource="http://purl.org/stc/ontology#Testware"/>
        <isInISTQBGlossary rdf:datatype="http://www.w3.org/2001/XMLSchema#boolean">true</isInISTQBGlossary>
        <rdfs:comment xml:lang="en">The set of conditions for officially completing a defined task. (ISTQB Glossary v4.5)</rdfs:comment>
        <rdfs:label>entry criteria</rdfs:label>
        <rdfs:seeAlso>Foundation - v4.0</rdfs:seeAlso>
        <skos:altLabel xml:lang="en">test completion criteria
completion criteria</skos:altLabel>
        <skos:prefLabel xml:lang="en">entry criteria</skos:prefLabel>
    </owl:Class>
    


    <!-- http://purl.org/stc/ontology#equivalence_partitioning -->

    <owl:Class rdf:about="http://purl.org/stc/ontology#equivalence_partitioning">
        <rdfs:subClassOf rdf:resource="http://purl.org/stc/ontology#black_box_test_technique"/>
        <isInISTQBGlossary rdf:datatype="http://www.w3.org/2001/XMLSchema#boolean">true</isInISTQBGlossary>
        <rdfs:label>equivalence partitioning</rdfs:label>
        <skos:prefLabel xml:lang="en">equivalence partitioning</skos:prefLabel>
    </owl:Class>
    


    <!-- http://purl.org/stc/ontology#error -->

    <owl:Class rdf:about="http://purl.org/stc/ontology#error">
        <rdfs:subClassOf rdf:resource="http://purl.org/stc/ontology#basic_concepts"/>
    </owl:Class>
    


    <!-- http://purl.org/stc/ontology#error_guessing -->

    <owl:Class rdf:about="http://purl.org/stc/ontology#error_guessing">
        <rdfs:subClassOf rdf:resource="http://purl.org/stc/ontology#experience-based_testing"/>
        <isInISTQBGlossary rdf:datatype="http://www.w3.org/2001/XMLSchema#boolean">true</isInISTQBGlossary>
        <rdfs:label>error guessing</rdfs:label>
        <skos:prefLabel xml:lang="en">error guessing</skos:prefLabel>
    </owl:Class>
    


    <!-- http://purl.org/stc/ontology#exhaustive_testing -->

    <owl:Class rdf:about="http://purl.org/stc/ontology#exhaustive_testing">
        <rdfs:subClassOf rdf:resource="http://purl.org/stc/ontology#method_orientation_in_test_approach"/>
        <isInISTQBGlossary rdf:datatype="http://www.w3.org/2001/XMLSchema#boolean">true</isInISTQBGlossary>
        <rdfs:comment xml:lang="en">A test approach in which the test suite comprises all combinations of input values and preconditions.</rdfs:comment>
        <rdfs:label>exhaustive testing</rdfs:label>
        <skos:altLabel xml:lang="en">complete testing</skos:altLabel>
        <skos:prefLabel xml:lang="en">exhaustive testing</skos:prefLabel>
    </owl:Class>
    


    <!-- http://purl.org/stc/ontology#exit_criteria -->

    <owl:Class rdf:about="http://purl.org/stc/ontology#exit_criteria">
        <rdfs:subClassOf rdf:resource="http://purl.org/stc/ontology#Testware"/>
        <isInISTQBGlossary rdf:datatype="http://www.w3.org/2001/XMLSchema#boolean">true</isInISTQBGlossary>
        <rdfs:comment xml:lang="en">The set of conditions for officially starting a defined task. (ISTQB Glossary v4-5)</rdfs:comment>
        <rdfs:label>exit criteria</rdfs:label>
        <rdfs:seeAlso>Foundation - v4.0
Advanced Test Manager - 2012
Advanced Test Analyst - v3.1</rdfs:seeAlso>
        <skos:altLabel>test completion criteria
completion criteria</skos:altLabel>
        <skos:prefLabel xml:lang="en">exit criteria</skos:prefLabel>
    </owl:Class>
    


    <!-- http://purl.org/stc/ontology#experience-based_testing -->

    <owl:Class rdf:about="http://purl.org/stc/ontology#experience-based_testing">
        <rdfs:subClassOf rdf:resource="http://purl.org/stc/ontology#test_technique"/>
        <owl:disjointWith rdf:resource="http://purl.org/stc/ontology#grey_box_test_technique"/>
        <owl:disjointWith rdf:resource="http://purl.org/stc/ontology#white_box_test_technique"/>
        <isInISTQBGlossary rdf:datatype="http://www.w3.org/2001/XMLSchema#boolean">true</isInISTQBGlossary>
        <rdfs:label>experience-based testing</rdfs:label>
        <skos:altLabel xml:lang="en">experience based testing
experience-based test technique
experience based test technique</skos:altLabel>
        <skos:prefLabel xml:lang="en">experience-based testing</skos:prefLabel>
    </owl:Class>
    


    <!-- http://purl.org/stc/ontology#experience_based_test_metric -->

    <owl:Class rdf:about="http://purl.org/stc/ontology#experience_based_test_metric">
        <rdfs:subClassOf rdf:resource="http://purl.org/stc/ontology#coverage"/>
        <isInISTQBGlossary rdf:datatype="http://www.w3.org/2001/XMLSchema#boolean">false</isInISTQBGlossary>
        <rdfs:comment xml:lang="en">There is currently no industry agreed approach to calculating experience-based coverage. (ISO/IEC/IEEE 29119-4)</rdfs:comment>
        <rdfs:label>experience coverage</rdfs:label>
        <rdfs:seeAlso>ISO/IEC/IEEE 29119-4 (Software and systems engineering — Software testing — Part 4: Test techniques)</rdfs:seeAlso>
        <skos:altLabel xml:lang="en">experience based test metric</skos:altLabel>
        <skos:altLabel xml:lang="en">experience based test metric
experience-based test metric</skos:altLabel>
        <skos:prefLabel xml:lang="en">experience coverage</skos:prefLabel>
    </owl:Class>
    


    <!-- http://purl.org/stc/ontology#exploratory_testing -->

    <owl:Class rdf:about="http://purl.org/stc/ontology#exploratory_testing">
        <rdfs:subClassOf rdf:resource="http://purl.org/stc/ontology#method_orientation_in_test_approach"/>
        <isInISTQBGlossary rdf:datatype="http://www.w3.org/2001/XMLSchema#boolean">true</isInISTQBGlossary>
        <rdfs:comment xml:lang="en">An approach to testing in which the testers dynamically design and execute tests based on their knowledge, exploration of the test item and the results of previous tests. (ISTQB Glossary v4.5)</rdfs:comment>
        <rdfs:label>exploratory testing</rdfs:label>
        <rdfs:seeAlso>ISO/IEC/IEEE 29119-1:2022 (Software and systems engineering — Software testing — Part 1: Concepts and definitions)

Foundation - v4.0
Advanced Test Analyst - v3.1</rdfs:seeAlso>
        <skos:prefLabel xml:lang="en">exploratory testing</skos:prefLabel>
    </owl:Class>
    


    <!-- http://purl.org/stc/ontology#failure -->

    <owl:Class rdf:about="http://purl.org/stc/ontology#failure">
        <rdfs:subClassOf rdf:resource="http://purl.org/stc/ontology#basic_concepts"/>
    </owl:Class>
    


    <!-- http://purl.org/stc/ontology#feature-driven_development -->

    <owl:Class rdf:about="http://purl.org/stc/ontology#feature-driven_development">
        <rdfs:subClassOf rdf:resource="http://purl.org/stc/ontology#target_orientation_in_software_development"/>
        <isInISTQBGlossary rdf:datatype="http://www.w3.org/2001/XMLSchema#boolean">true</isInISTQBGlossary>
        <rdfs:label>feature-driven development</rdfs:label>
        <skos:prefLabel xml:lang="en">feature-driven development</skos:prefLabel>
    </owl:Class>
    


    <!-- http://purl.org/stc/ontology#formal_review -->

    <owl:Class rdf:about="http://purl.org/stc/ontology#formal_review">
        <rdfs:subClassOf rdf:resource="http://purl.org/stc/ontology#review"/>
        <rdfs:label>formal review</rdfs:label>
        <skos:prefLabel xml:lang="en">formal review</skos:prefLabel>
    </owl:Class>
    


    <!-- http://purl.org/stc/ontology#functional_testing -->

    <owl:Class rdf:about="http://purl.org/stc/ontology#functional_testing">
        <rdfs:subClassOf rdf:resource="http://purl.org/stc/ontology#test_type"/>
        <isInISTQBGlossary rdf:datatype="http://www.w3.org/2001/XMLSchema#boolean">true</isInISTQBGlossary>
        <rdfs:comment xml:lang="en">Testing performed to evaluate if a component or system satisfies functional requirements. (ISTQB Glossary v4.5)</rdfs:comment>
        <rdfs:label>functional testing</rdfs:label>
        <rdfs:seeAlso>Foundation - v4.0
Advanced Test Management - v3.0
Advanced Test Analyst - v4.0
Specialist - Game Testing - v1.0.1</rdfs:seeAlso>
        <skos:prefLabel xml:lang="en">functional testing</skos:prefLabel>
    </owl:Class>
    


    <!-- http://purl.org/stc/ontology#fundamental_test_process -->

    <owl:Class rdf:about="http://purl.org/stc/ontology#fundamental_test_process">
        <rdfs:subClassOf rdf:resource="http://purl.org/stc/ontology#test_process"/>
        <isInISTQBGlossary rdf:datatype="http://www.w3.org/2001/XMLSchema#boolean">false</isInISTQBGlossary>
        <rdfs:label>fundamental test process</rdfs:label>
        <skos:prefLabel xml:lang="en">fundamental test process</skos:prefLabel>
    </owl:Class>
    


    <!-- http://purl.org/stc/ontology#gambling_testing -->

    <owl:Class rdf:about="http://purl.org/stc/ontology#gambling_testing">
        <rdfs:subClassOf rdf:resource="http://purl.org/stc/ontology#domain-specific_test_types"/>
        <isInISTQBGlossary rdf:datatype="http://www.w3.org/2001/XMLSchema#boolean">false</isInISTQBGlossary>
        <rdfs:label>gambling testing</rdfs:label>
        <skos:prefLabel xml:lang="en">gambling testing</skos:prefLabel>
    </owl:Class>
    


    <!-- http://purl.org/stc/ontology#grey_box_test_technique -->

    <owl:Class rdf:about="http://purl.org/stc/ontology#grey_box_test_technique">
        <rdfs:subClassOf rdf:resource="http://purl.org/stc/ontology#test_technique"/>
        <owl:disjointWith rdf:resource="http://purl.org/stc/ontology#white_box_test_technique"/>
        <isInISTQBGlossary rdf:datatype="http://www.w3.org/2001/XMLSchema#boolean">true</isInISTQBGlossary>
        <rdfs:label>grey-box testing</rdfs:label>
        <skos:altLabel xml:lang="en">grey box testing
gray-box testing
gray box testing</skos:altLabel>
        <skos:prefLabel xml:lang="en">grey-box testing</skos:prefLabel>
    </owl:Class>
    


    <!-- http://purl.org/stc/ontology#high_level_test_case -->

    <owl:Class rdf:about="http://purl.org/stc/ontology#high_level_test_case">
        <rdfs:subClassOf rdf:resource="http://purl.org/stc/ontology#test_case"/>
        <isInISTQBGlossary rdf:datatype="http://www.w3.org/2001/XMLSchema#boolean">true</isInISTQBGlossary>
        <rdfs:comment xml:lang="en">A test case with abstract preconditions, input data, expected results, postconditions, and actions (where applicable). (ISTQB Glossary v4.5)</rdfs:comment>
        <rdfs:label>high-level test case</rdfs:label>
        <rdfs:seeAlso>Advanced Test Manager - 2012
Advanced Test Analyst - v3.1
Advanced Test Analyst - v4.0</rdfs:seeAlso>
        <skos:altLabel>high level test case
logical test case
abstract test case
high level testcase
logical testcase
abstract testcase</skos:altLabel>
        <skos:prefLabel xml:lang="en">high-level test case</skos:prefLabel>
    </owl:Class>
    


    <!-- http://purl.org/stc/ontology#incremental_software_development -->

    <owl:Class rdf:about="http://purl.org/stc/ontology#incremental_software_development">
        <rdfs:subClassOf rdf:resource="http://purl.org/stc/ontology#process_orientation_in_software_development"/>
        <isInISTQBGlossary rdf:datatype="http://www.w3.org/2001/XMLSchema#boolean">false</isInISTQBGlossary>
        <rdfs:label>incremental</rdfs:label>
        <skos:prefLabel xml:lang="en">incremental software development</skos:prefLabel>
    </owl:Class>
    


    <!-- http://purl.org/stc/ontology#informal_review -->

    <owl:Class rdf:about="http://purl.org/stc/ontology#informal_review">
        <rdfs:subClassOf rdf:resource="http://purl.org/stc/ontology#review"/>
        <rdfs:label>informal review</rdfs:label>
        <skos:prefLabel xml:lang="en">informal review</skos:prefLabel>
    </owl:Class>
    


    <!-- http://purl.org/stc/ontology#inspection -->

    <owl:Class rdf:about="http://purl.org/stc/ontology#inspection">
        <rdfs:subClassOf rdf:resource="http://purl.org/stc/ontology#formal_review"/>
        <isInISTQBGlossary rdf:datatype="http://www.w3.org/2001/XMLSchema#boolean">true</isInISTQBGlossary>
        <rdfs:comment xml:lang="en">A type of formal review that uses defined team roles and measurement to identify defects in a work product, and improve the review process and the software development process. (ISTQB Glossary v4.5)</rdfs:comment>
        <rdfs:label>inspection</rdfs:label>
        <rdfs:seeAlso>Foundation - v4.0
Advanced Test Manager - 2012</rdfs:seeAlso>
        <skos:prefLabel xml:lang="en">inspection</skos:prefLabel>
    </owl:Class>
    


    <!-- http://purl.org/stc/ontology#integration -->

    <owl:Class rdf:about="http://purl.org/stc/ontology#integration">
        <rdfs:subClassOf rdf:resource="http://purl.org/stc/ontology#software_engineering_activity"/>
    </owl:Class>
    


    <!-- http://purl.org/stc/ontology#integration_testing -->

    <owl:Class rdf:about="http://purl.org/stc/ontology#integration_testing">
        <rdfs:subClassOf rdf:resource="http://purl.org/stc/ontology#test_level"/>
        <owl:disjointWith rdf:resource="http://purl.org/stc/ontology#system_testing"/>
        <isInISTQBGlossary rdf:datatype="http://www.w3.org/2001/XMLSchema#boolean">true</isInISTQBGlossary>
        <rdfs:label>integration testing</rdfs:label>
        <skos:prefLabel xml:lang="en">integration testing</skos:prefLabel>
    </owl:Class>
    


    <!-- http://purl.org/stc/ontology#interactive_application_security_testing -->

    <owl:Class rdf:about="http://purl.org/stc/ontology#interactive_application_security_testing">
        <rdfs:subClassOf rdf:resource="http://purl.org/stc/ontology#security_testing"/>
        <isInISTQBGlossary rdf:datatype="http://www.w3.org/2001/XMLSchema#boolean">true</isInISTQBGlossary>
        <rdfs:label>interactive application security testing</rdfs:label>
        <skos:prefLabel xml:lang="en">interactive application security testing</skos:prefLabel>
    </owl:Class>
    


    <!-- http://purl.org/stc/ontology#interface_testing -->

    <owl:Class rdf:about="http://purl.org/stc/ontology#interface_testing">
        <rdfs:subClassOf rdf:resource="http://purl.org/stc/ontology#target_orientation_in_test_approach"/>
        <isInISTQBGlossary rdf:datatype="http://www.w3.org/2001/XMLSchema#boolean">true</isInISTQBGlossary>
        <rdfs:label>interface testing</rdfs:label>
        <skos:prefLabel xml:lang="en">interface testing</skos:prefLabel>
    </owl:Class>
    


    <!-- http://purl.org/stc/ontology#interoperability_testing -->

    <owl:Class rdf:about="http://purl.org/stc/ontology#interoperability_testing">
        <rdfs:subClassOf rdf:resource="http://purl.org/stc/ontology#protocol_or_service_testing"/>
        <isInISTQBGlossary rdf:datatype="http://www.w3.org/2001/XMLSchema#boolean">false</isInISTQBGlossary>
        <rdfs:comment xml:lang="en">Testing conducted to ensure that a modified system retains the capability of exchanging information with systems of different types, and of using that information (ISO/IEC/IEEE 24765:2017)</rdfs:comment>
        <rdfs:label>interoperability testing</rdfs:label>
        <rdfs:seeAlso>ISO/IEC/IEEE 24765:2017 (Systems and software engineering —
Vocabulary)</rdfs:seeAlso>
        <skos:prefLabel xml:lang="en">interoperability testing</skos:prefLabel>
    </owl:Class>
    


    <!-- http://purl.org/stc/ontology#iterative_software_development -->

    <owl:Class rdf:about="http://purl.org/stc/ontology#iterative_software_development">
        <rdfs:subClassOf rdf:resource="http://purl.org/stc/ontology#process_orientation_in_software_development"/>
        <isInISTQBGlossary rdf:datatype="http://www.w3.org/2001/XMLSchema#boolean">true</isInISTQBGlossary>
        <rdfs:label>iterative</rdfs:label>
        <skos:prefLabel xml:lang="en">iterative software development</skos:prefLabel>
    </owl:Class>
    


    <!-- http://purl.org/stc/ontology#level_test_plan -->

    <owl:Class rdf:about="http://purl.org/stc/ontology#level_test_plan">
        <rdfs:subClassOf rdf:resource="http://purl.org/stc/ontology#test_plan"/>
        <isInISTQBGlossary rdf:datatype="http://www.w3.org/2001/XMLSchema#boolean">true</isInISTQBGlossary>
        <rdfs:comment xml:lang="en">A test plan that typically addresses one test level. (ISTQB Glossary v4.5)</rdfs:comment>
        <rdfs:label>level test plan</rdfs:label>
        <rdfs:seeAlso>Advanced Test Manager - 2012</rdfs:seeAlso>
        <skos:altLabel xml:lang="en">level testplan</skos:altLabel>
        <skos:prefLabel xml:lang="en">level test plan</skos:prefLabel>
    </owl:Class>
    


    <!-- http://purl.org/stc/ontology#load_testing -->

    <owl:Class rdf:about="http://purl.org/stc/ontology#load_testing">
        <rdfs:subClassOf rdf:resource="http://purl.org/stc/ontology#performance_testing"/>
        <isInISTQBGlossary rdf:datatype="http://www.w3.org/2001/XMLSchema#boolean">true</isInISTQBGlossary>
        <rdfs:label>load testing</rdfs:label>
        <skos:prefLabel xml:lang="en">load testing</skos:prefLabel>
    </owl:Class>
    


    <!-- http://purl.org/stc/ontology#low_level_test_case -->

    <owl:Class rdf:about="http://purl.org/stc/ontology#low_level_test_case">
        <rdfs:subClassOf rdf:resource="http://purl.org/stc/ontology#test_case"/>
        <isInISTQBGlossary rdf:datatype="http://www.w3.org/2001/XMLSchema#boolean">true</isInISTQBGlossary>
        <rdfs:comment xml:lang="en">A test case with concrete values for preconditions, input data, expected results, postconditions, and a detailed description of actions (where applicable). (ISTQB Glossary v4.5)</rdfs:comment>
        <rdfs:label>low-level test case</rdfs:label>
        <rdfs:seeAlso>Advanced Test Analyst - v3.1
Advanced Test Analyst - v4.0</rdfs:seeAlso>
        <skos:altLabel xml:lang="en">low level test case
concrete test case
physical test case
low level testcase
concrete testcase
physical testcase</skos:altLabel>
        <skos:prefLabel xml:lang="en">low-level test case</skos:prefLabel>
    </owl:Class>
    


    <!-- http://purl.org/stc/ontology#maintenance -->

    <owl:Class rdf:about="http://purl.org/stc/ontology#maintenance">
        <rdfs:subClassOf rdf:resource="http://purl.org/stc/ontology#software_lifecycle"/>
    </owl:Class>
    


    <!-- http://purl.org/stc/ontology#maintenance_testing -->

    <owl:Class rdf:about="http://purl.org/stc/ontology#maintenance_testing">
        <rdfs:subClassOf rdf:resource="http://purl.org/stc/ontology#change_orientation_in_test_approach"/>
        <isInISTQBGlossary rdf:datatype="http://www.w3.org/2001/XMLSchema#boolean">true</isInISTQBGlossary>
        <rdfs:comment xml:lang="en">Testing the changes to an operational system or the impact of a changed environment to an operational system. (ISTQB Glossary v4.5)</rdfs:comment>
        <rdfs:label>maintenance testing</rdfs:label>
        <rdfs:seeAlso>Foundation - v4.0</rdfs:seeAlso>
        <skos:prefLabel xml:lang="en">maintenance testing</skos:prefLabel>
    </owl:Class>
    


    <!-- http://purl.org/stc/ontology#manual_testing -->

    <owl:Class rdf:about="http://purl.org/stc/ontology#manual_testing">
        <rdfs:subClassOf rdf:resource="http://purl.org/stc/ontology#test_execution"/>
        <isInISTQBGlossary rdf:datatype="http://www.w3.org/2001/XMLSchema#boolean">false</isInISTQBGlossary>
        <rdfs:comment xml:lang="en">Humans performing tests by entering information into a test item and verifying the results. (ISO/IEC/IEEE 29119-1:2022)</rdfs:comment>
        <rdfs:comment xml:lang="en">ISO/IEC/IEEE 29119-1:2022 (Software and systems engineering — Software testing — Part 1: Concepts and definitions)</rdfs:comment>
        <rdfs:label>manual testing</rdfs:label>
        <skos:altLabel>unscripted testing</skos:altLabel>
        <skos:prefLabel xml:lang="en">manual testing</skos:prefLabel>
    </owl:Class>
    


    <!-- http://purl.org/stc/ontology#master_test_plan -->

    <owl:Class rdf:about="http://purl.org/stc/ontology#master_test_plan">
        <rdfs:subClassOf rdf:resource="http://purl.org/stc/ontology#test_plan"/>
        <isInISTQBGlossary rdf:datatype="http://www.w3.org/2001/XMLSchema#boolean">true</isInISTQBGlossary>
        <rdfs:comment xml:lang="en">A test plan that is used to coordinate multiple test levels or test types. (ISTQB Glossary v4.5)</rdfs:comment>
        <rdfs:label>master test plan</rdfs:label>
        <rdfs:seeAlso>Advanced Test Manager - 2012</rdfs:seeAlso>
        <skos:altLabel xml:lang="en">master testplan</skos:altLabel>
        <skos:prefLabel xml:lang="en">master test plan</skos:prefLabel>
    </owl:Class>
    


    <!-- http://purl.org/stc/ontology#math_testing -->

    <owl:Class rdf:about="http://purl.org/stc/ontology#math_testing">
        <rdfs:subClassOf rdf:resource="http://purl.org/stc/ontology#gambling_testing"/>
        <isInISTQBGlossary rdf:datatype="http://www.w3.org/2001/XMLSchema#boolean">true</isInISTQBGlossary>
        <rdfs:label>math testing</rdfs:label>
        <skos:prefLabel xml:lang="en">math testing</skos:prefLabel>
    </owl:Class>
    


    <!-- http://purl.org/stc/ontology#method_orientation_in_test_approach -->

    <owl:Class rdf:about="http://purl.org/stc/ontology#method_orientation_in_test_approach">
        <rdfs:subClassOf rdf:resource="http://purl.org/stc/ontology#test_approach"/>
        <isInISTQBGlossary rdf:datatype="http://www.w3.org/2001/XMLSchema#boolean">false</isInISTQBGlossary>
        <rdfs:label>method orientation</rdfs:label>
        <skos:prefLabel xml:lang="en">method orientation in test approach</skos:prefLabel>
    </owl:Class>
    


    <!-- http://purl.org/stc/ontology#metric -->

    <owl:Class rdf:about="http://purl.org/stc/ontology#metric">
        <rdfs:subClassOf rdf:resource="http://purl.org/stc/ontology#basic_concepts"/>
        <isInISTQBGlossary rdf:datatype="http://www.w3.org/2001/XMLSchema#boolean">true</isInISTQBGlossary>
        <rdfs:comment xml:lang="en">A measurement scale and the method used for measurement. (ISTQB Glossary v4.5) 

A quantitative measure of the degree to which a system, component, or process possesses a given attribute. (ISO/IEC/IEEE 24765:2017)</rdfs:comment>
        <rdfs:label>metric</rdfs:label>
        <rdfs:seeAlso>ISO/IEC/IEEE 24765:2017 (Systems and Software Engineering – Vocabulary)

Foundation - v4.0
Advanced Test Manager - 2012
Advanced Test Management - v3.0
Advanced Test Analyst - v3.1
Advanced Test Analyst - v4.0
Advanced Technical Test Analyst - v4.0
Advanced Test Automation Engineering - v2.0
Expert Improving the Test Process - 2011
Expert Test Management - 2011
Foundation Agile Tester - 2014
Advanced Agile Technical Tester - 2019
Agile Test Leadership at Scale - v1.0
Specialist - Acceptance Testing - 2019
Specialist - Agile Test Leadership at Scale - v2.0
Specialist - AI Testing - v1.0
Specialist - Automotive Software Tester - 2018
Specialist - Automotive Software Tester - v1.1
Specialist - Gambling Industry Tester - 2018
Specialist - Game Testing - v1.0.1
Specialist - Model-Based Tester - 2015
Specialist - Model-Based Testing - v1.1
Specialist - Performance Testing - 2018
Specialist - Security Tester - 2016
Specialist - Security Test Engineer - v1.0
Specialist - Test Automation Engineer - 2016
Specialist - Test Automation Strategy - v1.0</rdfs:seeAlso>
        <skos:prefLabel xml:lang="en">metric</skos:prefLabel>
    </owl:Class>
    


    <!-- http://purl.org/stc/ontology#mobile_app_testing -->

    <owl:Class rdf:about="http://purl.org/stc/ontology#mobile_app_testing">
        <rdfs:subClassOf rdf:resource="http://purl.org/stc/ontology#domain-specific_test_types"/>
        <isInISTQBGlossary rdf:datatype="http://www.w3.org/2001/XMLSchema#boolean">false</isInISTQBGlossary>
        <rdfs:label>mobile app testing</rdfs:label>
        <skos:altLabel xml:lang="en">mobile application testing</skos:altLabel>
        <skos:prefLabel xml:lang="en">mobile app testing</skos:prefLabel>
    </owl:Class>
    


    <!-- http://purl.org/stc/ontology#model -->

    <owl:Class rdf:about="http://purl.org/stc/ontology#model">
        <rdfs:subClassOf rdf:resource="http://purl.org/stc/ontology#basic_concepts"/>
    </owl:Class>
    


    <!-- http://purl.org/stc/ontology#model_based_testing -->

    <owl:Class rdf:about="http://purl.org/stc/ontology#model_based_testing">
        <rdfs:subClassOf rdf:resource="http://purl.org/stc/ontology#black_box_test_technique"/>
        <isInISTQBGlossary rdf:datatype="http://www.w3.org/2001/XMLSchema#boolean">true</isInISTQBGlossary>
        <rdfs:comment xml:lang="en">Testing based on or involving models. (ISTQB Glossary v4.5)</rdfs:comment>
        <rdfs:label>model-based testing</rdfs:label>
        <rdfs:seeAlso>Advanced Test Analyst - v4.0
Advanced Technical Test Analyst - v4.0
Advanced Test Automation Engineering - v2.0
Specialist - Acceptance Testing - 2019
Specialist - Model-Based Tester - 2015
Specialist - Model-Based Testing - v1.1
Specialist - Test Automation Engineer - 2016</rdfs:seeAlso>
        <skos:altLabel xml:lang="en">model based testing
mbt
MBT
model driven testing
model-driven testing
mdt
MDT</skos:altLabel>
        <skos:prefLabel xml:lang="en">model-based testing</skos:prefLabel>
    </owl:Class>
    


    <!-- http://purl.org/stc/ontology#model_coverage -->

    <owl:Class rdf:about="http://purl.org/stc/ontology#model_coverage">
        <rdfs:subClassOf rdf:resource="http://purl.org/stc/ontology#specification_coverage"/>
        <isInISTQBGlossary rdf:datatype="http://www.w3.org/2001/XMLSchema#boolean">true</isInISTQBGlossary>
        <rdfs:comment xml:lang="en">The coverage of model elements. (ISTQB Glossary v4.5)</rdfs:comment>
        <rdfs:label>model coverage</rdfs:label>
        <rdfs:seeAlso>Specialist - Model-Based Testing - v1.1</rdfs:seeAlso>
        <skos:prefLabel xml:lang="en">model coverage</skos:prefLabel>
    </owl:Class>
    


    <!-- http://purl.org/stc/ontology#model_verification -->

    <owl:Class rdf:about="http://purl.org/stc/ontology#model_verification">
        <rdfs:subClassOf rdf:resource="http://purl.org/stc/ontology#static_testing"/>
        <isInISTQBGlossary rdf:datatype="http://www.w3.org/2001/XMLSchema#boolean">false</isInISTQBGlossary>
        <rdfs:comment xml:lang="en">The process of determining that a model accurately represents the required conceptual description and specifications. (own)</rdfs:comment>
        <rdfs:label>model verification</rdfs:label>
        <skos:prefLabel xml:lang="en">model verification</skos:prefLabel>
    </owl:Class>
    


    <!-- http://purl.org/stc/ontology#modified_condition_decision_coverage -->

    <owl:Class rdf:about="http://purl.org/stc/ontology#modified_condition_decision_coverage">
        <rdfs:subClassOf rdf:resource="http://purl.org/stc/ontology#structural_coverage"/>
        <isInISTQBGlossary rdf:datatype="http://www.w3.org/2001/XMLSchema#boolean">true</isInISTQBGlossary>
        <rdfs:comment xml:lang="en">The coverage of all outcomes of the atomic conditions that independently affect the overall decision outcome. (ISTQB Glossary v4.5)

Coverage for modified condition/decision coverage testing. (ISO/IEC/IEEE 29119-4)</rdfs:comment>
        <rdfs:label>modified condition/decision coverage</rdfs:label>
        <rdfs:seeAlso>ISO/IEC/IEEE 29119-4 (Software and systems engineering — Software testing — Part 4: Test techniques)</rdfs:seeAlso>
        <skos:altLabel xml:lang="en">mc/dc
MC/DC
condition determination coverage
modified multiple condition coverage</skos:altLabel>
        <skos:prefLabel xml:lang="en">modified condition/decision coverage</skos:prefLabel>
    </owl:Class>
    


    <!-- http://purl.org/stc/ontology#multiple_condition_coverage -->

    <owl:Class rdf:about="http://purl.org/stc/ontology#multiple_condition_coverage">
        <rdfs:subClassOf rdf:resource="http://purl.org/stc/ontology#structural_coverage"/>
        <isInISTQBGlossary rdf:datatype="http://www.w3.org/2001/XMLSchema#boolean">true</isInISTQBGlossary>
        <rdfs:comment xml:lang="en">The coverage of all possible combinations of all single condition outcomes within one statement. (ISTQB Glossary v4.5)

Coverage for branch condition combination testing. (ISO/IEC/IEEE 29119-4 as branch condition combination coverage)</rdfs:comment>
        <rdfs:label>multiple condition coverage</rdfs:label>
        <rdfs:seeAlso>ISO/IEC/IEEE 29119-4 (Software and systems engineering — Software testing — Part 4: Test techniques)</rdfs:seeAlso>
        <skos:altLabel>branch condition combination coverage
condition combination coverage</skos:altLabel>
        <skos:prefLabel xml:lang="en">multiple condition coverage</skos:prefLabel>
    </owl:Class>
    


    <!-- http://purl.org/stc/ontology#neuron_coverage -->

    <owl:Class rdf:about="http://purl.org/stc/ontology#neuron_coverage">
        <rdfs:subClassOf rdf:resource="http://purl.org/stc/ontology#LLM_structural_coverage"/>
        <isInISTQBGlossary rdf:datatype="http://www.w3.org/2001/XMLSchema#boolean">true</isInISTQBGlossary>
        <rdfs:comment xml:lang="en">The coverage of activated neurons in the neural network for a set of tests. (ISTQB Glossary v4.5)</rdfs:comment>
        <rdfs:label>neuron coverage</rdfs:label>
        <rdfs:seeAlso>Specialist - AI Testing - v1.0</rdfs:seeAlso>
        <skos:prefLabel xml:lang="en">neuron coverage</skos:prefLabel>
    </owl:Class>
    


    <!-- http://purl.org/stc/ontology#non-functional_testing -->

    <owl:Class rdf:about="http://purl.org/stc/ontology#non-functional_testing">
        <rdfs:subClassOf rdf:resource="http://purl.org/stc/ontology#test_type"/>
        <isInISTQBGlossary rdf:datatype="http://www.w3.org/2001/XMLSchema#boolean">true</isInISTQBGlossary>
        <rdfs:comment xml:lang="en">Testing performed to evaluate that a component or system complies with non-functional requirements. (ISTQB Glossary v4.5)</rdfs:comment>
        <rdfs:label>non-functional testing</rdfs:label>
        <rdfs:seeAlso>Foundation - v4.0
Advanced Test Management - v3.0</rdfs:seeAlso>
        <skos:altLabel xml:lang="en">extra-functional testing</skos:altLabel>
        <skos:prefLabel xml:lang="en">non-functional testing</skos:prefLabel>
    </owl:Class>
    


    <!-- http://purl.org/stc/ontology#operation -->

    <owl:Class rdf:about="http://purl.org/stc/ontology#operation">
        <rdfs:subClassOf rdf:resource="http://purl.org/stc/ontology#software_lifecycle"/>
    </owl:Class>
    


    <!-- http://purl.org/stc/ontology#oracle_orientation_in_test_approach -->

    <owl:Class rdf:about="http://purl.org/stc/ontology#oracle_orientation_in_test_approach">
        <rdfs:subClassOf rdf:resource="http://purl.org/stc/ontology#test_approach"/>
        <isInISTQBGlossary rdf:datatype="http://www.w3.org/2001/XMLSchema#boolean">false</isInISTQBGlossary>
        <rdfs:label>oracle orientation</rdfs:label>
        <skos:prefLabel xml:lang="en">oracle orientation in test approach</skos:prefLabel>
    </owl:Class>
    


    <!-- http://purl.org/stc/ontology#pair_testing -->

    <owl:Class rdf:about="http://purl.org/stc/ontology#pair_testing">
        <rdfs:subClassOf rdf:resource="http://purl.org/stc/ontology#tester_orientation_in_test_approach"/>
        <isInISTQBGlossary rdf:datatype="http://www.w3.org/2001/XMLSchema#boolean">true</isInISTQBGlossary>
        <rdfs:label>pair testing</rdfs:label>
        <skos:prefLabel xml:lang="en">pair testing</skos:prefLabel>
    </owl:Class>
    


    <!-- http://purl.org/stc/ontology#peer_review -->

    <owl:Class rdf:about="http://purl.org/stc/ontology#peer_review">
        <rdfs:subClassOf rdf:resource="http://purl.org/stc/ontology#informal_review"/>
        <isInISTQBGlossary rdf:datatype="http://www.w3.org/2001/XMLSchema#boolean">true</isInISTQBGlossary>
        <rdfs:comment xml:lang="en">A type of review performed on a work product by persons that have the abilities required to create it.  (ISTQB Glossary v4.5)</rdfs:comment>
        <rdfs:label>peer review</rdfs:label>
        <rdfs:seeAlso></rdfs:seeAlso>
        <skos:prefLabel xml:lang="en">peer review</skos:prefLabel>
    </owl:Class>
    


    <!-- http://purl.org/stc/ontology#performance_testing -->

    <owl:Class rdf:about="http://purl.org/stc/ontology#performance_testing">
        <rdfs:subClassOf rdf:resource="http://purl.org/stc/ontology#non-functional_testing"/>
        <isInISTQBGlossary rdf:datatype="http://www.w3.org/2001/XMLSchema#boolean">true</isInISTQBGlossary>
        <rdfs:label>performance testing</rdfs:label>
        <skos:prefLabel xml:lang="en">performance testing</skos:prefLabel>
    </owl:Class>
    


    <!-- http://purl.org/stc/ontology#process_improvement -->

    <owl:Class rdf:about="http://purl.org/stc/ontology#process_improvement">
        <rdfs:subClassOf rdf:resource="http://purl.org/stc/ontology#support_processes"/>
    </owl:Class>
    


    <!-- http://purl.org/stc/ontology#process_orientation_in_software_development -->

    <owl:Class rdf:about="http://purl.org/stc/ontology#process_orientation_in_software_development">
        <rdfs:subClassOf rdf:resource="http://purl.org/stc/ontology#software_development_model"/>
        <isInISTQBGlossary rdf:datatype="http://www.w3.org/2001/XMLSchema#boolean">false</isInISTQBGlossary>
        <rdfs:label>process orientation</rdfs:label>
        <skos:prefLabel xml:lang="en">process orientation in software development</skos:prefLabel>
    </owl:Class>
    


    <!-- http://purl.org/stc/ontology#process_orientation_in_test_approach -->

    <owl:Class rdf:about="http://purl.org/stc/ontology#process_orientation_in_test_approach">
        <rdfs:subClassOf rdf:resource="http://purl.org/stc/ontology#test_approach"/>
        <isInISTQBGlossary rdf:datatype="http://www.w3.org/2001/XMLSchema#boolean">false</isInISTQBGlossary>
        <rdfs:label>process orientation</rdfs:label>
        <skos:prefLabel xml:lang="en">process orientation in test approach</skos:prefLabel>
    </owl:Class>
    


    <!-- http://purl.org/stc/ontology#project_management -->

    <owl:Class rdf:about="http://purl.org/stc/ontology#project_management">
        <rdfs:subClassOf rdf:resource="http://purl.org/stc/ontology#support_processes"/>
    </owl:Class>
    


    <!-- http://purl.org/stc/ontology#property-based_testing -->

    <owl:Class rdf:about="http://purl.org/stc/ontology#property-based_testing">
        <rdfs:subClassOf rdf:resource="http://purl.org/stc/ontology#target_orientation_in_test_approach"/>
        <isInISTQBGlossary rdf:datatype="http://www.w3.org/2001/XMLSchema#boolean">true</isInISTQBGlossary>
        <rdfs:label>property-based testing</rdfs:label>
        <skos:prefLabel xml:lang="en">property-based testing</skos:prefLabel>
    </owl:Class>
    


    <!-- http://purl.org/stc/ontology#protocol_or_service_testing -->

    <owl:Class rdf:about="http://purl.org/stc/ontology#protocol_or_service_testing">
        <rdfs:subClassOf rdf:resource="http://purl.org/stc/ontology#domain-specific_test_types"/>
        <isInISTQBGlossary rdf:datatype="http://www.w3.org/2001/XMLSchema#boolean">false</isInISTQBGlossary>
        <rdfs:label>protocol or service testing</rdfs:label>
        <skos:prefLabel xml:lang="en">protocol or service testing</skos:prefLabel>
    </owl:Class>
    


    <!-- http://purl.org/stc/ontology#quality_assurance -->

    <owl:Class rdf:about="http://purl.org/stc/ontology#quality_assurance">
        <rdfs:subClassOf rdf:resource="http://purl.org/stc/ontology#support_processes"/>
    </owl:Class>
    


    <!-- http://purl.org/stc/ontology#reactive_testing -->

    <owl:Class rdf:about="http://purl.org/stc/ontology#reactive_testing">
        <rdfs:subClassOf rdf:resource="http://purl.org/stc/ontology#dynamic_testing"/>
        <isInISTQBGlossary rdf:datatype="http://www.w3.org/2001/XMLSchema#boolean">true</isInISTQBGlossary>
        <rdfs:label>reactive testing</rdfs:label>
        <skos:prefLabel xml:lang="en">reactive testing</skos:prefLabel>
    </owl:Class>
    


    <!-- http://purl.org/stc/ontology#regression_testing -->

    <owl:Class rdf:about="http://purl.org/stc/ontology#regression_testing">
        <rdfs:subClassOf rdf:resource="http://purl.org/stc/ontology#change_orientation_in_test_approach"/>
        <isInISTQBGlossary rdf:datatype="http://www.w3.org/2001/XMLSchema#boolean">true</isInISTQBGlossary>
        <rdfs:comment xml:lang="en">A type of change-related testing to detect whether defects have been introduced or uncovered in unchanged areas of the software. (ISTQB Glossary v4.5)

Testingperformed following modifications to a test item or to its operational environment, to identify whether failures in unmodified parts of the test item occur. (ISO/IEC/IEEE 29119-1:2022)</rdfs:comment>
        <rdfs:label>regression testing</rdfs:label>
        <rdfs:seeAlso>ISO/IEC/IEEE 29119-1:2022 (Software and systems engineering — Software testing — Part 1: Concepts and definitions)

Foundation - v4.0
Advanced Test Analyst - v4.0
Specialist - Test Automation Engineer - 2016</rdfs:seeAlso>
        <skos:prefLabel xml:lang="en">regression testing</skos:prefLabel>
    </owl:Class>
    


    <!-- http://purl.org/stc/ontology#regulatory_acceptance_testing -->

    <owl:Class rdf:about="http://purl.org/stc/ontology#regulatory_acceptance_testing">
        <rdfs:subClassOf rdf:resource="http://purl.org/stc/ontology#acceptance_testing"/>
        <isInISTQBGlossary rdf:datatype="http://www.w3.org/2001/XMLSchema#boolean">true</isInISTQBGlossary>
        <rdfs:label>regulatory acceptance testing</rdfs:label>
        <skos:prefLabel xml:lang="en">regulatory acceptance testing</skos:prefLabel>
    </owl:Class>
    


    <!-- http://purl.org/stc/ontology#related_to_role -->

    <owl:Class rdf:about="http://purl.org/stc/ontology#related_to_role">
        <rdfs:subClassOf rdf:resource="http://purl.org/stc/ontology#test_work_force"/>
        <isInISTQBGlossary rdf:datatype="http://www.w3.org/2001/XMLSchema#boolean">false</isInISTQBGlossary>
        <rdfs:label>related to role</rdfs:label>
        <skos:prefLabel xml:lang="en">related to role</skos:prefLabel>
    </owl:Class>
    


    <!-- http://purl.org/stc/ontology#related_to_team -->

    <owl:Class rdf:about="http://purl.org/stc/ontology#related_to_team">
        <rdfs:subClassOf rdf:resource="http://purl.org/stc/ontology#test_work_force"/>
        <isInISTQBGlossary rdf:datatype="http://www.w3.org/2001/XMLSchema#boolean">false</isInISTQBGlossary>
        <rdfs:label>related to team</rdfs:label>
        <skos:prefLabel xml:lang="en">related to team</skos:prefLabel>
    </owl:Class>
    


    <!-- http://purl.org/stc/ontology#release -->

    <owl:Class rdf:about="http://purl.org/stc/ontology#release">
        <rdfs:subClassOf rdf:resource="http://purl.org/stc/ontology#software_lifecycle"/>
    </owl:Class>
    


    <!-- http://purl.org/stc/ontology#requirements-based_testing -->

    <owl:Class rdf:about="http://purl.org/stc/ontology#requirements-based_testing">
        <rdfs:subClassOf rdf:resource="http://purl.org/stc/ontology#black_box_test_technique"/>
        <isInISTQBGlossary rdf:datatype="http://www.w3.org/2001/XMLSchema#boolean">true</isInISTQBGlossary>
        <rdfs:label>requirements-based testing</rdfs:label>
        <skos:prefLabel xml:lang="en">requirements-based testing</skos:prefLabel>
    </owl:Class>
    


    <!-- http://purl.org/stc/ontology#requirements_coverage -->

    <owl:Class rdf:about="http://purl.org/stc/ontology#requirements_coverage">
        <rdfs:subClassOf rdf:resource="http://purl.org/stc/ontology#specification_coverage"/>
        <isInISTQBGlossary rdf:datatype="http://www.w3.org/2001/XMLSchema#boolean">false</isInISTQBGlossary>
        <rdfs:comment xml:lang="en">Number of requirements covered by executed tests (ISO/IEC/IEEE 29119-1:2022, defined as test coverage)</rdfs:comment>
        <rdfs:label>requirement coverage</rdfs:label>
        <rdfs:seeAlso>ISO/IEC/IEEE 29119-1:2022 (Software and systems engineering — Software testing — Part 1: Concepts and definitions)</rdfs:seeAlso>
        <skos:altLabel xml:lang="en">requirements coverage</skos:altLabel>
        <skos:prefLabel xml:lang="en">requirement coverage</skos:prefLabel>
    </owl:Class>
    


    <!-- http://purl.org/stc/ontology#requirements_engineering -->

    <owl:Class rdf:about="http://purl.org/stc/ontology#requirements_engineering">
        <rdfs:subClassOf rdf:resource="http://purl.org/stc/ontology#software_engineering_activity"/>
    </owl:Class>
    


    <!-- http://purl.org/stc/ontology#review -->

    <owl:Class rdf:about="http://purl.org/stc/ontology#review">
        <rdfs:subClassOf rdf:resource="http://purl.org/stc/ontology#static_testing"/>
    </owl:Class>
    


    <!-- http://purl.org/stc/ontology#risk-based_testing -->

    <owl:Class rdf:about="http://purl.org/stc/ontology#risk-based_testing">
        <rdfs:subClassOf rdf:resource="http://purl.org/stc/ontology#target_orientation_in_test_approach"/>
        <isInISTQBGlossary rdf:datatype="http://www.w3.org/2001/XMLSchema#boolean">true</isInISTQBGlossary>
        <rdfs:label>risk-based testing</rdfs:label>
        <skos:prefLabel xml:lang="en">risk-based testing</skos:prefLabel>
    </owl:Class>
    


    <!-- http://purl.org/stc/ontology#risk_oriented_metric -->

    <owl:Class rdf:about="http://purl.org/stc/ontology#risk_oriented_metric">
        <rdfs:subClassOf rdf:resource="http://purl.org/stc/ontology#test_metric"/>
        <isInISTQBGlossary rdf:datatype="http://www.w3.org/2001/XMLSchema#boolean">false</isInISTQBGlossary>
        <rdfs:label>risk oriented metric</rdfs:label>
        <skos:altLabel xml:lang="en">risk-oriented metric
risk metric</skos:altLabel>
        <skos:prefLabel xml:lang="en">risk oriented metric</skos:prefLabel>
    </owl:Class>
    


    <!-- http://purl.org/stc/ontology#safety_testing -->

    <owl:Class rdf:about="http://purl.org/stc/ontology#safety_testing">
        <rdfs:subClassOf rdf:resource="http://purl.org/stc/ontology#non-functional_testing"/>
        <isInISTQBGlossary rdf:datatype="http://www.w3.org/2001/XMLSchema#boolean">false</isInISTQBGlossary>
        <rdfs:label>safety testing</rdfs:label>
        <skos:prefLabel xml:lang="en">safety testing</skos:prefLabel>
    </owl:Class>
    


    <!-- http://purl.org/stc/ontology#scripted_testing -->

    <owl:Class rdf:about="http://purl.org/stc/ontology#scripted_testing">
        <rdfs:subClassOf rdf:resource="http://purl.org/stc/ontology#manual_testing"/>
        <isInISTQBGlossary rdf:datatype="http://www.w3.org/2001/XMLSchema#boolean">true</isInISTQBGlossary>
        <rdfs:comment xml:lang="en">Testing performed based on a documented test script. (ISO/IEC/IEEE 29119-1:2022)</rdfs:comment>
        <rdfs:label>scripted testing</rdfs:label>
        <rdfs:seeAlso>ISO/IEC/IEEE 29119-1:2022 (Software and systems engineering — Software testing — Part 1: Concepts and definitions)</rdfs:seeAlso>
        <skos:prefLabel xml:lang="en">scripted testing</skos:prefLabel>
    </owl:Class>
    


    <!-- http://purl.org/stc/ontology#security_testing -->

    <owl:Class rdf:about="http://purl.org/stc/ontology#security_testing">
        <rdfs:subClassOf rdf:resource="http://purl.org/stc/ontology#non-functional_testing"/>
        <isInISTQBGlossary rdf:datatype="http://www.w3.org/2001/XMLSchema#boolean">true</isInISTQBGlossary>
        <rdfs:comment xml:lang="en">A test type to determine the security of a component or system. (ISTQB Glossary v4.5)

Test type conducted to evaluate the degree to which a test item, and associated data and information, are protected so that unauthorized persons or systems cannot use, read, or modify them, and authorized persons or systems are not denied access to them. (ISO/IEC/IEEE 29119-1:2022)</rdfs:comment>
        <rdfs:label>security testing</rdfs:label>
        <rdfs:seeAlso>ISO/IEC/IEEE 29119-1:2022 (Software and systems engineering — Software testing — Part 1: Concepts and definitions)

Specialist - Mobile Application Testing - 2019
Specialist - Security Tester - 2016
Specialist - Security Test Engineer - v1.0</rdfs:seeAlso>
        <skos:prefLabel xml:lang="en">security testing</skos:prefLabel>
    </owl:Class>
    


    <!-- http://purl.org/stc/ontology#sequential_development_model -->

    <owl:Class rdf:about="http://purl.org/stc/ontology#sequential_development_model">
        <rdfs:subClassOf rdf:resource="http://purl.org/stc/ontology#process_orientation_in_software_development"/>
        <isInISTQBGlossary rdf:datatype="http://www.w3.org/2001/XMLSchema#boolean">true</isInISTQBGlossary>
        <rdfs:label>sequential</rdfs:label>
        <skos:prefLabel xml:lang="en">sequential development model</skos:prefLabel>
    </owl:Class>
    


    <!-- http://purl.org/stc/ontology#session-based_testing -->

    <owl:Class rdf:about="http://purl.org/stc/ontology#session-based_testing">
        <rdfs:subClassOf rdf:resource="http://purl.org/stc/ontology#process_orientation_in_test_approach"/>
        <isInISTQBGlossary rdf:datatype="http://www.w3.org/2001/XMLSchema#boolean">true</isInISTQBGlossary>
        <rdfs:label>session-based testing</rdfs:label>
        <skos:altLabel xml:lang="en">session based testing
session-oriented testing
session oriented testing</skos:altLabel>
        <skos:prefLabel xml:lang="en">session-based testing</skos:prefLabel>
    </owl:Class>
    


    <!-- http://purl.org/stc/ontology#software -->

    <owl:Class rdf:about="http://purl.org/stc/ontology#software">
        <rdfs:subClassOf rdf:resource="http://purl.org/stc/ontology#software_engineering_concepts"/>
    </owl:Class>
    


    <!-- http://purl.org/stc/ontology#software_development_model -->

    <owl:Class rdf:about="http://purl.org/stc/ontology#software_development_model">
        <rdfs:subClassOf rdf:resource="http://purl.org/stc/ontology#software_engineering_concepts"/>
        <isInISTQBGlossary rdf:datatype="http://www.w3.org/2001/XMLSchema#boolean">false</isInISTQBGlossary>
        <rdfs:label>software development model</rdfs:label>
        <skos:prefLabel xml:lang="en">software development model</skos:prefLabel>
    </owl:Class>
    


    <!-- http://purl.org/stc/ontology#software_engineering -->

    <owl:Class rdf:about="http://purl.org/stc/ontology#software_engineering">
        <rdfs:subClassOf rdf:resource="http://purl.org/stc/ontology#basic_concepts"/>
        <isInISTQBGlossary rdf:datatype="http://www.w3.org/2001/XMLSchema#boolean">false</isInISTQBGlossary>
        <rdfs:comment xml:lang="en">The application of a systematic, disciplined, quantifiable approach to the development, operation, and maintenance of software; that is, the application of engineering to software. (IEEE 610.12-1990, ISO/IEC/IEEE 24765:2017)

A set of systematic processes for the acquisition, supply, development, operation, maintenance, and disposal of software products. (ISO/IEC 12207:2017)</rdfs:comment>
        <rdfs:label>software engineering</rdfs:label>
        <rdfs:seeAlso>ISO/IEC/IEEE 24765:2017 (Systems and Software Engineering – Vocabulary)
ISO/IEC 12207:2017 (Systems and software engineering — Software life cycle processes)
ISO/IEC 12207:2017 (Systems and software engineering — Software life cycle processes)</rdfs:seeAlso>
        <skos:altLabel xml:lang="en">se
software development</skos:altLabel>
        <skos:prefLabel xml:lang="en">software engineering</skos:prefLabel>
    </owl:Class>
    


    <!-- http://purl.org/stc/ontology#software_engineering_activity -->

    <owl:Class rdf:about="http://purl.org/stc/ontology#software_engineering_activity">
        <rdfs:subClassOf rdf:resource="http://purl.org/stc/ontology#software_engineering_concepts"/>
    </owl:Class>
    


    <!-- http://purl.org/stc/ontology#software_engineering_concepts -->

    <owl:Class rdf:about="http://purl.org/stc/ontology#software_engineering_concepts">
        <rdfs:subClassOf rdf:resource="http://purl.org/nemo/gufo#AbstractIndividualType"/>
        <rdfs:comment xml:lang="en">Selection of software engineering concepts that relate to software testing concepts.</rdfs:comment>
        <rdfs:label>software engineering concepts</rdfs:label>
        <skos:prefLabel xml:lang="en">software engineering concepts</skos:prefLabel>
    </owl:Class>
    


    <!-- http://purl.org/stc/ontology#software_lifecycle -->

    <owl:Class rdf:about="http://purl.org/stc/ontology#software_lifecycle">
        <rdfs:subClassOf rdf:resource="http://purl.org/stc/ontology#software_engineering_concepts"/>
    </owl:Class>
    


    <!-- http://purl.org/stc/ontology#software_testing_concepts -->

    <owl:Class rdf:about="http://purl.org/stc/ontology#software_testing_concepts">
        <rdfs:subClassOf rdf:resource="http://purl.org/nemo/gufo#AbstractIndividualType"/>
        <rdfs:comment xml:lang="en">Rather exhaustive collection of software testing concepts</rdfs:comment>
        <rdfs:label>software testing concepts</rdfs:label>
        <skos:prefLabel xml:lang="en">software testing concepts</skos:prefLabel>
    </owl:Class>
    


    <!-- http://purl.org/stc/ontology#specialist_tester -->

    <owl:Class rdf:about="http://purl.org/stc/ontology#specialist_tester">
        <rdfs:subClassOf rdf:resource="http://purl.org/stc/ontology#related_to_role"/>
        <isInISTQBGlossary rdf:datatype="http://www.w3.org/2001/XMLSchema#boolean">false</isInISTQBGlossary>
        <rdfs:comment xml:lang="en">Performs testing for specific quality characteristics, such as usability, accessibility,
security, performance. (ISO/IEC/IEEE 29119-1:2022)</rdfs:comment>
        <rdfs:label>specialist tester</rdfs:label>
        <rdfs:seeAlso>ISO/IEC/IEEE 29119-1:2022 (Software and systems engineering — Software testing — Part 1: Concepts and definitions)</rdfs:seeAlso>
        <skos:prefLabel xml:lang="en">specialist tester</skos:prefLabel>
    </owl:Class>
    


    <!-- http://purl.org/stc/ontology#specification_coverage -->

    <owl:Class rdf:about="http://purl.org/stc/ontology#specification_coverage">
        <rdfs:subClassOf rdf:resource="http://purl.org/stc/ontology#coverage"/>
        <isInISTQBGlossary rdf:datatype="http://www.w3.org/2001/XMLSchema#boolean">false</isInISTQBGlossary>
        <rdfs:comment xml:lang="en">There is currently no industry agreed approach to calculating experience-based coverage. (ISO/IEC/IEEE 29119-4)</rdfs:comment>
        <rdfs:label>specification coverage</rdfs:label>
        <rdfs:seeAlso>ISO/IEC/IEEE 29119-4 (Software and systems engineering — Software testing — Part 4: Test techniques)</rdfs:seeAlso>
        <skos:altLabel xml:lang="en">black-box test metric
black box test metric
specification-based test metric
specification based test metric</skos:altLabel>
        <skos:prefLabel xml:lang="en">specification coverage</skos:prefLabel>
    </owl:Class>
    


    <!-- http://purl.org/stc/ontology#state_transition_testing -->

    <owl:Class rdf:about="http://purl.org/stc/ontology#state_transition_testing">
        <rdfs:subClassOf rdf:resource="http://purl.org/stc/ontology#black_box_test_technique"/>
        <isInISTQBGlossary rdf:datatype="http://www.w3.org/2001/XMLSchema#boolean">true</isInISTQBGlossary>
        <rdfs:label>state transition testing</rdfs:label>
        <skos:prefLabel xml:lang="en">state transition testing</skos:prefLabel>
    </owl:Class>
    


    <!-- http://purl.org/stc/ontology#statement_coverage -->

    <owl:Class rdf:about="http://purl.org/stc/ontology#statement_coverage">
        <rdfs:subClassOf rdf:resource="http://purl.org/stc/ontology#structural_coverage"/>
        <isInISTQBGlossary rdf:datatype="http://www.w3.org/2001/XMLSchema#boolean">true</isInISTQBGlossary>
        <rdfs:comment xml:lang="en">The coverage of executable statements. (ISTQB Glossary v4.5)

Coverage for statement testing. (ISO/IEC/IEEE 29119-4)</rdfs:comment>
        <rdfs:label>statement coverage</rdfs:label>
        <rdfs:seeAlso>ISO/IEC/IEEE 29119-4 (Software and systems engineering — Software testing — Part 4: Test techniques)

Foundation - v4.0</rdfs:seeAlso>
        <skos:altLabel xml:lang="en">statement testing coverage</skos:altLabel>
        <skos:prefLabel xml:lang="en">statement coverage</skos:prefLabel>
    </owl:Class>
    


    <!-- http://purl.org/stc/ontology#statement_testing -->

    <owl:Class rdf:about="http://purl.org/stc/ontology#statement_testing">
        <rdfs:subClassOf rdf:resource="http://purl.org/stc/ontology#white_box_test_technique"/>
        <isInISTQBGlossary rdf:datatype="http://www.w3.org/2001/XMLSchema#boolean">true</isInISTQBGlossary>
        <rdfs:label>statement testing</rdfs:label>
        <skos:prefLabel xml:lang="en">statement testing</skos:prefLabel>
    </owl:Class>
    


    <!-- http://purl.org/stc/ontology#static_analysis -->

    <owl:Class rdf:about="http://purl.org/stc/ontology#static_analysis">
        <rdfs:subClassOf rdf:resource="http://purl.org/stc/ontology#static_testing"/>
        <isInISTQBGlossary rdf:datatype="http://www.w3.org/2001/XMLSchema#boolean">true</isInISTQBGlossary>
        <rdfs:comment xml:lang="en">The process of evaluating a component or system without executing it, based on its form, structure, content, or documentation. (ISTQB Glossary v4.5)</rdfs:comment>
        <rdfs:label>static analysis</rdfs:label>
        <rdfs:seeAlso>Foundation - v4.0
Advanced Technical Test Analyst - v4.0
Advanced Test Automation Engineering - v2.0</rdfs:seeAlso>
        <skos:prefLabel xml:lang="en">static analysis</skos:prefLabel>
    </owl:Class>
    


    <!-- http://purl.org/stc/ontology#static_application_security_testing -->

    <owl:Class rdf:about="http://purl.org/stc/ontology#static_application_security_testing">
        <rdfs:subClassOf rdf:resource="http://purl.org/stc/ontology#security_testing"/>
        <isInISTQBGlossary rdf:datatype="http://www.w3.org/2001/XMLSchema#boolean">true</isInISTQBGlossary>
        <rdfs:label>static application security testing</rdfs:label>
        <skos:prefLabel xml:lang="en">static application security testing</skos:prefLabel>
    </owl:Class>
    


    <!-- http://purl.org/stc/ontology#static_testing -->

    <owl:Class rdf:about="http://purl.org/stc/ontology#static_testing">
        <rdfs:subClassOf rdf:resource="http://purl.org/stc/ontology#testing"/>
        <isInISTQBGlossary rdf:datatype="http://www.w3.org/2001/XMLSchema#boolean">true</isInISTQBGlossary>
        <rdfs:comment xml:lang="en">Testing that does not involve the execution of a test item. (ISTQB Glossary v4.5)

Testing in which a test item is examined against a set of quality or other criteria without the test item being executed. (ISO/IEC/IEEE 29119-1:2022)</rdfs:comment>
        <rdfs:label>static testing</rdfs:label>
        <rdfs:seeAlso>ISO/IEC/IEEE 29119-1:2022 (Software and systems engineering — Software testing — Part 1: Concepts and definitions)

Foundation - v4.0</rdfs:seeAlso>
        <skos:prefLabel xml:lang="en">static testing</skos:prefLabel>
    </owl:Class>
    


    <!-- http://purl.org/stc/ontology#stress_testing -->

    <owl:Class rdf:about="http://purl.org/stc/ontology#stress_testing">
        <rdfs:subClassOf rdf:resource="http://purl.org/stc/ontology#performance_testing"/>
        <isInISTQBGlossary rdf:datatype="http://www.w3.org/2001/XMLSchema#boolean">true</isInISTQBGlossary>
        <rdfs:label>stress testing</rdfs:label>
        <skos:prefLabel xml:lang="en">stress testing</skos:prefLabel>
    </owl:Class>
    


    <!-- http://purl.org/stc/ontology#structural_coverage -->

    <owl:Class rdf:about="http://purl.org/stc/ontology#structural_coverage">
        <rdfs:subClassOf rdf:resource="http://purl.org/stc/ontology#coverage"/>
        <isInISTQBGlossary rdf:datatype="http://www.w3.org/2001/XMLSchema#boolean">true</isInISTQBGlossary>
        <rdfs:comment xml:lang="en">Coverage measures based on the internal structure of a component or system. (ISTQB Glossary v4.5)</rdfs:comment>
        <rdfs:label>structural coverage</rdfs:label>
        <rdfs:seeAlso>ISO/IEC/IEEE 29119-4 (Software and systems engineering — Software testing — Part 4: Test techniques)</rdfs:seeAlso>
        <skos:altLabel xml:lang="en">white box test metric
white-box test metric
structure-based test metric
structure based test metric</skos:altLabel>
        <skos:prefLabel xml:lang="en">structural coverage</skos:prefLabel>
    </owl:Class>
    


    <!-- http://purl.org/stc/ontology#support_processes -->

    <owl:Class rdf:about="http://purl.org/stc/ontology#support_processes">
        <rdfs:subClassOf rdf:resource="http://purl.org/stc/ontology#software_lifecycle"/>
    </owl:Class>
    


    <!-- http://purl.org/stc/ontology#system_integration_testing -->

    <owl:Class rdf:about="http://purl.org/stc/ontology#system_integration_testing">
        <rdfs:subClassOf rdf:resource="http://purl.org/stc/ontology#integration_testing"/>
        <isInISTQBGlossary rdf:datatype="http://www.w3.org/2001/XMLSchema#boolean">true</isInISTQBGlossary>
        <rdfs:comment xml:lang="en">The integration testing of systems. (ISTQB Glossary v4.5)</rdfs:comment>
        <rdfs:label>system integration testing</rdfs:label>
        <rdfs:seeAlso>Foundation - v4.0</rdfs:seeAlso>
        <skos:prefLabel xml:lang="en">system integration testing</skos:prefLabel>
    </owl:Class>
    


    <!-- http://purl.org/stc/ontology#system_testing -->

    <owl:Class rdf:about="http://purl.org/stc/ontology#system_testing">
        <rdfs:subClassOf rdf:resource="http://purl.org/stc/ontology#test_level"/>
        <isInISTQBGlossary rdf:datatype="http://www.w3.org/2001/XMLSchema#boolean">true</isInISTQBGlossary>
        <rdfs:label>system testing</rdfs:label>
        <skos:prefLabel xml:lang="en">system testing</skos:prefLabel>
    </owl:Class>
    


    <!-- http://purl.org/stc/ontology#target_orientation_in_software_development -->

    <owl:Class rdf:about="http://purl.org/stc/ontology#target_orientation_in_software_development">
        <rdfs:subClassOf rdf:resource="http://purl.org/stc/ontology#software_development_model"/>
        <isInISTQBGlossary rdf:datatype="http://www.w3.org/2001/XMLSchema#boolean">false</isInISTQBGlossary>
        <rdfs:label>target orientation</rdfs:label>
        <skos:prefLabel xml:lang="en">target orientation in software development</skos:prefLabel>
    </owl:Class>
    


    <!-- http://purl.org/stc/ontology#target_orientation_in_test_approach -->

    <owl:Class rdf:about="http://purl.org/stc/ontology#target_orientation_in_test_approach">
        <rdfs:subClassOf rdf:resource="http://purl.org/stc/ontology#test_approach"/>
        <isInISTQBGlossary rdf:datatype="http://www.w3.org/2001/XMLSchema#boolean">false</isInISTQBGlossary>
        <rdfs:label>target orientation</rdfs:label>
        <skos:prefLabel xml:lang="en">target orientation in test approach</skos:prefLabel>
    </owl:Class>
    


    <!-- http://purl.org/stc/ontology#technical_review -->

    <owl:Class rdf:about="http://purl.org/stc/ontology#technical_review">
        <rdfs:subClassOf rdf:resource="http://purl.org/stc/ontology#formal_review"/>
        <isInISTQBGlossary rdf:datatype="http://www.w3.org/2001/XMLSchema#boolean">true</isInISTQBGlossary>
        <rdfs:comment xml:lang="en">A formal review by technical experts that examine the quality of a work product and identify discrepancies from specifications and standards. (ISTQB Glossary v4.5)</rdfs:comment>
        <rdfs:label>technical review</rdfs:label>
        <rdfs:seeAlso>Foundation - v4.0
Advanced Test Manager - 2012
Advanced Technical Test Analyst - v4.0</rdfs:seeAlso>
        <skos:prefLabel xml:lang="en">technical review</skos:prefLabel>
    </owl:Class>
    


    <!-- http://purl.org/stc/ontology#test_activity -->

    <owl:Class rdf:about="http://purl.org/stc/ontology#test_activity">
        <rdfs:subClassOf rdf:resource="http://purl.org/stc/ontology#software_engineering_activity"/>
        <rdfs:subClassOf rdf:resource="http://purl.org/stc/ontology#software_testing_concepts"/>
        <isInISTQBGlossary rdf:datatype="http://www.w3.org/2001/XMLSchema#boolean">false</isInISTQBGlossary>
        <rdfs:label>test activity</rdfs:label>
        <skos:prefLabel xml:lang="en">test activity</skos:prefLabel>
    </owl:Class>
    


    <!-- http://purl.org/stc/ontology#test_analysis -->

    <owl:Class rdf:about="http://purl.org/stc/ontology#test_analysis">
        <rdfs:subClassOf rdf:resource="http://purl.org/stc/ontology#test_activity"/>
        <isInISTQBGlossary rdf:datatype="http://www.w3.org/2001/XMLSchema#boolean">true</isInISTQBGlossary>
        <rdfs:comment xml:lang="en">The activity that identifies test conditions by analyzing the test basis. (ISTQB Glossary v4.5)</rdfs:comment>
        <rdfs:label>test analysis</rdfs:label>
        <rdfs:seeAlso>Foundation - v4.0
Advanced Test Analyst - v3.1
Advanced Test Analyst - v4.0</rdfs:seeAlso>
        <skos:prefLabel xml:lang="en">test analysis</skos:prefLabel>
    </owl:Class>
    


    <!-- http://purl.org/stc/ontology#test_analyst -->

    <owl:Class rdf:about="http://purl.org/stc/ontology#test_analyst">
        <rdfs:subClassOf rdf:resource="http://purl.org/stc/ontology#related_to_role"/>
        <isInISTQBGlossary rdf:datatype="http://www.w3.org/2001/XMLSchema#boolean">false</isInISTQBGlossary>
        <rdfs:comment xml:lang="en">Develops oracles and/or analyses test results for correctness and issues.  (ISO/IEC/IEEE 29119-1:2022)</rdfs:comment>
        <rdfs:label>test analyst</rdfs:label>
        <rdfs:seeAlso>ISO/IEC/IEEE 29119-1:2022 (Software and systems engineering — Software testing — Part 1: Concepts and definitions)</rdfs:seeAlso>
        <skos:altLabel xml:lang="en">TA</skos:altLabel>
        <skos:prefLabel xml:lang="en">test analyst</skos:prefLabel>
    </owl:Class>
    


    <!-- http://purl.org/stc/ontology#test_approach -->

    <owl:Class rdf:about="http://purl.org/stc/ontology#test_approach">
        <rdfs:subClassOf rdf:resource="http://purl.org/stc/ontology#software_testing_concepts"/>
        <isInISTQBGlossary rdf:datatype="http://www.w3.org/2001/XMLSchema#boolean">true</isInISTQBGlossary>
        <rdfs:comment xml:lang="en">The manner of implementing testing tasks. (ISTQB Glossary v4.5)</rdfs:comment>
        <rdfs:label>test approach</rdfs:label>
        <rdfs:seeAlso>Foundation - v4.0
Advanced Test Manager - 2012</rdfs:seeAlso>
        <skos:prefLabel xml:lang="en">test approach</skos:prefLabel>
    </owl:Class>
    


    <!-- http://purl.org/stc/ontology#test_architect -->

    <owl:Class rdf:about="http://purl.org/stc/ontology#test_architect">
        <rdfs:subClassOf rdf:resource="http://purl.org/stc/ontology#related_to_role"/>
        <isInISTQBGlossary rdf:datatype="http://www.w3.org/2001/XMLSchema#boolean">false</isInISTQBGlossary>
        <rdfs:comment xml:lang="en">Defines the test strategy, test environment and test plan for programmes and projects. Specifies the organizational test requirements and helps ensure conformance to these requirements. (ISO/IEC/IEEE 29119-1:2022)</rdfs:comment>
        <rdfs:label>test architect</rdfs:label>
        <rdfs:seeAlso>ISO/IEC/IEEE 29119-1:2022 (Software and systems engineering — Software testing — Part 1: Concepts and definitions)</rdfs:seeAlso>
        <skos:prefLabel xml:lang="en">test architect</skos:prefLabel>
    </owl:Class>
    


    <!-- http://purl.org/stc/ontology#test_automation -->

    <owl:Class rdf:about="http://purl.org/stc/ontology#test_automation">
        <rdfs:subClassOf rdf:resource="http://purl.org/stc/ontology#test_activity"/>
        <isInISTQBGlossary rdf:datatype="http://www.w3.org/2001/XMLSchema#boolean">true</isInISTQBGlossary>
        <rdfs:comment xml:lang="en">The conversion of test activities to automatic operation. (ISTQB Glossary v4.5)</rdfs:comment>
        <rdfs:label>test automation</rdfs:label>
        <rdfs:seeAlso>Advanced Test Automation Engineering - v2.0
Specialist - Test Automation Engineer - 2016</rdfs:seeAlso>
        <skos:prefLabel xml:lang="en">test automation</skos:prefLabel>
    </owl:Class>
    


    <!-- http://purl.org/stc/ontology#test_automation_engineer -->

    <owl:Class rdf:about="http://purl.org/stc/ontology#test_automation_engineer">
        <rdfs:subClassOf rdf:resource="http://purl.org/stc/ontology#related_to_role"/>
        <isInISTQBGlossary rdf:datatype="http://www.w3.org/2001/XMLSchema#boolean">false</isInISTQBGlossary>
        <rdfs:comment xml:lang="en">Implements tests cases/scripts within a test automation framework. (ISO/IEC/IEEE 29119-1:2022)</rdfs:comment>
        <rdfs:label>test automation engineer</rdfs:label>
        <rdfs:seeAlso>ISO/IEC/IEEE 29119-1:2022 (Software and systems engineering — Software testing — Part 1: Concepts and definitions)</rdfs:seeAlso>
        <skos:altLabel xml:lang="en">TAE
test automator</skos:altLabel>
        <skos:prefLabel xml:lang="en">test automation engineer</skos:prefLabel>
    </owl:Class>
    


    <!-- http://purl.org/stc/ontology#test_basis -->

    <owl:Class rdf:about="http://purl.org/stc/ontology#test_basis">
        <rdfs:subClassOf rdf:resource="http://purl.org/stc/ontology#Testware"/>
        <isInISTQBGlossary rdf:datatype="http://www.w3.org/2001/XMLSchema#boolean">true</isInISTQBGlossary>
        <rdfs:comment xml:lang="en">The body of knowledge used as the basis for test analysis and test design. (ISTQB Glossary v4.5)

Information used as the basis for designing and implementing test cases. (ISO/IEC/IEEE 29119-1:2022)</rdfs:comment>
        <rdfs:label>test basis</rdfs:label>
        <rdfs:seeAlso>ISO/IEC/IEEE 29119-1 (2022) Software and systems engineering -- Software testing -- Part 1: Concepts and definitions

Foundation - v4.0
Advanced Test Analyst - v3.1</rdfs:seeAlso>
        <skos:prefLabel xml:lang="en">test basis</skos:prefLabel>
    </owl:Class>
    


    <!-- http://purl.org/stc/ontology#test_case -->

    <owl:Class rdf:about="http://purl.org/stc/ontology#test_case">
        <rdfs:subClassOf rdf:resource="http://purl.org/stc/ontology#Testware"/>
        <isInISTQBGlossary rdf:datatype="http://www.w3.org/2001/XMLSchema#boolean">true</isInISTQBGlossary>
        <rdfs:comment xml:lang="en">A set of preconditions, inputs, actions (where applicable), expected results and postconditions, developed based on test conditions. (ISTQB Glossary v4.5)

Set of preconditions, inputs and expected results, developed to drive the execution of a test item to meet test objectives. (ISO/IEC/IEEE 29119-1:2022)</rdfs:comment>
        <rdfs:label>test case</rdfs:label>
        <rdfs:seeAlso>ISO/IEC/IEEE 29119-1 (2022) Software and systems engineering -- Software testing -- Part 1: Concepts and definitions

Foundation - v4.0
Advanced Test Manager - 2012
Advanced Test Management - v3.0
Advanced Test Analyst - v4.0
Specialist - Acceptance Testing - 2019</rdfs:seeAlso>
        <skos:altLabel xml:lang="en">testcase</skos:altLabel>
        <skos:prefLabel xml:lang="en">test case</skos:prefLabel>
    </owl:Class>
    


    <!-- http://purl.org/stc/ontology#test_completion -->

    <owl:Class rdf:about="http://purl.org/stc/ontology#test_completion">
        <rdfs:subClassOf rdf:resource="http://purl.org/stc/ontology#test_activity"/>
        <isInISTQBGlossary rdf:datatype="http://www.w3.org/2001/XMLSchema#boolean">true</isInISTQBGlossary>
        <rdfs:comment xml:lang="en">The activity that makes testware available for later use, leaves test environments in a satisfactory condition and communicates the results of testing to relevant stakeholders. (ISTQB Glossary v4.5)</rdfs:comment>
        <rdfs:label>test completion</rdfs:label>
        <rdfs:seeAlso>Foundation - v4.0
Advanced Test Management - v3.0</rdfs:seeAlso>
        <skos:prefLabel xml:lang="en">test completion</skos:prefLabel>
    </owl:Class>
    


    <!-- http://purl.org/stc/ontology#test_completion_report -->

    <owl:Class rdf:about="http://purl.org/stc/ontology#test_completion_report">
        <rdfs:subClassOf rdf:resource="http://purl.org/stc/ontology#test_report"/>
        <isInISTQBGlossary rdf:datatype="http://www.w3.org/2001/XMLSchema#boolean">true</isInISTQBGlossary>
        <rdfs:comment xml:lang="en">A type of test report produced at completion milestones that provides an evaluation of the corresponding test items against exit criteria. (ISTQB Glossary v4.5)

Report that provides a summary of the testing that was performed. (ISO/IEC/IEEE 29119-1:2022)</rdfs:comment>
        <rdfs:label>test completion report</rdfs:label>
        <rdfs:seeAlso>ISO/IEC/IEEE 29119-1:2022 (Software and systems engineering — Software testing — Part 1: Concepts and definitions)

Foundation - v4.0
Advanced Test Manager - 2012</rdfs:seeAlso>
        <skos:altLabel xml:lang="en">test summary report</skos:altLabel>
        <skos:prefLabel xml:lang="en">test completion report</skos:prefLabel>
    </owl:Class>
    


    <!-- http://purl.org/stc/ontology#test_condition -->

    <owl:Class rdf:about="http://purl.org/stc/ontology#test_condition">
        <rdfs:subClassOf rdf:resource="http://purl.org/stc/ontology#Testware"/>
        <isInISTQBGlossary rdf:datatype="http://www.w3.org/2001/XMLSchema#boolean">true</isInISTQBGlossary>
        <rdfs:comment xml:lang="en">A testable aspect of a component or system identified as a basis for testing. (ISTQB Glossary v4.5)

Testable aspect of a component or system, such as a function, transaction, feature, quality attribute, or structural element identified as a basis for testing. (ISO/IEC/IEEE 29119-1:2022)</rdfs:comment>
        <rdfs:label>test condition</rdfs:label>
        <rdfs:seeAlso>ISO/IEC/IEEE 29119-1:2022 (Software and systems engineering — Software testing — Part 1: Concepts and definitions)

Foundation - v4.0
Advanced Test Manager - 2012
Advanced Test Analyst - v3.1
Advanced Test Analyst - v4.0
Specialist - Test Automation Strategy - v1.0</rdfs:seeAlso>
        <skos:altLabel xml:lang="en">test situation
test requirement</skos:altLabel>
        <skos:prefLabel xml:lang="en">test condition</skos:prefLabel>
    </owl:Class>
    


    <!-- http://purl.org/stc/ontology#test_control -->

    <owl:Class rdf:about="http://purl.org/stc/ontology#test_control">
        <rdfs:subClassOf rdf:resource="http://purl.org/stc/ontology#test_activity"/>
        <isInISTQBGlossary rdf:datatype="http://www.w3.org/2001/XMLSchema#boolean">true</isInISTQBGlossary>
        <rdfs:comment xml:lang="en">The activity that develops and applies corrective actions to get a test project on track when it deviates from what was planned. (ISTQB Glossary v4.5)</rdfs:comment>
        <rdfs:label>test control</rdfs:label>
        <rdfs:seeAlso>Foundation - v4.0
Advanced Test Manager - 2012
Advanced Test Management - v3.0</rdfs:seeAlso>
        <skos:prefLabel xml:lang="en">test control</skos:prefLabel>
    </owl:Class>
    


    <!-- http://purl.org/stc/ontology#test_data -->

    <owl:Class rdf:about="http://purl.org/stc/ontology#test_data">
        <rdfs:subClassOf rdf:resource="http://purl.org/stc/ontology#Testware"/>
        <isInISTQBGlossary rdf:datatype="http://www.w3.org/2001/XMLSchema#boolean">true</isInISTQBGlossary>
        <rdfs:comment xml:lang="en">Data needed for test execution. (ISTQB Glossary v4.5)

Data created or selected to satisfy the input requirements for executing one or more test cases, which may be defined in the test plan, test case or test procedure. (ISO/IEC/IEEE 29119-1:2022)</rdfs:comment>
        <rdfs:label>test data</rdfs:label>
        <rdfs:seeAlso>ISO/IEC/IEEE 29119-1:2022 (Software and systems engineering — Software testing — Part 1: Concepts and definitions)

Foundation - v4.0
Advanced Test Analyst - v3.1
Advanced Test Analyst - v4.0</rdfs:seeAlso>
        <skos:altLabel xml:lang="en">testdata
test data set
testdata set</skos:altLabel>
        <skos:prefLabel xml:lang="en">test data</skos:prefLabel>
    </owl:Class>
    


    <!-- http://purl.org/stc/ontology#test_design -->

    <owl:Class rdf:about="http://purl.org/stc/ontology#test_design">
        <rdfs:subClassOf rdf:resource="http://purl.org/stc/ontology#test_activity"/>
        <isInISTQBGlossary rdf:datatype="http://www.w3.org/2001/XMLSchema#boolean">true</isInISTQBGlossary>
        <rdfs:comment xml:lang="en">The activity that derives and specifies test cases from test conditions. (ISTQB Glossary v4.5)</rdfs:comment>
        <rdfs:label>test design</rdfs:label>
        <rdfs:seeAlso>Foundation - v4.0
Advanced Test Manager - 2012
Advanced Test Analyst - v3.1
Advanced Test Analyst - v4.0</rdfs:seeAlso>
        <skos:prefLabel xml:lang="en">test design</skos:prefLabel>
    </owl:Class>
    


    <!-- http://purl.org/stc/ontology#test_designer -->

    <owl:Class rdf:about="http://purl.org/stc/ontology#test_designer">
        <rdfs:subClassOf rdf:resource="http://purl.org/stc/ontology#related_to_role"/>
        <isInISTQBGlossary rdf:datatype="http://www.w3.org/2001/XMLSchema#boolean">false</isInISTQBGlossary>
        <rdfs:comment xml:lang="en">Develops the test design artefacts. (ISO/IEC/IEEE 29119-1:2022)</rdfs:comment>
        <rdfs:label>test designer</rdfs:label>
        <rdfs:seeAlso>ISO/IEC/IEEE 29119-1:2022 (Software and systems engineering — Software testing — Part 1: Concepts and definitions)</rdfs:seeAlso>
        <skos:prefLabel xml:lang="en">test designer</skos:prefLabel>
    </owl:Class>
    


    <!-- http://purl.org/stc/ontology#test_director -->

    <owl:Class rdf:about="http://purl.org/stc/ontology#test_director">
        <rdfs:subClassOf rdf:resource="http://purl.org/stc/ontology#related_to_role"/>
        <isInISTQBGlossary rdf:datatype="http://www.w3.org/2001/XMLSchema#boolean">true</isInISTQBGlossary>
        <rdfs:comment xml:lang="en">A senior manager who manages test managers.</rdfs:comment>
        <rdfs:label>test director</rdfs:label>
        <rdfs:seeAlso>Advanced Test Manager - 2012</rdfs:seeAlso>
        <skos:prefLabel xml:lang="en">test director</skos:prefLabel>
    </owl:Class>
    


    <!-- http://purl.org/stc/ontology#test_driven_development -->

    <owl:Class rdf:about="http://purl.org/stc/ontology#test_driven_development">
        <rdfs:subClassOf rdf:resource="http://purl.org/stc/ontology#target_orientation_in_software_development"/>
        <isInISTQBGlossary rdf:datatype="http://www.w3.org/2001/XMLSchema#boolean">true</isInISTQBGlossary>
        <rdfs:comment xml:lang="en">A software development technique in which the test cases are developed, automated and then the software is developed incrementally to pass those test cases. (ISTQB Glossary v4.5)</rdfs:comment>
        <rdfs:label>test-driven</rdfs:label>
        <rdfs:seeAlso>Foundation - v4.0
Advanced Test Manager - 2012
Advanced Test Management - v3.0
Advanced Test Automation Engineering - v2.0
Advanced Agile Technical Tester - 2019
Specialist - Agile Test Leadership at Scale - v2.0
Specialist - Test Automation Strategy - v1.0</rdfs:seeAlso>
        <skos:altLabel xml:lang="en">test driven development
tdd
TDD</skos:altLabel>
        <skos:prefLabel xml:lang="en">test-driven development</skos:prefLabel>
    </owl:Class>
    


    <!-- http://purl.org/stc/ontology#test_execution -->

    <owl:Class rdf:about="http://purl.org/stc/ontology#test_execution">
        <rdfs:subClassOf rdf:resource="http://purl.org/stc/ontology#test_activity"/>
        <isInISTQBGlossary rdf:datatype="http://www.w3.org/2001/XMLSchema#boolean">true</isInISTQBGlossary>
        <rdfs:comment xml:lang="en">The activity that runs a test on a component or system producing actual results. (ISTQB Glossary v4.5)</rdfs:comment>
        <rdfs:label>test execution</rdfs:label>
        <rdfs:seeAlso>Foundation - v4.0
Advanced Test Manager - 2012
Advanced Test Analyst - v3.1
Advanced Test Analyst - v4.0
Advanced Technical Test Analyst - v4.0</rdfs:seeAlso>
        <skos:prefLabel xml:lang="en">test execution</skos:prefLabel>
    </owl:Class>
    


    <!-- http://purl.org/stc/ontology#test_first_approach -->

    <owl:Class rdf:about="http://purl.org/stc/ontology#test_first_approach">
        <rdfs:subClassOf rdf:resource="http://purl.org/stc/ontology#test_driven_development"/>
        <isInISTQBGlossary rdf:datatype="http://www.w3.org/2001/XMLSchema#boolean">true</isInISTQBGlossary>
        <rdfs:comment xml:lang="en">An approach to software development in which the test cases are designed and implemented before the associated component or system is developed. (ISTQB Glossary v4.5)</rdfs:comment>
        <rdfs:label>test-first approach</rdfs:label>
        <rdfs:seeAlso>Foundation - v4.0
Advanced Test Analyst - v3.1
Foundation Agile Tester - 2014
Specialist - Agile Test Leadership at Scale - v2.0</rdfs:seeAlso>
        <skos:altLabel xml:lang="en">test first approach</skos:altLabel>
        <skos:prefLabel xml:lang="en">test-first approach</skos:prefLabel>
    </owl:Class>
    


    <!-- http://purl.org/stc/ontology#test_implementation -->

    <owl:Class rdf:about="http://purl.org/stc/ontology#test_implementation">
        <rdfs:subClassOf rdf:resource="http://purl.org/stc/ontology#test_activity"/>
        <isInISTQBGlossary rdf:datatype="http://www.w3.org/2001/XMLSchema#boolean">true</isInISTQBGlossary>
        <rdfs:comment xml:lang="en">The activity that prepares the testware needed for test execution based on test analysis and design. (ISTQB Glossary v4.5)</rdfs:comment>
        <rdfs:label>test implementation</rdfs:label>
        <rdfs:seeAlso>Foundation - v4.0
Advanced Test Manager - 2012
Advanced Test Analyst - v3.1
Advanced Test Analyst - v4.0</rdfs:seeAlso>
        <skos:prefLabel xml:lang="en">test implementation</skos:prefLabel>
    </owl:Class>
    


    <!-- http://purl.org/stc/ontology#test_item -->

    <owl:Class rdf:about="http://purl.org/stc/ontology#test_item">
        <rdfs:subClassOf rdf:resource="http://purl.org/stc/ontology#Testware"/>
        <isInISTQBGlossary rdf:datatype="http://www.w3.org/2001/XMLSchema#boolean">true</isInISTQBGlossary>
        <rdfs:comment xml:lang="en">A part of a test object used in the test process. (ISTQB Glossary v4.5)</rdfs:comment>
        <rdfs:comment xml:lang="en">ISO/IEC/IEEE 29119-1:2022 defines the term test item differently: as a synonym to test object.</rdfs:comment>
        <rdfs:label>test item</rdfs:label>
        <skos:prefLabel xml:lang="en">test item</skos:prefLabel>
    </owl:Class>
    


    <!-- http://purl.org/stc/ontology#test_leader -->

    <owl:Class rdf:about="http://purl.org/stc/ontology#test_leader">
        <rdfs:subClassOf rdf:resource="http://purl.org/stc/ontology#related_to_role"/>
        <isInISTQBGlossary rdf:datatype="http://www.w3.org/2001/XMLSchema#boolean">true</isInISTQBGlossary>
        <rdfs:comment xml:lang="en">On large projects, the person who reports to the test manager and is responsible for project management of a particular test level or a particular set of testing activities. (ISTQB Glossary v4.5)</rdfs:comment>
        <rdfs:label>test leader</rdfs:label>
        <rdfs:seeAlso>Advanced Test Manager - 2012</rdfs:seeAlso>
        <skos:altLabel xml:lang="en">lead tester</skos:altLabel>
        <skos:prefLabel xml:lang="en">test leader</skos:prefLabel>
    </owl:Class>
    


    <!-- http://purl.org/stc/ontology#test_level -->

    <owl:Class rdf:about="http://purl.org/stc/ontology#test_level">
        <rdfs:subClassOf rdf:resource="http://purl.org/stc/ontology#software_testing_concepts"/>
        <isInISTQBGlossary rdf:datatype="http://www.w3.org/2001/XMLSchema#boolean">true</isInISTQBGlossary>
        <rdfs:comment xml:lang="en">A specific instantiation of a test process. (ISTQB Glossary v4.5)

One of a sequence of test stages each of which is typically associated with the achievement of particular
objectives and used to treat particular risks. (ISO/IEC/IEEE 29119-1:2022)</rdfs:comment>
        <rdfs:label>test level</rdfs:label>
        <rdfs:seeAlso>ISO/IEC/IEEE 29119-1:2022 (Software and systems engineering — Software testing — Part 1: Concepts and definitions)

Foundation - v4.0
Advanced Test Manager - 2012
Advanced Test Management - v3.0
Specialist - Mobile Application Testing - 2019
Specialist - Test Automation Strategy - v1.0</rdfs:seeAlso>
        <skos:altLabel xml:lang="en">test stage
test phase</skos:altLabel>
        <skos:prefLabel xml:lang="en">test level</skos:prefLabel>
    </owl:Class>
    


    <!-- http://purl.org/stc/ontology#test_management -->

    <owl:Class rdf:about="http://purl.org/stc/ontology#test_management">
        <rdfs:subClassOf rdf:resource="http://purl.org/stc/ontology#software_testing_concepts"/>
        <rdfs:subClassOf rdf:resource="http://purl.org/stc/ontology#test_activity"/>
        <isInISTQBGlossary rdf:datatype="http://www.w3.org/2001/XMLSchema#boolean">true</isInISTQBGlossary>
        <rdfs:comment xml:lang="en">The process of planning, scheduling, estimating, monitoring, reporting, controlling, and completing test activities. (ISTQB Glossary v4.5)</rdfs:comment>
        <rdfs:label>test management</rdfs:label>
        <skos:prefLabel xml:lang="en">test management</skos:prefLabel>
    </owl:Class>
    


    <!-- http://purl.org/stc/ontology#test_manager -->

    <owl:Class rdf:about="http://purl.org/stc/ontology#test_manager">
        <rdfs:subClassOf rdf:resource="http://purl.org/stc/ontology#related_to_role"/>
        <isInISTQBGlossary rdf:datatype="http://www.w3.org/2001/XMLSchema#boolean">true</isInISTQBGlossary>
        <rdfs:comment xml:lang="en">The person responsible for project management of testing activities, resources, and evaluation of a test object. (ISTQB Glossary v4.5)

Develops, manages, and helps to ensure conformance with the test management process. The test manager also plans and controls the dynamic test process. (ISO/IEC/IEEE 29119-1:2022)</rdfs:comment>
        <rdfs:label>test manager</rdfs:label>
        <rdfs:seeAlso>ISO/IEC/IEEE 29119-1:2022 (Software and systems engineering — Software testing — Part 1: Concepts and definitions)

Advanced Test Manager - 2012</rdfs:seeAlso>
        <skos:prefLabel xml:lang="en">test manager</skos:prefLabel>
    </owl:Class>
    


    <!-- http://purl.org/stc/ontology#test_metric -->

    <owl:Class rdf:about="http://purl.org/stc/ontology#test_metric">
        <rdfs:subClassOf rdf:resource="http://purl.org/stc/ontology#metric"/>
        <rdfs:subClassOf rdf:resource="http://purl.org/stc/ontology#software_testing_concepts"/>
        <isInISTQBGlossary rdf:datatype="http://www.w3.org/2001/XMLSchema#boolean">false</isInISTQBGlossary>
        <rdfs:comment xml:lang="en">A measurement of a characteristic of a test process, test activity, test object or testware. (own)</rdfs:comment>
        <rdfs:label>test metric</rdfs:label>
        <rdfs:seeAlso>ISO/IEC/IEEE 29119-4 (Software and systems engineering — Software testing — Part 4: Test techniques)</rdfs:seeAlso>
        <skos:altLabel xml:lang="en">testmetric</skos:altLabel>
        <skos:prefLabel xml:lang="en">test metric</skos:prefLabel>
    </owl:Class>
    


    <!-- http://purl.org/stc/ontology#test_model -->

    <owl:Class rdf:about="http://purl.org/stc/ontology#test_model">
        <rdfs:subClassOf rdf:resource="http://purl.org/stc/ontology#Testware"/>
        <isInISTQBGlossary rdf:datatype="http://www.w3.org/2001/XMLSchema#boolean">true</isInISTQBGlossary>
        <rdfs:comment xml:lang="en">A model describing testware that is used for testing a component or a system under test. (ISTQB Glossary v4.5)

Representation of the test item, which allows the testing to be focused on particular
characteristics or qualities. (ISO/IEC/IEEE 29119-1:2022)</rdfs:comment>
        <rdfs:label>test model</rdfs:label>
        <rdfs:seeAlso>ISO/IEC/IEEE 29119-1:2022 (Software and systems engineering — Software testing — Part 1: Concepts and definitions)

Specialist - Model-Based Tester - 2015
Specialist - Model-Based Testing - v1.1</rdfs:seeAlso>
        <skos:altLabel>test specification</skos:altLabel>
        <skos:prefLabel xml:lang="en">test model</skos:prefLabel>
    </owl:Class>
    


    <!-- http://purl.org/stc/ontology#test_monitoring -->

    <owl:Class rdf:about="http://purl.org/stc/ontology#test_monitoring">
        <rdfs:subClassOf rdf:resource="http://purl.org/stc/ontology#test_activity"/>
        <isInISTQBGlossary rdf:datatype="http://www.w3.org/2001/XMLSchema#boolean">true</isInISTQBGlossary>
        <rdfs:comment xml:lang="en">The activity that checks the status of testing activities, identifies any variances from planned or expected, and reports status to stakeholders. (ISTQB Glossary v4.5)</rdfs:comment>
        <rdfs:label>test monitoring</rdfs:label>
        <rdfs:seeAlso>Foundation - v4.0
Advanced Test Manager - 2012
Advanced Test Management - v3.0</rdfs:seeAlso>
        <skos:prefLabel xml:lang="en">test monitoring</skos:prefLabel>
    </owl:Class>
    


    <!-- http://purl.org/stc/ontology#test_object -->

    <owl:Class rdf:about="http://purl.org/stc/ontology#test_object">
        <rdfs:subClassOf rdf:resource="http://purl.org/stc/ontology#software"/>
        <isInISTQBGlossary rdf:datatype="http://www.w3.org/2001/XMLSchema#boolean">true</isInISTQBGlossary>
        <rdfs:comment xml:lang="en">The work product to be tested. (ISTQB Glossary v4.5)</rdfs:comment>
        <rdfs:label>test object</rdfs:label>
        <rdfs:seeAlso>Foundation - v4.0</rdfs:seeAlso>
        <skos:altLabel xml:lang="en">test target
system under test
sut
SUT
object under test</skos:altLabel>
        <skos:prefLabel xml:lang="en">test object</skos:prefLabel>
    </owl:Class>
    


    <!-- http://purl.org/stc/ontology#test_objective -->

    <owl:Class rdf:about="http://purl.org/stc/ontology#test_objective">
        <rdfs:subClassOf rdf:resource="http://purl.org/stc/ontology#Testware"/>
        <isInISTQBGlossary rdf:datatype="http://www.w3.org/2001/XMLSchema#boolean">true</isInISTQBGlossary>
        <rdfs:comment xml:lang="en">The purpose for testing. (ISTQB Gloassary v4.5)</rdfs:comment>
        <rdfs:comment xml:lang="en">test objective</rdfs:comment>
        <rdfs:seeAlso>Foundation - v4.0
Advanced Test Management - v3.0</rdfs:seeAlso>
        <skos:altLabel xml:lang="en">test goal</skos:altLabel>
        <skos:prefLabel xml:lang="en">test objective</skos:prefLabel>
    </owl:Class>
    


    <!-- http://purl.org/stc/ontology#test_oracle -->

    <owl:Class rdf:about="http://purl.org/stc/ontology#test_oracle">
        <rdfs:subClassOf rdf:resource="http://purl.org/stc/ontology#Testware"/>
        <isInISTQBGlossary rdf:datatype="http://www.w3.org/2001/XMLSchema#boolean">true</isInISTQBGlossary>
        <rdfs:comment xml:lang="en">A source to determine an expected result to compare with the actual result of the system under test.  (ISTQB Glossary v4.5)</rdfs:comment>
        <rdfs:label>test oracle</rdfs:label>
        <rdfs:seeAlso>Advanced Test Analyst - v4.0</rdfs:seeAlso>
        <skos:altLabel xml:lang="en">oracle</skos:altLabel>
        <skos:prefLabel xml:lang="en">test oracle</skos:prefLabel>
    </owl:Class>
    


    <!-- http://purl.org/stc/ontology#test_plan -->

    <owl:Class rdf:about="http://purl.org/stc/ontology#test_plan">
        <rdfs:subClassOf rdf:resource="http://purl.org/stc/ontology#Testware"/>
        <isInISTQBGlossary rdf:datatype="http://www.w3.org/2001/XMLSchema#boolean">true</isInISTQBGlossary>
        <rdfs:comment xml:lang="en">Documentation describing the test objectives to be achieved and the means and the schedule for achieving them, organized to coordinate testing activities. (ISTQB Glossary v4.5)

Detailed description of test objectives to be achieved and the means and schedule for achieving them, organized to coordinate testing activities for some test item or set of test items. (ISO/IEC/IEEE 29119-1:2022)</rdfs:comment>
        <rdfs:label>test plan</rdfs:label>
        <rdfs:seeAlso>ISO/IEC/IEEE 29119-1 (2022) Software and systems engineering -- Software testing -- Part 1: Concepts and definitions

Foundation - v4.0
Advanced Test Manager - 2012
Advanced Test Management - v3.0
Specialist - Performance Testing - 2018
Specialist - Security Test Engineer - v1.0</rdfs:seeAlso>
        <skos:altLabel xml:lang="en">testplan</skos:altLabel>
        <skos:prefLabel xml:lang="en">test plan</skos:prefLabel>
    </owl:Class>
    


    <!-- http://purl.org/stc/ontology#test_planning -->

    <owl:Class rdf:about="http://purl.org/stc/ontology#test_planning">
        <rdfs:subClassOf rdf:resource="http://purl.org/stc/ontology#test_activity"/>
        <isInISTQBGlossary rdf:datatype="http://www.w3.org/2001/XMLSchema#boolean">true</isInISTQBGlossary>
        <rdfs:comment xml:lang="en">The activity of establishing or updating a test plan. (ISTQB Glossary v4.5)</rdfs:comment>
        <rdfs:label>test planning</rdfs:label>
        <rdfs:seeAlso>Foundation - v4.0
Advanced Test Manager - 2012
Advanced Test Management - v3.0</rdfs:seeAlso>
        <skos:prefLabel xml:lang="en">test planning</skos:prefLabel>
    </owl:Class>
    


    <!-- http://purl.org/stc/ontology#test_process -->

    <owl:Class rdf:about="http://purl.org/stc/ontology#test_process">
        <rdfs:subClassOf rdf:resource="http://purl.org/stc/ontology#software_testing_concepts"/>
        <isInISTQBGlossary rdf:datatype="http://www.w3.org/2001/XMLSchema#boolean">true</isInISTQBGlossary>
        <rdfs:comment xml:lang="en">The set of interrelated activities comprising of test planning, test monitoring, test control, test analysis, test design, test implementation, test execution, and test completion.</rdfs:comment>
        <rdfs:comment xml:lang="en">The set of interrelated activities comprising of test planning, test monitoring, test control, test analysis, test design, test implementation, test execution, and test completion. (ISTQB Glossary v4.5)

Set of testing activities performed to achieve a test objective. (ISO/IEC/IEEE 29119-1:2022)</rdfs:comment>
        <rdfs:label>test process</rdfs:label>
        <rdfs:seeAlso>ISO/IEC/IEEE 29119-1:2022 (Software and Systems Engineering — Software Testing — Part 1: Concepts and Definitions)

Foundation - v4.0
Specialist - Mobile Application Testing - 2019
Specialist - Security Test Engineer - v1.0</rdfs:seeAlso>
        <skos:prefLabel xml:lang="en">test process</skos:prefLabel>
    </owl:Class>
    


    <!-- http://purl.org/stc/ontology#test_process_group -->

    <owl:Class rdf:about="http://purl.org/stc/ontology#test_process_group">
        <rdfs:subClassOf rdf:resource="http://purl.org/stc/ontology#related_to_team"/>
        <isInISTQBGlossary rdf:datatype="http://www.w3.org/2001/XMLSchema#boolean">true</isInISTQBGlossary>
        <rdfs:comment xml:lang="en">A collection of specialists who facilitate the definition, maintenance, and improvement of the test processes used by an organization. (ISTQB Glossary v4.5)</rdfs:comment>
        <rdfs:label>test process group</rdfs:label>
        <rdfs:seeAlso>Expert Improving the Test Process - v1.0.1</rdfs:seeAlso>
        <skos:altLabel xml:lang="en">TPG</skos:altLabel>
        <skos:prefLabel xml:lang="en">test process group</skos:prefLabel>
    </owl:Class>
    


    <!-- http://purl.org/stc/ontology#test_process_improvement -->

    <owl:Class rdf:about="http://purl.org/stc/ontology#test_process_improvement">
        <rdfs:subClassOf rdf:resource="http://purl.org/stc/ontology#test_management"/>
        <isInISTQBGlossary rdf:datatype="http://www.w3.org/2001/XMLSchema#boolean">true</isInISTQBGlossary>
        <rdfs:label>test process improvement</rdfs:label>
        <skos:prefLabel xml:lang="en">test process improvement</skos:prefLabel>
    </owl:Class>
    


    <!-- http://purl.org/stc/ontology#test_progress_report -->

    <owl:Class rdf:about="http://purl.org/stc/ontology#test_progress_report">
        <rdfs:subClassOf rdf:resource="http://purl.org/stc/ontology#test_report"/>
        <isInISTQBGlossary rdf:datatype="http://www.w3.org/2001/XMLSchema#boolean">true</isInISTQBGlossary>
        <rdfs:comment xml:lang="en">A type of periodic test report that includes the progress of test activities against a baseline, risks, and alternatives requiring a decision. (ISTQB Glossary v4.5)

Report that provides information about the status of the testing that is being performed in a specified reporting period. (ISO/IEC/IEEE 29119-1:2022, defined as test status report)</rdfs:comment>
        <rdfs:label>test progress report</rdfs:label>
        <rdfs:seeAlso>ISO/IEC/IEEE 29119-1:2022 (Software and systems engineering — Software testing — Part 1: Concepts and definitions)

Foundation - v4.0
Advanced Test Automation Engineering - v2.0</rdfs:seeAlso>
        <skos:altLabel xml:lang="en">test status report</skos:altLabel>
        <skos:prefLabel xml:lang="en">test progress report</skos:prefLabel>
    </owl:Class>
    


    <!-- http://purl.org/stc/ontology#test_report -->

    <owl:Class rdf:about="http://purl.org/stc/ontology#test_report">
        <rdfs:subClassOf rdf:resource="http://purl.org/stc/ontology#Testware"/>
        <isInISTQBGlossary rdf:datatype="http://www.w3.org/2001/XMLSchema#boolean">true</isInISTQBGlossary>
        <rdfs:comment xml:lang="en">Documentation summarizing testing and results. (ISTQB Glossary v4.5)</rdfs:comment>
        <rdfs:label>test report</rdfs:label>
        <rdfs:seeAlso>Specialist - Mobile Application Testing - 2019
Specialist - Security Test Engineer - v1.0
Specialist - Test Automation Strategy - v1.0</rdfs:seeAlso>
        <skos:altLabel xml:lang="en">testreport</skos:altLabel>
        <skos:prefLabel xml:lang="en">test report</skos:prefLabel>
    </owl:Class>
    


    <!-- http://purl.org/stc/ontology#test_script -->

    <owl:Class rdf:about="http://purl.org/stc/ontology#test_script">
        <rdfs:subClassOf rdf:resource="http://purl.org/stc/ontology#Testware"/>
        <isInISTQBGlossary rdf:datatype="http://www.w3.org/2001/XMLSchema#boolean">true</isInISTQBGlossary>
        <rdfs:comment xml:lang="en">A sequence of instructions for the execution of a test. (ISTQB Glossary v4.5)

Document specifying one or more test procedures. (ISO/IEC/IEEE 29119-1:2022)</rdfs:comment>
        <rdfs:label>test script</rdfs:label>
        <rdfs:seeAlso>ISO/IEC/IEEE 29119-1:2022 (Software and systems engineering — Software testing — Part 1: Concepts and definitions)

Advanced Test Manager - 2012
Advanced Test Analyst - v3.1
Advanced Test Analyst - v4.0
Advanced Test Automation Engineering - v2.0
Specialist - Test Automation Engineer - 2016</rdfs:seeAlso>
        <skos:altLabel xml:lang="en">test procedure specification</skos:altLabel>
        <skos:prefLabel xml:lang="en">test script</skos:prefLabel>
    </owl:Class>
    


    <!-- http://purl.org/stc/ontology#test_step -->

    <owl:Class rdf:about="http://purl.org/stc/ontology#test_step">
        <rdfs:subClassOf rdf:resource="http://purl.org/stc/ontology#Testware"/>
        <isInISTQBGlossary rdf:datatype="http://www.w3.org/2001/XMLSchema#boolean">true</isInISTQBGlossary>
        <rdfs:comment xml:lang="en">A single interaction between an actor and a test object consisting of an input, an action, and an expected result. (ISTQB Glossary v4.5)</rdfs:comment>
        <rdfs:comment xml:lang="en">Advanced Test Automation Engineering - v2.0</rdfs:comment>
        <rdfs:label>test step</rdfs:label>
        <skos:altLabel xml:lang="en">teststep</skos:altLabel>
        <skos:prefLabel xml:lang="en">test step</skos:prefLabel>
    </owl:Class>
    


    <!-- http://purl.org/stc/ontology#test_suite -->

    <owl:Class rdf:about="http://purl.org/stc/ontology#test_suite">
        <rdfs:subClassOf rdf:resource="http://purl.org/stc/ontology#Testware"/>
        <isInISTQBGlossary rdf:datatype="http://www.w3.org/2001/XMLSchema#boolean">true</isInISTQBGlossary>
        <rdfs:comment xml:lang="en">A set of test scripts or test procedures to be executed in a specific test run. (ISTQB Glossary v4.5)

Set of test cases or test procedures. (ISO/IEC/IEEE 29119-1:2022)</rdfs:comment>
        <rdfs:label>test suite</rdfs:label>
        <rdfs:seeAlso>Advanced Test Analyst - v3.1
Specialist - Test Automation Strategy - v1.0</rdfs:seeAlso>
        <skos:altLabel xml:lang="en">test set
test case suite
testsuite
testset
testcase suite</skos:altLabel>
        <skos:prefLabel xml:lang="en">test suite</skos:prefLabel>
    </owl:Class>
    


    <!-- http://purl.org/stc/ontology#test_technique -->

    <owl:Class rdf:about="http://purl.org/stc/ontology#test_technique">
        <rdfs:subClassOf rdf:resource="http://purl.org/stc/ontology#software_testing_concepts"/>
        <isInISTQBGlossary rdf:datatype="http://www.w3.org/2001/XMLSchema#boolean">true</isInISTQBGlossary>
        <rdfs:comment xml:lang="en">(ISTQB Glossary v4.5)</rdfs:comment>
        <rdfs:comment xml:lang="en">A procedure used to define test conditions, design test cases, and specify test data. (ISTQB Glossary v4.5)

Procedure used to create or select a test model, identify test coverage items, and derive
corresponding test cases. (ISO/IEC/IEEE 29119-1:2022, defined as test design technique)</rdfs:comment>
        <rdfs:label>test technique</rdfs:label>
        <rdfs:seeAlso>ISO/IEC/IEEE 29119-4 (Software and systems engineering — Software testing — Part 4: Test techniques)

Foundation - v4.0</rdfs:seeAlso>
        <skos:altLabel xml:lang="en">test design technique</skos:altLabel>
        <skos:altLabel xml:lang="en">test technique</skos:altLabel>
    </owl:Class>
    


    <!-- http://purl.org/stc/ontology#test_type -->

    <owl:Class rdf:about="http://purl.org/stc/ontology#test_type">
        <rdfs:subClassOf rdf:resource="http://purl.org/stc/ontology#software_testing_concepts"/>
        <isInISTQBGlossary rdf:datatype="http://www.w3.org/2001/XMLSchema#boolean">true</isInISTQBGlossary>
        <rdfs:comment xml:lang="en">A group of test activities based on specific test objectives aimed at specific characteristics of a component or system. (ISTQB Glossary v4.5)

Testing that is focused on specific quality characteristics. (ISO/IEC/IEEE 29119-1:2022)</rdfs:comment>
        <rdfs:label>test type</rdfs:label>
        <rdfs:seeAlso>ISO/IEC/IEEE 29119-1:2022 (Software and Systems Engineering — Software Testing — Part 1: Concepts and Definitions)

Foundation - v4.0
Advanced Test Manager - 2012
Advanced Test Management - v3.0
Advanced Test Analyst - v3.1
Advanced Test Analyst - v4.0
Advanced Technical Test Analyst - v4.0
Advanced Test Automation Engineering - v2.0
Specialist - Automotive Software Tester - 2018
Specialist - Automotive Software Tester - v1.1
Specialist - Gambling Industry Tester - 2018
Specialist - Game Testing - v1.0.1
Specialist - Mobile Application Testing - 2019
Specialist - Model-Based Testing - v1.1
Specialist - Test Automation Strategy - v1.0</rdfs:seeAlso>
        <skos:prefLabel xml:lang="en">test type</skos:prefLabel>
    </owl:Class>
    


    <!-- http://purl.org/stc/ontology#test_work_force -->

    <owl:Class rdf:about="http://purl.org/stc/ontology#test_work_force">
        <rdfs:subClassOf rdf:resource="http://purl.org/stc/ontology#software_testing_concepts"/>
        <isInISTQBGlossary rdf:datatype="http://www.w3.org/2001/XMLSchema#boolean">false</isInISTQBGlossary>
        <rdfs:comment xml:lang="en">Professions and roles in software testing</rdfs:comment>
        <rdfs:label>test work force</rdfs:label>
        <rdfs:seeAlso>GTB: The Professional profile for testing. The reference scheme for people and organizations involved in the topics of quality and testing of software-based components and systems. 2018.</rdfs:seeAlso>
        <skos:prefLabel xml:lang="en">test work force</skos:prefLabel>
    </owl:Class>
    


    <!-- http://purl.org/stc/ontology#tester -->

    <owl:Class rdf:about="http://purl.org/stc/ontology#tester">
        <rdfs:subClassOf rdf:resource="http://purl.org/stc/ontology#related_to_role"/>
        <isInISTQBGlossary rdf:datatype="http://www.w3.org/2001/XMLSchema#boolean">true</isInISTQBGlossary>
        <rdfs:comment xml:lang="en">A person who performs testing. (ISTQB Glossary v4.5)

Develops the test deliverables and completes the processes associated with the
dynamic test process. (ISO/IEC/IEEE 29119-1:2022)</rdfs:comment>
        <rdfs:label>tester</rdfs:label>
        <rdfs:seeAlso>ISO/IEC/IEEE 29119-1:2022 (Software and systems engineering — Software testing — Part 1: Concepts and definitions)</rdfs:seeAlso>
        <skos:prefLabel xml:lang="en">tester</skos:prefLabel>
    </owl:Class>
    


    <!-- http://purl.org/stc/ontology#tester_orientation_in_test_approach -->

    <owl:Class rdf:about="http://purl.org/stc/ontology#tester_orientation_in_test_approach">
        <rdfs:subClassOf rdf:resource="http://purl.org/stc/ontology#test_approach"/>
        <isInISTQBGlossary rdf:datatype="http://www.w3.org/2001/XMLSchema#boolean">false</isInISTQBGlossary>
        <rdfs:label>tester orientation</rdfs:label>
        <skos:prefLabel xml:lang="en">tester orientation in test approach</skos:prefLabel>
    </owl:Class>
    


    <!-- http://purl.org/stc/ontology#testing -->

    <owl:Class rdf:about="http://purl.org/stc/ontology#testing">
        <rdfs:subClassOf rdf:resource="http://purl.org/stc/ontology#software_testing_concepts"/>
        <isInISTQBGlossary rdf:datatype="http://www.w3.org/2001/XMLSchema#boolean">true</isInISTQBGlossary>
        <rdfs:comment xml:lang="en">Set of activities conducted to facilitate discovery and evaluation of properties of test items (ISO/IEC/IEEE 29119-1:2022, defined as test)

The process that consists of determining the degree to which a software product satisfies specified requirements (verification) and fulfills its intended purpose (validation). (ISO/IEC/IEEE 12207:2017)

The process of executing a system or component under specified conditions, observing or recording the results, and making an evaluation of some aspect of the system or component. (IEEE 610.12-1990)</rdfs:comment>
        <rdfs:seeAlso>Foundation - v4.0</rdfs:seeAlso>
        <rdfs:seeAlso>IEEE Standard 610.12-1990 (IEEE Standard Glossary of Software Engineering Terminology)
ISO/IEC/IEEE 29119-1:2022 (Software and Systems Engineering — Software Testing — Part 1: Concepts and Definitions)
ISO/IEC/IEEE 12207:2017 (Software Life Cycle Processes)</rdfs:seeAlso>
        <skos:prefLabel xml:lang="en">testing</skos:prefLabel>
    </owl:Class>
    


    <!-- http://purl.org/stc/ontology#testing_in_production -->

    <owl:Class rdf:about="http://purl.org/stc/ontology#testing_in_production">
        <rdfs:subClassOf rdf:resource="http://purl.org/stc/ontology#system_testing"/>
        <isInISTQBGlossary rdf:datatype="http://www.w3.org/2001/XMLSchema#boolean">true</isInISTQBGlossary>
        <rdfs:label>testing in production</rdfs:label>
        <skos:prefLabel xml:lang="en">testing in production</skos:prefLabel>
    </owl:Class>
    


    <!-- http://purl.org/stc/ontology#testing_quadrants -->

    <owl:Class rdf:about="http://purl.org/stc/ontology#testing_quadrants">
        <rdfs:subClassOf rdf:resource="http://purl.org/stc/ontology#test_approach"/>
        <isInISTQBGlossary rdf:datatype="http://www.w3.org/2001/XMLSchema#boolean">true</isInISTQBGlossary>
        <rdfs:comment xml:lang="en">A classification model of test types/test levels in four quadrants, relating them to two dimensions of test objectives: supporting the product team versus critiquing the product, and technology-facing versus business-facing. (ISTQB Glossary v4.5)</rdfs:comment>
        <rdfs:label>testing quadrants</rdfs:label>
        <rdfs:seeAlso>Foundation - v4.0</rdfs:seeAlso>
        <skos:prefLabel xml:lang="en">testing quadrants</skos:prefLabel>
    </owl:Class>
    


    <!-- http://purl.org/stc/ontology#usability_testing -->

    <owl:Class rdf:about="http://purl.org/stc/ontology#usability_testing">
        <rdfs:subClassOf rdf:resource="http://purl.org/stc/ontology#non-functional_testing"/>
        <isInISTQBGlossary rdf:datatype="http://www.w3.org/2001/XMLSchema#boolean">true</isInISTQBGlossary>
        <rdfs:comment xml:lang="en">Testing to evaluate the degree to which the system can be used by specified users with effectiveness, efficiency and satisfaction in a specified context of use. (ISTQB Glossary v4.5)</rdfs:comment>
        <rdfs:label>usability testing</rdfs:label>
        <rdfs:seeAlso>Specialist - Mobile Application Testing - 2019
Specialist - Usability Testing - 2018</rdfs:seeAlso>
        <skos:prefLabel xml:lang="en">usability testing</skos:prefLabel>
    </owl:Class>
    


    <!-- http://purl.org/stc/ontology#user-agent_based_testing -->

    <owl:Class rdf:about="http://purl.org/stc/ontology#user-agent_based_testing">
        <rdfs:subClassOf rdf:resource="http://purl.org/stc/ontology#mobile_app_testing"/>
        <isInISTQBGlossary rdf:datatype="http://www.w3.org/2001/XMLSchema#boolean">true</isInISTQBGlossary>
        <rdfs:label>user-agent based testing</rdfs:label>
        <skos:prefLabel xml:lang="en">user-agent based testing</skos:prefLabel>
    </owl:Class>
    


    <!-- http://purl.org/stc/ontology#user_acceptance_testing -->

    <owl:Class rdf:about="http://purl.org/stc/ontology#user_acceptance_testing">
        <rdfs:subClassOf rdf:resource="http://purl.org/stc/ontology#acceptance_testing"/>
        <isInISTQBGlossary rdf:datatype="http://www.w3.org/2001/XMLSchema#boolean">true</isInISTQBGlossary>
        <rdfs:label>user acceptance testing</rdfs:label>
        <skos:prefLabel xml:lang="en">user acceptance testing</skos:prefLabel>
    </owl:Class>
    


    <!-- http://purl.org/stc/ontology#validation -->

    <owl:Class rdf:about="http://purl.org/stc/ontology#validation">
        <rdfs:subClassOf rdf:resource="http://purl.org/stc/ontology#basic_concepts"/>
    </owl:Class>
    


    <!-- http://purl.org/stc/ontology#verification -->

    <owl:Class rdf:about="http://purl.org/stc/ontology#verification">
        <rdfs:subClassOf rdf:resource="http://purl.org/stc/ontology#basic_concepts"/>
    </owl:Class>
    


    <!-- http://purl.org/stc/ontology#walkthrough -->

    <owl:Class rdf:about="http://purl.org/stc/ontology#walkthrough">
        <rdfs:subClassOf rdf:resource="http://purl.org/stc/ontology#informal_review"/>
        <isInISTQBGlossary rdf:datatype="http://www.w3.org/2001/XMLSchema#boolean">true</isInISTQBGlossary>
        <rdfs:comment xml:lang="en">A type of review in which an author leads members of the review through a work product and the members ask questions and make comments about possible issues.  (ISTQB Glossary v4.5)</rdfs:comment>
        <rdfs:label>walkthrough</rdfs:label>
        <rdfs:seeAlso>Foundation - v4.0
Advanced Test Manager - 2012</rdfs:seeAlso>
        <skos:altLabel xml:lang="en">structured walkthrough</skos:altLabel>
        <skos:prefLabel xml:lang="en">walkthrough</skos:prefLabel>
    </owl:Class>
    


    <!-- http://purl.org/stc/ontology#white_box_test_technique -->

    <owl:Class rdf:about="http://purl.org/stc/ontology#white_box_test_technique">
        <rdfs:subClassOf rdf:resource="http://purl.org/stc/ontology#test_technique"/>
        <isInISTQBGlossary rdf:datatype="http://www.w3.org/2001/XMLSchema#boolean">true</isInISTQBGlossary>
        <rdfs:label>white box test technique</rdfs:label>
        <skos:altLabel xml:lang="en">white-box test technique
structure-based test design technique
structure based test design technique
structure-based test technique
structure based test technique
glass-box testing</skos:altLabel>
        <skos:prefLabel xml:lang="en">white box test technique</skos:prefLabel>
    </owl:Class>
    


    <!-- 
    ///////////////////////////////////////////////////////////////////////////////////////
    //
    // Individuals
    //
    ///////////////////////////////////////////////////////////////////////////////////////
     -->

    


    <!-- http://purl.org/stc/terms#AI_testing -->

    <owl:NamedIndividual rdf:about="http://purl.org/stc/terms#AI_testing">
        <terms:hasParent rdf:resource="http://purl.org/stc/terms#domain-specific_test_types"/>
        <isInISTQBGlossary rdf:datatype="http://www.w3.org/2001/XMLSchema#boolean">true</isInISTQBGlossary>
        <rdfs:label>AI testing</rdfs:label>
        <skos:prefLabel xml:lang="en">ai testing</skos:prefLabel>
    </owl:NamedIndividual>
    


    <!-- http://purl.org/stc/terms#API_testing -->

    <owl:NamedIndividual rdf:about="http://purl.org/stc/terms#API_testing">
        <terms:hasParent rdf:resource="http://purl.org/stc/terms#interface_testing"/>
        <isInISTQBGlossary rdf:datatype="http://www.w3.org/2001/XMLSchema#boolean">true</isInISTQBGlossary>
        <rdfs:label>API testing</rdfs:label>
        <skos:prefLabel xml:lang="en">api testing</skos:prefLabel>
    </owl:NamedIndividual>
    


    <!-- http://purl.org/stc/terms#GUI_testing -->

    <owl:NamedIndividual rdf:about="http://purl.org/stc/terms#GUI_testing">
        <terms:hasParent rdf:resource="http://purl.org/stc/terms#interface_testing"/>
        <isInISTQBGlossary rdf:datatype="http://www.w3.org/2001/XMLSchema#boolean">true</isInISTQBGlossary>
        <rdfs:label>GUI testing</rdfs:label>
        <skos:altLabel xml:lang="en">graphical user interface testing</skos:altLabel>
        <skos:prefLabel xml:lang="en">GUI testing</skos:prefLabel>
    </owl:NamedIndividual>
    


    <!-- http://purl.org/stc/terms#LLM_structural_coverage -->

    <owl:NamedIndividual rdf:about="http://purl.org/stc/terms#LLM_structural_coverage">
        <terms:hasParent rdf:resource="http://purl.org/stc/terms#structural_coverage"/>
        <isInISTQBGlossary rdf:datatype="http://www.w3.org/2001/XMLSchema#boolean">false</isInISTQBGlossary>
        <rdfs:comment xml:lang="en">Coverage measures based on the internal structure of an LLM. (own))</rdfs:comment>
        <rdfs:label>LLM structural coverage</rdfs:label>
        <skos:prefLabel xml:lang="en">llm structural coverage</skos:prefLabel>
    </owl:NamedIndividual>
    


    <!-- http://purl.org/stc/terms#MBT_modeller -->

    <owl:NamedIndividual rdf:about="http://purl.org/stc/terms#MBT_modeller">
        <terms:hasParent rdf:resource="http://purl.org/stc/terms#related_to_role"/>
        <isInISTQBGlossary rdf:datatype="http://www.w3.org/2001/XMLSchema#boolean">false</isInISTQBGlossary>
        <rdfs:comment xml:lang="en">Develops formal test specifications in the form of models used to generate test cases as part of model-based testing. (ISO/IEC/IEEE 29119-1:2022)</rdfs:comment>
        <rdfs:label>MBT modeller</rdfs:label>
        <rdfs:seeAlso>ISO/IEC/IEEE 29119-1:2022 (Software and systems engineering — Software testing — Part 1: Concepts and definitions)</rdfs:seeAlso>
        <skos:prefLabel xml:lang="en">MBT modeller</skos:prefLabel>
    </owl:NamedIndividual>
    


    <!-- http://purl.org/stc/terms#N-switch_coverage -->

    <owl:NamedIndividual rdf:about="http://purl.org/stc/terms#N-switch_coverage">
        <terms:hasParent rdf:resource="http://purl.org/stc/terms#structural_coverage"/>
        <isInISTQBGlossary rdf:datatype="http://www.w3.org/2001/XMLSchema#boolean">true</isInISTQBGlossary>
        <rdfs:comment xml:lang="en">The coverage of sequences of N+1 transitions. (ISTQB Glossary v4.5)</rdfs:comment>
        <rdfs:label>N-switch coverage</rdfs:label>
        <rdfs:seeAlso></rdfs:seeAlso>
        <skos:altLabel xml:lang="en">chow&apos;s coverage metric</skos:altLabel>
        <skos:prefLabel xml:lang="en">n-switch coverage
N-switch coverage</skos:prefLabel>
    </owl:NamedIndividual>
    


    <!-- http://purl.org/stc/terms#Testware -->

    <owl:NamedIndividual rdf:about="http://purl.org/stc/terms#Testware">
        <terms:hasParent rdf:resource="http://purl.org/stc/terms#software"/>
        <terms:hasParent rdf:resource="http://purl.org/stc/terms#software_testing_concepts"/>
        <isInISTQBGlossary rdf:datatype="http://www.w3.org/2001/XMLSchema#boolean">true</isInISTQBGlossary>
        <rdfs:comment xml:lang="en">Work products produced during the test process for use in planning, designing, executing, evaluating and reporting on testing. (ISTQB Glossary v4.5)

Artefacts produced during the test process required to plan, design, and execute tests. (ISO/IEC/IEEE 29119-1:2022)</rdfs:comment>
        <rdfs:label>testware</rdfs:label>
        <rdfs:seeAlso>ISO/IEC/IEEE 29119-1 (2022) Software and systems engineering -- Software testing -- Part 1: Concepts and definitions

Foundation - v4.0
Advanced Test Manager - 2012
Advanced Test Management - v3.0
Advanced Test Analyst - v3.1
Advanced Test Analyst - v4.0
Advanced Test Automation Engineering - v2.0
Specialist - Automotive Software Tester - v1.1
Specialist - Game Testing - v1.0.1
Specialist - Model-Based Testing - v1.1
Specialist - Performance Testing - 2018
Specialist - Test Automation Engineer - 2016
Specialist - Test Automation Strategy - v1.0</rdfs:seeAlso>
        <skos:altLabel>test artefact
test artifact</skos:altLabel>
        <skos:prefLabel xml:lang="en">testware</skos:prefLabel>
    </owl:NamedIndividual>
    


    <!-- http://purl.org/stc/terms#a_b_testing -->

    <owl:NamedIndividual rdf:about="http://purl.org/stc/terms#a_b_testing">
        <terms:hasParent rdf:resource="http://purl.org/stc/terms#oracle_orientation_in_test_approach"/>
        <isInISTQBGlossary rdf:datatype="http://www.w3.org/2001/XMLSchema#boolean">true</isInISTQBGlossary>
        <rdfs:comment xml:lang="en">A test approach in which two components or systems are statistically evaluated to determine which performs better for specified criteria. (ISTQB Glossary v4.5) 

Statistical testing approach that allows testers to determine which of two systems or components performs better. (ISO/IEC/IEEE 29119-1:2022)</rdfs:comment>
        <rdfs:label>a/b testing</rdfs:label>
        <skos:prefLabel xml:lang="en">a/b testing</skos:prefLabel>
    </owl:NamedIndividual>
    


    <!-- http://purl.org/stc/terms#acceptance -->

    <owl:NamedIndividual rdf:about="http://purl.org/stc/terms#acceptance">
        <terms:hasParent rdf:resource="http://purl.org/stc/terms#software_engineering_activity"/>
    </owl:NamedIndividual>
    


    <!-- http://purl.org/stc/terms#acceptance_criteria -->

    <owl:NamedIndividual rdf:about="http://purl.org/stc/terms#acceptance_criteria">
        <terms:hasParent rdf:resource="http://purl.org/stc/terms#Testware"/>
        <isInISTQBGlossary rdf:datatype="http://www.w3.org/2001/XMLSchema#boolean">true</isInISTQBGlossary>
        <rdfs:comment xml:lang="en">The criteria that a work product must satisfy to be accepted by the stakeholders. (ISTQB Glossary v4.5, after IREB Glossary)

Criteria that a system or system component must satisfy to be accepted by a user, customer, or other authorized entity.(ISO/IEC/IEEE 29148:2018)</rdfs:comment>
        <rdfs:label>acceptance criteria</rdfs:label>
        <rdfs:seeAlso>ISO/IEC/IEEE 29148:2018 (Systems and software engineering — Life cycle processes — Requirements engineering)</rdfs:seeAlso>
        <skos:prefLabel xml:lang="en">acceptance criteria</skos:prefLabel>
    </owl:NamedIndividual>
    


    <!-- http://purl.org/stc/terms#acceptance_test-driven_development -->

    <owl:NamedIndividual rdf:about="http://purl.org/stc/terms#acceptance_test-driven_development">
        <terms:hasParent rdf:resource="http://purl.org/stc/terms#test_first_approach"/>
        <isInISTQBGlossary rdf:datatype="http://www.w3.org/2001/XMLSchema#boolean">true</isInISTQBGlossary>
        <rdfs:label>acceptance test-driven development</rdfs:label>
        <skos:prefLabel xml:lang="en">acceptance test-driven development</skos:prefLabel>
    </owl:NamedIndividual>
    


    <!-- http://purl.org/stc/terms#acceptance_testing -->

    <owl:NamedIndividual rdf:about="http://purl.org/stc/terms#acceptance_testing">
        <terms:hasParent rdf:resource="http://purl.org/stc/terms#test_level"/>
        <isInISTQBGlossary rdf:datatype="http://www.w3.org/2001/XMLSchema#boolean">true</isInISTQBGlossary>
        <rdfs:label>acceptance testing</rdfs:label>
        <skos:prefLabel xml:lang="en">acceptance testing</skos:prefLabel>
    </owl:NamedIndividual>
    


    <!-- http://purl.org/stc/terms#accessibility_testing -->

    <owl:NamedIndividual rdf:about="http://purl.org/stc/terms#accessibility_testing">
        <terms:hasParent rdf:resource="http://purl.org/stc/terms#system_testing"/>
        <isInISTQBGlossary rdf:datatype="http://www.w3.org/2001/XMLSchema#boolean">false</isInISTQBGlossary>
        <rdfs:label>accessibility testing</rdfs:label>
        <skos:prefLabel xml:lang="en">accessibility testing</skos:prefLabel>
    </owl:NamedIndividual>
    


    <!-- http://purl.org/stc/terms#ad_hoc_testing -->

    <owl:NamedIndividual rdf:about="http://purl.org/stc/terms#ad_hoc_testing">
        <terms:hasParent rdf:resource="http://purl.org/stc/terms#method_orientation_in_test_approach"/>
        <isInISTQBGlossary rdf:datatype="http://www.w3.org/2001/XMLSchema#boolean">true</isInISTQBGlossary>
        <rdfs:comment xml:lang="en">Informal testing performed without test analysis and test design.</rdfs:comment>
        <rdfs:label>ad hoc testing</rdfs:label>
        <rdfs:seeAlso>Specialist - Game Testing - v1.0.1</rdfs:seeAlso>
        <skos:altLabel xml:lang="en">adhoc testing
ad hoc-testing</skos:altLabel>
        <skos:prefLabel xml:lang="en">ad hoc testing</skos:prefLabel>
    </owl:NamedIndividual>
    


    <!-- http://purl.org/stc/terms#adversarial_testing -->

    <owl:NamedIndividual rdf:about="http://purl.org/stc/terms#adversarial_testing">
        <terms:hasParent rdf:resource="http://purl.org/stc/terms#AI_testing"/>
        <isInISTQBGlossary rdf:datatype="http://www.w3.org/2001/XMLSchema#boolean">true</isInISTQBGlossary>
        <rdfs:label>adversarial testing</rdfs:label>
        <skos:prefLabel xml:lang="en">adversarial testing</skos:prefLabel>
    </owl:NamedIndividual>
    


    <!-- http://purl.org/stc/terms#agile_software_development -->

    <owl:NamedIndividual rdf:about="http://purl.org/stc/terms#agile_software_development">
        <terms:hasParent rdf:resource="http://purl.org/stc/terms#process_orientation_in_software_development"/>
        <isInISTQBGlossary rdf:datatype="http://www.w3.org/2001/XMLSchema#boolean">true</isInISTQBGlossary>
        <rdfs:label>agile</rdfs:label>
        <skos:prefLabel xml:lang="en">agile software development</skos:prefLabel>
    </owl:NamedIndividual>
    


    <!-- http://purl.org/stc/terms#agile_test_leader -->

    <owl:NamedIndividual rdf:about="http://purl.org/stc/terms#agile_test_leader">
        <terms:hasParent rdf:resource="http://purl.org/stc/terms#test_leader"/>
        <isInISTQBGlossary rdf:datatype="http://www.w3.org/2001/XMLSchema#boolean">true</isInISTQBGlossary>
        <rdfs:comment xml:lang="en">A leadership role that serves agile teams, championing testing and quality at the organizational level. (ISTQB Glossary v4.5)</rdfs:comment>
        <rdfs:label>agile test leader</rdfs:label>
        <rdfs:seeAlso>Agile Test Leadership at Scale - v1.0
Specialist - Agile Test Leadership at Scale - v2.0</rdfs:seeAlso>
        <skos:altLabel xml:lang="en">quality coach
agile test manager
quality leader</skos:altLabel>
        <skos:prefLabel xml:lang="en">agile test leader</skos:prefLabel>
    </owl:NamedIndividual>
    


    <!-- http://purl.org/stc/terms#agile_test_team_leader -->

    <owl:NamedIndividual rdf:about="http://purl.org/stc/terms#agile_test_team_leader">
        <terms:hasParent rdf:resource="http://purl.org/stc/terms#test_manager"/>
        <isInISTQBGlossary rdf:datatype="http://www.w3.org/2001/XMLSchema#boolean">true</isInISTQBGlossary>
        <rdfs:comment xml:lang="en">A role that is responsible for maintaining solution quality within an agile delivery team. (ISTQB Glossary v4.5)</rdfs:comment>
        <rdfs:label>agile test team leader</rdfs:label>
        <rdfs:seeAlso>Agile Test Leadership at Scale - v1.0
Specialist - Agile Test Leadership at Scale - v2.0</rdfs:seeAlso>
        <skos:prefLabel xml:lang="en">agile test team leader</skos:prefLabel>
    </owl:NamedIndividual>
    


    <!-- http://purl.org/stc/terms#alpha_testing -->

    <owl:NamedIndividual rdf:about="http://purl.org/stc/terms#alpha_testing">
        <terms:hasParent rdf:resource="http://purl.org/stc/terms#acceptance_testing"/>
        <isInISTQBGlossary rdf:datatype="http://www.w3.org/2001/XMLSchema#boolean">true</isInISTQBGlossary>
        <rdfs:label>alpha testing</rdfs:label>
        <skos:prefLabel xml:lang="en">alpha testing</skos:prefLabel>
    </owl:NamedIndividual>
    


    <!-- http://purl.org/stc/terms#architectural_design -->

    <owl:NamedIndividual rdf:about="http://purl.org/stc/terms#architectural_design">
        <terms:hasParent rdf:resource="http://purl.org/stc/terms#software_engineering_activity"/>
    </owl:NamedIndividual>
    


    <!-- http://purl.org/stc/terms#automated_testing -->

    <owl:NamedIndividual rdf:about="http://purl.org/stc/terms#automated_testing">
        <terms:hasParent rdf:resource="http://purl.org/stc/terms#test_execution"/>
        <isInISTQBGlossary rdf:datatype="http://www.w3.org/2001/XMLSchema#boolean">false</isInISTQBGlossary>
        <rdfs:label>automated testing</rdfs:label>
        <skos:prefLabel xml:lang="en">automated testing</skos:prefLabel>
    </owl:NamedIndividual>
    


    <!-- http://purl.org/stc/terms#back-to-back_testing -->

    <owl:NamedIndividual rdf:about="http://purl.org/stc/terms#back-to-back_testing">
        <terms:hasParent rdf:resource="http://purl.org/stc/terms#oracle_orientation_in_test_approach"/>
        <isInISTQBGlossary rdf:datatype="http://www.w3.org/2001/XMLSchema#boolean">true</isInISTQBGlossary>
        <rdfs:label>back-to-back testing</rdfs:label>
        <skos:altLabel xml:lang="en">back to back testing</skos:altLabel>
        <skos:prefLabel xml:lang="en">back-to-back testing</skos:prefLabel>
    </owl:NamedIndividual>
    


    <!-- http://purl.org/stc/terms#base_choice_coverage -->

    <owl:NamedIndividual rdf:about="http://purl.org/stc/terms#base_choice_coverage">
        <terms:hasParent rdf:resource="http://purl.org/stc/terms#specification_coverage"/>
        <isInISTQBGlossary rdf:datatype="http://www.w3.org/2001/XMLSchema#boolean">true</isInISTQBGlossary>
        <rdfs:comment xml:lang="en">The coverage of parameter-value combinations in which each value of a parameter is combined with the base values of all other parameters, for a chosen base value per parameter. (ISTQB Glossary v4.5)

Coverage for base choice testing. (ISO/IEC/IEEE 29119-4)</rdfs:comment>
        <rdfs:label>base choice coverage</rdfs:label>
        <rdfs:seeAlso>ISO/IEC/IEEE 29119-4 (Software and systems engineering — Software testing — Part 4: Test techniques)</rdfs:seeAlso>
        <skos:altLabel xml:lang="en">p-v pair coverage</skos:altLabel>
        <skos:prefLabel xml:lang="en">base choice coverage</skos:prefLabel>
    </owl:NamedIndividual>
    


    <!-- http://purl.org/stc/terms#basic_concepts -->

    <owl:NamedIndividual rdf:about="http://purl.org/stc/terms#basic_concepts">
        <terms:hasParent rdf:resource="http://purl.org/stc/terms#software_engineering_concepts"/>
        <isInISTQBGlossary rdf:datatype="http://www.w3.org/2001/XMLSchema#boolean">false</isInISTQBGlossary>
        <rdfs:label>basic concepts</rdfs:label>
        <skos:prefLabel xml:lang="en">basic concepts</skos:prefLabel>
    </owl:NamedIndividual>
    


    <!-- http://purl.org/stc/terms#behavior-driven_development -->

    <owl:NamedIndividual rdf:about="http://purl.org/stc/terms#behavior-driven_development">
        <terms:hasParent rdf:resource="http://purl.org/stc/terms#target_orientation_in_software_development"/>
        <isInISTQBGlossary rdf:datatype="http://www.w3.org/2001/XMLSchema#boolean">true</isInISTQBGlossary>
        <rdfs:label>behavior-driven</rdfs:label>
        <skos:altLabel xml:lang="en">behavior driven development
bdd
BDD</skos:altLabel>
        <skos:prefLabel xml:lang="en">behavior-driven development</skos:prefLabel>
    </owl:NamedIndividual>
    


    <!-- http://purl.org/stc/terms#beta_testing -->

    <owl:NamedIndividual rdf:about="http://purl.org/stc/terms#beta_testing">
        <terms:hasParent rdf:resource="http://purl.org/stc/terms#acceptance_testing"/>
        <isInISTQBGlossary rdf:datatype="http://www.w3.org/2001/XMLSchema#boolean">true</isInISTQBGlossary>
        <rdfs:label>beta testing</rdfs:label>
        <skos:prefLabel xml:lang="en">beta testing</skos:prefLabel>
    </owl:NamedIndividual>
    


    <!-- http://purl.org/stc/terms#black_box_test_technique -->

    <owl:NamedIndividual rdf:about="http://purl.org/stc/terms#black_box_test_technique">
        <terms:hasParent rdf:resource="http://purl.org/stc/terms#test_technique"/>
        <isInISTQBGlossary rdf:datatype="http://www.w3.org/2001/XMLSchema#boolean">true</isInISTQBGlossary>
        <rdfs:comment xml:lang="en">(ISTQB Glossary v4.5)</rdfs:comment>
        <rdfs:label>black box test technique</rdfs:label>
        <skos:altLabel xml:lang="en">specification-based testing
specification based testing
closed box testing
black-box test technique</skos:altLabel>
        <skos:prefLabel xml:lang="en">black box test technique</skos:prefLabel>
    </owl:NamedIndividual>
    


    <!-- http://purl.org/stc/terms#boundary_value_analysis -->

    <owl:NamedIndividual rdf:about="http://purl.org/stc/terms#boundary_value_analysis">
        <terms:hasParent rdf:resource="http://purl.org/stc/terms#black_box_test_technique"/>
        <isInISTQBGlossary rdf:datatype="http://www.w3.org/2001/XMLSchema#boolean">true</isInISTQBGlossary>
        <rdfs:label>boundary value analysis</rdfs:label>
        <skos:prefLabel xml:lang="en">boundary value analysis</skos:prefLabel>
    </owl:NamedIndividual>
    


    <!-- http://purl.org/stc/terms#branch_coverage -->

    <owl:NamedIndividual rdf:about="http://purl.org/stc/terms#branch_coverage">
        <terms:hasParent rdf:resource="http://purl.org/stc/terms#structural_coverage"/>
        <isInISTQBGlossary rdf:datatype="http://www.w3.org/2001/XMLSchema#boolean">true</isInISTQBGlossary>
        <rdfs:comment xml:lang="en">The coverage of branches in a control flow graph.  (ISTQB Glossary v4.5)</rdfs:comment>
        <rdfs:label>branch coverage</rdfs:label>
        <rdfs:seeAlso>Foundation - v4.0</rdfs:seeAlso>
        <skos:prefLabel xml:lang="en">branch coverage</skos:prefLabel>
    </owl:NamedIndividual>
    


    <!-- http://purl.org/stc/terms#branch_testing -->

    <owl:NamedIndividual rdf:about="http://purl.org/stc/terms#branch_testing">
        <terms:hasParent rdf:resource="http://purl.org/stc/terms#white_box_test_technique"/>
        <isInISTQBGlossary rdf:datatype="http://www.w3.org/2001/XMLSchema#boolean">true</isInISTQBGlossary>
        <rdfs:label>branch testing</rdfs:label>
        <skos:prefLabel xml:lang="en">branch testing</skos:prefLabel>
    </owl:NamedIndividual>
    


    <!-- http://purl.org/stc/terms#change_orientation_in_test_approach -->

    <owl:NamedIndividual rdf:about="http://purl.org/stc/terms#change_orientation_in_test_approach">
        <terms:hasParent rdf:resource="http://purl.org/stc/terms#test_approach"/>
        <isInISTQBGlossary rdf:datatype="http://www.w3.org/2001/XMLSchema#boolean">false</isInISTQBGlossary>
        <rdfs:label>change orientation</rdfs:label>
        <skos:prefLabel xml:lang="en">change orientation in test approach</skos:prefLabel>
    </owl:NamedIndividual>
    


    <!-- http://purl.org/stc/terms#checklist_based_testing -->

    <owl:NamedIndividual rdf:about="http://purl.org/stc/terms#checklist_based_testing">
        <terms:hasParent rdf:resource="http://purl.org/stc/terms#experience-based_testing"/>
        <isInISTQBGlossary rdf:datatype="http://www.w3.org/2001/XMLSchema#boolean">true</isInISTQBGlossary>
        <rdfs:label>checklist based testing</rdfs:label>
        <skos:prefLabel xml:lang="en">checklist based testing</skos:prefLabel>
    </owl:NamedIndividual>
    


    <!-- http://purl.org/stc/terms#code -->

    <owl:NamedIndividual rdf:about="http://purl.org/stc/terms#code">
        <terms:hasParent rdf:resource="http://purl.org/stc/terms#basic_concepts"/>
    </owl:NamedIndividual>
    


    <!-- http://purl.org/stc/terms#coding -->

    <owl:NamedIndividual rdf:about="http://purl.org/stc/terms#coding">
        <terms:hasParent rdf:resource="http://purl.org/stc/terms#software_engineering_activity"/>
    </owl:NamedIndividual>
    


    <!-- http://purl.org/stc/terms#compliance_testing -->

    <owl:NamedIndividual rdf:about="http://purl.org/stc/terms#compliance_testing">
        <terms:hasParent rdf:resource="http://purl.org/stc/terms#functional_testing"/>
        <isInISTQBGlossary rdf:datatype="http://www.w3.org/2001/XMLSchema#boolean">true</isInISTQBGlossary>
        <rdfs:comment xml:lang="en">The term conformance testing (defined by ISTQB to be a synonym for compliance testing) is used differently in telecommunication/protocol testing - see also protocol testing.</rdfs:comment>
        <rdfs:label>compliance testing</rdfs:label>
        <rdfs:seeAlso>Specialist - Gambling Industry Tester - 2018</rdfs:seeAlso>
        <skos:altLabel>conformance testing
regulation testing
standards testing</skos:altLabel>
        <skos:prefLabel xml:lang="en">compliance testing</skos:prefLabel>
    </owl:NamedIndividual>
    


    <!-- http://purl.org/stc/terms#component_integration_testing -->

    <owl:NamedIndividual rdf:about="http://purl.org/stc/terms#component_integration_testing">
        <terms:hasParent rdf:resource="http://purl.org/stc/terms#integration_testing"/>
        <isInISTQBGlossary rdf:datatype="http://www.w3.org/2001/XMLSchema#boolean">true</isInISTQBGlossary>
        <rdfs:comment xml:lang="en">The integration testing of components. (ISTQB Glossary v4.5)</rdfs:comment>
        <rdfs:label>component integration testing</rdfs:label>
        <rdfs:seeAlso>Foundation - v4.0</rdfs:seeAlso>
        <skos:altLabel xml:lang="en">module integration testing
unit integration testing</skos:altLabel>
        <skos:prefLabel xml:lang="en">component integration testing</skos:prefLabel>
    </owl:NamedIndividual>
    


    <!-- http://purl.org/stc/terms#component_testing -->

    <owl:NamedIndividual rdf:about="http://purl.org/stc/terms#component_testing">
        <terms:hasParent rdf:resource="http://purl.org/stc/terms#test_level"/>
        <isInISTQBGlossary rdf:datatype="http://www.w3.org/2001/XMLSchema#boolean">true</isInISTQBGlossary>
        <rdfs:label>component testing</rdfs:label>
        <skos:prefLabel xml:lang="en">component testing</skos:prefLabel>
    </owl:NamedIndividual>
    


    <!-- http://purl.org/stc/terms#condition_coverage -->

    <owl:NamedIndividual rdf:about="http://purl.org/stc/terms#condition_coverage">
        <terms:hasParent rdf:resource="http://purl.org/stc/terms#structural_coverage"/>
        <isInISTQBGlossary rdf:datatype="http://www.w3.org/2001/XMLSchema#boolean">true</isInISTQBGlossary>
        <rdfs:comment xml:lang="en">The coverage of condition outcomes. (ISTQB Glossary v4.5)

Coverage for branch condition testing. (ISO/IEC/IEEE 29119-4)</rdfs:comment>
        <rdfs:label>condition coverage</rdfs:label>
        <rdfs:seeAlso>ISO/IEC/IEEE 29119-4 (Software and systems engineering — Software testing — Part 4: Test techniques)</rdfs:seeAlso>
        <skos:altLabel xml:lang="en">branch condition coverage</skos:altLabel>
        <skos:prefLabel xml:lang="en">condition coverage</skos:prefLabel>
    </owl:NamedIndividual>
    


    <!-- http://purl.org/stc/terms#configuration_management -->

    <owl:NamedIndividual rdf:about="http://purl.org/stc/terms#configuration_management">
        <terms:hasParent rdf:resource="http://purl.org/stc/terms#support_processes"/>
    </owl:NamedIndividual>
    


    <!-- http://purl.org/stc/terms#confirmation_testing -->

    <owl:NamedIndividual rdf:about="http://purl.org/stc/terms#confirmation_testing">
        <terms:hasParent rdf:resource="http://purl.org/stc/terms#defect_orientation_in_test_approach"/>
        <isInISTQBGlossary rdf:datatype="http://www.w3.org/2001/XMLSchema#boolean">true</isInISTQBGlossary>
        <rdfs:comment xml:lang="en">A type of change-related testing performed after fixing a defect to confirm that a failure caused by that defect does not reoccur. (ISTQB Glossary v4.5)

Testing performed to check that modifications made to correct a fault have successfully removed the fault. (ISO/IEC/IEEE 29119-1:2022)</rdfs:comment>
        <rdfs:label>confirmation testing</rdfs:label>
        <rdfs:seeAlso>ISO/IEC/IEEE 29119-1:2022 (Software and systems engineering — Software testing — Part 1: Concepts and definitions)

Foundation - v4.0
Specialist - Test Automation Engineer - 2016
Specialist - Test Automation Strategy - v1.0</rdfs:seeAlso>
        <skos:altLabel xml:lang="en">retesting</skos:altLabel>
        <skos:prefLabel xml:lang="en">confirmation testing</skos:prefLabel>
    </owl:NamedIndividual>
    


    <!-- http://purl.org/stc/terms#conformance_testing -->

    <owl:NamedIndividual rdf:about="http://purl.org/stc/terms#conformance_testing">
        <terms:hasParent rdf:resource="http://purl.org/stc/terms#protocol_or_service_testing"/>
        <isInISTQBGlossary rdf:datatype="http://www.w3.org/2001/XMLSchema#boolean">false</isInISTQBGlossary>
        <rdfs:comment xml:lang="en">The process of verifying that a system or component meets the requirements of a specified standard. (ISO/IEC 9646-1:1994)</rdfs:comment>
        <rdfs:label>conformance testing</rdfs:label>
        <rdfs:seeAlso>ISO/IEC 9646-1:1994 (Information technology — Open Systems Interconnection — Conformance testing methodology and framework. Part 1: General concepts)</rdfs:seeAlso>
        <skos:prefLabel xml:lang="en">conformance testing</skos:prefLabel>
    </owl:NamedIndividual>
    


    <!-- http://purl.org/stc/terms#continuous_testing -->

    <owl:NamedIndividual rdf:about="http://purl.org/stc/terms#continuous_testing">
        <terms:hasParent rdf:resource="http://purl.org/stc/terms#process_orientation_in_test_approach"/>
        <isInISTQBGlossary rdf:datatype="http://www.w3.org/2001/XMLSchema#boolean">true</isInISTQBGlossary>
        <rdfs:label>continuous testing</rdfs:label>
        <skos:prefLabel xml:lang="en">continuous testing</skos:prefLabel>
    </owl:NamedIndividual>
    


    <!-- http://purl.org/stc/terms#contract_testing -->

    <owl:NamedIndividual rdf:about="http://purl.org/stc/terms#contract_testing">
        <terms:hasParent rdf:resource="http://purl.org/stc/terms#target_orientation_in_test_approach"/>
        <isInISTQBGlossary rdf:datatype="http://www.w3.org/2001/XMLSchema#boolean">true</isInISTQBGlossary>
        <rdfs:label>contract testing</rdfs:label>
        <skos:prefLabel xml:lang="en">contract testing</skos:prefLabel>
    </owl:NamedIndividual>
    


    <!-- http://purl.org/stc/terms#coverage -->

    <owl:NamedIndividual rdf:about="http://purl.org/stc/terms#coverage">
        <terms:hasParent rdf:resource="http://purl.org/stc/terms#test_metric"/>
        <isInISTQBGlossary rdf:datatype="http://www.w3.org/2001/XMLSchema#boolean">true</isInISTQBGlossary>
        <rdfs:comment xml:lang="en">The degree to which specified coverage items are exercised by a test suite, expressed as a percentage. (ISTQB Glossary v4.5)</rdfs:comment>
        <rdfs:label>coverage</rdfs:label>
        <skos:altLabel xml:lang="en">coverage metric
test coverage
coverage-oriented metric</skos:altLabel>
        <skos:prefLabel xml:lang="en">coverage</skos:prefLabel>
    </owl:NamedIndividual>
    


    <!-- http://purl.org/stc/terms#coverage_item -->

    <owl:NamedIndividual rdf:about="http://purl.org/stc/terms#coverage_item">
        <terms:hasParent rdf:resource="http://purl.org/stc/terms#Testware"/>
        <isInISTQBGlossary rdf:datatype="http://www.w3.org/2001/XMLSchema#boolean">true</isInISTQBGlossary>
        <rdfs:comment xml:lang="en">An attribute or combination of attributes derived from one or more test conditions by using a test technique. (ISTQB Glossary v4.5)

Measurable attribute of a test item that is the focus of testing (ISO/IEC/IEEE 29119-1:2022, defined as test (coverage) item)</rdfs:comment>
        <rdfs:label>coverage item</rdfs:label>
        <rdfs:seeAlso>ISO/IEC/IEEE 29119-1:2022 (Software and systems engineering — Software testing — Part 1: Concepts and definitions)

Foundation - v4.0
Specialist - Model-Based Testing - v1.1</rdfs:seeAlso>
        <skos:altLabel xml:lang="en">test coverage item</skos:altLabel>
        <skos:prefLabel xml:lang="en">coverage item</skos:prefLabel>
    </owl:NamedIndividual>
    


    <!-- http://purl.org/stc/terms#crowd_testing -->

    <owl:NamedIndividual rdf:about="http://purl.org/stc/terms#crowd_testing">
        <terms:hasParent rdf:resource="http://purl.org/stc/terms#tester_orientation_in_test_approach"/>
        <isInISTQBGlossary rdf:datatype="http://www.w3.org/2001/XMLSchema#boolean">true</isInISTQBGlossary>
        <rdfs:label>crowd testing</rdfs:label>
        <skos:prefLabel xml:lang="en">crowd testing</skos:prefLabel>
    </owl:NamedIndividual>
    


    <!-- http://purl.org/stc/terms#data -->

    <owl:NamedIndividual rdf:about="http://purl.org/stc/terms#data">
        <terms:hasParent rdf:resource="http://purl.org/stc/terms#basic_concepts"/>
    </owl:NamedIndividual>
    


    <!-- http://purl.org/stc/terms#decision_coverage -->

    <owl:NamedIndividual rdf:about="http://purl.org/stc/terms#decision_coverage">
        <terms:hasParent rdf:resource="http://purl.org/stc/terms#structural_coverage"/>
        <isInISTQBGlossary rdf:datatype="http://www.w3.org/2001/XMLSchema#boolean">true</isInISTQBGlossary>
        <rdfs:comment xml:lang="en">The coverage of decision outcomes. (ISTQB Glossary v4.5)

Coverage for decision testing. (ISO/IEC/IEEE 29119-4)</rdfs:comment>
        <rdfs:label>decision coverage</rdfs:label>
        <rdfs:seeAlso>ISO/IEC/IEEE 29119-4 (Software and systems engineering — Software testing — Part 4: Test techniques)</rdfs:seeAlso>
        <skos:prefLabel xml:lang="en">decision coverage</skos:prefLabel>
    </owl:NamedIndividual>
    


    <!-- http://purl.org/stc/terms#decision_table_testing -->

    <owl:NamedIndividual rdf:about="http://purl.org/stc/terms#decision_table_testing">
        <terms:hasParent rdf:resource="http://purl.org/stc/terms#black_box_test_technique"/>
        <isInISTQBGlossary rdf:datatype="http://www.w3.org/2001/XMLSchema#boolean">true</isInISTQBGlossary>
        <rdfs:label>decision table testing</rdfs:label>
        <skos:prefLabel xml:lang="en">decision table testing</skos:prefLabel>
    </owl:NamedIndividual>
    


    <!-- http://purl.org/stc/terms#defect -->

    <owl:NamedIndividual rdf:about="http://purl.org/stc/terms#defect">
        <terms:hasParent rdf:resource="http://purl.org/stc/terms#basic_concepts"/>
    </owl:NamedIndividual>
    


    <!-- http://purl.org/stc/terms#defect_orientation_in_test_approach -->

    <owl:NamedIndividual rdf:about="http://purl.org/stc/terms#defect_orientation_in_test_approach">
        <terms:hasParent rdf:resource="http://purl.org/stc/terms#change_orientation_in_test_approach"/>
        <isInISTQBGlossary rdf:datatype="http://www.w3.org/2001/XMLSchema#boolean">false</isInISTQBGlossary>
        <rdfs:label>defect orientation</rdfs:label>
        <skos:prefLabel xml:lang="en">defect orientation in test approach</skos:prefLabel>
    </owl:NamedIndividual>
    


    <!-- http://purl.org/stc/terms#defect_oriented_metric -->

    <owl:NamedIndividual rdf:about="http://purl.org/stc/terms#defect_oriented_metric">
        <terms:hasParent rdf:resource="http://purl.org/stc/terms#test_metric"/>
        <isInISTQBGlossary rdf:datatype="http://www.w3.org/2001/XMLSchema#boolean">false</isInISTQBGlossary>
        <rdfs:label>defect oriented metric</rdfs:label>
        <skos:altLabel xml:lang="en">defect-oriented metric
defect metric</skos:altLabel>
        <skos:prefLabel xml:lang="en">defect oriented metric</skos:prefLabel>
    </owl:NamedIndividual>
    


    <!-- http://purl.org/stc/terms#destructive_testing -->

    <owl:NamedIndividual rdf:about="http://purl.org/stc/terms#destructive_testing">
        <terms:hasParent rdf:resource="http://purl.org/stc/terms#security_testing"/>
        <isInISTQBGlossary rdf:datatype="http://www.w3.org/2001/XMLSchema#boolean">true</isInISTQBGlossary>
        <rdfs:label>destructive testing</rdfs:label>
        <skos:prefLabel xml:lang="en">destructive testing</skos:prefLabel>
    </owl:NamedIndividual>
    


    <!-- http://purl.org/stc/terms#detailed_design -->

    <owl:NamedIndividual rdf:about="http://purl.org/stc/terms#detailed_design">
        <terms:hasParent rdf:resource="http://purl.org/stc/terms#software_engineering_activity"/>
    </owl:NamedIndividual>
    


    <!-- http://purl.org/stc/terms#development -->

    <owl:NamedIndividual rdf:about="http://purl.org/stc/terms#development">
        <terms:hasParent rdf:resource="http://purl.org/stc/terms#software_lifecycle"/>
    </owl:NamedIndividual>
    


    <!-- http://purl.org/stc/terms#device-based_testing -->

    <owl:NamedIndividual rdf:about="http://purl.org/stc/terms#device-based_testing">
        <terms:hasParent rdf:resource="http://purl.org/stc/terms#mobile_app_testing"/>
        <isInISTQBGlossary rdf:datatype="http://www.w3.org/2001/XMLSchema#boolean">true</isInISTQBGlossary>
        <rdfs:label>device-based testing</rdfs:label>
        <skos:prefLabel xml:lang="en">device-based testing</skos:prefLabel>
    </owl:NamedIndividual>
    


    <!-- http://purl.org/stc/terms#domain-specific_test_types -->

    <owl:NamedIndividual rdf:about="http://purl.org/stc/terms#domain-specific_test_types">
        <terms:hasParent rdf:resource="http://purl.org/stc/terms#test_type"/>
        <isInISTQBGlossary rdf:datatype="http://www.w3.org/2001/XMLSchema#boolean">false</isInISTQBGlossary>
        <rdfs:label>domain-specific test types</rdfs:label>
        <skos:prefLabel xml:lang="en">domain-specific test types</skos:prefLabel>
    </owl:NamedIndividual>
    


    <!-- http://purl.org/stc/terms#dynamic_application_security_testing -->

    <owl:NamedIndividual rdf:about="http://purl.org/stc/terms#dynamic_application_security_testing">
        <terms:hasParent rdf:resource="http://purl.org/stc/terms#security_testing"/>
        <isInISTQBGlossary rdf:datatype="http://www.w3.org/2001/XMLSchema#boolean">true</isInISTQBGlossary>
        <rdfs:label>dynamic application security testing</rdfs:label>
        <skos:prefLabel xml:lang="en">dynamic application security testing</skos:prefLabel>
    </owl:NamedIndividual>
    


    <!-- http://purl.org/stc/terms#dynamic_testing -->

    <owl:NamedIndividual rdf:about="http://purl.org/stc/terms#dynamic_testing">
        <terms:hasParent rdf:resource="http://purl.org/stc/terms#testing"/>
        <isInISTQBGlossary rdf:datatype="http://www.w3.org/2001/XMLSchema#boolean">true</isInISTQBGlossary>
        <rdfs:comment xml:lang="en">Testing that involves the execution of the test item. (ISTQB Glossary v4.5)

Testing in which a test item is evaluated by executing it. (ISO/IEC/IEEE 29119-1)</rdfs:comment>
        <rdfs:label>dynamic testing</rdfs:label>
        <rdfs:seeAlso>ISO/IEC/IEEE 29119-1:2022 (Software and systems engineering — Software testing — Part 1: Concepts and definitions)

Foundation - v4.0</rdfs:seeAlso>
        <skos:prefLabel xml:lang="en">dynamic testing</skos:prefLabel>
    </owl:NamedIndividual>
    


    <!-- http://purl.org/stc/terms#each_choice_coverage -->

    <owl:NamedIndividual rdf:about="http://purl.org/stc/terms#each_choice_coverage">
        <terms:hasParent rdf:resource="http://purl.org/stc/terms#specification_coverage"/>
        <isInISTQBGlossary rdf:datatype="http://www.w3.org/2001/XMLSchema#boolean">true</isInISTQBGlossary>
        <rdfs:comment xml:lang="en">The coverage of equivalence partitions in multiple sets of partitions. (ISTQB Glossary v4.5)

Coverage for each choice testing. (ISO/IEC/IEEE 29119-4:2015)</rdfs:comment>
        <rdfs:label>each choice coverage</rdfs:label>
        <rdfs:seeAlso>ISO/IEC/IEEE 29119-4 (Software and systems engineering — Software testing — Part 4: Test techniques)</rdfs:seeAlso>
        <skos:altLabel xml:lang="en">ecc
ECC</skos:altLabel>
        <skos:prefLabel xml:lang="en">each choice coverage</skos:prefLabel>
    </owl:NamedIndividual>
    


    <!-- http://purl.org/stc/terms#end-to-end_testing -->

    <owl:NamedIndividual rdf:about="http://purl.org/stc/terms#end-to-end_testing">
        <terms:hasParent rdf:resource="http://purl.org/stc/terms#system_testing"/>
        <isInISTQBGlossary rdf:datatype="http://www.w3.org/2001/XMLSchema#boolean">true</isInISTQBGlossary>
        <rdfs:label>end-to-end testing</rdfs:label>
        <skos:altLabel xml:lang="en">e2e testing
E2E testing</skos:altLabel>
        <skos:prefLabel xml:lang="en">end-to-end testing</skos:prefLabel>
    </owl:NamedIndividual>
    


    <!-- http://purl.org/stc/terms#entry_criteria -->

    <owl:NamedIndividual rdf:about="http://purl.org/stc/terms#entry_criteria">
        <terms:hasParent rdf:resource="http://purl.org/stc/terms#Testware"/>
        <isInISTQBGlossary rdf:datatype="http://www.w3.org/2001/XMLSchema#boolean">true</isInISTQBGlossary>
        <rdfs:comment xml:lang="en">The set of conditions for officially completing a defined task. (ISTQB Glossary v4.5)</rdfs:comment>
        <rdfs:label>entry criteria</rdfs:label>
        <rdfs:seeAlso>Foundation - v4.0</rdfs:seeAlso>
        <skos:altLabel xml:lang="en">test completion criteria
completion criteria</skos:altLabel>
        <skos:prefLabel xml:lang="en">entry criteria</skos:prefLabel>
    </owl:NamedIndividual>
    


    <!-- http://purl.org/stc/terms#equivalence_partitioning -->

    <owl:NamedIndividual rdf:about="http://purl.org/stc/terms#equivalence_partitioning">
        <terms:hasParent rdf:resource="http://purl.org/stc/terms#black_box_test_technique"/>
        <isInISTQBGlossary rdf:datatype="http://www.w3.org/2001/XMLSchema#boolean">true</isInISTQBGlossary>
        <rdfs:label>equivalence partitioning</rdfs:label>
        <skos:prefLabel xml:lang="en">equivalence partitioning</skos:prefLabel>
    </owl:NamedIndividual>
    


    <!-- http://purl.org/stc/terms#error -->

    <owl:NamedIndividual rdf:about="http://purl.org/stc/terms#error">
        <terms:hasParent rdf:resource="http://purl.org/stc/terms#basic_concepts"/>
    </owl:NamedIndividual>
    


    <!-- http://purl.org/stc/terms#error_guessing -->

    <owl:NamedIndividual rdf:about="http://purl.org/stc/terms#error_guessing">
        <terms:hasParent rdf:resource="http://purl.org/stc/terms#experience-based_testing"/>
        <isInISTQBGlossary rdf:datatype="http://www.w3.org/2001/XMLSchema#boolean">true</isInISTQBGlossary>
        <rdfs:label>error guessing</rdfs:label>
        <skos:prefLabel xml:lang="en">error guessing</skos:prefLabel>
    </owl:NamedIndividual>
    


    <!-- http://purl.org/stc/terms#exhaustive_testing -->

    <owl:NamedIndividual rdf:about="http://purl.org/stc/terms#exhaustive_testing">
        <terms:hasParent rdf:resource="http://purl.org/stc/terms#method_orientation_in_test_approach"/>
        <isInISTQBGlossary rdf:datatype="http://www.w3.org/2001/XMLSchema#boolean">true</isInISTQBGlossary>
        <rdfs:comment xml:lang="en">A test approach in which the test suite comprises all combinations of input values and preconditions.</rdfs:comment>
        <rdfs:label>exhaustive testing</rdfs:label>
        <skos:altLabel xml:lang="en">complete testing</skos:altLabel>
        <skos:prefLabel xml:lang="en">exhaustive testing</skos:prefLabel>
    </owl:NamedIndividual>
    


    <!-- http://purl.org/stc/terms#exit_criteria -->

    <owl:NamedIndividual rdf:about="http://purl.org/stc/terms#exit_criteria">
        <terms:hasParent rdf:resource="http://purl.org/stc/terms#Testware"/>
        <isInISTQBGlossary rdf:datatype="http://www.w3.org/2001/XMLSchema#boolean">true</isInISTQBGlossary>
        <rdfs:comment xml:lang="en">The set of conditions for officially starting a defined task. (ISTQB Glossary v4-5)</rdfs:comment>
        <rdfs:label>exit criteria</rdfs:label>
        <rdfs:seeAlso>Foundation - v4.0
Advanced Test Manager - 2012
Advanced Test Analyst - v3.1</rdfs:seeAlso>
        <skos:altLabel>test completion criteria
completion criteria</skos:altLabel>
        <skos:prefLabel xml:lang="en">exit criteria</skos:prefLabel>
    </owl:NamedIndividual>
    


    <!-- http://purl.org/stc/terms#experience-based_testing -->

    <owl:NamedIndividual rdf:about="http://purl.org/stc/terms#experience-based_testing">
        <terms:hasParent rdf:resource="http://purl.org/stc/terms#test_technique"/>
        <isInISTQBGlossary rdf:datatype="http://www.w3.org/2001/XMLSchema#boolean">true</isInISTQBGlossary>
        <rdfs:label>experience-based testing</rdfs:label>
        <skos:altLabel xml:lang="en">experience based testing
experience-based test technique
experience based test technique</skos:altLabel>
        <skos:prefLabel xml:lang="en">experience-based testing</skos:prefLabel>
    </owl:NamedIndividual>
    


    <!-- http://purl.org/stc/terms#experience_based_test_metric -->

    <owl:NamedIndividual rdf:about="http://purl.org/stc/terms#experience_based_test_metric">
        <terms:hasParent rdf:resource="http://purl.org/stc/terms#coverage"/>
        <isInISTQBGlossary rdf:datatype="http://www.w3.org/2001/XMLSchema#boolean">false</isInISTQBGlossary>
        <rdfs:comment xml:lang="en">There is currently no industry agreed approach to calculating experience-based coverage. (ISO/IEC/IEEE 29119-4)</rdfs:comment>
        <rdfs:label>experience coverage</rdfs:label>
        <rdfs:seeAlso>ISO/IEC/IEEE 29119-4 (Software and systems engineering — Software testing — Part 4: Test techniques)</rdfs:seeAlso>
        <skos:altLabel xml:lang="en">experience based test metric</skos:altLabel>
        <skos:altLabel xml:lang="en">experience based test metric
experience-based test metric</skos:altLabel>
        <skos:prefLabel xml:lang="en">experience coverage</skos:prefLabel>
    </owl:NamedIndividual>
    


    <!-- http://purl.org/stc/terms#exploratory_testing -->

    <owl:NamedIndividual rdf:about="http://purl.org/stc/terms#exploratory_testing">
        <terms:hasParent rdf:resource="http://purl.org/stc/terms#method_orientation_in_test_approach"/>
        <isInISTQBGlossary rdf:datatype="http://www.w3.org/2001/XMLSchema#boolean">true</isInISTQBGlossary>
        <rdfs:comment xml:lang="en">An approach to testing in which the testers dynamically design and execute tests based on their knowledge, exploration of the test item and the results of previous tests. (ISTQB Glossary v4.5)</rdfs:comment>
        <rdfs:label>exploratory testing</rdfs:label>
        <rdfs:seeAlso>ISO/IEC/IEEE 29119-1:2022 (Software and systems engineering — Software testing — Part 1: Concepts and definitions)

Foundation - v4.0
Advanced Test Analyst - v3.1</rdfs:seeAlso>
        <skos:prefLabel xml:lang="en">exploratory testing</skos:prefLabel>
    </owl:NamedIndividual>
    


    <!-- http://purl.org/stc/terms#failure -->

    <owl:NamedIndividual rdf:about="http://purl.org/stc/terms#failure">
        <terms:hasParent rdf:resource="http://purl.org/stc/terms#basic_concepts"/>
    </owl:NamedIndividual>
    


    <!-- http://purl.org/stc/terms#feature-driven_development -->

    <owl:NamedIndividual rdf:about="http://purl.org/stc/terms#feature-driven_development">
        <terms:hasParent rdf:resource="http://purl.org/stc/terms#target_orientation_in_software_development"/>
        <isInISTQBGlossary rdf:datatype="http://www.w3.org/2001/XMLSchema#boolean">true</isInISTQBGlossary>
        <rdfs:label>feature-driven development</rdfs:label>
        <skos:prefLabel xml:lang="en">feature-driven development</skos:prefLabel>
    </owl:NamedIndividual>
    


    <!-- http://purl.org/stc/terms#formal_review -->

    <owl:NamedIndividual rdf:about="http://purl.org/stc/terms#formal_review">
        <terms:hasParent rdf:resource="http://purl.org/stc/terms#review"/>
        <rdfs:label>formal review</rdfs:label>
        <skos:prefLabel xml:lang="en">formal review</skos:prefLabel>
    </owl:NamedIndividual>
    


    <!-- http://purl.org/stc/terms#functional_testing -->

    <owl:NamedIndividual rdf:about="http://purl.org/stc/terms#functional_testing">
        <terms:hasParent rdf:resource="http://purl.org/stc/terms#test_type"/>
        <isInISTQBGlossary rdf:datatype="http://www.w3.org/2001/XMLSchema#boolean">true</isInISTQBGlossary>
        <rdfs:comment xml:lang="en">Testing performed to evaluate if a component or system satisfies functional requirements. (ISTQB Glossary v4.5)</rdfs:comment>
        <rdfs:label>functional testing</rdfs:label>
        <rdfs:seeAlso>Foundation - v4.0
Advanced Test Management - v3.0
Advanced Test Analyst - v4.0
Specialist - Game Testing - v1.0.1</rdfs:seeAlso>
        <skos:prefLabel xml:lang="en">functional testing</skos:prefLabel>
    </owl:NamedIndividual>
    


    <!-- http://purl.org/stc/terms#fundamental_test_process -->

    <owl:NamedIndividual rdf:about="http://purl.org/stc/terms#fundamental_test_process">
        <terms:hasParent rdf:resource="http://purl.org/stc/terms#test_process"/>
        <isInISTQBGlossary rdf:datatype="http://www.w3.org/2001/XMLSchema#boolean">false</isInISTQBGlossary>
        <rdfs:label>fundamental test process</rdfs:label>
        <skos:prefLabel xml:lang="en">fundamental test process</skos:prefLabel>
    </owl:NamedIndividual>
    


    <!-- http://purl.org/stc/terms#gambling_testing -->

    <owl:NamedIndividual rdf:about="http://purl.org/stc/terms#gambling_testing">
        <terms:hasParent rdf:resource="http://purl.org/stc/terms#domain-specific_test_types"/>
        <isInISTQBGlossary rdf:datatype="http://www.w3.org/2001/XMLSchema#boolean">false</isInISTQBGlossary>
        <rdfs:label>gambling testing</rdfs:label>
        <skos:prefLabel xml:lang="en">gambling testing</skos:prefLabel>
    </owl:NamedIndividual>
    


    <!-- http://purl.org/stc/terms#grey_box_test_technique -->

    <owl:NamedIndividual rdf:about="http://purl.org/stc/terms#grey_box_test_technique">
        <terms:hasParent rdf:resource="http://purl.org/stc/terms#test_technique"/>
        <isInISTQBGlossary rdf:datatype="http://www.w3.org/2001/XMLSchema#boolean">true</isInISTQBGlossary>
        <rdfs:label>grey-box testing</rdfs:label>
        <skos:altLabel xml:lang="en">grey box testing
gray-box testing
gray box testing</skos:altLabel>
        <skos:prefLabel xml:lang="en">grey-box testing</skos:prefLabel>
    </owl:NamedIndividual>
    


    <!-- http://purl.org/stc/terms#high_level_test_case -->

    <owl:NamedIndividual rdf:about="http://purl.org/stc/terms#high_level_test_case">
        <terms:hasParent rdf:resource="http://purl.org/stc/terms#test_case"/>
        <isInISTQBGlossary rdf:datatype="http://www.w3.org/2001/XMLSchema#boolean">true</isInISTQBGlossary>
        <rdfs:comment xml:lang="en">A test case with abstract preconditions, input data, expected results, postconditions, and actions (where applicable). (ISTQB Glossary v4.5)</rdfs:comment>
        <rdfs:label>high-level test case</rdfs:label>
        <rdfs:seeAlso>Advanced Test Manager - 2012
Advanced Test Analyst - v3.1
Advanced Test Analyst - v4.0</rdfs:seeAlso>
        <skos:altLabel>high level test case
logical test case
abstract test case
high level testcase
logical testcase
abstract testcase</skos:altLabel>
        <skos:prefLabel xml:lang="en">high-level test case</skos:prefLabel>
    </owl:NamedIndividual>
    


    <!-- http://purl.org/stc/terms#incremental_software_development -->

    <owl:NamedIndividual rdf:about="http://purl.org/stc/terms#incremental_software_development">
        <terms:hasParent rdf:resource="http://purl.org/stc/terms#process_orientation_in_software_development"/>
        <isInISTQBGlossary rdf:datatype="http://www.w3.org/2001/XMLSchema#boolean">false</isInISTQBGlossary>
        <rdfs:label>incremental</rdfs:label>
        <skos:prefLabel xml:lang="en">incremental software development</skos:prefLabel>
    </owl:NamedIndividual>
    


    <!-- http://purl.org/stc/terms#informal_review -->

    <owl:NamedIndividual rdf:about="http://purl.org/stc/terms#informal_review">
        <terms:hasParent rdf:resource="http://purl.org/stc/terms#review"/>
        <rdfs:label>informal review</rdfs:label>
        <skos:prefLabel xml:lang="en">informal review</skos:prefLabel>
    </owl:NamedIndividual>
    


    <!-- http://purl.org/stc/terms#inspection -->

    <owl:NamedIndividual rdf:about="http://purl.org/stc/terms#inspection">
        <terms:hasParent rdf:resource="http://purl.org/stc/terms#formal_review"/>
        <isInISTQBGlossary rdf:datatype="http://www.w3.org/2001/XMLSchema#boolean">true</isInISTQBGlossary>
        <rdfs:comment xml:lang="en">A type of formal review that uses defined team roles and measurement to identify defects in a work product, and improve the review process and the software development process. (ISTQB Glossary v4.5)</rdfs:comment>
        <rdfs:label>inspection</rdfs:label>
        <rdfs:seeAlso>Foundation - v4.0
Advanced Test Manager - 2012</rdfs:seeAlso>
        <skos:prefLabel xml:lang="en">inspection</skos:prefLabel>
    </owl:NamedIndividual>
    


    <!-- http://purl.org/stc/terms#integration -->

    <owl:NamedIndividual rdf:about="http://purl.org/stc/terms#integration">
        <terms:hasParent rdf:resource="http://purl.org/stc/terms#software_engineering_activity"/>
    </owl:NamedIndividual>
    


    <!-- http://purl.org/stc/terms#integration_testing -->

    <owl:NamedIndividual rdf:about="http://purl.org/stc/terms#integration_testing">
        <terms:hasParent rdf:resource="http://purl.org/stc/terms#test_level"/>
        <isInISTQBGlossary rdf:datatype="http://www.w3.org/2001/XMLSchema#boolean">true</isInISTQBGlossary>
        <rdfs:label>integration testing</rdfs:label>
        <skos:prefLabel xml:lang="en">integration testing</skos:prefLabel>
    </owl:NamedIndividual>
    


    <!-- http://purl.org/stc/terms#interactive_application_security_testing -->

    <owl:NamedIndividual rdf:about="http://purl.org/stc/terms#interactive_application_security_testing">
        <terms:hasParent rdf:resource="http://purl.org/stc/terms#security_testing"/>
        <isInISTQBGlossary rdf:datatype="http://www.w3.org/2001/XMLSchema#boolean">true</isInISTQBGlossary>
        <rdfs:label>interactive application security testing</rdfs:label>
        <skos:prefLabel xml:lang="en">interactive application security testing</skos:prefLabel>
    </owl:NamedIndividual>
    


    <!-- http://purl.org/stc/terms#interface_testing -->

    <owl:NamedIndividual rdf:about="http://purl.org/stc/terms#interface_testing">
        <terms:hasParent rdf:resource="http://purl.org/stc/terms#target_orientation_in_test_approach"/>
        <isInISTQBGlossary rdf:datatype="http://www.w3.org/2001/XMLSchema#boolean">true</isInISTQBGlossary>
        <rdfs:label>interface testing</rdfs:label>
        <skos:prefLabel xml:lang="en">interface testing</skos:prefLabel>
    </owl:NamedIndividual>
    


    <!-- http://purl.org/stc/terms#interoperability_testing -->

    <owl:NamedIndividual rdf:about="http://purl.org/stc/terms#interoperability_testing">
        <terms:hasParent rdf:resource="http://purl.org/stc/terms#protocol_or_service_testing"/>
        <isInISTQBGlossary rdf:datatype="http://www.w3.org/2001/XMLSchema#boolean">false</isInISTQBGlossary>
        <rdfs:comment xml:lang="en">Testing conducted to ensure that a modified system retains the capability of exchanging information with systems of different types, and of using that information (ISO/IEC/IEEE 24765:2017)</rdfs:comment>
        <rdfs:label>interoperability testing</rdfs:label>
        <rdfs:seeAlso>ISO/IEC/IEEE 24765:2017 (Systems and software engineering —
Vocabulary)</rdfs:seeAlso>
        <skos:prefLabel xml:lang="en">interoperability testing</skos:prefLabel>
    </owl:NamedIndividual>
    


    <!-- http://purl.org/stc/terms#iterative_software_development -->

    <owl:NamedIndividual rdf:about="http://purl.org/stc/terms#iterative_software_development">
        <terms:hasParent rdf:resource="http://purl.org/stc/terms#process_orientation_in_software_development"/>
        <isInISTQBGlossary rdf:datatype="http://www.w3.org/2001/XMLSchema#boolean">true</isInISTQBGlossary>
        <rdfs:label>iterative</rdfs:label>
        <skos:prefLabel xml:lang="en">iterative software development</skos:prefLabel>
    </owl:NamedIndividual>
    


    <!-- http://purl.org/stc/terms#level_test_plan -->

    <owl:NamedIndividual rdf:about="http://purl.org/stc/terms#level_test_plan">
        <terms:hasParent rdf:resource="http://purl.org/stc/terms#test_plan"/>
        <isInISTQBGlossary rdf:datatype="http://www.w3.org/2001/XMLSchema#boolean">true</isInISTQBGlossary>
        <rdfs:comment xml:lang="en">A test plan that typically addresses one test level. (ISTQB Glossary v4.5)</rdfs:comment>
        <rdfs:label>level test plan</rdfs:label>
        <rdfs:seeAlso>Advanced Test Manager - 2012</rdfs:seeAlso>
        <skos:altLabel xml:lang="en">level testplan</skos:altLabel>
        <skos:prefLabel xml:lang="en">level test plan</skos:prefLabel>
    </owl:NamedIndividual>
    


    <!-- http://purl.org/stc/terms#load_testing -->

    <owl:NamedIndividual rdf:about="http://purl.org/stc/terms#load_testing">
        <terms:hasParent rdf:resource="http://purl.org/stc/terms#performance_testing"/>
        <isInISTQBGlossary rdf:datatype="http://www.w3.org/2001/XMLSchema#boolean">true</isInISTQBGlossary>
        <rdfs:label>load testing</rdfs:label>
        <skos:prefLabel xml:lang="en">load testing</skos:prefLabel>
    </owl:NamedIndividual>
    


    <!-- http://purl.org/stc/terms#low_level_test_case -->

    <owl:NamedIndividual rdf:about="http://purl.org/stc/terms#low_level_test_case">
        <terms:hasParent rdf:resource="http://purl.org/stc/terms#test_case"/>
        <isInISTQBGlossary rdf:datatype="http://www.w3.org/2001/XMLSchema#boolean">true</isInISTQBGlossary>
        <rdfs:comment xml:lang="en">A test case with concrete values for preconditions, input data, expected results, postconditions, and a detailed description of actions (where applicable). (ISTQB Glossary v4.5)</rdfs:comment>
        <rdfs:label>low-level test case</rdfs:label>
        <rdfs:seeAlso>Advanced Test Analyst - v3.1
Advanced Test Analyst - v4.0</rdfs:seeAlso>
        <skos:altLabel xml:lang="en">low level test case
concrete test case
physical test case
low level testcase
concrete testcase
physical testcase</skos:altLabel>
        <skos:prefLabel xml:lang="en">low-level test case</skos:prefLabel>
    </owl:NamedIndividual>
    


    <!-- http://purl.org/stc/terms#maintenance -->

    <owl:NamedIndividual rdf:about="http://purl.org/stc/terms#maintenance">
        <terms:hasParent rdf:resource="http://purl.org/stc/terms#software_lifecycle"/>
    </owl:NamedIndividual>
    


    <!-- http://purl.org/stc/terms#maintenance_testing -->

    <owl:NamedIndividual rdf:about="http://purl.org/stc/terms#maintenance_testing">
        <terms:hasParent rdf:resource="http://purl.org/stc/terms#change_orientation_in_test_approach"/>
        <isInISTQBGlossary rdf:datatype="http://www.w3.org/2001/XMLSchema#boolean">true</isInISTQBGlossary>
        <rdfs:comment xml:lang="en">Testing the changes to an operational system or the impact of a changed environment to an operational system. (ISTQB Glossary v4.5)</rdfs:comment>
        <rdfs:label>maintenance testing</rdfs:label>
        <rdfs:seeAlso>Foundation - v4.0</rdfs:seeAlso>
        <skos:prefLabel xml:lang="en">maintenance testing</skos:prefLabel>
    </owl:NamedIndividual>
    


    <!-- http://purl.org/stc/terms#manual_testing -->

    <owl:NamedIndividual rdf:about="http://purl.org/stc/terms#manual_testing">
        <terms:hasParent rdf:resource="http://purl.org/stc/terms#test_execution"/>
        <isInISTQBGlossary rdf:datatype="http://www.w3.org/2001/XMLSchema#boolean">false</isInISTQBGlossary>
        <rdfs:comment xml:lang="en">Humans performing tests by entering information into a test item and verifying the results. (ISO/IEC/IEEE 29119-1:2022)</rdfs:comment>
        <rdfs:comment xml:lang="en">ISO/IEC/IEEE 29119-1:2022 (Software and systems engineering — Software testing — Part 1: Concepts and definitions)</rdfs:comment>
        <rdfs:label>manual testing</rdfs:label>
        <skos:altLabel>unscripted testing</skos:altLabel>
        <skos:prefLabel xml:lang="en">manual testing</skos:prefLabel>
    </owl:NamedIndividual>
    


    <!-- http://purl.org/stc/terms#master_test_plan -->

    <owl:NamedIndividual rdf:about="http://purl.org/stc/terms#master_test_plan">
        <terms:hasParent rdf:resource="http://purl.org/stc/terms#test_plan"/>
        <isInISTQBGlossary rdf:datatype="http://www.w3.org/2001/XMLSchema#boolean">true</isInISTQBGlossary>
        <rdfs:comment xml:lang="en">A test plan that is used to coordinate multiple test levels or test types. (ISTQB Glossary v4.5)</rdfs:comment>
        <rdfs:label>master test plan</rdfs:label>
        <rdfs:seeAlso>Advanced Test Manager - 2012</rdfs:seeAlso>
        <skos:altLabel xml:lang="en">master testplan</skos:altLabel>
        <skos:prefLabel xml:lang="en">master test plan</skos:prefLabel>
    </owl:NamedIndividual>
    


    <!-- http://purl.org/stc/terms#math_testing -->

    <owl:NamedIndividual rdf:about="http://purl.org/stc/terms#math_testing">
        <terms:hasParent rdf:resource="http://purl.org/stc/terms#gambling_testing"/>
        <isInISTQBGlossary rdf:datatype="http://www.w3.org/2001/XMLSchema#boolean">true</isInISTQBGlossary>
        <rdfs:label>math testing</rdfs:label>
        <skos:prefLabel xml:lang="en">math testing</skos:prefLabel>
    </owl:NamedIndividual>
    


    <!-- http://purl.org/stc/terms#method_orientation_in_test_approach -->

    <owl:NamedIndividual rdf:about="http://purl.org/stc/terms#method_orientation_in_test_approach">
        <terms:hasParent rdf:resource="http://purl.org/stc/terms#test_approach"/>
        <isInISTQBGlossary rdf:datatype="http://www.w3.org/2001/XMLSchema#boolean">false</isInISTQBGlossary>
        <rdfs:label>method orientation</rdfs:label>
        <skos:prefLabel xml:lang="en">method orientation in test approach</skos:prefLabel>
    </owl:NamedIndividual>
    


    <!-- http://purl.org/stc/terms#metric -->

    <owl:NamedIndividual rdf:about="http://purl.org/stc/terms#metric">
        <terms:hasParent rdf:resource="http://purl.org/stc/terms#basic_concepts"/>
        <isInISTQBGlossary rdf:datatype="http://www.w3.org/2001/XMLSchema#boolean">true</isInISTQBGlossary>
        <rdfs:comment xml:lang="en">A measurement scale and the method used for measurement. (ISTQB Glossary v4.5) 

A quantitative measure of the degree to which a system, component, or process possesses a given attribute. (ISO/IEC/IEEE 24765:2017)</rdfs:comment>
        <rdfs:label>metric</rdfs:label>
        <rdfs:seeAlso>ISO/IEC/IEEE 24765:2017 (Systems and Software Engineering – Vocabulary)

Foundation - v4.0
Advanced Test Manager - 2012
Advanced Test Management - v3.0
Advanced Test Analyst - v3.1
Advanced Test Analyst - v4.0
Advanced Technical Test Analyst - v4.0
Advanced Test Automation Engineering - v2.0
Expert Improving the Test Process - 2011
Expert Test Management - 2011
Foundation Agile Tester - 2014
Advanced Agile Technical Tester - 2019
Agile Test Leadership at Scale - v1.0
Specialist - Acceptance Testing - 2019
Specialist - Agile Test Leadership at Scale - v2.0
Specialist - AI Testing - v1.0
Specialist - Automotive Software Tester - 2018
Specialist - Automotive Software Tester - v1.1
Specialist - Gambling Industry Tester - 2018
Specialist - Game Testing - v1.0.1
Specialist - Model-Based Tester - 2015
Specialist - Model-Based Testing - v1.1
Specialist - Performance Testing - 2018
Specialist - Security Tester - 2016
Specialist - Security Test Engineer - v1.0
Specialist - Test Automation Engineer - 2016
Specialist - Test Automation Strategy - v1.0</rdfs:seeAlso>
        <skos:prefLabel xml:lang="en">metric</skos:prefLabel>
    </owl:NamedIndividual>
    


    <!-- http://purl.org/stc/terms#mobile_app_testing -->

    <owl:NamedIndividual rdf:about="http://purl.org/stc/terms#mobile_app_testing">
        <terms:hasParent rdf:resource="http://purl.org/stc/terms#domain-specific_test_types"/>
        <isInISTQBGlossary rdf:datatype="http://www.w3.org/2001/XMLSchema#boolean">false</isInISTQBGlossary>
        <rdfs:label>mobile app testing</rdfs:label>
        <skos:altLabel xml:lang="en">mobile application testing</skos:altLabel>
        <skos:prefLabel xml:lang="en">mobile app testing</skos:prefLabel>
    </owl:NamedIndividual>
    


    <!-- http://purl.org/stc/terms#model -->

    <owl:NamedIndividual rdf:about="http://purl.org/stc/terms#model">
        <terms:hasParent rdf:resource="http://purl.org/stc/terms#basic_concepts"/>
    </owl:NamedIndividual>
    


    <!-- http://purl.org/stc/terms#model_based_testing -->

    <owl:NamedIndividual rdf:about="http://purl.org/stc/terms#model_based_testing">
        <terms:hasParent rdf:resource="http://purl.org/stc/terms#black_box_test_technique"/>
        <isInISTQBGlossary rdf:datatype="http://www.w3.org/2001/XMLSchema#boolean">true</isInISTQBGlossary>
        <rdfs:comment xml:lang="en">Testing based on or involving models. (ISTQB Glossary v4.5)</rdfs:comment>
        <rdfs:label>model-based testing</rdfs:label>
        <rdfs:seeAlso>Advanced Test Analyst - v4.0
Advanced Technical Test Analyst - v4.0
Advanced Test Automation Engineering - v2.0
Specialist - Acceptance Testing - 2019
Specialist - Model-Based Tester - 2015
Specialist - Model-Based Testing - v1.1
Specialist - Test Automation Engineer - 2016</rdfs:seeAlso>
        <skos:altLabel xml:lang="en">model based testing
mbt
MBT
model driven testing
model-driven testing
mdt
MDT</skos:altLabel>
        <skos:prefLabel xml:lang="en">model-based testing</skos:prefLabel>
    </owl:NamedIndividual>
    


    <!-- http://purl.org/stc/terms#model_coverage -->

    <owl:NamedIndividual rdf:about="http://purl.org/stc/terms#model_coverage">
        <terms:hasParent rdf:resource="http://purl.org/stc/terms#specification_coverage"/>
        <isInISTQBGlossary rdf:datatype="http://www.w3.org/2001/XMLSchema#boolean">true</isInISTQBGlossary>
        <rdfs:comment xml:lang="en">The coverage of model elements. (ISTQB Glossary v4.5)</rdfs:comment>
        <rdfs:label>model coverage</rdfs:label>
        <rdfs:seeAlso>Specialist - Model-Based Testing - v1.1</rdfs:seeAlso>
        <skos:prefLabel xml:lang="en">model coverage</skos:prefLabel>
    </owl:NamedIndividual>
    


    <!-- http://purl.org/stc/terms#model_verification -->

    <owl:NamedIndividual rdf:about="http://purl.org/stc/terms#model_verification">
        <terms:hasParent rdf:resource="http://purl.org/stc/terms#static_testing"/>
        <isInISTQBGlossary rdf:datatype="http://www.w3.org/2001/XMLSchema#boolean">false</isInISTQBGlossary>
        <rdfs:comment xml:lang="en">The process of determining that a model accurately represents the required conceptual description and specifications. (own)</rdfs:comment>
        <rdfs:label>model verification</rdfs:label>
        <skos:prefLabel xml:lang="en">model verification</skos:prefLabel>
    </owl:NamedIndividual>
    


    <!-- http://purl.org/stc/terms#modified_condition_decision_coverage -->

    <owl:NamedIndividual rdf:about="http://purl.org/stc/terms#modified_condition_decision_coverage">
        <terms:hasParent rdf:resource="http://purl.org/stc/terms#structural_coverage"/>
        <isInISTQBGlossary rdf:datatype="http://www.w3.org/2001/XMLSchema#boolean">true</isInISTQBGlossary>
        <rdfs:comment xml:lang="en">The coverage of all outcomes of the atomic conditions that independently affect the overall decision outcome. (ISTQB Glossary v4.5)

Coverage for modified condition/decision coverage testing. (ISO/IEC/IEEE 29119-4)</rdfs:comment>
        <rdfs:label>modified condition/decision coverage</rdfs:label>
        <rdfs:seeAlso>ISO/IEC/IEEE 29119-4 (Software and systems engineering — Software testing — Part 4: Test techniques)</rdfs:seeAlso>
        <skos:altLabel xml:lang="en">mc/dc
MC/DC
condition determination coverage
modified multiple condition coverage</skos:altLabel>
        <skos:prefLabel xml:lang="en">modified condition/decision coverage</skos:prefLabel>
    </owl:NamedIndividual>
    


    <!-- http://purl.org/stc/terms#multiple_condition_coverage -->

    <owl:NamedIndividual rdf:about="http://purl.org/stc/terms#multiple_condition_coverage">
        <terms:hasParent rdf:resource="http://purl.org/stc/terms#structural_coverage"/>
        <isInISTQBGlossary rdf:datatype="http://www.w3.org/2001/XMLSchema#boolean">true</isInISTQBGlossary>
        <rdfs:comment xml:lang="en">The coverage of all possible combinations of all single condition outcomes within one statement. (ISTQB Glossary v4.5)

Coverage for branch condition combination testing. (ISO/IEC/IEEE 29119-4 as branch condition combination coverage)</rdfs:comment>
        <rdfs:label>multiple condition coverage</rdfs:label>
        <rdfs:seeAlso>ISO/IEC/IEEE 29119-4 (Software and systems engineering — Software testing — Part 4: Test techniques)</rdfs:seeAlso>
        <skos:altLabel>branch condition combination coverage
condition combination coverage</skos:altLabel>
        <skos:prefLabel xml:lang="en">multiple condition coverage</skos:prefLabel>
    </owl:NamedIndividual>
    


    <!-- http://purl.org/stc/terms#neuron_coverage -->

    <owl:NamedIndividual rdf:about="http://purl.org/stc/terms#neuron_coverage">
        <terms:hasParent rdf:resource="http://purl.org/stc/terms#LLM_structural_coverage"/>
        <isInISTQBGlossary rdf:datatype="http://www.w3.org/2001/XMLSchema#boolean">true</isInISTQBGlossary>
        <rdfs:comment xml:lang="en">The coverage of activated neurons in the neural network for a set of tests. (ISTQB Glossary v4.5)</rdfs:comment>
        <rdfs:label>neuron coverage</rdfs:label>
        <rdfs:seeAlso>Specialist - AI Testing - v1.0</rdfs:seeAlso>
        <skos:prefLabel xml:lang="en">neuron coverage</skos:prefLabel>
    </owl:NamedIndividual>
    


    <!-- http://purl.org/stc/terms#non-functional_testing -->

    <owl:NamedIndividual rdf:about="http://purl.org/stc/terms#non-functional_testing">
        <terms:hasParent rdf:resource="http://purl.org/stc/terms#test_type"/>
        <isInISTQBGlossary rdf:datatype="http://www.w3.org/2001/XMLSchema#boolean">true</isInISTQBGlossary>
        <rdfs:comment xml:lang="en">Testing performed to evaluate that a component or system complies with non-functional requirements. (ISTQB Glossary v4.5)</rdfs:comment>
        <rdfs:label>non-functional testing</rdfs:label>
        <rdfs:seeAlso>Foundation - v4.0
Advanced Test Management - v3.0</rdfs:seeAlso>
        <skos:altLabel xml:lang="en">extra-functional testing</skos:altLabel>
        <skos:prefLabel xml:lang="en">non-functional testing</skos:prefLabel>
    </owl:NamedIndividual>
    


    <!-- http://purl.org/stc/terms#operation -->

    <owl:NamedIndividual rdf:about="http://purl.org/stc/terms#operation">
        <terms:hasParent rdf:resource="http://purl.org/stc/terms#software_lifecycle"/>
    </owl:NamedIndividual>
    


    <!-- http://purl.org/stc/terms#oracle_orientation_in_test_approach -->

    <owl:NamedIndividual rdf:about="http://purl.org/stc/terms#oracle_orientation_in_test_approach">
        <terms:hasParent rdf:resource="http://purl.org/stc/terms#test_approach"/>
        <isInISTQBGlossary rdf:datatype="http://www.w3.org/2001/XMLSchema#boolean">false</isInISTQBGlossary>
        <rdfs:label>oracle orientation</rdfs:label>
        <skos:prefLabel xml:lang="en">oracle orientation in test approach</skos:prefLabel>
    </owl:NamedIndividual>
    


    <!-- http://purl.org/stc/terms#pair_testing -->

    <owl:NamedIndividual rdf:about="http://purl.org/stc/terms#pair_testing">
        <terms:hasParent rdf:resource="http://purl.org/stc/terms#tester_orientation_in_test_approach"/>
        <isInISTQBGlossary rdf:datatype="http://www.w3.org/2001/XMLSchema#boolean">true</isInISTQBGlossary>
        <rdfs:label>pair testing</rdfs:label>
        <skos:prefLabel xml:lang="en">pair testing</skos:prefLabel>
    </owl:NamedIndividual>
    


    <!-- http://purl.org/stc/terms#peer_review -->

    <owl:NamedIndividual rdf:about="http://purl.org/stc/terms#peer_review">
        <terms:hasParent rdf:resource="http://purl.org/stc/terms#informal_review"/>
        <isInISTQBGlossary rdf:datatype="http://www.w3.org/2001/XMLSchema#boolean">true</isInISTQBGlossary>
        <rdfs:comment xml:lang="en">A type of review performed on a work product by persons that have the abilities required to create it.  (ISTQB Glossary v4.5)</rdfs:comment>
        <rdfs:label>peer review</rdfs:label>
        <rdfs:seeAlso></rdfs:seeAlso>
        <skos:prefLabel xml:lang="en">peer review</skos:prefLabel>
    </owl:NamedIndividual>
    


    <!-- http://purl.org/stc/terms#performance_testing -->

    <owl:NamedIndividual rdf:about="http://purl.org/stc/terms#performance_testing">
        <terms:hasParent rdf:resource="http://purl.org/stc/terms#non-functional_testing"/>
        <isInISTQBGlossary rdf:datatype="http://www.w3.org/2001/XMLSchema#boolean">true</isInISTQBGlossary>
        <rdfs:label>performance testing</rdfs:label>
        <skos:prefLabel xml:lang="en">performance testing</skos:prefLabel>
    </owl:NamedIndividual>
    


    <!-- http://purl.org/stc/terms#process_improvement -->

    <owl:NamedIndividual rdf:about="http://purl.org/stc/terms#process_improvement">
        <terms:hasParent rdf:resource="http://purl.org/stc/terms#support_processes"/>
    </owl:NamedIndividual>
    


    <!-- http://purl.org/stc/terms#process_orientation_in_software_development -->

    <owl:NamedIndividual rdf:about="http://purl.org/stc/terms#process_orientation_in_software_development">
        <terms:hasParent rdf:resource="http://purl.org/stc/terms#software_development_model"/>
        <isInISTQBGlossary rdf:datatype="http://www.w3.org/2001/XMLSchema#boolean">false</isInISTQBGlossary>
        <rdfs:label>process orientation</rdfs:label>
        <skos:prefLabel xml:lang="en">process orientation in software development</skos:prefLabel>
    </owl:NamedIndividual>
    


    <!-- http://purl.org/stc/terms#process_orientation_in_test_approach -->

    <owl:NamedIndividual rdf:about="http://purl.org/stc/terms#process_orientation_in_test_approach">
        <terms:hasParent rdf:resource="http://purl.org/stc/terms#test_approach"/>
        <isInISTQBGlossary rdf:datatype="http://www.w3.org/2001/XMLSchema#boolean">false</isInISTQBGlossary>
        <rdfs:label>process orientation</rdfs:label>
        <skos:prefLabel xml:lang="en">process orientation in test approach</skos:prefLabel>
    </owl:NamedIndividual>
    


    <!-- http://purl.org/stc/terms#project_management -->

    <owl:NamedIndividual rdf:about="http://purl.org/stc/terms#project_management">
        <terms:hasParent rdf:resource="http://purl.org/stc/terms#support_processes"/>
    </owl:NamedIndividual>
    


    <!-- http://purl.org/stc/terms#property-based_testing -->

    <owl:NamedIndividual rdf:about="http://purl.org/stc/terms#property-based_testing">
        <terms:hasParent rdf:resource="http://purl.org/stc/terms#target_orientation_in_test_approach"/>
        <isInISTQBGlossary rdf:datatype="http://www.w3.org/2001/XMLSchema#boolean">true</isInISTQBGlossary>
        <rdfs:label>property-based testing</rdfs:label>
        <skos:prefLabel xml:lang="en">property-based testing</skos:prefLabel>
    </owl:NamedIndividual>
    


    <!-- http://purl.org/stc/terms#protocol_or_service_testing -->

    <owl:NamedIndividual rdf:about="http://purl.org/stc/terms#protocol_or_service_testing">
        <terms:hasParent rdf:resource="http://purl.org/stc/terms#domain-specific_test_types"/>
        <isInISTQBGlossary rdf:datatype="http://www.w3.org/2001/XMLSchema#boolean">false</isInISTQBGlossary>
        <rdfs:label>protocol or service testing</rdfs:label>
        <skos:prefLabel xml:lang="en">protocol or service testing</skos:prefLabel>
    </owl:NamedIndividual>
    


    <!-- http://purl.org/stc/terms#quality_assurance -->

    <owl:NamedIndividual rdf:about="http://purl.org/stc/terms#quality_assurance">
        <terms:hasParent rdf:resource="http://purl.org/stc/terms#support_processes"/>
    </owl:NamedIndividual>
    


    <!-- http://purl.org/stc/terms#reactive_testing -->

    <owl:NamedIndividual rdf:about="http://purl.org/stc/terms#reactive_testing">
        <terms:hasParent rdf:resource="http://purl.org/stc/terms#dynamic_testing"/>
        <isInISTQBGlossary rdf:datatype="http://www.w3.org/2001/XMLSchema#boolean">true</isInISTQBGlossary>
        <rdfs:label>reactive testing</rdfs:label>
        <skos:prefLabel xml:lang="en">reactive testing</skos:prefLabel>
    </owl:NamedIndividual>
    


    <!-- http://purl.org/stc/terms#regression_testing -->

    <owl:NamedIndividual rdf:about="http://purl.org/stc/terms#regression_testing">
        <terms:hasParent rdf:resource="http://purl.org/stc/terms#change_orientation_in_test_approach"/>
        <isInISTQBGlossary rdf:datatype="http://www.w3.org/2001/XMLSchema#boolean">true</isInISTQBGlossary>
        <rdfs:comment xml:lang="en">A type of change-related testing to detect whether defects have been introduced or uncovered in unchanged areas of the software. (ISTQB Glossary v4.5)

Testingperformed following modifications to a test item or to its operational environment, to identify whether failures in unmodified parts of the test item occur. (ISO/IEC/IEEE 29119-1:2022)</rdfs:comment>
        <rdfs:label>regression testing</rdfs:label>
        <rdfs:seeAlso>ISO/IEC/IEEE 29119-1:2022 (Software and systems engineering — Software testing — Part 1: Concepts and definitions)

Foundation - v4.0
Advanced Test Analyst - v4.0
Specialist - Test Automation Engineer - 2016</rdfs:seeAlso>
        <skos:prefLabel xml:lang="en">regression testing</skos:prefLabel>
    </owl:NamedIndividual>
    


    <!-- http://purl.org/stc/terms#regulatory_acceptance_testing -->

    <owl:NamedIndividual rdf:about="http://purl.org/stc/terms#regulatory_acceptance_testing">
        <terms:hasParent rdf:resource="http://purl.org/stc/terms#acceptance_testing"/>
        <isInISTQBGlossary rdf:datatype="http://www.w3.org/2001/XMLSchema#boolean">true</isInISTQBGlossary>
        <rdfs:label>regulatory acceptance testing</rdfs:label>
        <skos:prefLabel xml:lang="en">regulatory acceptance testing</skos:prefLabel>
    </owl:NamedIndividual>
    


    <!-- http://purl.org/stc/terms#related_to_role -->

    <owl:NamedIndividual rdf:about="http://purl.org/stc/terms#related_to_role">
        <terms:hasParent rdf:resource="http://purl.org/stc/terms#test_work_force"/>
        <isInISTQBGlossary rdf:datatype="http://www.w3.org/2001/XMLSchema#boolean">false</isInISTQBGlossary>
        <rdfs:label>related to role</rdfs:label>
        <skos:prefLabel xml:lang="en">related to role</skos:prefLabel>
    </owl:NamedIndividual>
    


    <!-- http://purl.org/stc/terms#related_to_team -->

    <owl:NamedIndividual rdf:about="http://purl.org/stc/terms#related_to_team">
        <terms:hasParent rdf:resource="http://purl.org/stc/terms#test_work_force"/>
        <isInISTQBGlossary rdf:datatype="http://www.w3.org/2001/XMLSchema#boolean">false</isInISTQBGlossary>
        <rdfs:label>related to team</rdfs:label>
        <skos:prefLabel xml:lang="en">related to team</skos:prefLabel>
    </owl:NamedIndividual>
    


    <!-- http://purl.org/stc/terms#release -->

    <owl:NamedIndividual rdf:about="http://purl.org/stc/terms#release">
        <terms:hasParent rdf:resource="http://purl.org/stc/terms#software_lifecycle"/>
    </owl:NamedIndividual>
    


    <!-- http://purl.org/stc/terms#requirements-based_testing -->

    <owl:NamedIndividual rdf:about="http://purl.org/stc/terms#requirements-based_testing">
        <terms:hasParent rdf:resource="http://purl.org/stc/terms#black_box_test_technique"/>
        <isInISTQBGlossary rdf:datatype="http://www.w3.org/2001/XMLSchema#boolean">true</isInISTQBGlossary>
        <rdfs:label>requirements-based testing</rdfs:label>
        <skos:prefLabel xml:lang="en">requirements-based testing</skos:prefLabel>
    </owl:NamedIndividual>
    


    <!-- http://purl.org/stc/terms#requirements_coverage -->

    <owl:NamedIndividual rdf:about="http://purl.org/stc/terms#requirements_coverage">
        <terms:hasParent rdf:resource="http://purl.org/stc/terms#specification_coverage"/>
        <isInISTQBGlossary rdf:datatype="http://www.w3.org/2001/XMLSchema#boolean">false</isInISTQBGlossary>
        <rdfs:comment xml:lang="en">Number of requirements covered by executed tests (ISO/IEC/IEEE 29119-1:2022, defined as test coverage)</rdfs:comment>
        <rdfs:label>requirement coverage</rdfs:label>
        <rdfs:seeAlso>ISO/IEC/IEEE 29119-1:2022 (Software and systems engineering — Software testing — Part 1: Concepts and definitions)</rdfs:seeAlso>
        <skos:altLabel xml:lang="en">requirements coverage</skos:altLabel>
        <skos:prefLabel xml:lang="en">requirement coverage</skos:prefLabel>
    </owl:NamedIndividual>
    


    <!-- http://purl.org/stc/terms#requirements_engineering -->

    <owl:NamedIndividual rdf:about="http://purl.org/stc/terms#requirements_engineering">
        <terms:hasParent rdf:resource="http://purl.org/stc/terms#software_engineering_activity"/>
    </owl:NamedIndividual>
    


    <!-- http://purl.org/stc/terms#review -->

    <owl:NamedIndividual rdf:about="http://purl.org/stc/terms#review">
        <terms:hasParent rdf:resource="http://purl.org/stc/terms#static_testing"/>
    </owl:NamedIndividual>
    


    <!-- http://purl.org/stc/terms#risk-based_testing -->

    <owl:NamedIndividual rdf:about="http://purl.org/stc/terms#risk-based_testing">
        <terms:hasParent rdf:resource="http://purl.org/stc/terms#target_orientation_in_test_approach"/>
        <isInISTQBGlossary rdf:datatype="http://www.w3.org/2001/XMLSchema#boolean">true</isInISTQBGlossary>
        <rdfs:label>risk-based testing</rdfs:label>
        <skos:prefLabel xml:lang="en">risk-based testing</skos:prefLabel>
    </owl:NamedIndividual>
    


    <!-- http://purl.org/stc/terms#risk_oriented_metric -->

    <owl:NamedIndividual rdf:about="http://purl.org/stc/terms#risk_oriented_metric">
        <terms:hasParent rdf:resource="http://purl.org/stc/terms#test_metric"/>
        <isInISTQBGlossary rdf:datatype="http://www.w3.org/2001/XMLSchema#boolean">false</isInISTQBGlossary>
        <rdfs:label>risk oriented metric</rdfs:label>
        <skos:altLabel xml:lang="en">risk-oriented metric
risk metric</skos:altLabel>
        <skos:prefLabel xml:lang="en">risk oriented metric</skos:prefLabel>
    </owl:NamedIndividual>
    


    <!-- http://purl.org/stc/terms#safety_testing -->

    <owl:NamedIndividual rdf:about="http://purl.org/stc/terms#safety_testing">
        <terms:hasParent rdf:resource="http://purl.org/stc/terms#non-functional_testing"/>
        <isInISTQBGlossary rdf:datatype="http://www.w3.org/2001/XMLSchema#boolean">false</isInISTQBGlossary>
        <rdfs:label>safety testing</rdfs:label>
        <skos:prefLabel xml:lang="en">safety testing</skos:prefLabel>
    </owl:NamedIndividual>
    


    <!-- http://purl.org/stc/terms#scripted_testing -->

    <owl:NamedIndividual rdf:about="http://purl.org/stc/terms#scripted_testing">
        <terms:hasParent rdf:resource="http://purl.org/stc/terms#manual_testing"/>
        <isInISTQBGlossary rdf:datatype="http://www.w3.org/2001/XMLSchema#boolean">true</isInISTQBGlossary>
        <rdfs:comment xml:lang="en">Testing performed based on a documented test script. (ISO/IEC/IEEE 29119-1:2022)</rdfs:comment>
        <rdfs:label>scripted testing</rdfs:label>
        <rdfs:seeAlso>ISO/IEC/IEEE 29119-1:2022 (Software and systems engineering — Software testing — Part 1: Concepts and definitions)</rdfs:seeAlso>
        <skos:prefLabel xml:lang="en">scripted testing</skos:prefLabel>
    </owl:NamedIndividual>
    


    <!-- http://purl.org/stc/terms#security_testing -->

    <owl:NamedIndividual rdf:about="http://purl.org/stc/terms#security_testing">
        <terms:hasParent rdf:resource="http://purl.org/stc/terms#non-functional_testing"/>
        <isInISTQBGlossary rdf:datatype="http://www.w3.org/2001/XMLSchema#boolean">true</isInISTQBGlossary>
        <rdfs:comment xml:lang="en">A test type to determine the security of a component or system. (ISTQB Glossary v4.5)

Test type conducted to evaluate the degree to which a test item, and associated data and information, are protected so that unauthorized persons or systems cannot use, read, or modify them, and authorized persons or systems are not denied access to them. (ISO/IEC/IEEE 29119-1:2022)</rdfs:comment>
        <rdfs:label>security testing</rdfs:label>
        <rdfs:seeAlso>ISO/IEC/IEEE 29119-1:2022 (Software and systems engineering — Software testing — Part 1: Concepts and definitions)

Specialist - Mobile Application Testing - 2019
Specialist - Security Tester - 2016
Specialist - Security Test Engineer - v1.0</rdfs:seeAlso>
        <skos:prefLabel xml:lang="en">security testing</skos:prefLabel>
    </owl:NamedIndividual>
    


    <!-- http://purl.org/stc/terms#sequential_development_model -->

    <owl:NamedIndividual rdf:about="http://purl.org/stc/terms#sequential_development_model">
        <terms:hasParent rdf:resource="http://purl.org/stc/terms#process_orientation_in_software_development"/>
        <isInISTQBGlossary rdf:datatype="http://www.w3.org/2001/XMLSchema#boolean">true</isInISTQBGlossary>
        <rdfs:label>sequential</rdfs:label>
        <skos:prefLabel xml:lang="en">sequential development model</skos:prefLabel>
    </owl:NamedIndividual>
    


    <!-- http://purl.org/stc/terms#session-based_testing -->

    <owl:NamedIndividual rdf:about="http://purl.org/stc/terms#session-based_testing">
        <terms:hasParent rdf:resource="http://purl.org/stc/terms#process_orientation_in_test_approach"/>
        <isInISTQBGlossary rdf:datatype="http://www.w3.org/2001/XMLSchema#boolean">true</isInISTQBGlossary>
        <rdfs:label>session-based testing</rdfs:label>
        <skos:altLabel xml:lang="en">session based testing
session-oriented testing
session oriented testing</skos:altLabel>
        <skos:prefLabel xml:lang="en">session-based testing</skos:prefLabel>
    </owl:NamedIndividual>
    


    <!-- http://purl.org/stc/terms#software -->

    <owl:NamedIndividual rdf:about="http://purl.org/stc/terms#software">
        <terms:hasParent rdf:resource="http://purl.org/stc/terms#software_engineering_concepts"/>
    </owl:NamedIndividual>
    


    <!-- http://purl.org/stc/terms#software_development_model -->

    <owl:NamedIndividual rdf:about="http://purl.org/stc/terms#software_development_model">
        <terms:hasParent rdf:resource="http://purl.org/stc/terms#software_engineering_concepts"/>
        <isInISTQBGlossary rdf:datatype="http://www.w3.org/2001/XMLSchema#boolean">false</isInISTQBGlossary>
        <rdfs:label>software development model</rdfs:label>
        <skos:prefLabel xml:lang="en">software development model</skos:prefLabel>
    </owl:NamedIndividual>
    


    <!-- http://purl.org/stc/terms#software_engineering -->

    <owl:NamedIndividual rdf:about="http://purl.org/stc/terms#software_engineering">
        <terms:hasParent rdf:resource="http://purl.org/stc/terms#basic_concepts"/>
        <isInISTQBGlossary rdf:datatype="http://www.w3.org/2001/XMLSchema#boolean">false</isInISTQBGlossary>
        <rdfs:comment xml:lang="en">The application of a systematic, disciplined, quantifiable approach to the development, operation, and maintenance of software; that is, the application of engineering to software. (IEEE 610.12-1990, ISO/IEC/IEEE 24765:2017)

A set of systematic processes for the acquisition, supply, development, operation, maintenance, and disposal of software products. (ISO/IEC 12207:2017)</rdfs:comment>
        <rdfs:label>software engineering</rdfs:label>
        <rdfs:seeAlso>ISO/IEC/IEEE 24765:2017 (Systems and Software Engineering – Vocabulary)
ISO/IEC 12207:2017 (Systems and software engineering — Software life cycle processes)
ISO/IEC 12207:2017 (Systems and software engineering — Software life cycle processes)</rdfs:seeAlso>
        <skos:altLabel xml:lang="en">se
software development</skos:altLabel>
        <skos:prefLabel xml:lang="en">software engineering</skos:prefLabel>
    </owl:NamedIndividual>
    


    <!-- http://purl.org/stc/terms#software_engineering_activity -->

    <owl:NamedIndividual rdf:about="http://purl.org/stc/terms#software_engineering_activity">
        <terms:hasParent rdf:resource="http://purl.org/stc/terms#software_engineering_concepts"/>
    </owl:NamedIndividual>
    


    <!-- http://purl.org/stc/terms#software_engineering_concepts -->

    <owl:NamedIndividual rdf:about="http://purl.org/stc/terms#software_engineering_concepts">
        <rdfs:comment xml:lang="en">Selection of software engineering concepts that relate to software testing concepts.</rdfs:comment>
        <rdfs:label>software engineering concepts</rdfs:label>
        <skos:prefLabel xml:lang="en">software engineering concepts</skos:prefLabel>
    </owl:NamedIndividual>
    


    <!-- http://purl.org/stc/terms#software_lifecycle -->

    <owl:NamedIndividual rdf:about="http://purl.org/stc/terms#software_lifecycle">
        <terms:hasParent rdf:resource="http://purl.org/stc/terms#software_engineering_concepts"/>
    </owl:NamedIndividual>
    


    <!-- http://purl.org/stc/terms#software_testing_concepts -->

    <owl:NamedIndividual rdf:about="http://purl.org/stc/terms#software_testing_concepts">
        <rdfs:comment xml:lang="en">Rather exhaustive collection of software testing concepts</rdfs:comment>
        <rdfs:label>software testing concepts</rdfs:label>
        <skos:prefLabel xml:lang="en">software testing concepts</skos:prefLabel>
    </owl:NamedIndividual>
    


    <!-- http://purl.org/stc/terms#specialist_tester -->

    <owl:NamedIndividual rdf:about="http://purl.org/stc/terms#specialist_tester">
        <terms:hasParent rdf:resource="http://purl.org/stc/terms#related_to_role"/>
        <isInISTQBGlossary rdf:datatype="http://www.w3.org/2001/XMLSchema#boolean">false</isInISTQBGlossary>
        <rdfs:comment xml:lang="en">Performs testing for specific quality characteristics, such as usability, accessibility,
security, performance. (ISO/IEC/IEEE 29119-1:2022)</rdfs:comment>
        <rdfs:label>specialist tester</rdfs:label>
        <rdfs:seeAlso>ISO/IEC/IEEE 29119-1:2022 (Software and systems engineering — Software testing — Part 1: Concepts and definitions)</rdfs:seeAlso>
        <skos:prefLabel xml:lang="en">specialist tester</skos:prefLabel>
    </owl:NamedIndividual>
    


    <!-- http://purl.org/stc/terms#specification_coverage -->

    <owl:NamedIndividual rdf:about="http://purl.org/stc/terms#specification_coverage">
        <terms:hasParent rdf:resource="http://purl.org/stc/terms#coverage"/>
        <isInISTQBGlossary rdf:datatype="http://www.w3.org/2001/XMLSchema#boolean">false</isInISTQBGlossary>
        <rdfs:comment xml:lang="en">There is currently no industry agreed approach to calculating experience-based coverage. (ISO/IEC/IEEE 29119-4)</rdfs:comment>
        <rdfs:label>specification coverage</rdfs:label>
        <rdfs:seeAlso>ISO/IEC/IEEE 29119-4 (Software and systems engineering — Software testing — Part 4: Test techniques)</rdfs:seeAlso>
        <skos:altLabel xml:lang="en">black-box test metric
black box test metric
specification-based test metric
specification based test metric</skos:altLabel>
        <skos:prefLabel xml:lang="en">specification coverage</skos:prefLabel>
    </owl:NamedIndividual>
    


    <!-- http://purl.org/stc/terms#state_transition_testing -->

    <owl:NamedIndividual rdf:about="http://purl.org/stc/terms#state_transition_testing">
        <terms:hasParent rdf:resource="http://purl.org/stc/terms#black_box_test_technique"/>
        <isInISTQBGlossary rdf:datatype="http://www.w3.org/2001/XMLSchema#boolean">true</isInISTQBGlossary>
        <rdfs:label>state transition testing</rdfs:label>
        <skos:prefLabel xml:lang="en">state transition testing</skos:prefLabel>
    </owl:NamedIndividual>
    


    <!-- http://purl.org/stc/terms#statement_coverage -->

    <owl:NamedIndividual rdf:about="http://purl.org/stc/terms#statement_coverage">
        <terms:hasParent rdf:resource="http://purl.org/stc/terms#structural_coverage"/>
        <isInISTQBGlossary rdf:datatype="http://www.w3.org/2001/XMLSchema#boolean">true</isInISTQBGlossary>
        <rdfs:comment xml:lang="en">The coverage of executable statements. (ISTQB Glossary v4.5)

Coverage for statement testing. (ISO/IEC/IEEE 29119-4)</rdfs:comment>
        <rdfs:label>statement coverage</rdfs:label>
        <rdfs:seeAlso>ISO/IEC/IEEE 29119-4 (Software and systems engineering — Software testing — Part 4: Test techniques)

Foundation - v4.0</rdfs:seeAlso>
        <skos:altLabel xml:lang="en">statement testing coverage</skos:altLabel>
        <skos:prefLabel xml:lang="en">statement coverage</skos:prefLabel>
    </owl:NamedIndividual>
    


    <!-- http://purl.org/stc/terms#statement_testing -->

    <owl:NamedIndividual rdf:about="http://purl.org/stc/terms#statement_testing">
        <terms:hasParent rdf:resource="http://purl.org/stc/terms#white_box_test_technique"/>
        <isInISTQBGlossary rdf:datatype="http://www.w3.org/2001/XMLSchema#boolean">true</isInISTQBGlossary>
        <rdfs:label>statement testing</rdfs:label>
        <skos:prefLabel xml:lang="en">statement testing</skos:prefLabel>
    </owl:NamedIndividual>
    


    <!-- http://purl.org/stc/terms#static_analysis -->

    <owl:NamedIndividual rdf:about="http://purl.org/stc/terms#static_analysis">
        <terms:hasParent rdf:resource="http://purl.org/stc/terms#static_testing"/>
        <isInISTQBGlossary rdf:datatype="http://www.w3.org/2001/XMLSchema#boolean">true</isInISTQBGlossary>
        <rdfs:comment xml:lang="en">The process of evaluating a component or system without executing it, based on its form, structure, content, or documentation. (ISTQB Glossary v4.5)</rdfs:comment>
        <rdfs:label>static analysis</rdfs:label>
        <rdfs:seeAlso>Foundation - v4.0
Advanced Technical Test Analyst - v4.0
Advanced Test Automation Engineering - v2.0</rdfs:seeAlso>
        <skos:prefLabel xml:lang="en">static analysis</skos:prefLabel>
    </owl:NamedIndividual>
    


    <!-- http://purl.org/stc/terms#static_application_security_testing -->

    <owl:NamedIndividual rdf:about="http://purl.org/stc/terms#static_application_security_testing">
        <terms:hasParent rdf:resource="http://purl.org/stc/terms#security_testing"/>
        <isInISTQBGlossary rdf:datatype="http://www.w3.org/2001/XMLSchema#boolean">true</isInISTQBGlossary>
        <rdfs:label>static application security testing</rdfs:label>
        <skos:prefLabel xml:lang="en">static application security testing</skos:prefLabel>
    </owl:NamedIndividual>
    


    <!-- http://purl.org/stc/terms#static_testing -->

    <owl:NamedIndividual rdf:about="http://purl.org/stc/terms#static_testing">
        <terms:hasParent rdf:resource="http://purl.org/stc/terms#testing"/>
        <isInISTQBGlossary rdf:datatype="http://www.w3.org/2001/XMLSchema#boolean">true</isInISTQBGlossary>
        <rdfs:comment xml:lang="en">Testing that does not involve the execution of a test item. (ISTQB Glossary v4.5)

Testing in which a test item is examined against a set of quality or other criteria without the test item being executed. (ISO/IEC/IEEE 29119-1:2022)</rdfs:comment>
        <rdfs:label>static testing</rdfs:label>
        <rdfs:seeAlso>ISO/IEC/IEEE 29119-1:2022 (Software and systems engineering — Software testing — Part 1: Concepts and definitions)

Foundation - v4.0</rdfs:seeAlso>
        <skos:prefLabel xml:lang="en">static testing</skos:prefLabel>
    </owl:NamedIndividual>
    


    <!-- http://purl.org/stc/terms#stress_testing -->

    <owl:NamedIndividual rdf:about="http://purl.org/stc/terms#stress_testing">
        <terms:hasParent rdf:resource="http://purl.org/stc/terms#performance_testing"/>
        <isInISTQBGlossary rdf:datatype="http://www.w3.org/2001/XMLSchema#boolean">true</isInISTQBGlossary>
        <rdfs:label>stress testing</rdfs:label>
        <skos:prefLabel xml:lang="en">stress testing</skos:prefLabel>
    </owl:NamedIndividual>
    


    <!-- http://purl.org/stc/terms#structural_coverage -->

    <owl:NamedIndividual rdf:about="http://purl.org/stc/terms#structural_coverage">
        <terms:hasParent rdf:resource="http://purl.org/stc/terms#coverage"/>
        <isInISTQBGlossary rdf:datatype="http://www.w3.org/2001/XMLSchema#boolean">true</isInISTQBGlossary>
        <rdfs:comment xml:lang="en">Coverage measures based on the internal structure of a component or system. (ISTQB Glossary v4.5)</rdfs:comment>
        <rdfs:label>structural coverage</rdfs:label>
        <rdfs:seeAlso>ISO/IEC/IEEE 29119-4 (Software and systems engineering — Software testing — Part 4: Test techniques)</rdfs:seeAlso>
        <skos:altLabel xml:lang="en">white box test metric
white-box test metric
structure-based test metric
structure based test metric</skos:altLabel>
        <skos:prefLabel xml:lang="en">structural coverage</skos:prefLabel>
    </owl:NamedIndividual>
    


    <!-- http://purl.org/stc/terms#support_processes -->

    <owl:NamedIndividual rdf:about="http://purl.org/stc/terms#support_processes">
        <terms:hasParent rdf:resource="http://purl.org/stc/terms#software_lifecycle"/>
    </owl:NamedIndividual>
    


    <!-- http://purl.org/stc/terms#system_integration_testing -->

    <owl:NamedIndividual rdf:about="http://purl.org/stc/terms#system_integration_testing">
        <terms:hasParent rdf:resource="http://purl.org/stc/terms#integration_testing"/>
        <isInISTQBGlossary rdf:datatype="http://www.w3.org/2001/XMLSchema#boolean">true</isInISTQBGlossary>
        <rdfs:comment xml:lang="en">The integration testing of systems. (ISTQB Glossary v4.5)</rdfs:comment>
        <rdfs:label>system integration testing</rdfs:label>
        <rdfs:seeAlso>Foundation - v4.0</rdfs:seeAlso>
        <skos:prefLabel xml:lang="en">system integration testing</skos:prefLabel>
    </owl:NamedIndividual>
    


    <!-- http://purl.org/stc/terms#system_testing -->

    <owl:NamedIndividual rdf:about="http://purl.org/stc/terms#system_testing">
        <terms:hasParent rdf:resource="http://purl.org/stc/terms#test_level"/>
        <isInISTQBGlossary rdf:datatype="http://www.w3.org/2001/XMLSchema#boolean">true</isInISTQBGlossary>
        <rdfs:label>system testing</rdfs:label>
        <skos:prefLabel xml:lang="en">system testing</skos:prefLabel>
    </owl:NamedIndividual>
    


    <!-- http://purl.org/stc/terms#target_orientation_in_software_development -->

    <owl:NamedIndividual rdf:about="http://purl.org/stc/terms#target_orientation_in_software_development">
        <terms:hasParent rdf:resource="http://purl.org/stc/terms#software_development_model"/>
        <isInISTQBGlossary rdf:datatype="http://www.w3.org/2001/XMLSchema#boolean">false</isInISTQBGlossary>
        <rdfs:label>target orientation</rdfs:label>
        <skos:prefLabel xml:lang="en">target orientation in software development</skos:prefLabel>
    </owl:NamedIndividual>
    


    <!-- http://purl.org/stc/terms#target_orientation_in_test_approach -->

    <owl:NamedIndividual rdf:about="http://purl.org/stc/terms#target_orientation_in_test_approach">
        <terms:hasParent rdf:resource="http://purl.org/stc/terms#test_approach"/>
        <isInISTQBGlossary rdf:datatype="http://www.w3.org/2001/XMLSchema#boolean">false</isInISTQBGlossary>
        <rdfs:label>target orientation</rdfs:label>
        <skos:prefLabel xml:lang="en">target orientation in test approach</skos:prefLabel>
    </owl:NamedIndividual>
    


    <!-- http://purl.org/stc/terms#technical_review -->

    <owl:NamedIndividual rdf:about="http://purl.org/stc/terms#technical_review">
        <terms:hasParent rdf:resource="http://purl.org/stc/terms#formal_review"/>
        <isInISTQBGlossary rdf:datatype="http://www.w3.org/2001/XMLSchema#boolean">true</isInISTQBGlossary>
        <rdfs:comment xml:lang="en">A formal review by technical experts that examine the quality of a work product and identify discrepancies from specifications and standards. (ISTQB Glossary v4.5)</rdfs:comment>
        <rdfs:label>technical review</rdfs:label>
        <rdfs:seeAlso>Foundation - v4.0
Advanced Test Manager - 2012
Advanced Technical Test Analyst - v4.0</rdfs:seeAlso>
        <skos:prefLabel xml:lang="en">technical review</skos:prefLabel>
    </owl:NamedIndividual>
    


    <!-- http://purl.org/stc/terms#test_activity -->

    <owl:NamedIndividual rdf:about="http://purl.org/stc/terms#test_activity">
        <terms:hasParent rdf:resource="http://purl.org/stc/terms#software_engineering_activity"/>
        <terms:hasParent rdf:resource="http://purl.org/stc/terms#software_testing_concepts"/>
        <isInISTQBGlossary rdf:datatype="http://www.w3.org/2001/XMLSchema#boolean">false</isInISTQBGlossary>
        <rdfs:label>test activity</rdfs:label>
        <skos:prefLabel xml:lang="en">test activity</skos:prefLabel>
    </owl:NamedIndividual>
    


    <!-- http://purl.org/stc/terms#test_analysis -->

    <owl:NamedIndividual rdf:about="http://purl.org/stc/terms#test_analysis">
        <terms:hasParent rdf:resource="http://purl.org/stc/terms#test_activity"/>
        <isInISTQBGlossary rdf:datatype="http://www.w3.org/2001/XMLSchema#boolean">true</isInISTQBGlossary>
        <rdfs:comment xml:lang="en">The activity that identifies test conditions by analyzing the test basis. (ISTQB Glossary v4.5)</rdfs:comment>
        <rdfs:label>test analysis</rdfs:label>
        <rdfs:seeAlso>Foundation - v4.0
Advanced Test Analyst - v3.1
Advanced Test Analyst - v4.0</rdfs:seeAlso>
        <skos:prefLabel xml:lang="en">test analysis</skos:prefLabel>
    </owl:NamedIndividual>
    


    <!-- http://purl.org/stc/terms#test_analyst -->

    <owl:NamedIndividual rdf:about="http://purl.org/stc/terms#test_analyst">
        <terms:hasParent rdf:resource="http://purl.org/stc/terms#related_to_role"/>
        <isInISTQBGlossary rdf:datatype="http://www.w3.org/2001/XMLSchema#boolean">false</isInISTQBGlossary>
        <rdfs:comment xml:lang="en">Develops oracles and/or analyses test results for correctness and issues.  (ISO/IEC/IEEE 29119-1:2022)</rdfs:comment>
        <rdfs:label>test analyst</rdfs:label>
        <rdfs:seeAlso>ISO/IEC/IEEE 29119-1:2022 (Software and systems engineering — Software testing — Part 1: Concepts and definitions)</rdfs:seeAlso>
        <skos:altLabel xml:lang="en">TA</skos:altLabel>
        <skos:prefLabel xml:lang="en">test analyst</skos:prefLabel>
    </owl:NamedIndividual>
    


    <!-- http://purl.org/stc/terms#test_approach -->

    <owl:NamedIndividual rdf:about="http://purl.org/stc/terms#test_approach">
        <terms:hasParent rdf:resource="http://purl.org/stc/terms#software_testing_concepts"/>
        <isInISTQBGlossary rdf:datatype="http://www.w3.org/2001/XMLSchema#boolean">true</isInISTQBGlossary>
        <rdfs:comment xml:lang="en">The manner of implementing testing tasks. (ISTQB Glossary v4.5)</rdfs:comment>
        <rdfs:label>test approach</rdfs:label>
        <rdfs:seeAlso>Foundation - v4.0
Advanced Test Manager - 2012</rdfs:seeAlso>
        <skos:prefLabel xml:lang="en">test approach</skos:prefLabel>
    </owl:NamedIndividual>
    


    <!-- http://purl.org/stc/terms#test_architect -->

    <owl:NamedIndividual rdf:about="http://purl.org/stc/terms#test_architect">
        <terms:hasParent rdf:resource="http://purl.org/stc/terms#related_to_role"/>
        <isInISTQBGlossary rdf:datatype="http://www.w3.org/2001/XMLSchema#boolean">false</isInISTQBGlossary>
        <rdfs:comment xml:lang="en">Defines the test strategy, test environment and test plan for programmes and projects. Specifies the organizational test requirements and helps ensure conformance to these requirements. (ISO/IEC/IEEE 29119-1:2022)</rdfs:comment>
        <rdfs:label>test architect</rdfs:label>
        <rdfs:seeAlso>ISO/IEC/IEEE 29119-1:2022 (Software and systems engineering — Software testing — Part 1: Concepts and definitions)</rdfs:seeAlso>
        <skos:prefLabel xml:lang="en">test architect</skos:prefLabel>
    </owl:NamedIndividual>
    


    <!-- http://purl.org/stc/terms#test_automation -->

    <owl:NamedIndividual rdf:about="http://purl.org/stc/terms#test_automation">
        <terms:hasParent rdf:resource="http://purl.org/stc/terms#test_activity"/>
        <isInISTQBGlossary rdf:datatype="http://www.w3.org/2001/XMLSchema#boolean">true</isInISTQBGlossary>
        <rdfs:comment xml:lang="en">The conversion of test activities to automatic operation. (ISTQB Glossary v4.5)</rdfs:comment>
        <rdfs:label>test automation</rdfs:label>
        <rdfs:seeAlso>Advanced Test Automation Engineering - v2.0
Specialist - Test Automation Engineer - 2016</rdfs:seeAlso>
        <skos:prefLabel xml:lang="en">test automation</skos:prefLabel>
    </owl:NamedIndividual>
    


    <!-- http://purl.org/stc/terms#test_automation_engineer -->

    <owl:NamedIndividual rdf:about="http://purl.org/stc/terms#test_automation_engineer">
        <terms:hasParent rdf:resource="http://purl.org/stc/terms#related_to_role"/>
        <isInISTQBGlossary rdf:datatype="http://www.w3.org/2001/XMLSchema#boolean">false</isInISTQBGlossary>
        <rdfs:comment xml:lang="en">Implements tests cases/scripts within a test automation framework. (ISO/IEC/IEEE 29119-1:2022)</rdfs:comment>
        <rdfs:label>test automation engineer</rdfs:label>
        <rdfs:seeAlso>ISO/IEC/IEEE 29119-1:2022 (Software and systems engineering — Software testing — Part 1: Concepts and definitions)</rdfs:seeAlso>
        <skos:altLabel xml:lang="en">TAE
test automator</skos:altLabel>
        <skos:prefLabel xml:lang="en">test automation engineer</skos:prefLabel>
    </owl:NamedIndividual>
    


    <!-- http://purl.org/stc/terms#test_basis -->

    <owl:NamedIndividual rdf:about="http://purl.org/stc/terms#test_basis">
        <terms:hasParent rdf:resource="http://purl.org/stc/terms#Testware"/>
        <isInISTQBGlossary rdf:datatype="http://www.w3.org/2001/XMLSchema#boolean">true</isInISTQBGlossary>
        <rdfs:comment xml:lang="en">The body of knowledge used as the basis for test analysis and test design. (ISTQB Glossary v4.5)

Information used as the basis for designing and implementing test cases. (ISO/IEC/IEEE 29119-1:2022)</rdfs:comment>
        <rdfs:label>test basis</rdfs:label>
        <rdfs:seeAlso>ISO/IEC/IEEE 29119-1 (2022) Software and systems engineering -- Software testing -- Part 1: Concepts and definitions

Foundation - v4.0
Advanced Test Analyst - v3.1</rdfs:seeAlso>
        <skos:prefLabel xml:lang="en">test basis</skos:prefLabel>
    </owl:NamedIndividual>
    


    <!-- http://purl.org/stc/terms#test_case -->

    <owl:NamedIndividual rdf:about="http://purl.org/stc/terms#test_case">
        <terms:hasParent rdf:resource="http://purl.org/stc/terms#Testware"/>
        <isInISTQBGlossary rdf:datatype="http://www.w3.org/2001/XMLSchema#boolean">true</isInISTQBGlossary>
        <rdfs:comment xml:lang="en">A set of preconditions, inputs, actions (where applicable), expected results and postconditions, developed based on test conditions. (ISTQB Glossary v4.5)

Set of preconditions, inputs and expected results, developed to drive the execution of a test item to meet test objectives. (ISO/IEC/IEEE 29119-1:2022)</rdfs:comment>
        <rdfs:label>test case</rdfs:label>
        <rdfs:seeAlso>ISO/IEC/IEEE 29119-1 (2022) Software and systems engineering -- Software testing -- Part 1: Concepts and definitions

Foundation - v4.0
Advanced Test Manager - 2012
Advanced Test Management - v3.0
Advanced Test Analyst - v4.0
Specialist - Acceptance Testing - 2019</rdfs:seeAlso>
        <skos:altLabel xml:lang="en">testcase</skos:altLabel>
        <skos:prefLabel xml:lang="en">test case</skos:prefLabel>
    </owl:NamedIndividual>
    


    <!-- http://purl.org/stc/terms#test_completion -->

    <owl:NamedIndividual rdf:about="http://purl.org/stc/terms#test_completion">
        <terms:hasParent rdf:resource="http://purl.org/stc/terms#test_activity"/>
        <isInISTQBGlossary rdf:datatype="http://www.w3.org/2001/XMLSchema#boolean">true</isInISTQBGlossary>
        <rdfs:comment xml:lang="en">The activity that makes testware available for later use, leaves test environments in a satisfactory condition and communicates the results of testing to relevant stakeholders. (ISTQB Glossary v4.5)</rdfs:comment>
        <rdfs:label>test completion</rdfs:label>
        <rdfs:seeAlso>Foundation - v4.0
Advanced Test Management - v3.0</rdfs:seeAlso>
        <skos:prefLabel xml:lang="en">test completion</skos:prefLabel>
    </owl:NamedIndividual>
    


    <!-- http://purl.org/stc/terms#test_completion_report -->

    <owl:NamedIndividual rdf:about="http://purl.org/stc/terms#test_completion_report">
        <terms:hasParent rdf:resource="http://purl.org/stc/terms#test_report"/>
        <isInISTQBGlossary rdf:datatype="http://www.w3.org/2001/XMLSchema#boolean">true</isInISTQBGlossary>
        <rdfs:comment xml:lang="en">A type of test report produced at completion milestones that provides an evaluation of the corresponding test items against exit criteria. (ISTQB Glossary v4.5)

Report that provides a summary of the testing that was performed. (ISO/IEC/IEEE 29119-1:2022)</rdfs:comment>
        <rdfs:label>test completion report</rdfs:label>
        <rdfs:seeAlso>ISO/IEC/IEEE 29119-1:2022 (Software and systems engineering — Software testing — Part 1: Concepts and definitions)

Foundation - v4.0
Advanced Test Manager - 2012</rdfs:seeAlso>
        <skos:altLabel xml:lang="en">test summary report</skos:altLabel>
        <skos:prefLabel xml:lang="en">test completion report</skos:prefLabel>
    </owl:NamedIndividual>
    


    <!-- http://purl.org/stc/terms#test_condition -->

    <owl:NamedIndividual rdf:about="http://purl.org/stc/terms#test_condition">
        <terms:hasParent rdf:resource="http://purl.org/stc/terms#Testware"/>
        <isInISTQBGlossary rdf:datatype="http://www.w3.org/2001/XMLSchema#boolean">true</isInISTQBGlossary>
        <rdfs:comment xml:lang="en">A testable aspect of a component or system identified as a basis for testing. (ISTQB Glossary v4.5)

Testable aspect of a component or system, such as a function, transaction, feature, quality attribute, or structural element identified as a basis for testing. (ISO/IEC/IEEE 29119-1:2022)</rdfs:comment>
        <rdfs:label>test condition</rdfs:label>
        <rdfs:seeAlso>ISO/IEC/IEEE 29119-1:2022 (Software and systems engineering — Software testing — Part 1: Concepts and definitions)

Foundation - v4.0
Advanced Test Manager - 2012
Advanced Test Analyst - v3.1
Advanced Test Analyst - v4.0
Specialist - Test Automation Strategy - v1.0</rdfs:seeAlso>
        <skos:altLabel xml:lang="en">test situation
test requirement</skos:altLabel>
        <skos:prefLabel xml:lang="en">test condition</skos:prefLabel>
    </owl:NamedIndividual>
    


    <!-- http://purl.org/stc/terms#test_control -->

    <owl:NamedIndividual rdf:about="http://purl.org/stc/terms#test_control">
        <terms:hasParent rdf:resource="http://purl.org/stc/terms#test_activity"/>
        <isInISTQBGlossary rdf:datatype="http://www.w3.org/2001/XMLSchema#boolean">true</isInISTQBGlossary>
        <rdfs:comment xml:lang="en">The activity that develops and applies corrective actions to get a test project on track when it deviates from what was planned. (ISTQB Glossary v4.5)</rdfs:comment>
        <rdfs:label>test control</rdfs:label>
        <rdfs:seeAlso>Foundation - v4.0
Advanced Test Manager - 2012
Advanced Test Management - v3.0</rdfs:seeAlso>
        <skos:prefLabel xml:lang="en">test control</skos:prefLabel>
    </owl:NamedIndividual>
    


    <!-- http://purl.org/stc/terms#test_data -->

    <owl:NamedIndividual rdf:about="http://purl.org/stc/terms#test_data">
        <terms:hasParent rdf:resource="http://purl.org/stc/terms#Testware"/>
        <isInISTQBGlossary rdf:datatype="http://www.w3.org/2001/XMLSchema#boolean">true</isInISTQBGlossary>
        <rdfs:comment xml:lang="en">Data needed for test execution. (ISTQB Glossary v4.5)

Data created or selected to satisfy the input requirements for executing one or more test cases, which may be defined in the test plan, test case or test procedure. (ISO/IEC/IEEE 29119-1:2022)</rdfs:comment>
        <rdfs:label>test data</rdfs:label>
        <rdfs:seeAlso>ISO/IEC/IEEE 29119-1:2022 (Software and systems engineering — Software testing — Part 1: Concepts and definitions)

Foundation - v4.0
Advanced Test Analyst - v3.1
Advanced Test Analyst - v4.0</rdfs:seeAlso>
        <skos:altLabel xml:lang="en">testdata
test data set
testdata set</skos:altLabel>
        <skos:prefLabel xml:lang="en">test data</skos:prefLabel>
    </owl:NamedIndividual>
    


    <!-- http://purl.org/stc/terms#test_design -->

    <owl:NamedIndividual rdf:about="http://purl.org/stc/terms#test_design">
        <terms:hasParent rdf:resource="http://purl.org/stc/terms#test_activity"/>
        <isInISTQBGlossary rdf:datatype="http://www.w3.org/2001/XMLSchema#boolean">true</isInISTQBGlossary>
        <rdfs:comment xml:lang="en">The activity that derives and specifies test cases from test conditions. (ISTQB Glossary v4.5)</rdfs:comment>
        <rdfs:label>test design</rdfs:label>
        <rdfs:seeAlso>Foundation - v4.0
Advanced Test Manager - 2012
Advanced Test Analyst - v3.1
Advanced Test Analyst - v4.0</rdfs:seeAlso>
        <skos:prefLabel xml:lang="en">test design</skos:prefLabel>
    </owl:NamedIndividual>
    


    <!-- http://purl.org/stc/terms#test_designer -->

    <owl:NamedIndividual rdf:about="http://purl.org/stc/terms#test_designer">
        <terms:hasParent rdf:resource="http://purl.org/stc/terms#related_to_role"/>
        <isInISTQBGlossary rdf:datatype="http://www.w3.org/2001/XMLSchema#boolean">false</isInISTQBGlossary>
        <rdfs:comment xml:lang="en">Develops the test design artefacts. (ISO/IEC/IEEE 29119-1:2022)</rdfs:comment>
        <rdfs:label>test designer</rdfs:label>
        <rdfs:seeAlso>ISO/IEC/IEEE 29119-1:2022 (Software and systems engineering — Software testing — Part 1: Concepts and definitions)</rdfs:seeAlso>
        <skos:prefLabel xml:lang="en">test designer</skos:prefLabel>
    </owl:NamedIndividual>
    


    <!-- http://purl.org/stc/terms#test_director -->

    <owl:NamedIndividual rdf:about="http://purl.org/stc/terms#test_director">
        <terms:hasParent rdf:resource="http://purl.org/stc/terms#related_to_role"/>
        <isInISTQBGlossary rdf:datatype="http://www.w3.org/2001/XMLSchema#boolean">true</isInISTQBGlossary>
        <rdfs:comment xml:lang="en">A senior manager who manages test managers.</rdfs:comment>
        <rdfs:label>test director</rdfs:label>
        <rdfs:seeAlso>Advanced Test Manager - 2012</rdfs:seeAlso>
        <skos:prefLabel xml:lang="en">test director</skos:prefLabel>
    </owl:NamedIndividual>
    


    <!-- http://purl.org/stc/terms#test_driven_development -->

    <owl:NamedIndividual rdf:about="http://purl.org/stc/terms#test_driven_development">
        <terms:hasParent rdf:resource="http://purl.org/stc/terms#target_orientation_in_software_development"/>
        <isInISTQBGlossary rdf:datatype="http://www.w3.org/2001/XMLSchema#boolean">true</isInISTQBGlossary>
        <rdfs:comment xml:lang="en">A software development technique in which the test cases are developed, automated and then the software is developed incrementally to pass those test cases. (ISTQB Glossary v4.5)</rdfs:comment>
        <rdfs:label>test-driven</rdfs:label>
        <rdfs:seeAlso>Foundation - v4.0
Advanced Test Manager - 2012
Advanced Test Management - v3.0
Advanced Test Automation Engineering - v2.0
Advanced Agile Technical Tester - 2019
Specialist - Agile Test Leadership at Scale - v2.0
Specialist - Test Automation Strategy - v1.0</rdfs:seeAlso>
        <skos:altLabel xml:lang="en">test driven development
tdd
TDD</skos:altLabel>
        <skos:prefLabel xml:lang="en">test-driven development</skos:prefLabel>
    </owl:NamedIndividual>
    


    <!-- http://purl.org/stc/terms#test_execution -->

    <owl:NamedIndividual rdf:about="http://purl.org/stc/terms#test_execution">
        <terms:hasParent rdf:resource="http://purl.org/stc/terms#test_activity"/>
        <isInISTQBGlossary rdf:datatype="http://www.w3.org/2001/XMLSchema#boolean">true</isInISTQBGlossary>
        <rdfs:comment xml:lang="en">The activity that runs a test on a component or system producing actual results. (ISTQB Glossary v4.5)</rdfs:comment>
        <rdfs:label>test execution</rdfs:label>
        <rdfs:seeAlso>Foundation - v4.0
Advanced Test Manager - 2012
Advanced Test Analyst - v3.1
Advanced Test Analyst - v4.0
Advanced Technical Test Analyst - v4.0</rdfs:seeAlso>
        <skos:prefLabel xml:lang="en">test execution</skos:prefLabel>
    </owl:NamedIndividual>
    


    <!-- http://purl.org/stc/terms#test_first_approach -->

    <owl:NamedIndividual rdf:about="http://purl.org/stc/terms#test_first_approach">
        <terms:hasParent rdf:resource="http://purl.org/stc/terms#test_driven_development"/>
        <isInISTQBGlossary rdf:datatype="http://www.w3.org/2001/XMLSchema#boolean">true</isInISTQBGlossary>
        <rdfs:comment xml:lang="en">An approach to software development in which the test cases are designed and implemented before the associated component or system is developed. (ISTQB Glossary v4.5)</rdfs:comment>
        <rdfs:label>test-first approach</rdfs:label>
        <rdfs:seeAlso>Foundation - v4.0
Advanced Test Analyst - v3.1
Foundation Agile Tester - 2014
Specialist - Agile Test Leadership at Scale - v2.0</rdfs:seeAlso>
        <skos:altLabel xml:lang="en">test first approach</skos:altLabel>
        <skos:prefLabel xml:lang="en">test-first approach</skos:prefLabel>
    </owl:NamedIndividual>
    


    <!-- http://purl.org/stc/terms#test_implementation -->

    <owl:NamedIndividual rdf:about="http://purl.org/stc/terms#test_implementation">
        <terms:hasParent rdf:resource="http://purl.org/stc/terms#test_activity"/>
        <isInISTQBGlossary rdf:datatype="http://www.w3.org/2001/XMLSchema#boolean">true</isInISTQBGlossary>
        <rdfs:comment xml:lang="en">The activity that prepares the testware needed for test execution based on test analysis and design. (ISTQB Glossary v4.5)</rdfs:comment>
        <rdfs:label>test implementation</rdfs:label>
        <rdfs:seeAlso>Foundation - v4.0
Advanced Test Manager - 2012
Advanced Test Analyst - v3.1
Advanced Test Analyst - v4.0</rdfs:seeAlso>
        <skos:prefLabel xml:lang="en">test implementation</skos:prefLabel>
    </owl:NamedIndividual>
    


    <!-- http://purl.org/stc/terms#test_item -->

    <owl:NamedIndividual rdf:about="http://purl.org/stc/terms#test_item">
        <terms:hasParent rdf:resource="http://purl.org/stc/terms#Testware"/>
        <isInISTQBGlossary rdf:datatype="http://www.w3.org/2001/XMLSchema#boolean">true</isInISTQBGlossary>
        <rdfs:comment xml:lang="en">A part of a test object used in the test process. (ISTQB Glossary v4.5)</rdfs:comment>
        <rdfs:comment xml:lang="en">ISO/IEC/IEEE 29119-1:2022 defines the term test item differently: as a synonym to test object.</rdfs:comment>
        <rdfs:label>test item</rdfs:label>
        <skos:prefLabel xml:lang="en">test item</skos:prefLabel>
    </owl:NamedIndividual>
    


    <!-- http://purl.org/stc/terms#test_leader -->

    <owl:NamedIndividual rdf:about="http://purl.org/stc/terms#test_leader">
        <terms:hasParent rdf:resource="http://purl.org/stc/terms#related_to_role"/>
        <isInISTQBGlossary rdf:datatype="http://www.w3.org/2001/XMLSchema#boolean">true</isInISTQBGlossary>
        <rdfs:comment xml:lang="en">On large projects, the person who reports to the test manager and is responsible for project management of a particular test level or a particular set of testing activities. (ISTQB Glossary v4.5)</rdfs:comment>
        <rdfs:label>test leader</rdfs:label>
        <rdfs:seeAlso>Advanced Test Manager - 2012</rdfs:seeAlso>
        <skos:altLabel xml:lang="en">lead tester</skos:altLabel>
        <skos:prefLabel xml:lang="en">test leader</skos:prefLabel>
    </owl:NamedIndividual>
    


    <!-- http://purl.org/stc/terms#test_level -->

    <owl:NamedIndividual rdf:about="http://purl.org/stc/terms#test_level">
        <terms:hasParent rdf:resource="http://purl.org/stc/terms#software_testing_concepts"/>
        <isInISTQBGlossary rdf:datatype="http://www.w3.org/2001/XMLSchema#boolean">true</isInISTQBGlossary>
        <rdfs:comment xml:lang="en">A specific instantiation of a test process. (ISTQB Glossary v4.5)

One of a sequence of test stages each of which is typically associated with the achievement of particular
objectives and used to treat particular risks. (ISO/IEC/IEEE 29119-1:2022)</rdfs:comment>
        <rdfs:label>test level</rdfs:label>
        <rdfs:seeAlso>ISO/IEC/IEEE 29119-1:2022 (Software and systems engineering — Software testing — Part 1: Concepts and definitions)

Foundation - v4.0
Advanced Test Manager - 2012
Advanced Test Management - v3.0
Specialist - Mobile Application Testing - 2019
Specialist - Test Automation Strategy - v1.0</rdfs:seeAlso>
        <skos:altLabel xml:lang="en">test stage
test phase</skos:altLabel>
        <skos:prefLabel xml:lang="en">test level</skos:prefLabel>
    </owl:NamedIndividual>
    


    <!-- http://purl.org/stc/terms#test_management -->

    <owl:NamedIndividual rdf:about="http://purl.org/stc/terms#test_management">
        <terms:hasParent rdf:resource="http://purl.org/stc/terms#software_testing_concepts"/>
        <terms:hasParent rdf:resource="http://purl.org/stc/terms#test_activity"/>
        <isInISTQBGlossary rdf:datatype="http://www.w3.org/2001/XMLSchema#boolean">true</isInISTQBGlossary>
        <rdfs:comment xml:lang="en">The process of planning, scheduling, estimating, monitoring, reporting, controlling, and completing test activities. (ISTQB Glossary v4.5)</rdfs:comment>
        <rdfs:label>test management</rdfs:label>
        <skos:prefLabel xml:lang="en">test management</skos:prefLabel>
    </owl:NamedIndividual>
    


    <!-- http://purl.org/stc/terms#test_manager -->

    <owl:NamedIndividual rdf:about="http://purl.org/stc/terms#test_manager">
        <terms:hasParent rdf:resource="http://purl.org/stc/terms#related_to_role"/>
        <isInISTQBGlossary rdf:datatype="http://www.w3.org/2001/XMLSchema#boolean">true</isInISTQBGlossary>
        <rdfs:comment xml:lang="en">The person responsible for project management of testing activities, resources, and evaluation of a test object. (ISTQB Glossary v4.5)

Develops, manages, and helps to ensure conformance with the test management process. The test manager also plans and controls the dynamic test process. (ISO/IEC/IEEE 29119-1:2022)</rdfs:comment>
        <rdfs:label>test manager</rdfs:label>
        <rdfs:seeAlso>ISO/IEC/IEEE 29119-1:2022 (Software and systems engineering — Software testing — Part 1: Concepts and definitions)

Advanced Test Manager - 2012</rdfs:seeAlso>
        <skos:prefLabel xml:lang="en">test manager</skos:prefLabel>
    </owl:NamedIndividual>
    


    <!-- http://purl.org/stc/terms#test_metric -->

    <owl:NamedIndividual rdf:about="http://purl.org/stc/terms#test_metric">
        <terms:hasParent rdf:resource="http://purl.org/stc/terms#metric"/>
        <terms:hasParent rdf:resource="http://purl.org/stc/terms#software_testing_concepts"/>
        <isInISTQBGlossary rdf:datatype="http://www.w3.org/2001/XMLSchema#boolean">false</isInISTQBGlossary>
        <rdfs:comment xml:lang="en">A measurement of a characteristic of a test process, test activity, test object or testware. (own)</rdfs:comment>
        <rdfs:label>test metric</rdfs:label>
        <rdfs:seeAlso>ISO/IEC/IEEE 29119-4 (Software and systems engineering — Software testing — Part 4: Test techniques)</rdfs:seeAlso>
        <skos:altLabel xml:lang="en">testmetric</skos:altLabel>
        <skos:prefLabel xml:lang="en">test metric</skos:prefLabel>
    </owl:NamedIndividual>
    


    <!-- http://purl.org/stc/terms#test_model -->

    <owl:NamedIndividual rdf:about="http://purl.org/stc/terms#test_model">
        <terms:hasParent rdf:resource="http://purl.org/stc/terms#Testware"/>
        <isInISTQBGlossary rdf:datatype="http://www.w3.org/2001/XMLSchema#boolean">true</isInISTQBGlossary>
        <rdfs:comment xml:lang="en">A model describing testware that is used for testing a component or a system under test. (ISTQB Glossary v4.5)

Representation of the test item, which allows the testing to be focused on particular
characteristics or qualities. (ISO/IEC/IEEE 29119-1:2022)</rdfs:comment>
        <rdfs:label>test model</rdfs:label>
        <rdfs:seeAlso>ISO/IEC/IEEE 29119-1:2022 (Software and systems engineering — Software testing — Part 1: Concepts and definitions)

Specialist - Model-Based Tester - 2015
Specialist - Model-Based Testing - v1.1</rdfs:seeAlso>
        <skos:altLabel>test specification</skos:altLabel>
        <skos:prefLabel xml:lang="en">test model</skos:prefLabel>
    </owl:NamedIndividual>
    


    <!-- http://purl.org/stc/terms#test_monitoring -->

    <owl:NamedIndividual rdf:about="http://purl.org/stc/terms#test_monitoring">
        <terms:hasParent rdf:resource="http://purl.org/stc/terms#test_activity"/>
        <isInISTQBGlossary rdf:datatype="http://www.w3.org/2001/XMLSchema#boolean">true</isInISTQBGlossary>
        <rdfs:comment xml:lang="en">The activity that checks the status of testing activities, identifies any variances from planned or expected, and reports status to stakeholders. (ISTQB Glossary v4.5)</rdfs:comment>
        <rdfs:label>test monitoring</rdfs:label>
        <rdfs:seeAlso>Foundation - v4.0
Advanced Test Manager - 2012
Advanced Test Management - v3.0</rdfs:seeAlso>
        <skos:prefLabel xml:lang="en">test monitoring</skos:prefLabel>
    </owl:NamedIndividual>
    


    <!-- http://purl.org/stc/terms#test_object -->

    <owl:NamedIndividual rdf:about="http://purl.org/stc/terms#test_object">
        <terms:hasParent rdf:resource="http://purl.org/stc/terms#Testware"/>
        <isInISTQBGlossary rdf:datatype="http://www.w3.org/2001/XMLSchema#boolean">true</isInISTQBGlossary>
        <rdfs:comment xml:lang="en">The work product to be tested. (ISTQB Glossary v4.5)</rdfs:comment>
        <rdfs:label>test object</rdfs:label>
        <rdfs:seeAlso>Foundation - v4.0</rdfs:seeAlso>
        <skos:altLabel xml:lang="en">test target
system under test
sut
SUT
object under test</skos:altLabel>
        <skos:prefLabel xml:lang="en">test object</skos:prefLabel>
    </owl:NamedIndividual>
    


    <!-- http://purl.org/stc/terms#test_objective -->

    <owl:NamedIndividual rdf:about="http://purl.org/stc/terms#test_objective">
        <terms:hasParent rdf:resource="http://purl.org/stc/terms#Testware"/>
        <isInISTQBGlossary rdf:datatype="http://www.w3.org/2001/XMLSchema#boolean">true</isInISTQBGlossary>
        <rdfs:comment xml:lang="en">The purpose for testing. (ISTQB Gloassary v4.5)</rdfs:comment>
        <rdfs:comment xml:lang="en">test objective</rdfs:comment>
        <rdfs:seeAlso>Foundation - v4.0
Advanced Test Management - v3.0</rdfs:seeAlso>
        <skos:altLabel xml:lang="en">test goal</skos:altLabel>
        <skos:prefLabel xml:lang="en">test objective</skos:prefLabel>
    </owl:NamedIndividual>
    


    <!-- http://purl.org/stc/terms#test_oracle -->

    <owl:NamedIndividual rdf:about="http://purl.org/stc/terms#test_oracle">
        <terms:hasParent rdf:resource="http://purl.org/stc/terms#Testware"/>
        <isInISTQBGlossary rdf:datatype="http://www.w3.org/2001/XMLSchema#boolean">true</isInISTQBGlossary>
        <rdfs:comment xml:lang="en">A source to determine an expected result to compare with the actual result of the system under test.  (ISTQB Glossary v4.5)</rdfs:comment>
        <rdfs:label>test oracle</rdfs:label>
        <rdfs:seeAlso>Advanced Test Analyst - v4.0</rdfs:seeAlso>
        <skos:altLabel xml:lang="en">oracle</skos:altLabel>
        <skos:prefLabel xml:lang="en">test oracle</skos:prefLabel>
    </owl:NamedIndividual>
    


    <!-- http://purl.org/stc/terms#test_plan -->

    <owl:NamedIndividual rdf:about="http://purl.org/stc/terms#test_plan">
        <terms:hasParent rdf:resource="http://purl.org/stc/terms#Testware"/>
        <isInISTQBGlossary rdf:datatype="http://www.w3.org/2001/XMLSchema#boolean">true</isInISTQBGlossary>
        <rdfs:comment xml:lang="en">Documentation describing the test objectives to be achieved and the means and the schedule for achieving them, organized to coordinate testing activities. (ISTQB Glossary v4.5)

Detailed description of test objectives to be achieved and the means and schedule for achieving them, organized to coordinate testing activities for some test item or set of test items. (ISO/IEC/IEEE 29119-1:2022)</rdfs:comment>
        <rdfs:label>test plan</rdfs:label>
        <rdfs:seeAlso>ISO/IEC/IEEE 29119-1 (2022) Software and systems engineering -- Software testing -- Part 1: Concepts and definitions

Foundation - v4.0
Advanced Test Manager - 2012
Advanced Test Management - v3.0
Specialist - Performance Testing - 2018
Specialist - Security Test Engineer - v1.0</rdfs:seeAlso>
        <skos:altLabel xml:lang="en">testplan</skos:altLabel>
        <skos:prefLabel xml:lang="en">test plan</skos:prefLabel>
    </owl:NamedIndividual>
    


    <!-- http://purl.org/stc/terms#test_planning -->

    <owl:NamedIndividual rdf:about="http://purl.org/stc/terms#test_planning">
        <terms:hasParent rdf:resource="http://purl.org/stc/terms#test_activity"/>
        <isInISTQBGlossary rdf:datatype="http://www.w3.org/2001/XMLSchema#boolean">true</isInISTQBGlossary>
        <rdfs:comment xml:lang="en">The activity of establishing or updating a test plan. (ISTQB Glossary v4.5)</rdfs:comment>
        <rdfs:label>test planning</rdfs:label>
        <rdfs:seeAlso>Foundation - v4.0
Advanced Test Manager - 2012
Advanced Test Management - v3.0</rdfs:seeAlso>
        <skos:prefLabel xml:lang="en">test planning</skos:prefLabel>
    </owl:NamedIndividual>
    


    <!-- http://purl.org/stc/terms#test_process -->

    <owl:NamedIndividual rdf:about="http://purl.org/stc/terms#test_process">
        <terms:hasParent rdf:resource="http://purl.org/stc/terms#software_testing_concepts"/>
        <isInISTQBGlossary rdf:datatype="http://www.w3.org/2001/XMLSchema#boolean">true</isInISTQBGlossary>
        <rdfs:comment xml:lang="en">The set of interrelated activities comprising of test planning, test monitoring, test control, test analysis, test design, test implementation, test execution, and test completion.</rdfs:comment>
        <rdfs:comment xml:lang="en">The set of interrelated activities comprising of test planning, test monitoring, test control, test analysis, test design, test implementation, test execution, and test completion. (ISTQB Glossary v4.5)

Set of testing activities performed to achieve a test objective. (ISO/IEC/IEEE 29119-1:2022)</rdfs:comment>
        <rdfs:label>test process</rdfs:label>
        <rdfs:seeAlso>ISO/IEC/IEEE 29119-1:2022 (Software and Systems Engineering — Software Testing — Part 1: Concepts and Definitions)

Foundation - v4.0
Specialist - Mobile Application Testing - 2019
Specialist - Security Test Engineer - v1.0</rdfs:seeAlso>
        <skos:prefLabel xml:lang="en">test process</skos:prefLabel>
    </owl:NamedIndividual>
    


    <!-- http://purl.org/stc/terms#test_process_group -->

    <owl:NamedIndividual rdf:about="http://purl.org/stc/terms#test_process_group">
        <terms:hasParent rdf:resource="http://purl.org/stc/terms#related_to_team"/>
        <isInISTQBGlossary rdf:datatype="http://www.w3.org/2001/XMLSchema#boolean">true</isInISTQBGlossary>
        <rdfs:comment xml:lang="en">A collection of specialists who facilitate the definition, maintenance, and improvement of the test processes used by an organization. (ISTQB Glossary v4.5)</rdfs:comment>
        <rdfs:label>test process group</rdfs:label>
        <rdfs:seeAlso>Expert Improving the Test Process - v1.0.1</rdfs:seeAlso>
        <skos:altLabel xml:lang="en">TPG</skos:altLabel>
        <skos:prefLabel xml:lang="en">test process group</skos:prefLabel>
    </owl:NamedIndividual>
    


    <!-- http://purl.org/stc/terms#test_process_improvement -->

    <owl:NamedIndividual rdf:about="http://purl.org/stc/terms#test_process_improvement">
        <terms:hasParent rdf:resource="http://purl.org/stc/terms#test_management"/>
        <isInISTQBGlossary rdf:datatype="http://www.w3.org/2001/XMLSchema#boolean">true</isInISTQBGlossary>
        <rdfs:label>test process improvement</rdfs:label>
        <skos:prefLabel xml:lang="en">test process improvement</skos:prefLabel>
    </owl:NamedIndividual>
    


    <!-- http://purl.org/stc/terms#test_progress_report -->

    <owl:NamedIndividual rdf:about="http://purl.org/stc/terms#test_progress_report">
        <terms:hasParent rdf:resource="http://purl.org/stc/terms#test_report"/>
        <isInISTQBGlossary rdf:datatype="http://www.w3.org/2001/XMLSchema#boolean">true</isInISTQBGlossary>
        <rdfs:comment xml:lang="en">A type of periodic test report that includes the progress of test activities against a baseline, risks, and alternatives requiring a decision. (ISTQB Glossary v4.5)

Report that provides information about the status of the testing that is being performed in a specified reporting period. (ISO/IEC/IEEE 29119-1:2022, defined as test status report)</rdfs:comment>
        <rdfs:label>test progress report</rdfs:label>
        <rdfs:seeAlso>ISO/IEC/IEEE 29119-1:2022 (Software and systems engineering — Software testing — Part 1: Concepts and definitions)

Foundation - v4.0
Advanced Test Automation Engineering - v2.0</rdfs:seeAlso>
        <skos:altLabel xml:lang="en">test status report</skos:altLabel>
        <skos:prefLabel xml:lang="en">test progress report</skos:prefLabel>
    </owl:NamedIndividual>
    


    <!-- http://purl.org/stc/terms#test_report -->

    <owl:NamedIndividual rdf:about="http://purl.org/stc/terms#test_report">
        <terms:hasParent rdf:resource="http://purl.org/stc/terms#Testware"/>
        <isInISTQBGlossary rdf:datatype="http://www.w3.org/2001/XMLSchema#boolean">true</isInISTQBGlossary>
        <rdfs:comment xml:lang="en">Documentation summarizing testing and results. (ISTQB Glossary v4.5)</rdfs:comment>
        <rdfs:label>test report</rdfs:label>
        <rdfs:seeAlso>Specialist - Mobile Application Testing - 2019
Specialist - Security Test Engineer - v1.0
Specialist - Test Automation Strategy - v1.0</rdfs:seeAlso>
        <skos:altLabel xml:lang="en">testreport</skos:altLabel>
        <skos:prefLabel xml:lang="en">test report</skos:prefLabel>
    </owl:NamedIndividual>
    


    <!-- http://purl.org/stc/terms#test_script -->

    <owl:NamedIndividual rdf:about="http://purl.org/stc/terms#test_script">
        <terms:hasParent rdf:resource="http://purl.org/stc/terms#Testware"/>
        <isInISTQBGlossary rdf:datatype="http://www.w3.org/2001/XMLSchema#boolean">true</isInISTQBGlossary>
        <rdfs:comment xml:lang="en">A sequence of instructions for the execution of a test. (ISTQB Glossary v4.5)

Document specifying one or more test procedures. (ISO/IEC/IEEE 29119-1:2022)</rdfs:comment>
        <rdfs:label>test script</rdfs:label>
        <rdfs:seeAlso>ISO/IEC/IEEE 29119-1:2022 (Software and systems engineering — Software testing — Part 1: Concepts and definitions)

Advanced Test Manager - 2012
Advanced Test Analyst - v3.1
Advanced Test Analyst - v4.0
Advanced Test Automation Engineering - v2.0
Specialist - Test Automation Engineer - 2016</rdfs:seeAlso>
        <skos:altLabel xml:lang="en">test procedure specification</skos:altLabel>
        <skos:prefLabel xml:lang="en">test script</skos:prefLabel>
    </owl:NamedIndividual>
    


    <!-- http://purl.org/stc/terms#test_step -->

    <owl:NamedIndividual rdf:about="http://purl.org/stc/terms#test_step">
        <terms:hasParent rdf:resource="http://purl.org/stc/terms#Testware"/>
        <isInISTQBGlossary rdf:datatype="http://www.w3.org/2001/XMLSchema#boolean">true</isInISTQBGlossary>
        <rdfs:comment xml:lang="en">A single interaction between an actor and a test object consisting of an input, an action, and an expected result. (ISTQB Glossary v4.5)</rdfs:comment>
        <rdfs:comment xml:lang="en">Advanced Test Automation Engineering - v2.0</rdfs:comment>
        <rdfs:label>test step</rdfs:label>
        <skos:altLabel xml:lang="en">teststep</skos:altLabel>
        <skos:prefLabel xml:lang="en">test step</skos:prefLabel>
    </owl:NamedIndividual>
    


    <!-- http://purl.org/stc/terms#test_suite -->

    <owl:NamedIndividual rdf:about="http://purl.org/stc/terms#test_suite">
        <terms:hasParent rdf:resource="http://purl.org/stc/terms#Testware"/>
        <isInISTQBGlossary rdf:datatype="http://www.w3.org/2001/XMLSchema#boolean">true</isInISTQBGlossary>
        <rdfs:comment xml:lang="en">A set of test scripts or test procedures to be executed in a specific test run. (ISTQB Glossary v4.5)

Set of test cases or test procedures. (ISO/IEC/IEEE 29119-1:2022)</rdfs:comment>
        <rdfs:label>test suite</rdfs:label>
        <rdfs:seeAlso>Advanced Test Analyst - v3.1
Specialist - Test Automation Strategy - v1.0</rdfs:seeAlso>
        <skos:altLabel xml:lang="en">test set
test case suite
testsuite
testset
testcase suite</skos:altLabel>
        <skos:prefLabel xml:lang="en">test suite</skos:prefLabel>
    </owl:NamedIndividual>
    


    <!-- http://purl.org/stc/terms#test_technique -->

    <owl:NamedIndividual rdf:about="http://purl.org/stc/terms#test_technique">
        <terms:hasParent rdf:resource="http://purl.org/stc/terms#software_testing_concepts"/>
        <isInISTQBGlossary rdf:datatype="http://www.w3.org/2001/XMLSchema#boolean">true</isInISTQBGlossary>
        <rdfs:comment xml:lang="en">(ISTQB Glossary v4.5)</rdfs:comment>
        <rdfs:comment xml:lang="en">A procedure used to define test conditions, design test cases, and specify test data. (ISTQB Glossary v4.5)

Procedure used to create or select a test model, identify test coverage items, and derive
corresponding test cases. (ISO/IEC/IEEE 29119-1:2022, defined as test design technique)</rdfs:comment>
        <rdfs:label>test technique</rdfs:label>
        <rdfs:seeAlso>ISO/IEC/IEEE 29119-4 (Software and systems engineering — Software testing — Part 4: Test techniques)

Foundation - v4.0</rdfs:seeAlso>
        <skos:altLabel xml:lang="en">test design technique</skos:altLabel>
        <skos:altLabel xml:lang="en">test technique</skos:altLabel>
    </owl:NamedIndividual>
    


    <!-- http://purl.org/stc/terms#test_type -->

    <owl:NamedIndividual rdf:about="http://purl.org/stc/terms#test_type">
        <terms:hasParent rdf:resource="http://purl.org/stc/terms#software_testing_concepts"/>
        <isInISTQBGlossary rdf:datatype="http://www.w3.org/2001/XMLSchema#boolean">true</isInISTQBGlossary>
        <rdfs:comment xml:lang="en">A group of test activities based on specific test objectives aimed at specific characteristics of a component or system. (ISTQB Glossary v4.5)

Testing that is focused on specific quality characteristics. (ISO/IEC/IEEE 29119-1:2022)</rdfs:comment>
        <rdfs:label>test type</rdfs:label>
        <rdfs:seeAlso>ISO/IEC/IEEE 29119-1:2022 (Software and Systems Engineering — Software Testing — Part 1: Concepts and Definitions)

Foundation - v4.0
Advanced Test Manager - 2012
Advanced Test Management - v3.0
Advanced Test Analyst - v3.1
Advanced Test Analyst - v4.0
Advanced Technical Test Analyst - v4.0
Advanced Test Automation Engineering - v2.0
Specialist - Automotive Software Tester - 2018
Specialist - Automotive Software Tester - v1.1
Specialist - Gambling Industry Tester - 2018
Specialist - Game Testing - v1.0.1
Specialist - Mobile Application Testing - 2019
Specialist - Model-Based Testing - v1.1
Specialist - Test Automation Strategy - v1.0</rdfs:seeAlso>
        <skos:prefLabel xml:lang="en">test type</skos:prefLabel>
    </owl:NamedIndividual>
    


    <!-- http://purl.org/stc/terms#test_work_force -->

    <owl:NamedIndividual rdf:about="http://purl.org/stc/terms#test_work_force">
        <terms:hasParent rdf:resource="http://purl.org/stc/terms#software_testing_concepts"/>
        <isInISTQBGlossary rdf:datatype="http://www.w3.org/2001/XMLSchema#boolean">false</isInISTQBGlossary>
        <rdfs:comment xml:lang="en">Professions and roles in software testing</rdfs:comment>
        <rdfs:label>test work force</rdfs:label>
        <rdfs:seeAlso>GTB: The Professional profile for testing. The reference scheme for people and organizations involved in the topics of quality and testing of software-based components and systems. 2018.</rdfs:seeAlso>
        <skos:prefLabel xml:lang="en">test work force</skos:prefLabel>
    </owl:NamedIndividual>
    


    <!-- http://purl.org/stc/terms#tester -->

    <owl:NamedIndividual rdf:about="http://purl.org/stc/terms#tester">
        <terms:hasParent rdf:resource="http://purl.org/stc/terms#related_to_role"/>
        <isInISTQBGlossary rdf:datatype="http://www.w3.org/2001/XMLSchema#boolean">true</isInISTQBGlossary>
        <rdfs:comment xml:lang="en">A person who performs testing. (ISTQB Glossary v4.5)

Develops the test deliverables and completes the processes associated with the
dynamic test process. (ISO/IEC/IEEE 29119-1:2022)</rdfs:comment>
        <rdfs:label>tester</rdfs:label>
        <rdfs:seeAlso>ISO/IEC/IEEE 29119-1:2022 (Software and systems engineering — Software testing — Part 1: Concepts and definitions)</rdfs:seeAlso>
        <skos:prefLabel xml:lang="en">tester</skos:prefLabel>
    </owl:NamedIndividual>
    


    <!-- http://purl.org/stc/terms#tester_orientation_in_test_approach -->

    <owl:NamedIndividual rdf:about="http://purl.org/stc/terms#tester_orientation_in_test_approach">
        <terms:hasParent rdf:resource="http://purl.org/stc/terms#test_approach"/>
        <isInISTQBGlossary rdf:datatype="http://www.w3.org/2001/XMLSchema#boolean">false</isInISTQBGlossary>
        <rdfs:label>tester orientation</rdfs:label>
        <skos:prefLabel xml:lang="en">tester orientation in test approach</skos:prefLabel>
    </owl:NamedIndividual>
    


    <!-- http://purl.org/stc/terms#testing -->

    <owl:NamedIndividual rdf:about="http://purl.org/stc/terms#testing">
        <terms:hasParent rdf:resource="http://purl.org/stc/terms#software_testing_concepts"/>
        <isInISTQBGlossary rdf:datatype="http://www.w3.org/2001/XMLSchema#boolean">true</isInISTQBGlossary>
        <rdfs:comment xml:lang="en">Set of activities conducted to facilitate discovery and evaluation of properties of test items (ISO/IEC/IEEE 29119-1:2022, defined as test)

The process that consists of determining the degree to which a software product satisfies specified requirements (verification) and fulfills its intended purpose (validation). (ISO/IEC/IEEE 12207:2017)

The process of executing a system or component under specified conditions, observing or recording the results, and making an evaluation of some aspect of the system or component. (IEEE 610.12-1990)</rdfs:comment>
        <rdfs:seeAlso>Foundation - v4.0</rdfs:seeAlso>
        <rdfs:seeAlso>IEEE Standard 610.12-1990 (IEEE Standard Glossary of Software Engineering Terminology)
ISO/IEC/IEEE 29119-1:2022 (Software and Systems Engineering — Software Testing — Part 1: Concepts and Definitions)
ISO/IEC/IEEE 12207:2017 (Software Life Cycle Processes)</rdfs:seeAlso>
        <skos:prefLabel xml:lang="en">testing</skos:prefLabel>
    </owl:NamedIndividual>
    


    <!-- http://purl.org/stc/terms#testing_in_production -->

    <owl:NamedIndividual rdf:about="http://purl.org/stc/terms#testing_in_production">
        <terms:hasParent rdf:resource="http://purl.org/stc/terms#system_testing"/>
        <isInISTQBGlossary rdf:datatype="http://www.w3.org/2001/XMLSchema#boolean">true</isInISTQBGlossary>
        <rdfs:label>testing in production</rdfs:label>
        <skos:prefLabel xml:lang="en">testing in production</skos:prefLabel>
    </owl:NamedIndividual>
    


    <!-- http://purl.org/stc/terms#testing_quadrants -->

    <owl:NamedIndividual rdf:about="http://purl.org/stc/terms#testing_quadrants">
        <terms:hasParent rdf:resource="http://purl.org/stc/terms#test_approach"/>
        <isInISTQBGlossary rdf:datatype="http://www.w3.org/2001/XMLSchema#boolean">true</isInISTQBGlossary>
        <rdfs:comment xml:lang="en">A classification model of test types/test levels in four quadrants, relating them to two dimensions of test objectives: supporting the product team versus critiquing the product, and technology-facing versus business-facing. (ISTQB Glossary v4.5)</rdfs:comment>
        <rdfs:label>testing quadrants</rdfs:label>
        <rdfs:seeAlso>Foundation - v4.0</rdfs:seeAlso>
        <skos:prefLabel xml:lang="en">testing quadrants</skos:prefLabel>
    </owl:NamedIndividual>
    


    <!-- http://purl.org/stc/terms#usability_testing -->

    <owl:NamedIndividual rdf:about="http://purl.org/stc/terms#usability_testing">
        <terms:hasParent rdf:resource="http://purl.org/stc/terms#non-functional_testing"/>
        <isInISTQBGlossary rdf:datatype="http://www.w3.org/2001/XMLSchema#boolean">true</isInISTQBGlossary>
        <rdfs:comment xml:lang="en">Testing to evaluate the degree to which the system can be used by specified users with effectiveness, efficiency and satisfaction in a specified context of use. (ISTQB Glossary v4.5)</rdfs:comment>
        <rdfs:label>usability testing</rdfs:label>
        <rdfs:seeAlso>Specialist - Mobile Application Testing - 2019
Specialist - Usability Testing - 2018</rdfs:seeAlso>
        <skos:prefLabel xml:lang="en">usability testing</skos:prefLabel>
    </owl:NamedIndividual>
    


    <!-- http://purl.org/stc/terms#user-agent_based_testing -->

    <owl:NamedIndividual rdf:about="http://purl.org/stc/terms#user-agent_based_testing">
        <terms:hasParent rdf:resource="http://purl.org/stc/terms#mobile_app_testing"/>
        <isInISTQBGlossary rdf:datatype="http://www.w3.org/2001/XMLSchema#boolean">true</isInISTQBGlossary>
        <rdfs:label>user-agent based testing</rdfs:label>
        <skos:prefLabel xml:lang="en">user-agent based testing</skos:prefLabel>
    </owl:NamedIndividual>
    


    <!-- http://purl.org/stc/terms#user_acceptance_testing -->

    <owl:NamedIndividual rdf:about="http://purl.org/stc/terms#user_acceptance_testing">
        <terms:hasParent rdf:resource="http://purl.org/stc/terms#acceptance_testing"/>
        <isInISTQBGlossary rdf:datatype="http://www.w3.org/2001/XMLSchema#boolean">true</isInISTQBGlossary>
        <rdfs:label>user acceptance testing</rdfs:label>
        <skos:prefLabel xml:lang="en">user acceptance testing</skos:prefLabel>
    </owl:NamedIndividual>
    


    <!-- http://purl.org/stc/terms#validation -->

    <owl:NamedIndividual rdf:about="http://purl.org/stc/terms#validation">
        <terms:hasParent rdf:resource="http://purl.org/stc/terms#basic_concepts"/>
    </owl:NamedIndividual>
    


    <!-- http://purl.org/stc/terms#verification -->

    <owl:NamedIndividual rdf:about="http://purl.org/stc/terms#verification">
        <terms:hasParent rdf:resource="http://purl.org/stc/terms#basic_concepts"/>
    </owl:NamedIndividual>
    


    <!-- http://purl.org/stc/terms#walkthrough -->

    <owl:NamedIndividual rdf:about="http://purl.org/stc/terms#walkthrough">
        <terms:hasParent rdf:resource="http://purl.org/stc/terms#informal_review"/>
        <isInISTQBGlossary rdf:datatype="http://www.w3.org/2001/XMLSchema#boolean">true</isInISTQBGlossary>
        <rdfs:comment xml:lang="en">A type of review in which an author leads members of the review through a work product and the members ask questions and make comments about possible issues.  (ISTQB Glossary v4.5)</rdfs:comment>
        <rdfs:label>walkthrough</rdfs:label>
        <rdfs:seeAlso>Foundation - v4.0
Advanced Test Manager - 2012</rdfs:seeAlso>
        <skos:altLabel xml:lang="en">structured walkthrough</skos:altLabel>
        <skos:prefLabel xml:lang="en">walkthrough</skos:prefLabel>
    </owl:NamedIndividual>
    


    <!-- http://purl.org/stc/terms#white_box_test_technique -->

    <owl:NamedIndividual rdf:about="http://purl.org/stc/terms#white_box_test_technique">
        <terms:hasParent rdf:resource="http://purl.org/stc/terms#test_technique"/>
        <isInISTQBGlossary rdf:datatype="http://www.w3.org/2001/XMLSchema#boolean">true</isInISTQBGlossary>
        <rdfs:label>white box test technique</rdfs:label>
        <skos:altLabel xml:lang="en">white-box test technique
structure-based test design technique
structure based test design technique
structure-based test technique
structure based test technique
glass-box testing</skos:altLabel>
        <skos:prefLabel xml:lang="en">white box test technique</skos:prefLabel>
    </owl:NamedIndividual>
</rdf:RDF>



<!-- Generated by the OWL API (version 4.5.29.2024-05-13T12:11:03Z) https://github.com/owlcs/owlapi -->

