@prefix : <http://purl.org/stc/ontology#> .
@prefix owl: <http://www.w3.org/2002/07/owl#> .
@prefix rdf: <http://www.w3.org/1999/02/22-rdf-syntax-ns#> .
@prefix xml: <http://www.w3.org/XML/1998/namespace> .
@prefix xsd: <http://www.w3.org/2001/XMLSchema#> .
@prefix rdfs: <http://www.w3.org/2000/01/rdf-schema#> .
@base <http://purl.org/stc/ontology#> .

<http://purl.org/stc/ontology#> rdf:type owl:Ontology ;
                                 owl:versionIRI <http://purl.org/stc/ontology#/1.0.0> ;
                                 owl:imports <http://purl.org/nemo/gufo#/1.0.0> ;
                                 <http://purl.org/dc/elements/1.1/title> "stc - The Software Testing Concepts Ontology"@en ;
                                 <http://purl.org/dc/terms/bibliographicCitation> "Schieferdecker, I.K.: \"stc: The software testing concepts ontology\", 2025, http://purl.org/stc"@en ;
                                 <http://purl.org/dc/terms/license> "http://creativecommons.org/licenses/by/4.0/legalcode.en" ;
                                 :preferredNamespacePrefix "stc:"@en ;
                                 :preferredNamespaceURI "http://purl.org/stc/ontology#" ;
                                 rdfs:comment """ISTQB test process mind map.pdf reflected, but 
- collaboration-based approach not contained (as it is too general)
- acceptance test-driven development being a test-first approach represented as a software development model (and not as a test approach)

ISTQB static & dynamic testing mind map.pdf reflected, but 
- with a lot more detailed reflection of test types, test approaches, and test techniques

Top software testing concepts like testing, test activity, etc. put in relation to each other and/or to software engineering conceps

ISTQB test techniques mind map.pdf reflected"""@en ;
                                 owl:versionInfo 1 ;
                                 <http://www.w3.org/2004/02/skos/core#prefLabel> "stc"@en .

#################################################################
#    Annotation properties
#################################################################

###  http://purl.org/dc/elements/1.1/title
<http://purl.org/dc/elements/1.1/title> rdf:type owl:AnnotationProperty .


###  http://purl.org/dc/terms/bibliographicCitation
<http://purl.org/dc/terms/bibliographicCitation> rdf:type owl:AnnotationProperty .


###  http://purl.org/dc/terms/license
<http://purl.org/dc/terms/license> rdf:type owl:AnnotationProperty .


###  http://purl.org/stc/ontology#isInISTQBGlossary
:isInISTQBGlossary rdf:type owl:AnnotationProperty ;
                   rdfs:comment "A flag indicating if this concept is defined by the ISTQB glossary" ;
                   rdfs:label "is in ISTQB glossary" ;
                   <http://www.w3.org/2004/02/skos/core#prefLabel> "is in ISTQB glossary"@en ;
                   rdfs:range xsd:boolean .


###  http://purl.org/stc/ontology#preferredNamespacePrefix
:preferredNamespacePrefix rdf:type owl:AnnotationProperty .


###  http://purl.org/stc/ontology#preferredNamespaceURI
:preferredNamespaceURI rdf:type owl:AnnotationProperty .


###  http://www.w3.org/2004/02/skos/core#altLabel
<http://www.w3.org/2004/02/skos/core#altLabel> rdf:type owl:AnnotationProperty .


###  http://www.w3.org/2004/02/skos/core#prefLabel
<http://www.w3.org/2004/02/skos/core#prefLabel> rdf:type owl:AnnotationProperty .


#################################################################
#    Object Properties
#################################################################

###  http://purl.org/stc/ontology#creates
:creates rdf:type owl:ObjectProperty ;
         rdfs:domain :software_engineering_activity ;
         rdfs:range :software ;
         rdfs:comment "Indicates that the subject concept creates instances of the object concept."@en ;
         rdfs:label "creates" ;
         <http://www.w3.org/2004/02/skos/core#prefLabel> "creates"@en .


###  http://purl.org/stc/ontology#createsTestCompletionReport
:createsTestCompletionReport rdf:type owl:ObjectProperty ;
                             rdfs:subPropertyOf :creates ;
                             rdfs:domain :test_completion ;
                             rdfs:range :test_completion_report ;
                             rdfs:comment "Indicates that a test completion report is created by the test completion activity."@en ;
                             <http://www.w3.org/2004/02/skos/core#prefLabel> "createsTestCompletionReport"@en .


###  http://purl.org/stc/ontology#createsTestCondition
:createsTestCondition rdf:type owl:ObjectProperty ;
                      rdfs:subPropertyOf :creates ;
                      rdfs:domain :test_analysis ;
                      rdfs:range :test_condition ;
                      rdfs:comment "Indicates that a test condition is created by the test analysis activity."@en ;
                      <http://www.w3.org/2004/02/skos/core#prefLabel> "createsTestCondition"@en .


###  http://purl.org/stc/ontology#createsTestPlan
:createsTestPlan rdf:type owl:ObjectProperty ;
                 rdfs:subPropertyOf :creates ;
                 rdfs:domain :test_planning ;
                 rdfs:range :test_plan ;
                 rdfs:comment "Indicates that a test plan is created by the test planning activity."@en ;
                 <http://www.w3.org/2004/02/skos/core#prefLabel> "createsTestPlan"@en .


###  http://purl.org/stc/ontology#createsTestProgressReport
:createsTestProgressReport rdf:type owl:ObjectProperty ;
                           rdfs:subPropertyOf :creates ;
                           rdfs:domain :test_monitoring ;
                           rdfs:range :test_progress_report ;
                           rdfs:comment "Indicates that a test progress report  is created by the test monitoring activity."@en ;
                           <http://www.w3.org/2004/02/skos/core#prefLabel> "createsTestProgressReport"@en .


###  http://purl.org/stc/ontology#createsTests
:createsTests rdf:type owl:ObjectProperty ;
              rdfs:subPropertyOf :creates ;
              rdfs:domain :test_design ;
              rdfs:range :test_case ,
                         :test_data ;
              rdfs:comment "Indicates that a test case and/or test data are created by the test design activity."@en ;
              <http://www.w3.org/2004/02/skos/core#prefLabel> "createsTests"@en .


###  http://purl.org/stc/ontology#isPartOf
:isPartOf rdf:type owl:ObjectProperty ;
          rdfs:comment "Indicates that the subject concept is part of the object concept."@en ;
          rdfs:label "isPartOf" ;
          <http://www.w3.org/2004/02/skos/core#prefLabel> "is part of"@en .


###  http://purl.org/stc/ontology#isPartOfTestObject
:isPartOfTestObject rdf:type owl:ObjectProperty ;
                    rdfs:subPropertyOf :isPartOf ;
                    rdfs:domain :test_item ;
                    rdfs:range :test_object ;
                    rdfs:comment "Indicates that test items are part of a test object."@en ;
                    <http://www.w3.org/2004/02/skos/core#prefLabel> "isPartOfTestObject"@en .


###  http://purl.org/stc/ontology#useInGreyBoxTesting
:useInGreyBoxTesting rdf:type owl:ObjectProperty ;
                     rdfs:subPropertyOf :uses ;
                     rdfs:domain :grey_box_test_technique ;
                     rdfs:range :black_box_test_technique ,
                                :white_box_test_technique ;
                     rdfs:comment "Indicates that a grey-box test technique utilizes principles, knowledge, or aspects from black-box and  white-box test techniques."@en ;
                     <http://www.w3.org/2004/02/skos/core#prefLabel> "useInGreyBoxTesting"@en .


###  http://purl.org/stc/ontology#useInTestActivity
:useInTestActivity rdf:type owl:ObjectProperty ;
                   rdfs:subPropertyOf :uses ;
                   rdfs:domain :test_activity ;
                   rdfs:range :Testware ,
                              :software ;
                   rdfs:label "Indicates that a test activity uses testware and software (of the test object)." ,
                              "useInTestActivity" ;
                   <http://www.w3.org/2004/02/skos/core#prefLabel> "useInTestActivity"@en .


###  http://purl.org/stc/ontology#useInTestAnalysis
:useInTestAnalysis rdf:type owl:ObjectProperty ;
                   rdfs:subPropertyOf :uses ;
                   rdfs:domain :test_analysis ;
                   rdfs:range :test_basis ;
                   rdfs:comment "Indicates that a test analysis utilizes the test basis."@en ;
                   <http://www.w3.org/2004/02/skos/core#prefLabel> "useInTestAnalysis"@en .


###  http://purl.org/stc/ontology#useInTestCase
:useInTestCase rdf:type owl:ObjectProperty ;
               rdfs:subPropertyOf :uses ;
               rdfs:domain :test_case ;
               rdfs:range :test_data ,
                          :test_step ;
               rdfs:comment "Indicates that a test case may utilizes test steps and/or test data."@en ;
               <http://www.w3.org/2004/02/skos/core#prefLabel> "useInTestCase"@en .


###  http://purl.org/stc/ontology#useInTestCondition
:useInTestCondition rdf:type owl:ObjectProperty ;
                    rdfs:subPropertyOf :uses ;
                    rdfs:domain :test_condition ;
                    rdfs:range :acceptance_criteria ,
                               :coverage_item ;
                    rdfs:comment "Indicates that a test condition utilizes acceptance criteria and coverage items."@en ;
                    <http://www.w3.org/2004/02/skos/core#prefLabel> "useInTestCondition"@en .


###  http://purl.org/stc/ontology#useInTestDesign
:useInTestDesign rdf:type owl:ObjectProperty ;
                 rdfs:subPropertyOf :uses ;
                 rdfs:domain :test_design ;
                 rdfs:range :test_condition ,
                            :test_technique ;
                 rdfs:comment "Indicates that a test design utilizes test techniques and test conditions."@en ;
                 <http://www.w3.org/2004/02/skos/core#prefLabel> "useInTestDesign"@en .


###  http://purl.org/stc/ontology#useInTestExecution
:useInTestExecution rdf:type owl:ObjectProperty ;
                    rdfs:subPropertyOf :uses ;
                    rdfs:domain :test_execution ;
                    rdfs:range :test_object ,
                               :test_suite ;
                    rdfs:comment "Indicates that a test execution utilizes test objects and test suites."@en ;
                    <http://www.w3.org/2004/02/skos/core#prefLabel> "useInTestExecution"@en .


###  http://purl.org/stc/ontology#useInTestPlan
:useInTestPlan rdf:type owl:ObjectProperty ;
               rdfs:subPropertyOf :uses ;
               rdfs:domain :test_plan ;
               rdfs:range :entry_criteria ,
                          :exit_criteria ,
                          :test_approach ,
                          :test_objective ;
               rdfs:comment "Indicates that a test plan utilizes test approaches, test objectives, and entry and exit criteria."@en ;
               <http://www.w3.org/2004/02/skos/core#prefLabel> "useInTestPlan"@en .


###  http://purl.org/stc/ontology#useInTestProcess
:useInTestProcess rdf:type owl:ObjectProperty ;
                  rdfs:subPropertyOf :uses ;
                  rdfs:domain :test_process ;
                  rdfs:range :Testware ,
                             :test_activity ,
                             :test_approach ,
                             :test_level ,
                             :test_metric ,
                             :test_type ;
                  rdfs:comment "Indicates that a test process utilizes test activities, testware, test metrics, test levels, test approaches and test types."@en ;
                  <http://www.w3.org/2004/02/skos/core#prefLabel> "useInTestProcess"@en .


###  http://purl.org/stc/ontology#useInTestQuadrants
:useInTestQuadrants rdf:type owl:ObjectProperty ;
                    rdfs:subPropertyOf :uses ;
                    rdfs:domain :testing_quadrants ;
                    rdfs:range :test_approach ,
                               :test_level ,
                               :test_type ;
                    rdfs:comment "Indicates that a test quadrant utilizes test levels and test types/test approaches."@en ;
                    <http://www.w3.org/2004/02/skos/core#prefLabel> "useInTestQuadrants"@en .


###  http://purl.org/stc/ontology#useInTesting
:useInTesting rdf:type owl:ObjectProperty ;
              rdfs:subPropertyOf :uses ;
              rdfs:domain :testing ;
              rdfs:range :test_management ,
                         :test_process ,
                         :test_work_force ;
              rdfs:comment "Indicates that testing is done by a test work force along a test process that is to be managed."@en ;
              rdfs:label "useInTesting" ;
              <http://www.w3.org/2004/02/skos/core#prefLabel> "useInTesting"@en .


###  http://purl.org/stc/ontology#uses
:uses rdf:type owl:ObjectProperty ;
      rdfs:comment "Indicates that the subject concept utilizes principles, knowledge, or aspects commonly associated with the object concept."@en ;
      rdfs:label "uses" ;
      <http://www.w3.org/2004/02/skos/core#prefLabel> "uses"@en .


###  http://purl.org/stc/terms#hasParent
<http://purl.org/stc/terms#hasParent> rdf:type owl:ObjectProperty .


#################################################################
#    Classes
#################################################################

###  http://purl.org/stc/ontology#AI_testing
:AI_testing rdf:type owl:Class ;
            rdfs:subClassOf :domain-specific_test_types ;
            :isInISTQBGlossary "true"^^xsd:boolean ;
            rdfs:label "AI testing" ;
            <http://www.w3.org/2004/02/skos/core#prefLabel> "ai testing"@en .


###  http://purl.org/stc/ontology#API_testing
:API_testing rdf:type owl:Class ;
             rdfs:subClassOf :interface_testing ;
             :isInISTQBGlossary "true"^^xsd:boolean ;
             rdfs:label "API testing" ;
             <http://www.w3.org/2004/02/skos/core#prefLabel> "api testing"@en .


###  http://purl.org/stc/ontology#GUI_testing
:GUI_testing rdf:type owl:Class ;
             rdfs:subClassOf :interface_testing ;
             :isInISTQBGlossary "true"^^xsd:boolean ;
             rdfs:label "GUI testing" ;
             <http://www.w3.org/2004/02/skos/core#altLabel> "graphical user interface testing"@en ;
             <http://www.w3.org/2004/02/skos/core#prefLabel> "GUI testing"@en .


###  http://purl.org/stc/ontology#LLM_structural_coverage
:LLM_structural_coverage rdf:type owl:Class ;
                         rdfs:subClassOf :structural_coverage ;
                         :isInISTQBGlossary "false"^^xsd:boolean ;
                         rdfs:comment "Coverage measures based on the internal structure of an LLM. (own))"@en ;
                         rdfs:label "LLM structural coverage" ;
                         <http://www.w3.org/2004/02/skos/core#prefLabel> "llm structural coverage"@en .


###  http://purl.org/stc/ontology#MBT_modeller
:MBT_modeller rdf:type owl:Class ;
              rdfs:subClassOf :related_to_role ;
              :isInISTQBGlossary "false"^^xsd:boolean ;
              rdfs:comment "Develops formal test specifications in the form of models used to generate test cases as part of model-based testing. (ISO/IEC/IEEE 29119-1:2022)"@en ;
              rdfs:label "MBT modeller" ;
              rdfs:seeAlso "ISO/IEC/IEEE 29119-1:2022 (Software and systems engineering — Software testing — Part 1: Concepts and definitions)" ;
              <http://www.w3.org/2004/02/skos/core#prefLabel> "MBT modeller"@en .


###  http://purl.org/stc/ontology#N-switch_coverage
:N-switch_coverage rdf:type owl:Class ;
                   rdfs:subClassOf :structural_coverage ;
                   :isInISTQBGlossary "true"^^xsd:boolean ;
                   rdfs:comment "The coverage of sequences of N+1 transitions. (ISTQB Glossary v4.5)"@en ;
                   rdfs:label "N-switch coverage" ;
                   rdfs:seeAlso "" ;
                   <http://www.w3.org/2004/02/skos/core#altLabel> "chow's coverage metric"@en ;
                   <http://www.w3.org/2004/02/skos/core#prefLabel> """n-switch coverage
N-switch coverage"""@en .


###  http://purl.org/stc/ontology#Testware
:Testware rdf:type owl:Class ;
          rdfs:subClassOf :software_testing_concepts ;
          :isInISTQBGlossary "true"^^xsd:boolean ;
          rdfs:comment """Work products produced during the test process for use in planning, designing, executing, evaluating and reporting on testing. (ISTQB Glossary v4.5)

Artefacts produced during the test process required to plan, design, and execute tests. (ISO/IEC/IEEE 29119-1:2022)"""@en ;
          rdfs:label "testware" ;
          rdfs:seeAlso """ISO/IEC/IEEE 29119-1 (2022) Software and systems engineering -- Software testing -- Part 1: Concepts and definitions

Foundation - v4.0
Advanced Test Manager - 2012
Advanced Test Management - v3.0
Advanced Test Analyst - v3.1
Advanced Test Analyst - v4.0
Advanced Test Automation Engineering - v2.0
Specialist - Automotive Software Tester - v1.1
Specialist - Game Testing - v1.0.1
Specialist - Model-Based Testing - v1.1
Specialist - Performance Testing - 2018
Specialist - Test Automation Engineer - 2016
Specialist - Test Automation Strategy - v1.0""" ;
          <http://www.w3.org/2004/02/skos/core#altLabel> """test artefact
test artifact""" ;
          <http://www.w3.org/2004/02/skos/core#prefLabel> "testware"@en .


###  http://purl.org/stc/ontology#a_b_testing
:a_b_testing rdf:type owl:Class ;
             rdfs:subClassOf :oracle_orientation_in_test_approach ;
             :isInISTQBGlossary "true"^^xsd:boolean ;
             rdfs:comment """A test approach in which two components or systems are statistically evaluated to determine which performs better for specified criteria. (ISTQB Glossary v4.5) 

Statistical testing approach that allows testers to determine which of two systems or components performs better. (ISO/IEC/IEEE 29119-1:2022)"""@en ;
             rdfs:label "a/b testing" ;
             <http://www.w3.org/2004/02/skos/core#prefLabel> "a/b testing"@en .


###  http://purl.org/stc/ontology#acceptance
:acceptance rdf:type owl:Class ;
            rdfs:subClassOf :software_engineering_activity .


###  http://purl.org/stc/ontology#acceptance_criteria
:acceptance_criteria rdf:type owl:Class ;
                     rdfs:subClassOf :Testware ;
                     :isInISTQBGlossary "true"^^xsd:boolean ;
                     rdfs:comment """The criteria that a work product must satisfy to be accepted by the stakeholders. (ISTQB Glossary v4.5, after IREB Glossary)

Criteria that a system or system component must satisfy to be accepted by a user, customer, or other authorized entity.(ISO/IEC/IEEE 29148:2018)"""@en ;
                     rdfs:label "acceptance criteria" ;
                     rdfs:seeAlso "ISO/IEC/IEEE 29148:2018 (Systems and software engineering — Life cycle processes — Requirements engineering)" ;
                     <http://www.w3.org/2004/02/skos/core#prefLabel> "acceptance criteria"@en .


###  http://purl.org/stc/ontology#acceptance_test-driven_development
:acceptance_test-driven_development rdf:type owl:Class ;
                                    rdfs:subClassOf :test_first_approach ;
                                    :isInISTQBGlossary "true"^^xsd:boolean ;
                                    rdfs:label "acceptance test-driven development" ;
                                    <http://www.w3.org/2004/02/skos/core#prefLabel> "acceptance test-driven development"@en .


###  http://purl.org/stc/ontology#acceptance_testing
:acceptance_testing rdf:type owl:Class ;
                    rdfs:subClassOf :test_level ;
                    owl:disjointWith :component_testing ,
                                     :integration_testing ,
                                     :system_testing ;
                    :isInISTQBGlossary "true"^^xsd:boolean ;
                    rdfs:label "acceptance testing" ;
                    <http://www.w3.org/2004/02/skos/core#prefLabel> "acceptance testing"@en .


###  http://purl.org/stc/ontology#accessibility_testing
:accessibility_testing rdf:type owl:Class ;
                       rdfs:subClassOf :system_testing ;
                       :isInISTQBGlossary "false"^^xsd:boolean ;
                       rdfs:label "accessibility testing" ;
                       <http://www.w3.org/2004/02/skos/core#prefLabel> "accessibility testing"@en .


###  http://purl.org/stc/ontology#ad_hoc_testing
:ad_hoc_testing rdf:type owl:Class ;
                rdfs:subClassOf :method_orientation_in_test_approach ;
                :isInISTQBGlossary "true"^^xsd:boolean ;
                rdfs:comment "Informal testing performed without test analysis and test design."@en ;
                rdfs:label "ad hoc testing" ;
                rdfs:seeAlso "Specialist - Game Testing - v1.0.1" ;
                <http://www.w3.org/2004/02/skos/core#altLabel> """adhoc testing
ad hoc-testing"""@en ;
                <http://www.w3.org/2004/02/skos/core#prefLabel> "ad hoc testing"@en .


###  http://purl.org/stc/ontology#adversarial_testing
:adversarial_testing rdf:type owl:Class ;
                     rdfs:subClassOf :AI_testing ;
                     :isInISTQBGlossary "true"^^xsd:boolean ;
                     rdfs:label "adversarial testing" ;
                     <http://www.w3.org/2004/02/skos/core#prefLabel> "adversarial testing"@en .


###  http://purl.org/stc/ontology#agile_software_development
:agile_software_development rdf:type owl:Class ;
                            rdfs:subClassOf :process_orientation_in_software_development ;
                            :isInISTQBGlossary "true"^^xsd:boolean ;
                            rdfs:label "agile" ;
                            <http://www.w3.org/2004/02/skos/core#prefLabel> "agile software development"@en .


###  http://purl.org/stc/ontology#agile_test_leader
:agile_test_leader rdf:type owl:Class ;
                   rdfs:subClassOf :test_leader ;
                   :isInISTQBGlossary "true"^^xsd:boolean ;
                   rdfs:comment "A leadership role that serves agile teams, championing testing and quality at the organizational level. (ISTQB Glossary v4.5)"@en ;
                   rdfs:label "agile test leader" ;
                   rdfs:seeAlso """Agile Test Leadership at Scale - v1.0
Specialist - Agile Test Leadership at Scale - v2.0""" ;
                   <http://www.w3.org/2004/02/skos/core#altLabel> """quality coach
agile test manager
quality leader"""@en ;
                   <http://www.w3.org/2004/02/skos/core#prefLabel> "agile test leader"@en .


###  http://purl.org/stc/ontology#agile_test_team_leader
:agile_test_team_leader rdf:type owl:Class ;
                        rdfs:subClassOf :test_manager ;
                        :isInISTQBGlossary "true"^^xsd:boolean ;
                        rdfs:comment "A role that is responsible for maintaining solution quality within an agile delivery team. (ISTQB Glossary v4.5)"@en ;
                        rdfs:label "agile test team leader" ;
                        rdfs:seeAlso """Agile Test Leadership at Scale - v1.0
Specialist - Agile Test Leadership at Scale - v2.0""" ;
                        <http://www.w3.org/2004/02/skos/core#prefLabel> "agile test team leader"@en .


###  http://purl.org/stc/ontology#alpha_testing
:alpha_testing rdf:type owl:Class ;
               rdfs:subClassOf :acceptance_testing ;
               :isInISTQBGlossary "true"^^xsd:boolean ;
               rdfs:label "alpha testing" ;
               <http://www.w3.org/2004/02/skos/core#prefLabel> "alpha testing"@en .


###  http://purl.org/stc/ontology#architectural_design
:architectural_design rdf:type owl:Class ;
                      rdfs:subClassOf :software_engineering_activity .


###  http://purl.org/stc/ontology#automated_testing
:automated_testing rdf:type owl:Class ;
                   rdfs:subClassOf :test_execution ;
                   :isInISTQBGlossary "false"^^xsd:boolean ;
                   rdfs:label "automated testing" ;
                   <http://www.w3.org/2004/02/skos/core#prefLabel> "automated testing"@en .


###  http://purl.org/stc/ontology#back-to-back_testing
:back-to-back_testing rdf:type owl:Class ;
                      rdfs:subClassOf :oracle_orientation_in_test_approach ;
                      :isInISTQBGlossary "true"^^xsd:boolean ;
                      rdfs:label "back-to-back testing" ;
                      <http://www.w3.org/2004/02/skos/core#altLabel> "back to back testing"@en ;
                      <http://www.w3.org/2004/02/skos/core#prefLabel> "back-to-back testing"@en .


###  http://purl.org/stc/ontology#base_choice_coverage
:base_choice_coverage rdf:type owl:Class ;
                      rdfs:subClassOf :specification_coverage ;
                      :isInISTQBGlossary "true"^^xsd:boolean ;
                      rdfs:comment """The coverage of parameter-value combinations in which each value of a parameter is combined with the base values of all other parameters, for a chosen base value per parameter. (ISTQB Glossary v4.5)

Coverage for base choice testing. (ISO/IEC/IEEE 29119-4)"""@en ;
                      rdfs:label "base choice coverage" ;
                      rdfs:seeAlso "ISO/IEC/IEEE 29119-4 (Software and systems engineering — Software testing — Part 4: Test techniques)" ;
                      <http://www.w3.org/2004/02/skos/core#altLabel> "p-v pair coverage"@en ;
                      <http://www.w3.org/2004/02/skos/core#prefLabel> "base choice coverage"@en .


###  http://purl.org/stc/ontology#basic_concepts
:basic_concepts rdf:type owl:Class ;
                rdfs:subClassOf :software_engineering_concepts ;
                :isInISTQBGlossary "false"^^xsd:boolean ;
                rdfs:label "basic concepts" ;
                <http://www.w3.org/2004/02/skos/core#prefLabel> "basic concepts"@en .


###  http://purl.org/stc/ontology#behavior-driven_development
:behavior-driven_development rdf:type owl:Class ;
                             rdfs:subClassOf :target_orientation_in_software_development ;
                             :isInISTQBGlossary "true"^^xsd:boolean ;
                             rdfs:label "behavior-driven" ;
                             <http://www.w3.org/2004/02/skos/core#altLabel> """behavior driven development
bdd
BDD"""@en ;
                             <http://www.w3.org/2004/02/skos/core#prefLabel> "behavior-driven development"@en .


###  http://purl.org/stc/ontology#beta_testing
:beta_testing rdf:type owl:Class ;
              rdfs:subClassOf :acceptance_testing ;
              :isInISTQBGlossary "true"^^xsd:boolean ;
              rdfs:label "beta testing" ;
              <http://www.w3.org/2004/02/skos/core#prefLabel> "beta testing"@en .


###  http://purl.org/stc/ontology#black_box_test_technique
:black_box_test_technique rdf:type owl:Class ;
                          rdfs:subClassOf :test_technique ;
                          owl:disjointWith :experience-based_testing ,
                                           :grey_box_test_technique ,
                                           :white_box_test_technique ;
                          :isInISTQBGlossary "true"^^xsd:boolean ;
                          rdfs:comment "(ISTQB Glossary v4.5)"@en ;
                          rdfs:label "black box test technique" ;
                          <http://www.w3.org/2004/02/skos/core#altLabel> """specification-based testing
specification based testing
closed box testing
black-box test technique"""@en ;
                          <http://www.w3.org/2004/02/skos/core#prefLabel> "black box test technique"@en .


###  http://purl.org/stc/ontology#boundary_value_analysis
:boundary_value_analysis rdf:type owl:Class ;
                         rdfs:subClassOf :black_box_test_technique ;
                         :isInISTQBGlossary "true"^^xsd:boolean ;
                         rdfs:label "boundary value analysis" ;
                         <http://www.w3.org/2004/02/skos/core#prefLabel> "boundary value analysis"@en .


###  http://purl.org/stc/ontology#branch_coverage
:branch_coverage rdf:type owl:Class ;
                 rdfs:subClassOf :structural_coverage ;
                 :isInISTQBGlossary "true"^^xsd:boolean ;
                 rdfs:comment "The coverage of branches in a control flow graph.  (ISTQB Glossary v4.5)"@en ;
                 rdfs:label "branch coverage" ;
                 rdfs:seeAlso "Foundation - v4.0" ;
                 <http://www.w3.org/2004/02/skos/core#prefLabel> "branch coverage"@en .


###  http://purl.org/stc/ontology#branch_testing
:branch_testing rdf:type owl:Class ;
                rdfs:subClassOf :white_box_test_technique ;
                :isInISTQBGlossary "true"^^xsd:boolean ;
                rdfs:label "branch testing" ;
                <http://www.w3.org/2004/02/skos/core#prefLabel> "branch testing"@en .


###  http://purl.org/stc/ontology#change_orientation_in_test_approach
:change_orientation_in_test_approach rdf:type owl:Class ;
                                     rdfs:subClassOf :test_approach ;
                                     :isInISTQBGlossary "false"^^xsd:boolean ;
                                     rdfs:label "change orientation" ;
                                     <http://www.w3.org/2004/02/skos/core#prefLabel> "change orientation in test approach"@en .


###  http://purl.org/stc/ontology#checklist_based_testing
:checklist_based_testing rdf:type owl:Class ;
                         rdfs:subClassOf :experience-based_testing ;
                         :isInISTQBGlossary "true"^^xsd:boolean ;
                         rdfs:label "checklist based testing" ;
                         <http://www.w3.org/2004/02/skos/core#prefLabel> "checklist based testing"@en .


###  http://purl.org/stc/ontology#code
:code rdf:type owl:Class ;
      rdfs:subClassOf :basic_concepts .


###  http://purl.org/stc/ontology#coding
:coding rdf:type owl:Class ;
        rdfs:subClassOf :software_engineering_activity .


###  http://purl.org/stc/ontology#compliance_testing
:compliance_testing rdf:type owl:Class ;
                    rdfs:subClassOf :functional_testing ;
                    :isInISTQBGlossary "true"^^xsd:boolean ;
                    rdfs:comment "The term conformance testing (defined by ISTQB to be a synonym for compliance testing) is used differently in telecommunication/protocol testing - see also protocol testing."@en ;
                    rdfs:label "compliance testing" ;
                    rdfs:seeAlso "Specialist - Gambling Industry Tester - 2018" ;
                    <http://www.w3.org/2004/02/skos/core#altLabel> """conformance testing
regulation testing
standards testing""" ;
                    <http://www.w3.org/2004/02/skos/core#prefLabel> "compliance testing"@en .


###  http://purl.org/stc/ontology#component_integration_testing
:component_integration_testing rdf:type owl:Class ;
                               rdfs:subClassOf :integration_testing ;
                               :isInISTQBGlossary "true"^^xsd:boolean ;
                               rdfs:comment "The integration testing of components. (ISTQB Glossary v4.5)"@en ;
                               rdfs:label "component integration testing" ;
                               rdfs:seeAlso "Foundation - v4.0" ;
                               <http://www.w3.org/2004/02/skos/core#altLabel> """module integration testing
unit integration testing"""@en ;
                               <http://www.w3.org/2004/02/skos/core#prefLabel> "component integration testing"@en .


###  http://purl.org/stc/ontology#component_testing
:component_testing rdf:type owl:Class ;
                   rdfs:subClassOf :test_level ;
                   owl:disjointWith :integration_testing ,
                                    :system_testing ;
                   :isInISTQBGlossary "true"^^xsd:boolean ;
                   rdfs:label "component testing" ;
                   <http://www.w3.org/2004/02/skos/core#prefLabel> "component testing"@en .


###  http://purl.org/stc/ontology#condition_coverage
:condition_coverage rdf:type owl:Class ;
                    rdfs:subClassOf :structural_coverage ;
                    :isInISTQBGlossary "true"^^xsd:boolean ;
                    rdfs:comment """The coverage of condition outcomes. (ISTQB Glossary v4.5)

Coverage for branch condition testing. (ISO/IEC/IEEE 29119-4)"""@en ;
                    rdfs:label "condition coverage" ;
                    rdfs:seeAlso "ISO/IEC/IEEE 29119-4 (Software and systems engineering — Software testing — Part 4: Test techniques)" ;
                    <http://www.w3.org/2004/02/skos/core#altLabel> "branch condition coverage"@en ;
                    <http://www.w3.org/2004/02/skos/core#prefLabel> "condition coverage"@en .


###  http://purl.org/stc/ontology#configuration_management
:configuration_management rdf:type owl:Class ;
                          rdfs:subClassOf :support_processes .


###  http://purl.org/stc/ontology#confirmation_testing
:confirmation_testing rdf:type owl:Class ;
                      rdfs:subClassOf :defect_orientation_in_test_approach ;
                      :isInISTQBGlossary "true"^^xsd:boolean ;
                      rdfs:comment """A type of change-related testing performed after fixing a defect to confirm that a failure caused by that defect does not reoccur. (ISTQB Glossary v4.5)

Testing performed to check that modifications made to correct a fault have successfully removed the fault. (ISO/IEC/IEEE 29119-1:2022)"""@en ;
                      rdfs:label "confirmation testing" ;
                      rdfs:seeAlso """ISO/IEC/IEEE 29119-1:2022 (Software and systems engineering — Software testing — Part 1: Concepts and definitions)

Foundation - v4.0
Specialist - Test Automation Engineer - 2016
Specialist - Test Automation Strategy - v1.0""" ;
                      <http://www.w3.org/2004/02/skos/core#altLabel> "retesting"@en ;
                      <http://www.w3.org/2004/02/skos/core#prefLabel> "confirmation testing"@en .


###  http://purl.org/stc/ontology#conformance_testing
:conformance_testing rdf:type owl:Class ;
                     rdfs:subClassOf :protocol_or_service_testing ;
                     :isInISTQBGlossary "false"^^xsd:boolean ;
                     rdfs:comment "The process of verifying that a system or component meets the requirements of a specified standard. (ISO/IEC 9646-1:1994)"@en ;
                     rdfs:label "conformance testing" ;
                     rdfs:seeAlso "ISO/IEC 9646-1:1994 (Information technology — Open Systems Interconnection — Conformance testing methodology and framework. Part 1: General concepts)" ;
                     <http://www.w3.org/2004/02/skos/core#prefLabel> "conformance testing"@en .


###  http://purl.org/stc/ontology#continuous_testing
:continuous_testing rdf:type owl:Class ;
                    rdfs:subClassOf :process_orientation_in_test_approach ;
                    :isInISTQBGlossary "true"^^xsd:boolean ;
                    rdfs:label "continuous testing" ;
                    <http://www.w3.org/2004/02/skos/core#prefLabel> "continuous testing"@en .


###  http://purl.org/stc/ontology#contract_testing
:contract_testing rdf:type owl:Class ;
                  rdfs:subClassOf :target_orientation_in_test_approach ;
                  :isInISTQBGlossary "true"^^xsd:boolean ;
                  rdfs:label "contract testing" ;
                  <http://www.w3.org/2004/02/skos/core#prefLabel> "contract testing"@en .


###  http://purl.org/stc/ontology#coverage
:coverage rdf:type owl:Class ;
          rdfs:subClassOf :test_metric ;
          :isInISTQBGlossary "true"^^xsd:boolean ;
          rdfs:comment "The degree to which specified coverage items are exercised by a test suite, expressed as a percentage. (ISTQB Glossary v4.5)"@en ;
          rdfs:label "coverage" ;
          <http://www.w3.org/2004/02/skos/core#altLabel> """coverage metric
test coverage
coverage-oriented metric"""@en ;
          <http://www.w3.org/2004/02/skos/core#prefLabel> "coverage"@en .


###  http://purl.org/stc/ontology#coverage_item
:coverage_item rdf:type owl:Class ;
               rdfs:subClassOf :Testware ;
               :isInISTQBGlossary "true"^^xsd:boolean ;
               rdfs:comment """An attribute or combination of attributes derived from one or more test conditions by using a test technique. (ISTQB Glossary v4.5)

Measurable attribute of a test item that is the focus of testing (ISO/IEC/IEEE 29119-1:2022, defined as test (coverage) item)"""@en ;
               rdfs:label "coverage item" ;
               rdfs:seeAlso """ISO/IEC/IEEE 29119-1:2022 (Software and systems engineering — Software testing — Part 1: Concepts and definitions)

Foundation - v4.0
Specialist - Model-Based Testing - v1.1""" ;
               <http://www.w3.org/2004/02/skos/core#altLabel> "test coverage item"@en ;
               <http://www.w3.org/2004/02/skos/core#prefLabel> "coverage item"@en .


###  http://purl.org/stc/ontology#crowd_testing
:crowd_testing rdf:type owl:Class ;
               rdfs:subClassOf :tester_orientation_in_test_approach ;
               :isInISTQBGlossary "true"^^xsd:boolean ;
               rdfs:label "crowd testing" ;
               <http://www.w3.org/2004/02/skos/core#prefLabel> "crowd testing"@en .


###  http://purl.org/stc/ontology#data
:data rdf:type owl:Class ;
      rdfs:subClassOf :basic_concepts .


###  http://purl.org/stc/ontology#decision_coverage
:decision_coverage rdf:type owl:Class ;
                   rdfs:subClassOf :structural_coverage ;
                   :isInISTQBGlossary "true"^^xsd:boolean ;
                   rdfs:comment """The coverage of decision outcomes. (ISTQB Glossary v4.5)

Coverage for decision testing. (ISO/IEC/IEEE 29119-4)"""@en ;
                   rdfs:label "decision coverage" ;
                   rdfs:seeAlso "ISO/IEC/IEEE 29119-4 (Software and systems engineering — Software testing — Part 4: Test techniques)" ;
                   <http://www.w3.org/2004/02/skos/core#prefLabel> "decision coverage"@en .


###  http://purl.org/stc/ontology#decision_table_testing
:decision_table_testing rdf:type owl:Class ;
                        rdfs:subClassOf :black_box_test_technique ;
                        :isInISTQBGlossary "true"^^xsd:boolean ;
                        rdfs:label "decision table testing" ;
                        <http://www.w3.org/2004/02/skos/core#prefLabel> "decision table testing"@en .


###  http://purl.org/stc/ontology#defect
:defect rdf:type owl:Class ;
        rdfs:subClassOf :basic_concepts .


###  http://purl.org/stc/ontology#defect_orientation_in_test_approach
:defect_orientation_in_test_approach rdf:type owl:Class ;
                                     rdfs:subClassOf :change_orientation_in_test_approach ;
                                     :isInISTQBGlossary "false"^^xsd:boolean ;
                                     rdfs:label "defect orientation" ;
                                     <http://www.w3.org/2004/02/skos/core#prefLabel> "defect orientation in test approach"@en .


###  http://purl.org/stc/ontology#defect_oriented_metric
:defect_oriented_metric rdf:type owl:Class ;
                        rdfs:subClassOf :test_metric ;
                        :isInISTQBGlossary "false"^^xsd:boolean ;
                        rdfs:label "defect oriented metric" ;
                        <http://www.w3.org/2004/02/skos/core#altLabel> """defect-oriented metric
defect metric"""@en ;
                        <http://www.w3.org/2004/02/skos/core#prefLabel> "defect oriented metric"@en .


###  http://purl.org/stc/ontology#destructive_testing
:destructive_testing rdf:type owl:Class ;
                     rdfs:subClassOf :security_testing ;
                     :isInISTQBGlossary "true"^^xsd:boolean ;
                     rdfs:label "destructive testing" ;
                     <http://www.w3.org/2004/02/skos/core#prefLabel> "destructive testing"@en .


###  http://purl.org/stc/ontology#detailed_design
:detailed_design rdf:type owl:Class ;
                 rdfs:subClassOf :software_engineering_activity .


###  http://purl.org/stc/ontology#development
:development rdf:type owl:Class ;
             rdfs:subClassOf :software_lifecycle .


###  http://purl.org/stc/ontology#device-based_testing
:device-based_testing rdf:type owl:Class ;
                      rdfs:subClassOf :mobile_app_testing ;
                      :isInISTQBGlossary "true"^^xsd:boolean ;
                      rdfs:label "device-based testing" ;
                      <http://www.w3.org/2004/02/skos/core#prefLabel> "device-based testing"@en .


###  http://purl.org/stc/ontology#domain-specific_test_types
:domain-specific_test_types rdf:type owl:Class ;
                            rdfs:subClassOf :test_type ;
                            :isInISTQBGlossary "false"^^xsd:boolean ;
                            rdfs:label "domain-specific test types" ;
                            <http://www.w3.org/2004/02/skos/core#prefLabel> "domain-specific test types"@en .


###  http://purl.org/stc/ontology#dynamic_application_security_testing
:dynamic_application_security_testing rdf:type owl:Class ;
                                      rdfs:subClassOf :security_testing ;
                                      :isInISTQBGlossary "true"^^xsd:boolean ;
                                      rdfs:label "dynamic application security testing" ;
                                      <http://www.w3.org/2004/02/skos/core#prefLabel> "dynamic application security testing"@en .


###  http://purl.org/stc/ontology#dynamic_testing
:dynamic_testing rdf:type owl:Class ;
                 rdfs:subClassOf :testing ;
                 owl:disjointWith :static_testing ;
                 :isInISTQBGlossary "true"^^xsd:boolean ;
                 rdfs:comment """Testing that involves the execution of the test item. (ISTQB Glossary v4.5)

Testing in which a test item is evaluated by executing it. (ISO/IEC/IEEE 29119-1)"""@en ;
                 rdfs:label "dynamic testing" ;
                 rdfs:seeAlso """ISO/IEC/IEEE 29119-1:2022 (Software and systems engineering — Software testing — Part 1: Concepts and definitions)

Foundation - v4.0""" ;
                 <http://www.w3.org/2004/02/skos/core#prefLabel> "dynamic testing"@en .


###  http://purl.org/stc/ontology#each_choice_coverage
:each_choice_coverage rdf:type owl:Class ;
                      rdfs:subClassOf :specification_coverage ;
                      :isInISTQBGlossary "true"^^xsd:boolean ;
                      rdfs:comment """The coverage of equivalence partitions in multiple sets of partitions. (ISTQB Glossary v4.5)

Coverage for each choice testing. (ISO/IEC/IEEE 29119-4:2015)"""@en ;
                      rdfs:label "each choice coverage" ;
                      rdfs:seeAlso "ISO/IEC/IEEE 29119-4 (Software and systems engineering — Software testing — Part 4: Test techniques)" ;
                      <http://www.w3.org/2004/02/skos/core#altLabel> """ecc
ECC"""@en ;
                      <http://www.w3.org/2004/02/skos/core#prefLabel> "each choice coverage"@en .


###  http://purl.org/stc/ontology#end-to-end_testing
:end-to-end_testing rdf:type owl:Class ;
                    rdfs:subClassOf :system_testing ;
                    :isInISTQBGlossary "true"^^xsd:boolean ;
                    rdfs:label "end-to-end testing" ;
                    <http://www.w3.org/2004/02/skos/core#altLabel> """e2e testing
E2E testing"""@en ;
                    <http://www.w3.org/2004/02/skos/core#prefLabel> "end-to-end testing"@en .


###  http://purl.org/stc/ontology#entry_criteria
:entry_criteria rdf:type owl:Class ;
                rdfs:subClassOf :Testware ;
                :isInISTQBGlossary "true"^^xsd:boolean ;
                rdfs:comment "The set of conditions for officially completing a defined task. (ISTQB Glossary v4.5)"@en ;
                rdfs:label "entry criteria" ;
                rdfs:seeAlso "Foundation - v4.0" ;
                <http://www.w3.org/2004/02/skos/core#altLabel> """test completion criteria
completion criteria"""@en ;
                <http://www.w3.org/2004/02/skos/core#prefLabel> "entry criteria"@en .


###  http://purl.org/stc/ontology#equivalence_partitioning
:equivalence_partitioning rdf:type owl:Class ;
                          rdfs:subClassOf :black_box_test_technique ;
                          :isInISTQBGlossary "true"^^xsd:boolean ;
                          rdfs:label "equivalence partitioning" ;
                          <http://www.w3.org/2004/02/skos/core#prefLabel> "equivalence partitioning"@en .


###  http://purl.org/stc/ontology#error
:error rdf:type owl:Class ;
       rdfs:subClassOf :basic_concepts .


###  http://purl.org/stc/ontology#error_guessing
:error_guessing rdf:type owl:Class ;
                rdfs:subClassOf :experience-based_testing ;
                :isInISTQBGlossary "true"^^xsd:boolean ;
                rdfs:label "error guessing" ;
                <http://www.w3.org/2004/02/skos/core#prefLabel> "error guessing"@en .


###  http://purl.org/stc/ontology#exhaustive_testing
:exhaustive_testing rdf:type owl:Class ;
                    rdfs:subClassOf :method_orientation_in_test_approach ;
                    :isInISTQBGlossary "true"^^xsd:boolean ;
                    rdfs:comment "A test approach in which the test suite comprises all combinations of input values and preconditions."@en ;
                    rdfs:label "exhaustive testing" ;
                    <http://www.w3.org/2004/02/skos/core#altLabel> "complete testing"@en ;
                    <http://www.w3.org/2004/02/skos/core#prefLabel> "exhaustive testing"@en .


###  http://purl.org/stc/ontology#exit_criteria
:exit_criteria rdf:type owl:Class ;
               rdfs:subClassOf :Testware ;
               :isInISTQBGlossary "true"^^xsd:boolean ;
               rdfs:comment "The set of conditions for officially starting a defined task. (ISTQB Glossary v4-5)"@en ;
               rdfs:label "exit criteria" ;
               rdfs:seeAlso """Foundation - v4.0
Advanced Test Manager - 2012
Advanced Test Analyst - v3.1""" ;
               <http://www.w3.org/2004/02/skos/core#altLabel> """test completion criteria
completion criteria""" ;
               <http://www.w3.org/2004/02/skos/core#prefLabel> "exit criteria"@en .


###  http://purl.org/stc/ontology#experience-based_testing
:experience-based_testing rdf:type owl:Class ;
                          rdfs:subClassOf :test_technique ;
                          owl:disjointWith :grey_box_test_technique ,
                                           :white_box_test_technique ;
                          :isInISTQBGlossary "true"^^xsd:boolean ;
                          rdfs:label "experience-based testing" ;
                          <http://www.w3.org/2004/02/skos/core#altLabel> """experience based testing
experience-based test technique
experience based test technique"""@en ;
                          <http://www.w3.org/2004/02/skos/core#prefLabel> "experience-based testing"@en .


###  http://purl.org/stc/ontology#experience_based_test_metric
:experience_based_test_metric rdf:type owl:Class ;
                              rdfs:subClassOf :coverage ;
                              :isInISTQBGlossary "false"^^xsd:boolean ;
                              rdfs:comment "There is currently no industry agreed approach to calculating experience-based coverage. (ISO/IEC/IEEE 29119-4)"@en ;
                              rdfs:label "experience coverage" ;
                              rdfs:seeAlso "ISO/IEC/IEEE 29119-4 (Software and systems engineering — Software testing — Part 4: Test techniques)" ;
                              <http://www.w3.org/2004/02/skos/core#altLabel> "experience based test metric"@en ,
                                                                             """experience based test metric
experience-based test metric"""@en ;
                              <http://www.w3.org/2004/02/skos/core#prefLabel> "experience coverage"@en .


###  http://purl.org/stc/ontology#exploratory_testing
:exploratory_testing rdf:type owl:Class ;
                     rdfs:subClassOf :method_orientation_in_test_approach ;
                     :isInISTQBGlossary "true"^^xsd:boolean ;
                     rdfs:comment "An approach to testing in which the testers dynamically design and execute tests based on their knowledge, exploration of the test item and the results of previous tests. (ISTQB Glossary v4.5)"@en ;
                     rdfs:label "exploratory testing" ;
                     rdfs:seeAlso """ISO/IEC/IEEE 29119-1:2022 (Software and systems engineering — Software testing — Part 1: Concepts and definitions)

Foundation - v4.0
Advanced Test Analyst - v3.1""" ;
                     <http://www.w3.org/2004/02/skos/core#prefLabel> "exploratory testing"@en .


###  http://purl.org/stc/ontology#failure
:failure rdf:type owl:Class ;
         rdfs:subClassOf :basic_concepts .


###  http://purl.org/stc/ontology#feature-driven_development
:feature-driven_development rdf:type owl:Class ;
                            rdfs:subClassOf :target_orientation_in_software_development ;
                            :isInISTQBGlossary "true"^^xsd:boolean ;
                            rdfs:label "feature-driven development" ;
                            <http://www.w3.org/2004/02/skos/core#prefLabel> "feature-driven development"@en .


###  http://purl.org/stc/ontology#formal_review
:formal_review rdf:type owl:Class ;
               rdfs:subClassOf :review ;
               rdfs:label "formal review" ;
               <http://www.w3.org/2004/02/skos/core#prefLabel> "formal review"@en .


###  http://purl.org/stc/ontology#functional_testing
:functional_testing rdf:type owl:Class ;
                    rdfs:subClassOf :test_type ;
                    :isInISTQBGlossary "true"^^xsd:boolean ;
                    rdfs:comment "Testing performed to evaluate if a component or system satisfies functional requirements. (ISTQB Glossary v4.5)"@en ;
                    rdfs:label "functional testing" ;
                    rdfs:seeAlso """Foundation - v4.0
Advanced Test Management - v3.0
Advanced Test Analyst - v4.0
Specialist - Game Testing - v1.0.1""" ;
                    <http://www.w3.org/2004/02/skos/core#prefLabel> "functional testing"@en .


###  http://purl.org/stc/ontology#fundamental_test_process
:fundamental_test_process rdf:type owl:Class ;
                          rdfs:subClassOf :test_process ;
                          :isInISTQBGlossary "false"^^xsd:boolean ;
                          rdfs:label "fundamental test process" ;
                          <http://www.w3.org/2004/02/skos/core#prefLabel> "fundamental test process"@en .


###  http://purl.org/stc/ontology#gambling_testing
:gambling_testing rdf:type owl:Class ;
                  rdfs:subClassOf :domain-specific_test_types ;
                  :isInISTQBGlossary "false"^^xsd:boolean ;
                  rdfs:label "gambling testing" ;
                  <http://www.w3.org/2004/02/skos/core#prefLabel> "gambling testing"@en .


###  http://purl.org/stc/ontology#grey_box_test_technique
:grey_box_test_technique rdf:type owl:Class ;
                         rdfs:subClassOf :test_technique ;
                         owl:disjointWith :white_box_test_technique ;
                         :isInISTQBGlossary "true"^^xsd:boolean ;
                         rdfs:label "grey-box testing" ;
                         <http://www.w3.org/2004/02/skos/core#altLabel> """grey box testing
gray-box testing
gray box testing"""@en ;
                         <http://www.w3.org/2004/02/skos/core#prefLabel> "grey-box testing"@en .


###  http://purl.org/stc/ontology#high_level_test_case
:high_level_test_case rdf:type owl:Class ;
                      rdfs:subClassOf :test_case ;
                      :isInISTQBGlossary "true"^^xsd:boolean ;
                      rdfs:comment "A test case with abstract preconditions, input data, expected results, postconditions, and actions (where applicable). (ISTQB Glossary v4.5)"@en ;
                      rdfs:label "high-level test case" ;
                      rdfs:seeAlso """Advanced Test Manager - 2012
Advanced Test Analyst - v3.1
Advanced Test Analyst - v4.0""" ;
                      <http://www.w3.org/2004/02/skos/core#altLabel> """high level test case
logical test case
abstract test case
high level testcase
logical testcase
abstract testcase""" ;
                      <http://www.w3.org/2004/02/skos/core#prefLabel> "high-level test case"@en .


###  http://purl.org/stc/ontology#incremental_software_development
:incremental_software_development rdf:type owl:Class ;
                                  rdfs:subClassOf :process_orientation_in_software_development ;
                                  :isInISTQBGlossary "false"^^xsd:boolean ;
                                  rdfs:label "incremental" ;
                                  <http://www.w3.org/2004/02/skos/core#prefLabel> "incremental software development"@en .


###  http://purl.org/stc/ontology#informal_review
:informal_review rdf:type owl:Class ;
                 rdfs:subClassOf :review ;
                 rdfs:label "informal review" ;
                 <http://www.w3.org/2004/02/skos/core#prefLabel> "informal review"@en .


###  http://purl.org/stc/ontology#inspection
:inspection rdf:type owl:Class ;
            rdfs:subClassOf :formal_review ;
            :isInISTQBGlossary "true"^^xsd:boolean ;
            rdfs:comment "A type of formal review that uses defined team roles and measurement to identify defects in a work product, and improve the review process and the software development process. (ISTQB Glossary v4.5)"@en ;
            rdfs:label "inspection" ;
            rdfs:seeAlso """Foundation - v4.0
Advanced Test Manager - 2012""" ;
            <http://www.w3.org/2004/02/skos/core#prefLabel> "inspection"@en .


###  http://purl.org/stc/ontology#integration
:integration rdf:type owl:Class ;
             rdfs:subClassOf :software_engineering_activity .


###  http://purl.org/stc/ontology#integration_testing
:integration_testing rdf:type owl:Class ;
                     rdfs:subClassOf :test_level ;
                     owl:disjointWith :system_testing ;
                     :isInISTQBGlossary "true"^^xsd:boolean ;
                     rdfs:label "integration testing" ;
                     <http://www.w3.org/2004/02/skos/core#prefLabel> "integration testing"@en .


###  http://purl.org/stc/ontology#interactive_application_security_testing
:interactive_application_security_testing rdf:type owl:Class ;
                                          rdfs:subClassOf :security_testing ;
                                          :isInISTQBGlossary "true"^^xsd:boolean ;
                                          rdfs:label "interactive application security testing" ;
                                          <http://www.w3.org/2004/02/skos/core#prefLabel> "interactive application security testing"@en .


###  http://purl.org/stc/ontology#interface_testing
:interface_testing rdf:type owl:Class ;
                   rdfs:subClassOf :target_orientation_in_test_approach ;
                   :isInISTQBGlossary "true"^^xsd:boolean ;
                   rdfs:label "interface testing" ;
                   <http://www.w3.org/2004/02/skos/core#prefLabel> "interface testing"@en .


###  http://purl.org/stc/ontology#interoperability_testing
:interoperability_testing rdf:type owl:Class ;
                          rdfs:subClassOf :protocol_or_service_testing ;
                          :isInISTQBGlossary "false"^^xsd:boolean ;
                          rdfs:comment "Testing conducted to ensure that a modified system retains the capability of exchanging information with systems of different types, and of using that information (ISO/IEC/IEEE 24765:2017)"@en ;
                          rdfs:label "interoperability testing" ;
                          rdfs:seeAlso """ISO/IEC/IEEE 24765:2017 (Systems and software engineering —
Vocabulary)""" ;
                          <http://www.w3.org/2004/02/skos/core#prefLabel> "interoperability testing"@en .


###  http://purl.org/stc/ontology#iterative_software_development
:iterative_software_development rdf:type owl:Class ;
                                rdfs:subClassOf :process_orientation_in_software_development ;
                                :isInISTQBGlossary "true"^^xsd:boolean ;
                                rdfs:label "iterative" ;
                                <http://www.w3.org/2004/02/skos/core#prefLabel> "iterative software development"@en .


###  http://purl.org/stc/ontology#level_test_plan
:level_test_plan rdf:type owl:Class ;
                 rdfs:subClassOf :test_plan ;
                 :isInISTQBGlossary "true"^^xsd:boolean ;
                 rdfs:comment "A test plan that typically addresses one test level. (ISTQB Glossary v4.5)"@en ;
                 rdfs:label "level test plan" ;
                 rdfs:seeAlso "Advanced Test Manager - 2012" ;
                 <http://www.w3.org/2004/02/skos/core#altLabel> "level testplan"@en ;
                 <http://www.w3.org/2004/02/skos/core#prefLabel> "level test plan"@en .


###  http://purl.org/stc/ontology#load_testing
:load_testing rdf:type owl:Class ;
              rdfs:subClassOf :performance_testing ;
              :isInISTQBGlossary "true"^^xsd:boolean ;
              rdfs:label "load testing" ;
              <http://www.w3.org/2004/02/skos/core#prefLabel> "load testing"@en .


###  http://purl.org/stc/ontology#low_level_test_case
:low_level_test_case rdf:type owl:Class ;
                     rdfs:subClassOf :test_case ;
                     :isInISTQBGlossary "true"^^xsd:boolean ;
                     rdfs:comment "A test case with concrete values for preconditions, input data, expected results, postconditions, and a detailed description of actions (where applicable). (ISTQB Glossary v4.5)"@en ;
                     rdfs:label "low-level test case" ;
                     rdfs:seeAlso """Advanced Test Analyst - v3.1
Advanced Test Analyst - v4.0""" ;
                     <http://www.w3.org/2004/02/skos/core#altLabel> """low level test case
concrete test case
physical test case
low level testcase
concrete testcase
physical testcase"""@en ;
                     <http://www.w3.org/2004/02/skos/core#prefLabel> "low-level test case"@en .


###  http://purl.org/stc/ontology#maintenance
:maintenance rdf:type owl:Class ;
             rdfs:subClassOf :software_lifecycle .


###  http://purl.org/stc/ontology#maintenance_testing
:maintenance_testing rdf:type owl:Class ;
                     rdfs:subClassOf :change_orientation_in_test_approach ;
                     :isInISTQBGlossary "true"^^xsd:boolean ;
                     rdfs:comment "Testing the changes to an operational system or the impact of a changed environment to an operational system. (ISTQB Glossary v4.5)"@en ;
                     rdfs:label "maintenance testing" ;
                     rdfs:seeAlso "Foundation - v4.0" ;
                     <http://www.w3.org/2004/02/skos/core#prefLabel> "maintenance testing"@en .


###  http://purl.org/stc/ontology#manual_testing
:manual_testing rdf:type owl:Class ;
                rdfs:subClassOf :test_execution ;
                :isInISTQBGlossary "false"^^xsd:boolean ;
                rdfs:comment "Humans performing tests by entering information into a test item and verifying the results. (ISO/IEC/IEEE 29119-1:2022)"@en ,
                             "ISO/IEC/IEEE 29119-1:2022 (Software and systems engineering — Software testing — Part 1: Concepts and definitions)"@en ;
                rdfs:label "manual testing" ;
                <http://www.w3.org/2004/02/skos/core#altLabel> "unscripted testing" ;
                <http://www.w3.org/2004/02/skos/core#prefLabel> "manual testing"@en .


###  http://purl.org/stc/ontology#master_test_plan
:master_test_plan rdf:type owl:Class ;
                  rdfs:subClassOf :test_plan ;
                  :isInISTQBGlossary "true"^^xsd:boolean ;
                  rdfs:comment "A test plan that is used to coordinate multiple test levels or test types. (ISTQB Glossary v4.5)"@en ;
                  rdfs:label "master test plan" ;
                  rdfs:seeAlso "Advanced Test Manager - 2012" ;
                  <http://www.w3.org/2004/02/skos/core#altLabel> "master testplan"@en ;
                  <http://www.w3.org/2004/02/skos/core#prefLabel> "master test plan"@en .


###  http://purl.org/stc/ontology#math_testing
:math_testing rdf:type owl:Class ;
              rdfs:subClassOf :gambling_testing ;
              :isInISTQBGlossary "true"^^xsd:boolean ;
              rdfs:label "math testing" ;
              <http://www.w3.org/2004/02/skos/core#prefLabel> "math testing"@en .


###  http://purl.org/stc/ontology#method_orientation_in_test_approach
:method_orientation_in_test_approach rdf:type owl:Class ;
                                     rdfs:subClassOf :test_approach ;
                                     :isInISTQBGlossary "false"^^xsd:boolean ;
                                     rdfs:label "method orientation" ;
                                     <http://www.w3.org/2004/02/skos/core#prefLabel> "method orientation in test approach"@en .


###  http://purl.org/stc/ontology#metric
:metric rdf:type owl:Class ;
        rdfs:subClassOf :basic_concepts ;
        :isInISTQBGlossary "true"^^xsd:boolean ;
        rdfs:comment """A measurement scale and the method used for measurement. (ISTQB Glossary v4.5) 

A quantitative measure of the degree to which a system, component, or process possesses a given attribute. (ISO/IEC/IEEE 24765:2017)"""@en ;
        rdfs:label "metric" ;
        rdfs:seeAlso """ISO/IEC/IEEE 24765:2017 (Systems and Software Engineering – Vocabulary)

Foundation - v4.0
Advanced Test Manager - 2012
Advanced Test Management - v3.0
Advanced Test Analyst - v3.1
Advanced Test Analyst - v4.0
Advanced Technical Test Analyst - v4.0
Advanced Test Automation Engineering - v2.0
Expert Improving the Test Process - 2011
Expert Test Management - 2011
Foundation Agile Tester - 2014
Advanced Agile Technical Tester - 2019
Agile Test Leadership at Scale - v1.0
Specialist - Acceptance Testing - 2019
Specialist - Agile Test Leadership at Scale - v2.0
Specialist - AI Testing - v1.0
Specialist - Automotive Software Tester - 2018
Specialist - Automotive Software Tester - v1.1
Specialist - Gambling Industry Tester - 2018
Specialist - Game Testing - v1.0.1
Specialist - Model-Based Tester - 2015
Specialist - Model-Based Testing - v1.1
Specialist - Performance Testing - 2018
Specialist - Security Tester - 2016
Specialist - Security Test Engineer - v1.0
Specialist - Test Automation Engineer - 2016
Specialist - Test Automation Strategy - v1.0""" ;
        <http://www.w3.org/2004/02/skos/core#prefLabel> "metric"@en .


###  http://purl.org/stc/ontology#mobile_app_testing
:mobile_app_testing rdf:type owl:Class ;
                    rdfs:subClassOf :domain-specific_test_types ;
                    :isInISTQBGlossary "false"^^xsd:boolean ;
                    rdfs:label "mobile app testing" ;
                    <http://www.w3.org/2004/02/skos/core#altLabel> "mobile application testing"@en ;
                    <http://www.w3.org/2004/02/skos/core#prefLabel> "mobile app testing"@en .


###  http://purl.org/stc/ontology#model
:model rdf:type owl:Class ;
       rdfs:subClassOf :basic_concepts .


###  http://purl.org/stc/ontology#model_based_testing
:model_based_testing rdf:type owl:Class ;
                     rdfs:subClassOf :black_box_test_technique ;
                     :isInISTQBGlossary "true"^^xsd:boolean ;
                     rdfs:comment "Testing based on or involving models. (ISTQB Glossary v4.5)"@en ;
                     rdfs:label "model-based testing" ;
                     rdfs:seeAlso """Advanced Test Analyst - v4.0
Advanced Technical Test Analyst - v4.0
Advanced Test Automation Engineering - v2.0
Specialist - Acceptance Testing - 2019
Specialist - Model-Based Tester - 2015
Specialist - Model-Based Testing - v1.1
Specialist - Test Automation Engineer - 2016""" ;
                     <http://www.w3.org/2004/02/skos/core#altLabel> """model based testing
mbt
MBT
model driven testing
model-driven testing
mdt
MDT"""@en ;
                     <http://www.w3.org/2004/02/skos/core#prefLabel> "model-based testing"@en .


###  http://purl.org/stc/ontology#model_coverage
:model_coverage rdf:type owl:Class ;
                rdfs:subClassOf :specification_coverage ;
                :isInISTQBGlossary "true"^^xsd:boolean ;
                rdfs:comment "The coverage of model elements. (ISTQB Glossary v4.5)"@en ;
                rdfs:label "model coverage" ;
                rdfs:seeAlso "Specialist - Model-Based Testing - v1.1" ;
                <http://www.w3.org/2004/02/skos/core#prefLabel> "model coverage"@en .


###  http://purl.org/stc/ontology#model_verification
:model_verification rdf:type owl:Class ;
                    rdfs:subClassOf :static_testing ;
                    :isInISTQBGlossary "false"^^xsd:boolean ;
                    rdfs:comment "The process of determining that a model accurately represents the required conceptual description and specifications. (own)"@en ;
                    rdfs:label "model verification" ;
                    <http://www.w3.org/2004/02/skos/core#prefLabel> "model verification"@en .


###  http://purl.org/stc/ontology#modified_condition_decision_coverage
:modified_condition_decision_coverage rdf:type owl:Class ;
                                      rdfs:subClassOf :structural_coverage ;
                                      :isInISTQBGlossary "true"^^xsd:boolean ;
                                      rdfs:comment """The coverage of all outcomes of the atomic conditions that independently affect the overall decision outcome. (ISTQB Glossary v4.5)

Coverage for modified condition/decision coverage testing. (ISO/IEC/IEEE 29119-4)"""@en ;
                                      rdfs:label "modified condition/decision coverage" ;
                                      rdfs:seeAlso "ISO/IEC/IEEE 29119-4 (Software and systems engineering — Software testing — Part 4: Test techniques)" ;
                                      <http://www.w3.org/2004/02/skos/core#altLabel> """mc/dc
MC/DC
condition determination coverage
modified multiple condition coverage"""@en ;
                                      <http://www.w3.org/2004/02/skos/core#prefLabel> "modified condition/decision coverage"@en .


###  http://purl.org/stc/ontology#multiple_condition_coverage
:multiple_condition_coverage rdf:type owl:Class ;
                             rdfs:subClassOf :structural_coverage ;
                             :isInISTQBGlossary "true"^^xsd:boolean ;
                             rdfs:comment """The coverage of all possible combinations of all single condition outcomes within one statement. (ISTQB Glossary v4.5)

Coverage for branch condition combination testing. (ISO/IEC/IEEE 29119-4 as branch condition combination coverage)"""@en ;
                             rdfs:label "multiple condition coverage" ;
                             rdfs:seeAlso "ISO/IEC/IEEE 29119-4 (Software and systems engineering — Software testing — Part 4: Test techniques)" ;
                             <http://www.w3.org/2004/02/skos/core#altLabel> """branch condition combination coverage
condition combination coverage""" ;
                             <http://www.w3.org/2004/02/skos/core#prefLabel> "multiple condition coverage"@en .


###  http://purl.org/stc/ontology#neuron_coverage
:neuron_coverage rdf:type owl:Class ;
                 rdfs:subClassOf :LLM_structural_coverage ;
                 :isInISTQBGlossary "true"^^xsd:boolean ;
                 rdfs:comment "The coverage of activated neurons in the neural network for a set of tests. (ISTQB Glossary v4.5)"@en ;
                 rdfs:label "neuron coverage" ;
                 rdfs:seeAlso "Specialist - AI Testing - v1.0" ;
                 <http://www.w3.org/2004/02/skos/core#prefLabel> "neuron coverage"@en .


###  http://purl.org/stc/ontology#non-functional_testing
:non-functional_testing rdf:type owl:Class ;
                        rdfs:subClassOf :test_type ;
                        :isInISTQBGlossary "true"^^xsd:boolean ;
                        rdfs:comment "Testing performed to evaluate that a component or system complies with non-functional requirements. (ISTQB Glossary v4.5)"@en ;
                        rdfs:label "non-functional testing" ;
                        rdfs:seeAlso """Foundation - v4.0
Advanced Test Management - v3.0""" ;
                        <http://www.w3.org/2004/02/skos/core#altLabel> "extra-functional testing"@en ;
                        <http://www.w3.org/2004/02/skos/core#prefLabel> "non-functional testing"@en .


###  http://purl.org/stc/ontology#operation
:operation rdf:type owl:Class ;
           rdfs:subClassOf :software_lifecycle .


###  http://purl.org/stc/ontology#oracle_orientation_in_test_approach
:oracle_orientation_in_test_approach rdf:type owl:Class ;
                                     rdfs:subClassOf :test_approach ;
                                     :isInISTQBGlossary "false"^^xsd:boolean ;
                                     rdfs:label "oracle orientation" ;
                                     <http://www.w3.org/2004/02/skos/core#prefLabel> "oracle orientation in test approach"@en .


###  http://purl.org/stc/ontology#pair_testing
:pair_testing rdf:type owl:Class ;
              rdfs:subClassOf :tester_orientation_in_test_approach ;
              :isInISTQBGlossary "true"^^xsd:boolean ;
              rdfs:label "pair testing" ;
              <http://www.w3.org/2004/02/skos/core#prefLabel> "pair testing"@en .


###  http://purl.org/stc/ontology#peer_review
:peer_review rdf:type owl:Class ;
             rdfs:subClassOf :informal_review ;
             :isInISTQBGlossary "true"^^xsd:boolean ;
             rdfs:comment "A type of review performed on a work product by persons that have the abilities required to create it.  (ISTQB Glossary v4.5)"@en ;
             rdfs:label "peer review" ;
             rdfs:seeAlso "" ;
             <http://www.w3.org/2004/02/skos/core#prefLabel> "peer review"@en .


###  http://purl.org/stc/ontology#performance_testing
:performance_testing rdf:type owl:Class ;
                     rdfs:subClassOf :non-functional_testing ;
                     :isInISTQBGlossary "true"^^xsd:boolean ;
                     rdfs:label "performance testing" ;
                     <http://www.w3.org/2004/02/skos/core#prefLabel> "performance testing"@en .


###  http://purl.org/stc/ontology#process_improvement
:process_improvement rdf:type owl:Class ;
                     rdfs:subClassOf :support_processes .


###  http://purl.org/stc/ontology#process_orientation_in_software_development
:process_orientation_in_software_development rdf:type owl:Class ;
                                             rdfs:subClassOf :software_development_model ;
                                             :isInISTQBGlossary "false"^^xsd:boolean ;
                                             rdfs:label "process orientation" ;
                                             <http://www.w3.org/2004/02/skos/core#prefLabel> "process orientation in software development"@en .


###  http://purl.org/stc/ontology#process_orientation_in_test_approach
:process_orientation_in_test_approach rdf:type owl:Class ;
                                      rdfs:subClassOf :test_approach ;
                                      :isInISTQBGlossary "false"^^xsd:boolean ;
                                      rdfs:label "process orientation" ;
                                      <http://www.w3.org/2004/02/skos/core#prefLabel> "process orientation in test approach"@en .


###  http://purl.org/stc/ontology#project_management
:project_management rdf:type owl:Class ;
                    rdfs:subClassOf :support_processes .


###  http://purl.org/stc/ontology#property-based_testing
:property-based_testing rdf:type owl:Class ;
                        rdfs:subClassOf :target_orientation_in_test_approach ;
                        :isInISTQBGlossary "true"^^xsd:boolean ;
                        rdfs:label "property-based testing" ;
                        <http://www.w3.org/2004/02/skos/core#prefLabel> "property-based testing"@en .


###  http://purl.org/stc/ontology#protocol_or_service_testing
:protocol_or_service_testing rdf:type owl:Class ;
                             rdfs:subClassOf :domain-specific_test_types ;
                             :isInISTQBGlossary "false"^^xsd:boolean ;
                             rdfs:label "protocol or service testing" ;
                             <http://www.w3.org/2004/02/skos/core#prefLabel> "protocol or service testing"@en .


###  http://purl.org/stc/ontology#quality_assurance
:quality_assurance rdf:type owl:Class ;
                   rdfs:subClassOf :support_processes .


###  http://purl.org/stc/ontology#reactive_testing
:reactive_testing rdf:type owl:Class ;
                  rdfs:subClassOf :dynamic_testing ;
                  :isInISTQBGlossary "true"^^xsd:boolean ;
                  rdfs:label "reactive testing" ;
                  <http://www.w3.org/2004/02/skos/core#prefLabel> "reactive testing"@en .


###  http://purl.org/stc/ontology#regression_testing
:regression_testing rdf:type owl:Class ;
                    rdfs:subClassOf :change_orientation_in_test_approach ;
                    :isInISTQBGlossary "true"^^xsd:boolean ;
                    rdfs:comment """A type of change-related testing to detect whether defects have been introduced or uncovered in unchanged areas of the software. (ISTQB Glossary v4.5)

Testingperformed following modifications to a test item or to its operational environment, to identify whether failures in unmodified parts of the test item occur. (ISO/IEC/IEEE 29119-1:2022)"""@en ;
                    rdfs:label "regression testing" ;
                    rdfs:seeAlso """ISO/IEC/IEEE 29119-1:2022 (Software and systems engineering — Software testing — Part 1: Concepts and definitions)

Foundation - v4.0
Advanced Test Analyst - v4.0
Specialist - Test Automation Engineer - 2016""" ;
                    <http://www.w3.org/2004/02/skos/core#prefLabel> "regression testing"@en .


###  http://purl.org/stc/ontology#regulatory_acceptance_testing
:regulatory_acceptance_testing rdf:type owl:Class ;
                               rdfs:subClassOf :acceptance_testing ;
                               :isInISTQBGlossary "true"^^xsd:boolean ;
                               rdfs:label "regulatory acceptance testing" ;
                               <http://www.w3.org/2004/02/skos/core#prefLabel> "regulatory acceptance testing"@en .


###  http://purl.org/stc/ontology#related_to_role
:related_to_role rdf:type owl:Class ;
                 rdfs:subClassOf :test_work_force ;
                 :isInISTQBGlossary "false"^^xsd:boolean ;
                 rdfs:label "related to role" ;
                 <http://www.w3.org/2004/02/skos/core#prefLabel> "related to role"@en .


###  http://purl.org/stc/ontology#related_to_team
:related_to_team rdf:type owl:Class ;
                 rdfs:subClassOf :test_work_force ;
                 :isInISTQBGlossary "false"^^xsd:boolean ;
                 rdfs:label "related to team" ;
                 <http://www.w3.org/2004/02/skos/core#prefLabel> "related to team"@en .


###  http://purl.org/stc/ontology#release
:release rdf:type owl:Class ;
         rdfs:subClassOf :software_lifecycle .


###  http://purl.org/stc/ontology#requirements-based_testing
:requirements-based_testing rdf:type owl:Class ;
                            rdfs:subClassOf :black_box_test_technique ;
                            :isInISTQBGlossary "true"^^xsd:boolean ;
                            rdfs:label "requirements-based testing" ;
                            <http://www.w3.org/2004/02/skos/core#prefLabel> "requirements-based testing"@en .


###  http://purl.org/stc/ontology#requirements_coverage
:requirements_coverage rdf:type owl:Class ;
                       rdfs:subClassOf :specification_coverage ;
                       :isInISTQBGlossary "false"^^xsd:boolean ;
                       rdfs:comment "Number of requirements covered by executed tests (ISO/IEC/IEEE 29119-1:2022, defined as test coverage)"@en ;
                       rdfs:label "requirement coverage" ;
                       rdfs:seeAlso "ISO/IEC/IEEE 29119-1:2022 (Software and systems engineering — Software testing — Part 1: Concepts and definitions)" ;
                       <http://www.w3.org/2004/02/skos/core#altLabel> "requirements coverage"@en ;
                       <http://www.w3.org/2004/02/skos/core#prefLabel> "requirement coverage"@en .


###  http://purl.org/stc/ontology#requirements_engineering
:requirements_engineering rdf:type owl:Class ;
                          rdfs:subClassOf :software_engineering_activity .


###  http://purl.org/stc/ontology#review
:review rdf:type owl:Class ;
        rdfs:subClassOf :static_testing .


###  http://purl.org/stc/ontology#risk-based_testing
:risk-based_testing rdf:type owl:Class ;
                    rdfs:subClassOf :target_orientation_in_test_approach ;
                    :isInISTQBGlossary "true"^^xsd:boolean ;
                    rdfs:label "risk-based testing" ;
                    <http://www.w3.org/2004/02/skos/core#prefLabel> "risk-based testing"@en .


###  http://purl.org/stc/ontology#risk_oriented_metric
:risk_oriented_metric rdf:type owl:Class ;
                      rdfs:subClassOf :test_metric ;
                      :isInISTQBGlossary "false"^^xsd:boolean ;
                      rdfs:label "risk oriented metric" ;
                      <http://www.w3.org/2004/02/skos/core#altLabel> """risk-oriented metric
risk metric"""@en ;
                      <http://www.w3.org/2004/02/skos/core#prefLabel> "risk oriented metric"@en .


###  http://purl.org/stc/ontology#safety_testing
:safety_testing rdf:type owl:Class ;
                rdfs:subClassOf :non-functional_testing ;
                :isInISTQBGlossary "false"^^xsd:boolean ;
                rdfs:label "safety testing" ;
                <http://www.w3.org/2004/02/skos/core#prefLabel> "safety testing"@en .


###  http://purl.org/stc/ontology#scripted_testing
:scripted_testing rdf:type owl:Class ;
                  rdfs:subClassOf :manual_testing ;
                  :isInISTQBGlossary "true"^^xsd:boolean ;
                  rdfs:comment "Testing performed based on a documented test script. (ISO/IEC/IEEE 29119-1:2022)"@en ;
                  rdfs:label "scripted testing" ;
                  rdfs:seeAlso "ISO/IEC/IEEE 29119-1:2022 (Software and systems engineering — Software testing — Part 1: Concepts and definitions)" ;
                  <http://www.w3.org/2004/02/skos/core#prefLabel> "scripted testing"@en .


###  http://purl.org/stc/ontology#security_testing
:security_testing rdf:type owl:Class ;
                  rdfs:subClassOf :non-functional_testing ;
                  :isInISTQBGlossary "true"^^xsd:boolean ;
                  rdfs:comment """A test type to determine the security of a component or system. (ISTQB Glossary v4.5)

Test type conducted to evaluate the degree to which a test item, and associated data and information, are protected so that unauthorized persons or systems cannot use, read, or modify them, and authorized persons or systems are not denied access to them. (ISO/IEC/IEEE 29119-1:2022)"""@en ;
                  rdfs:label "security testing" ;
                  rdfs:seeAlso """ISO/IEC/IEEE 29119-1:2022 (Software and systems engineering — Software testing — Part 1: Concepts and definitions)

Specialist - Mobile Application Testing - 2019
Specialist - Security Tester - 2016
Specialist - Security Test Engineer - v1.0""" ;
                  <http://www.w3.org/2004/02/skos/core#prefLabel> "security testing"@en .


###  http://purl.org/stc/ontology#sequential_development_model
:sequential_development_model rdf:type owl:Class ;
                              rdfs:subClassOf :process_orientation_in_software_development ;
                              :isInISTQBGlossary "true"^^xsd:boolean ;
                              rdfs:label "sequential" ;
                              <http://www.w3.org/2004/02/skos/core#prefLabel> "sequential development model"@en .


###  http://purl.org/stc/ontology#session-based_testing
:session-based_testing rdf:type owl:Class ;
                       rdfs:subClassOf :process_orientation_in_test_approach ;
                       :isInISTQBGlossary "true"^^xsd:boolean ;
                       rdfs:label "session-based testing" ;
                       <http://www.w3.org/2004/02/skos/core#altLabel> """session based testing
session-oriented testing
session oriented testing"""@en ;
                       <http://www.w3.org/2004/02/skos/core#prefLabel> "session-based testing"@en .


###  http://purl.org/stc/ontology#software
:software rdf:type owl:Class ;
          rdfs:subClassOf :software_engineering_concepts .


###  http://purl.org/stc/ontology#software_development_model
:software_development_model rdf:type owl:Class ;
                            rdfs:subClassOf :software_engineering_concepts ;
                            :isInISTQBGlossary "false"^^xsd:boolean ;
                            rdfs:label "software development model" ;
                            <http://www.w3.org/2004/02/skos/core#prefLabel> "software development model"@en .


###  http://purl.org/stc/ontology#software_engineering
:software_engineering rdf:type owl:Class ;
                      rdfs:subClassOf :basic_concepts ;
                      :isInISTQBGlossary "false"^^xsd:boolean ;
                      rdfs:comment """The application of a systematic, disciplined, quantifiable approach to the development, operation, and maintenance of software; that is, the application of engineering to software. (IEEE 610.12-1990, ISO/IEC/IEEE 24765:2017)

A set of systematic processes for the acquisition, supply, development, operation, maintenance, and disposal of software products. (ISO/IEC 12207:2017)"""@en ;
                      rdfs:label "software engineering" ;
                      rdfs:seeAlso """ISO/IEC/IEEE 24765:2017 (Systems and Software Engineering – Vocabulary)
ISO/IEC 12207:2017 (Systems and software engineering — Software life cycle processes)
ISO/IEC 12207:2017 (Systems and software engineering — Software life cycle processes)""" ;
                      <http://www.w3.org/2004/02/skos/core#altLabel> """se
software development"""@en ;
                      <http://www.w3.org/2004/02/skos/core#prefLabel> "software engineering"@en .


###  http://purl.org/stc/ontology#software_engineering_activity
:software_engineering_activity rdf:type owl:Class ;
                               rdfs:subClassOf :software_engineering_concepts .


###  http://purl.org/stc/ontology#software_engineering_concepts
:software_engineering_concepts rdf:type owl:Class ;
                               rdfs:subClassOf <http://purl.org/nemo/gufo#AbstractIndividualType> ;
                               rdfs:comment "Selection of software engineering concepts that relate to software testing concepts."@en ;
                               rdfs:label "software engineering concepts" ;
                               <http://www.w3.org/2004/02/skos/core#prefLabel> "software engineering concepts"@en .


###  http://purl.org/stc/ontology#software_lifecycle
:software_lifecycle rdf:type owl:Class ;
                    rdfs:subClassOf :software_engineering_concepts .


###  http://purl.org/stc/ontology#software_testing_concepts
:software_testing_concepts rdf:type owl:Class ;
                           rdfs:subClassOf <http://purl.org/nemo/gufo#AbstractIndividualType> ;
                           rdfs:comment "Rather exhaustive collection of software testing concepts"@en ;
                           rdfs:label "software testing concepts" ;
                           <http://www.w3.org/2004/02/skos/core#prefLabel> "software testing concepts"@en .


###  http://purl.org/stc/ontology#specialist_tester
:specialist_tester rdf:type owl:Class ;
                   rdfs:subClassOf :related_to_role ;
                   :isInISTQBGlossary "false"^^xsd:boolean ;
                   rdfs:comment """Performs testing for specific quality characteristics, such as usability, accessibility,
security, performance. (ISO/IEC/IEEE 29119-1:2022)"""@en ;
                   rdfs:label "specialist tester" ;
                   rdfs:seeAlso "ISO/IEC/IEEE 29119-1:2022 (Software and systems engineering — Software testing — Part 1: Concepts and definitions)" ;
                   <http://www.w3.org/2004/02/skos/core#prefLabel> "specialist tester"@en .


###  http://purl.org/stc/ontology#specification_coverage
:specification_coverage rdf:type owl:Class ;
                        rdfs:subClassOf :coverage ;
                        :isInISTQBGlossary "false"^^xsd:boolean ;
                        rdfs:comment "There is currently no industry agreed approach to calculating experience-based coverage. (ISO/IEC/IEEE 29119-4)"@en ;
                        rdfs:label "specification coverage" ;
                        rdfs:seeAlso "ISO/IEC/IEEE 29119-4 (Software and systems engineering — Software testing — Part 4: Test techniques)" ;
                        <http://www.w3.org/2004/02/skos/core#altLabel> """black-box test metric
black box test metric
specification-based test metric
specification based test metric"""@en ;
                        <http://www.w3.org/2004/02/skos/core#prefLabel> "specification coverage"@en .


###  http://purl.org/stc/ontology#state_transition_testing
:state_transition_testing rdf:type owl:Class ;
                          rdfs:subClassOf :black_box_test_technique ;
                          :isInISTQBGlossary "true"^^xsd:boolean ;
                          rdfs:label "state transition testing" ;
                          <http://www.w3.org/2004/02/skos/core#prefLabel> "state transition testing"@en .


###  http://purl.org/stc/ontology#statement_coverage
:statement_coverage rdf:type owl:Class ;
                    rdfs:subClassOf :structural_coverage ;
                    :isInISTQBGlossary "true"^^xsd:boolean ;
                    rdfs:comment """The coverage of executable statements. (ISTQB Glossary v4.5)

Coverage for statement testing. (ISO/IEC/IEEE 29119-4)"""@en ;
                    rdfs:label "statement coverage" ;
                    rdfs:seeAlso """ISO/IEC/IEEE 29119-4 (Software and systems engineering — Software testing — Part 4: Test techniques)

Foundation - v4.0""" ;
                    <http://www.w3.org/2004/02/skos/core#altLabel> "statement testing coverage"@en ;
                    <http://www.w3.org/2004/02/skos/core#prefLabel> "statement coverage"@en .


###  http://purl.org/stc/ontology#statement_testing
:statement_testing rdf:type owl:Class ;
                   rdfs:subClassOf :white_box_test_technique ;
                   :isInISTQBGlossary "true"^^xsd:boolean ;
                   rdfs:label "statement testing" ;
                   <http://www.w3.org/2004/02/skos/core#prefLabel> "statement testing"@en .


###  http://purl.org/stc/ontology#static_analysis
:static_analysis rdf:type owl:Class ;
                 rdfs:subClassOf :static_testing ;
                 :isInISTQBGlossary "true"^^xsd:boolean ;
                 rdfs:comment "The process of evaluating a component or system without executing it, based on its form, structure, content, or documentation. (ISTQB Glossary v4.5)"@en ;
                 rdfs:label "static analysis" ;
                 rdfs:seeAlso """Foundation - v4.0
Advanced Technical Test Analyst - v4.0
Advanced Test Automation Engineering - v2.0""" ;
                 <http://www.w3.org/2004/02/skos/core#prefLabel> "static analysis"@en .


###  http://purl.org/stc/ontology#static_application_security_testing
:static_application_security_testing rdf:type owl:Class ;
                                     rdfs:subClassOf :security_testing ;
                                     :isInISTQBGlossary "true"^^xsd:boolean ;
                                     rdfs:label "static application security testing" ;
                                     <http://www.w3.org/2004/02/skos/core#prefLabel> "static application security testing"@en .


###  http://purl.org/stc/ontology#static_testing
:static_testing rdf:type owl:Class ;
                rdfs:subClassOf :testing ;
                :isInISTQBGlossary "true"^^xsd:boolean ;
                rdfs:comment """Testing that does not involve the execution of a test item. (ISTQB Glossary v4.5)

Testing in which a test item is examined against a set of quality or other criteria without the test item being executed. (ISO/IEC/IEEE 29119-1:2022)"""@en ;
                rdfs:label "static testing" ;
                rdfs:seeAlso """ISO/IEC/IEEE 29119-1:2022 (Software and systems engineering — Software testing — Part 1: Concepts and definitions)

Foundation - v4.0""" ;
                <http://www.w3.org/2004/02/skos/core#prefLabel> "static testing"@en .


###  http://purl.org/stc/ontology#stress_testing
:stress_testing rdf:type owl:Class ;
                rdfs:subClassOf :performance_testing ;
                :isInISTQBGlossary "true"^^xsd:boolean ;
                rdfs:label "stress testing" ;
                <http://www.w3.org/2004/02/skos/core#prefLabel> "stress testing"@en .


###  http://purl.org/stc/ontology#structural_coverage
:structural_coverage rdf:type owl:Class ;
                     rdfs:subClassOf :coverage ;
                     :isInISTQBGlossary "true"^^xsd:boolean ;
                     rdfs:comment "Coverage measures based on the internal structure of a component or system. (ISTQB Glossary v4.5)"@en ;
                     rdfs:label "structural coverage" ;
                     rdfs:seeAlso "ISO/IEC/IEEE 29119-4 (Software and systems engineering — Software testing — Part 4: Test techniques)" ;
                     <http://www.w3.org/2004/02/skos/core#altLabel> """white box test metric
white-box test metric
structure-based test metric
structure based test metric"""@en ;
                     <http://www.w3.org/2004/02/skos/core#prefLabel> "structural coverage"@en .


###  http://purl.org/stc/ontology#support_processes
:support_processes rdf:type owl:Class ;
                   rdfs:subClassOf :software_lifecycle .


###  http://purl.org/stc/ontology#system_integration_testing
:system_integration_testing rdf:type owl:Class ;
                            rdfs:subClassOf :integration_testing ;
                            :isInISTQBGlossary "true"^^xsd:boolean ;
                            rdfs:comment "The integration testing of systems. (ISTQB Glossary v4.5)"@en ;
                            rdfs:label "system integration testing" ;
                            rdfs:seeAlso "Foundation - v4.0" ;
                            <http://www.w3.org/2004/02/skos/core#prefLabel> "system integration testing"@en .


###  http://purl.org/stc/ontology#system_testing
:system_testing rdf:type owl:Class ;
                rdfs:subClassOf :test_level ;
                :isInISTQBGlossary "true"^^xsd:boolean ;
                rdfs:label "system testing" ;
                <http://www.w3.org/2004/02/skos/core#prefLabel> "system testing"@en .


###  http://purl.org/stc/ontology#target_orientation_in_software_development
:target_orientation_in_software_development rdf:type owl:Class ;
                                            rdfs:subClassOf :software_development_model ;
                                            :isInISTQBGlossary "false"^^xsd:boolean ;
                                            rdfs:label "target orientation" ;
                                            <http://www.w3.org/2004/02/skos/core#prefLabel> "target orientation in software development"@en .


###  http://purl.org/stc/ontology#target_orientation_in_test_approach
:target_orientation_in_test_approach rdf:type owl:Class ;
                                     rdfs:subClassOf :test_approach ;
                                     :isInISTQBGlossary "false"^^xsd:boolean ;
                                     rdfs:label "target orientation" ;
                                     <http://www.w3.org/2004/02/skos/core#prefLabel> "target orientation in test approach"@en .


###  http://purl.org/stc/ontology#technical_review
:technical_review rdf:type owl:Class ;
                  rdfs:subClassOf :formal_review ;
                  :isInISTQBGlossary "true"^^xsd:boolean ;
                  rdfs:comment "A formal review by technical experts that examine the quality of a work product and identify discrepancies from specifications and standards. (ISTQB Glossary v4.5)"@en ;
                  rdfs:label "technical review" ;
                  rdfs:seeAlso """Foundation - v4.0
Advanced Test Manager - 2012
Advanced Technical Test Analyst - v4.0""" ;
                  <http://www.w3.org/2004/02/skos/core#prefLabel> "technical review"@en .


###  http://purl.org/stc/ontology#test_activity
:test_activity rdf:type owl:Class ;
               rdfs:subClassOf :software_engineering_activity ,
                               :software_testing_concepts ;
               :isInISTQBGlossary "false"^^xsd:boolean ;
               rdfs:label "test activity" ;
               <http://www.w3.org/2004/02/skos/core#prefLabel> "test activity"@en .


###  http://purl.org/stc/ontology#test_analysis
:test_analysis rdf:type owl:Class ;
               rdfs:subClassOf :test_activity ;
               :isInISTQBGlossary "true"^^xsd:boolean ;
               rdfs:comment "The activity that identifies test conditions by analyzing the test basis. (ISTQB Glossary v4.5)"@en ;
               rdfs:label "test analysis" ;
               rdfs:seeAlso """Foundation - v4.0
Advanced Test Analyst - v3.1
Advanced Test Analyst - v4.0""" ;
               <http://www.w3.org/2004/02/skos/core#prefLabel> "test analysis"@en .


###  http://purl.org/stc/ontology#test_analyst
:test_analyst rdf:type owl:Class ;
              rdfs:subClassOf :related_to_role ;
              :isInISTQBGlossary "false"^^xsd:boolean ;
              rdfs:comment "Develops oracles and/or analyses test results for correctness and issues.  (ISO/IEC/IEEE 29119-1:2022)"@en ;
              rdfs:label "test analyst" ;
              rdfs:seeAlso "ISO/IEC/IEEE 29119-1:2022 (Software and systems engineering — Software testing — Part 1: Concepts and definitions)" ;
              <http://www.w3.org/2004/02/skos/core#altLabel> "TA"@en ;
              <http://www.w3.org/2004/02/skos/core#prefLabel> "test analyst"@en .


###  http://purl.org/stc/ontology#test_approach
:test_approach rdf:type owl:Class ;
               rdfs:subClassOf :software_testing_concepts ;
               :isInISTQBGlossary "true"^^xsd:boolean ;
               rdfs:comment "The manner of implementing testing tasks. (ISTQB Glossary v4.5)"@en ;
               rdfs:label "test approach" ;
               rdfs:seeAlso """Foundation - v4.0
Advanced Test Manager - 2012""" ;
               <http://www.w3.org/2004/02/skos/core#prefLabel> "test approach"@en .


###  http://purl.org/stc/ontology#test_architect
:test_architect rdf:type owl:Class ;
                rdfs:subClassOf :related_to_role ;
                :isInISTQBGlossary "false"^^xsd:boolean ;
                rdfs:comment "Defines the test strategy, test environment and test plan for programmes and projects. Specifies the organizational test requirements and helps ensure conformance to these requirements. (ISO/IEC/IEEE 29119-1:2022)"@en ;
                rdfs:label "test architect" ;
                rdfs:seeAlso "ISO/IEC/IEEE 29119-1:2022 (Software and systems engineering — Software testing — Part 1: Concepts and definitions)" ;
                <http://www.w3.org/2004/02/skos/core#prefLabel> "test architect"@en .


###  http://purl.org/stc/ontology#test_automation
:test_automation rdf:type owl:Class ;
                 rdfs:subClassOf :test_activity ;
                 :isInISTQBGlossary "true"^^xsd:boolean ;
                 rdfs:comment "The conversion of test activities to automatic operation. (ISTQB Glossary v4.5)"@en ;
                 rdfs:label "test automation" ;
                 rdfs:seeAlso """Advanced Test Automation Engineering - v2.0
Specialist - Test Automation Engineer - 2016""" ;
                 <http://www.w3.org/2004/02/skos/core#prefLabel> "test automation"@en .


###  http://purl.org/stc/ontology#test_automation_engineer
:test_automation_engineer rdf:type owl:Class ;
                          rdfs:subClassOf :related_to_role ;
                          :isInISTQBGlossary "false"^^xsd:boolean ;
                          rdfs:comment "Implements tests cases/scripts within a test automation framework. (ISO/IEC/IEEE 29119-1:2022)"@en ;
                          rdfs:label "test automation engineer" ;
                          rdfs:seeAlso "ISO/IEC/IEEE 29119-1:2022 (Software and systems engineering — Software testing — Part 1: Concepts and definitions)" ;
                          <http://www.w3.org/2004/02/skos/core#altLabel> """TAE
test automator"""@en ;
                          <http://www.w3.org/2004/02/skos/core#prefLabel> "test automation engineer"@en .


###  http://purl.org/stc/ontology#test_basis
:test_basis rdf:type owl:Class ;
            rdfs:subClassOf :Testware ;
            :isInISTQBGlossary "true"^^xsd:boolean ;
            rdfs:comment """The body of knowledge used as the basis for test analysis and test design. (ISTQB Glossary v4.5)

Information used as the basis for designing and implementing test cases. (ISO/IEC/IEEE 29119-1:2022)"""@en ;
            rdfs:label "test basis" ;
            rdfs:seeAlso """ISO/IEC/IEEE 29119-1 (2022) Software and systems engineering -- Software testing -- Part 1: Concepts and definitions

Foundation - v4.0
Advanced Test Analyst - v3.1""" ;
            <http://www.w3.org/2004/02/skos/core#prefLabel> "test basis"@en .


###  http://purl.org/stc/ontology#test_case
:test_case rdf:type owl:Class ;
           rdfs:subClassOf :Testware ;
           :isInISTQBGlossary "true"^^xsd:boolean ;
           rdfs:comment """A set of preconditions, inputs, actions (where applicable), expected results and postconditions, developed based on test conditions. (ISTQB Glossary v4.5)

Set of preconditions, inputs and expected results, developed to drive the execution of a test item to meet test objectives. (ISO/IEC/IEEE 29119-1:2022)"""@en ;
           rdfs:label "test case" ;
           rdfs:seeAlso """ISO/IEC/IEEE 29119-1 (2022) Software and systems engineering -- Software testing -- Part 1: Concepts and definitions

Foundation - v4.0
Advanced Test Manager - 2012
Advanced Test Management - v3.0
Advanced Test Analyst - v4.0
Specialist - Acceptance Testing - 2019""" ;
           <http://www.w3.org/2004/02/skos/core#altLabel> "testcase"@en ;
           <http://www.w3.org/2004/02/skos/core#prefLabel> "test case"@en .


###  http://purl.org/stc/ontology#test_completion
:test_completion rdf:type owl:Class ;
                 rdfs:subClassOf :test_activity ;
                 :isInISTQBGlossary "true"^^xsd:boolean ;
                 rdfs:comment "The activity that makes testware available for later use, leaves test environments in a satisfactory condition and communicates the results of testing to relevant stakeholders. (ISTQB Glossary v4.5)"@en ;
                 rdfs:label "test completion" ;
                 rdfs:seeAlso """Foundation - v4.0
Advanced Test Management - v3.0""" ;
                 <http://www.w3.org/2004/02/skos/core#prefLabel> "test completion"@en .


###  http://purl.org/stc/ontology#test_completion_report
:test_completion_report rdf:type owl:Class ;
                        rdfs:subClassOf :test_report ;
                        :isInISTQBGlossary "true"^^xsd:boolean ;
                        rdfs:comment """A type of test report produced at completion milestones that provides an evaluation of the corresponding test items against exit criteria. (ISTQB Glossary v4.5)

Report that provides a summary of the testing that was performed. (ISO/IEC/IEEE 29119-1:2022)"""@en ;
                        rdfs:label "test completion report" ;
                        rdfs:seeAlso """ISO/IEC/IEEE 29119-1:2022 (Software and systems engineering — Software testing — Part 1: Concepts and definitions)

Foundation - v4.0
Advanced Test Manager - 2012""" ;
                        <http://www.w3.org/2004/02/skos/core#altLabel> "test summary report"@en ;
                        <http://www.w3.org/2004/02/skos/core#prefLabel> "test completion report"@en .


###  http://purl.org/stc/ontology#test_condition
:test_condition rdf:type owl:Class ;
                rdfs:subClassOf :Testware ;
                :isInISTQBGlossary "true"^^xsd:boolean ;
                rdfs:comment """A testable aspect of a component or system identified as a basis for testing. (ISTQB Glossary v4.5)

Testable aspect of a component or system, such as a function, transaction, feature, quality attribute, or structural element identified as a basis for testing. (ISO/IEC/IEEE 29119-1:2022)"""@en ;
                rdfs:label "test condition" ;
                rdfs:seeAlso """ISO/IEC/IEEE 29119-1:2022 (Software and systems engineering — Software testing — Part 1: Concepts and definitions)

Foundation - v4.0
Advanced Test Manager - 2012
Advanced Test Analyst - v3.1
Advanced Test Analyst - v4.0
Specialist - Test Automation Strategy - v1.0""" ;
                <http://www.w3.org/2004/02/skos/core#altLabel> """test situation
test requirement"""@en ;
                <http://www.w3.org/2004/02/skos/core#prefLabel> "test condition"@en .


###  http://purl.org/stc/ontology#test_control
:test_control rdf:type owl:Class ;
              rdfs:subClassOf :test_activity ;
              :isInISTQBGlossary "true"^^xsd:boolean ;
              rdfs:comment "The activity that develops and applies corrective actions to get a test project on track when it deviates from what was planned. (ISTQB Glossary v4.5)"@en ;
              rdfs:label "test control" ;
              rdfs:seeAlso """Foundation - v4.0
Advanced Test Manager - 2012
Advanced Test Management - v3.0""" ;
              <http://www.w3.org/2004/02/skos/core#prefLabel> "test control"@en .


###  http://purl.org/stc/ontology#test_data
:test_data rdf:type owl:Class ;
           rdfs:subClassOf :Testware ;
           :isInISTQBGlossary "true"^^xsd:boolean ;
           rdfs:comment """Data needed for test execution. (ISTQB Glossary v4.5)

Data created or selected to satisfy the input requirements for executing one or more test cases, which may be defined in the test plan, test case or test procedure. (ISO/IEC/IEEE 29119-1:2022)"""@en ;
           rdfs:label "test data" ;
           rdfs:seeAlso """ISO/IEC/IEEE 29119-1:2022 (Software and systems engineering — Software testing — Part 1: Concepts and definitions)

Foundation - v4.0
Advanced Test Analyst - v3.1
Advanced Test Analyst - v4.0""" ;
           <http://www.w3.org/2004/02/skos/core#altLabel> """testdata
test data set
testdata set"""@en ;
           <http://www.w3.org/2004/02/skos/core#prefLabel> "test data"@en .


###  http://purl.org/stc/ontology#test_design
:test_design rdf:type owl:Class ;
             rdfs:subClassOf :test_activity ;
             :isInISTQBGlossary "true"^^xsd:boolean ;
             rdfs:comment "The activity that derives and specifies test cases from test conditions. (ISTQB Glossary v4.5)"@en ;
             rdfs:label "test design" ;
             rdfs:seeAlso """Foundation - v4.0
Advanced Test Manager - 2012
Advanced Test Analyst - v3.1
Advanced Test Analyst - v4.0""" ;
             <http://www.w3.org/2004/02/skos/core#prefLabel> "test design"@en .


###  http://purl.org/stc/ontology#test_designer
:test_designer rdf:type owl:Class ;
               rdfs:subClassOf :related_to_role ;
               :isInISTQBGlossary "false"^^xsd:boolean ;
               rdfs:comment "Develops the test design artefacts. (ISO/IEC/IEEE 29119-1:2022)"@en ;
               rdfs:label "test designer" ;
               rdfs:seeAlso "ISO/IEC/IEEE 29119-1:2022 (Software and systems engineering — Software testing — Part 1: Concepts and definitions)" ;
               <http://www.w3.org/2004/02/skos/core#prefLabel> "test designer"@en .


###  http://purl.org/stc/ontology#test_director
:test_director rdf:type owl:Class ;
               rdfs:subClassOf :related_to_role ;
               :isInISTQBGlossary "true"^^xsd:boolean ;
               rdfs:comment "A senior manager who manages test managers."@en ;
               rdfs:label "test director" ;
               rdfs:seeAlso "Advanced Test Manager - 2012" ;
               <http://www.w3.org/2004/02/skos/core#prefLabel> "test director"@en .


###  http://purl.org/stc/ontology#test_driven_development
:test_driven_development rdf:type owl:Class ;
                         rdfs:subClassOf :target_orientation_in_software_development ;
                         :isInISTQBGlossary "true"^^xsd:boolean ;
                         rdfs:comment "A software development technique in which the test cases are developed, automated and then the software is developed incrementally to pass those test cases. (ISTQB Glossary v4.5)"@en ;
                         rdfs:label "test-driven" ;
                         rdfs:seeAlso """Foundation - v4.0
Advanced Test Manager - 2012
Advanced Test Management - v3.0
Advanced Test Automation Engineering - v2.0
Advanced Agile Technical Tester - 2019
Specialist - Agile Test Leadership at Scale - v2.0
Specialist - Test Automation Strategy - v1.0""" ;
                         <http://www.w3.org/2004/02/skos/core#altLabel> """test driven development
tdd
TDD"""@en ;
                         <http://www.w3.org/2004/02/skos/core#prefLabel> "test-driven development"@en .


###  http://purl.org/stc/ontology#test_execution
:test_execution rdf:type owl:Class ;
                rdfs:subClassOf :test_activity ;
                :isInISTQBGlossary "true"^^xsd:boolean ;
                rdfs:comment "The activity that runs a test on a component or system producing actual results. (ISTQB Glossary v4.5)"@en ;
                rdfs:label "test execution" ;
                rdfs:seeAlso """Foundation - v4.0
Advanced Test Manager - 2012
Advanced Test Analyst - v3.1
Advanced Test Analyst - v4.0
Advanced Technical Test Analyst - v4.0""" ;
                <http://www.w3.org/2004/02/skos/core#prefLabel> "test execution"@en .


###  http://purl.org/stc/ontology#test_first_approach
:test_first_approach rdf:type owl:Class ;
                     rdfs:subClassOf :test_driven_development ;
                     :isInISTQBGlossary "true"^^xsd:boolean ;
                     rdfs:comment "An approach to software development in which the test cases are designed and implemented before the associated component or system is developed. (ISTQB Glossary v4.5)"@en ;
                     rdfs:label "test-first approach" ;
                     rdfs:seeAlso """Foundation - v4.0
Advanced Test Analyst - v3.1
Foundation Agile Tester - 2014
Specialist - Agile Test Leadership at Scale - v2.0""" ;
                     <http://www.w3.org/2004/02/skos/core#altLabel> "test first approach"@en ;
                     <http://www.w3.org/2004/02/skos/core#prefLabel> "test-first approach"@en .


###  http://purl.org/stc/ontology#test_implementation
:test_implementation rdf:type owl:Class ;
                     rdfs:subClassOf :test_activity ;
                     :isInISTQBGlossary "true"^^xsd:boolean ;
                     rdfs:comment "The activity that prepares the testware needed for test execution based on test analysis and design. (ISTQB Glossary v4.5)"@en ;
                     rdfs:label "test implementation" ;
                     rdfs:seeAlso """Foundation - v4.0
Advanced Test Manager - 2012
Advanced Test Analyst - v3.1
Advanced Test Analyst - v4.0""" ;
                     <http://www.w3.org/2004/02/skos/core#prefLabel> "test implementation"@en .


###  http://purl.org/stc/ontology#test_item
:test_item rdf:type owl:Class ;
           rdfs:subClassOf :Testware ;
           :isInISTQBGlossary "true"^^xsd:boolean ;
           rdfs:comment "A part of a test object used in the test process. (ISTQB Glossary v4.5)"@en ,
                        "ISO/IEC/IEEE 29119-1:2022 defines the term test item differently: as a synonym to test object."@en ;
           rdfs:label "test item" ;
           <http://www.w3.org/2004/02/skos/core#prefLabel> "test item"@en .


###  http://purl.org/stc/ontology#test_leader
:test_leader rdf:type owl:Class ;
             rdfs:subClassOf :related_to_role ;
             :isInISTQBGlossary "true"^^xsd:boolean ;
             rdfs:comment "On large projects, the person who reports to the test manager and is responsible for project management of a particular test level or a particular set of testing activities. (ISTQB Glossary v4.5)"@en ;
             rdfs:label "test leader" ;
             rdfs:seeAlso "Advanced Test Manager - 2012" ;
             <http://www.w3.org/2004/02/skos/core#altLabel> "lead tester"@en ;
             <http://www.w3.org/2004/02/skos/core#prefLabel> "test leader"@en .


###  http://purl.org/stc/ontology#test_level
:test_level rdf:type owl:Class ;
            rdfs:subClassOf :software_testing_concepts ;
            :isInISTQBGlossary "true"^^xsd:boolean ;
            rdfs:comment """A specific instantiation of a test process. (ISTQB Glossary v4.5)

One of a sequence of test stages each of which is typically associated with the achievement of particular
objectives and used to treat particular risks. (ISO/IEC/IEEE 29119-1:2022)"""@en ;
            rdfs:label "test level" ;
            rdfs:seeAlso """ISO/IEC/IEEE 29119-1:2022 (Software and systems engineering — Software testing — Part 1: Concepts and definitions)

Foundation - v4.0
Advanced Test Manager - 2012
Advanced Test Management - v3.0
Specialist - Mobile Application Testing - 2019
Specialist - Test Automation Strategy - v1.0""" ;
            <http://www.w3.org/2004/02/skos/core#altLabel> """test stage
test phase"""@en ;
            <http://www.w3.org/2004/02/skos/core#prefLabel> "test level"@en .


###  http://purl.org/stc/ontology#test_management
:test_management rdf:type owl:Class ;
                 rdfs:subClassOf :software_testing_concepts ,
                                 :test_activity ;
                 :isInISTQBGlossary "true"^^xsd:boolean ;
                 rdfs:comment "The process of planning, scheduling, estimating, monitoring, reporting, controlling, and completing test activities. (ISTQB Glossary v4.5)"@en ;
                 rdfs:label "test management" ;
                 <http://www.w3.org/2004/02/skos/core#prefLabel> "test management"@en .


###  http://purl.org/stc/ontology#test_manager
:test_manager rdf:type owl:Class ;
              rdfs:subClassOf :related_to_role ;
              :isInISTQBGlossary "true"^^xsd:boolean ;
              rdfs:comment """The person responsible for project management of testing activities, resources, and evaluation of a test object. (ISTQB Glossary v4.5)

Develops, manages, and helps to ensure conformance with the test management process. The test manager also plans and controls the dynamic test process. (ISO/IEC/IEEE 29119-1:2022)"""@en ;
              rdfs:label "test manager" ;
              rdfs:seeAlso """ISO/IEC/IEEE 29119-1:2022 (Software and systems engineering — Software testing — Part 1: Concepts and definitions)

Advanced Test Manager - 2012""" ;
              <http://www.w3.org/2004/02/skos/core#prefLabel> "test manager"@en .


###  http://purl.org/stc/ontology#test_metric
:test_metric rdf:type owl:Class ;
             rdfs:subClassOf :metric ,
                             :software_testing_concepts ;
             :isInISTQBGlossary "false"^^xsd:boolean ;
             rdfs:comment "A measurement of a characteristic of a test process, test activity, test object or testware. (own)"@en ;
             rdfs:label "test metric" ;
             rdfs:seeAlso "ISO/IEC/IEEE 29119-4 (Software and systems engineering — Software testing — Part 4: Test techniques)" ;
             <http://www.w3.org/2004/02/skos/core#altLabel> "testmetric"@en ;
             <http://www.w3.org/2004/02/skos/core#prefLabel> "test metric"@en .


###  http://purl.org/stc/ontology#test_model
:test_model rdf:type owl:Class ;
            rdfs:subClassOf :Testware ;
            :isInISTQBGlossary "true"^^xsd:boolean ;
            rdfs:comment """A model describing testware that is used for testing a component or a system under test. (ISTQB Glossary v4.5)

Representation of the test item, which allows the testing to be focused on particular
characteristics or qualities. (ISO/IEC/IEEE 29119-1:2022)"""@en ;
            rdfs:label "test model" ;
            rdfs:seeAlso """ISO/IEC/IEEE 29119-1:2022 (Software and systems engineering — Software testing — Part 1: Concepts and definitions)

Specialist - Model-Based Tester - 2015
Specialist - Model-Based Testing - v1.1""" ;
            <http://www.w3.org/2004/02/skos/core#altLabel> "test specification" ;
            <http://www.w3.org/2004/02/skos/core#prefLabel> "test model"@en .


###  http://purl.org/stc/ontology#test_monitoring
:test_monitoring rdf:type owl:Class ;
                 rdfs:subClassOf :test_activity ;
                 :isInISTQBGlossary "true"^^xsd:boolean ;
                 rdfs:comment "The activity that checks the status of testing activities, identifies any variances from planned or expected, and reports status to stakeholders. (ISTQB Glossary v4.5)"@en ;
                 rdfs:label "test monitoring" ;
                 rdfs:seeAlso """Foundation - v4.0
Advanced Test Manager - 2012
Advanced Test Management - v3.0""" ;
                 <http://www.w3.org/2004/02/skos/core#prefLabel> "test monitoring"@en .


###  http://purl.org/stc/ontology#test_object
:test_object rdf:type owl:Class ;
             rdfs:subClassOf :software ;
             :isInISTQBGlossary "true"^^xsd:boolean ;
             rdfs:comment "The work product to be tested. (ISTQB Glossary v4.5)"@en ;
             rdfs:label "test object" ;
             rdfs:seeAlso "Foundation - v4.0" ;
             <http://www.w3.org/2004/02/skos/core#altLabel> """test target
system under test
sut
SUT
object under test"""@en ;
             <http://www.w3.org/2004/02/skos/core#prefLabel> "test object"@en .


###  http://purl.org/stc/ontology#test_objective
:test_objective rdf:type owl:Class ;
                rdfs:subClassOf :Testware ;
                :isInISTQBGlossary "true"^^xsd:boolean ;
                rdfs:comment "The purpose for testing. (ISTQB Gloassary v4.5)"@en ,
                             "test objective"@en ;
                rdfs:seeAlso """Foundation - v4.0
Advanced Test Management - v3.0""" ;
                <http://www.w3.org/2004/02/skos/core#altLabel> "test goal"@en ;
                <http://www.w3.org/2004/02/skos/core#prefLabel> "test objective"@en .


###  http://purl.org/stc/ontology#test_oracle
:test_oracle rdf:type owl:Class ;
             rdfs:subClassOf :Testware ;
             :isInISTQBGlossary "true"^^xsd:boolean ;
             rdfs:comment "A source to determine an expected result to compare with the actual result of the system under test.  (ISTQB Glossary v4.5)"@en ;
             rdfs:label "test oracle" ;
             rdfs:seeAlso "Advanced Test Analyst - v4.0" ;
             <http://www.w3.org/2004/02/skos/core#altLabel> "oracle"@en ;
             <http://www.w3.org/2004/02/skos/core#prefLabel> "test oracle"@en .


###  http://purl.org/stc/ontology#test_plan
:test_plan rdf:type owl:Class ;
           rdfs:subClassOf :Testware ;
           :isInISTQBGlossary "true"^^xsd:boolean ;
           rdfs:comment """Documentation describing the test objectives to be achieved and the means and the schedule for achieving them, organized to coordinate testing activities. (ISTQB Glossary v4.5)

Detailed description of test objectives to be achieved and the means and schedule for achieving them, organized to coordinate testing activities for some test item or set of test items. (ISO/IEC/IEEE 29119-1:2022)"""@en ;
           rdfs:label "test plan" ;
           rdfs:seeAlso """ISO/IEC/IEEE 29119-1 (2022) Software and systems engineering -- Software testing -- Part 1: Concepts and definitions

Foundation - v4.0
Advanced Test Manager - 2012
Advanced Test Management - v3.0
Specialist - Performance Testing - 2018
Specialist - Security Test Engineer - v1.0""" ;
           <http://www.w3.org/2004/02/skos/core#altLabel> "testplan"@en ;
           <http://www.w3.org/2004/02/skos/core#prefLabel> "test plan"@en .


###  http://purl.org/stc/ontology#test_planning
:test_planning rdf:type owl:Class ;
               rdfs:subClassOf :test_activity ;
               :isInISTQBGlossary "true"^^xsd:boolean ;
               rdfs:comment "The activity of establishing or updating a test plan. (ISTQB Glossary v4.5)"@en ;
               rdfs:label "test planning" ;
               rdfs:seeAlso """Foundation - v4.0
Advanced Test Manager - 2012
Advanced Test Management - v3.0""" ;
               <http://www.w3.org/2004/02/skos/core#prefLabel> "test planning"@en .


###  http://purl.org/stc/ontology#test_process
:test_process rdf:type owl:Class ;
              rdfs:subClassOf :software_testing_concepts ;
              :isInISTQBGlossary "true"^^xsd:boolean ;
              rdfs:comment "The set of interrelated activities comprising of test planning, test monitoring, test control, test analysis, test design, test implementation, test execution, and test completion."@en ,
                           """The set of interrelated activities comprising of test planning, test monitoring, test control, test analysis, test design, test implementation, test execution, and test completion. (ISTQB Glossary v4.5)

Set of testing activities performed to achieve a test objective. (ISO/IEC/IEEE 29119-1:2022)"""@en ;
              rdfs:label "test process" ;
              rdfs:seeAlso """ISO/IEC/IEEE 29119-1:2022 (Software and Systems Engineering — Software Testing — Part 1: Concepts and Definitions)

Foundation - v4.0
Specialist - Mobile Application Testing - 2019
Specialist - Security Test Engineer - v1.0""" ;
              <http://www.w3.org/2004/02/skos/core#prefLabel> "test process"@en .


###  http://purl.org/stc/ontology#test_process_group
:test_process_group rdf:type owl:Class ;
                    rdfs:subClassOf :related_to_team ;
                    :isInISTQBGlossary "true"^^xsd:boolean ;
                    rdfs:comment "A collection of specialists who facilitate the definition, maintenance, and improvement of the test processes used by an organization. (ISTQB Glossary v4.5)"@en ;
                    rdfs:label "test process group" ;
                    rdfs:seeAlso "Expert Improving the Test Process - v1.0.1" ;
                    <http://www.w3.org/2004/02/skos/core#altLabel> "TPG"@en ;
                    <http://www.w3.org/2004/02/skos/core#prefLabel> "test process group"@en .


###  http://purl.org/stc/ontology#test_process_improvement
:test_process_improvement rdf:type owl:Class ;
                          rdfs:subClassOf :test_management ;
                          :isInISTQBGlossary "true"^^xsd:boolean ;
                          rdfs:label "test process improvement" ;
                          <http://www.w3.org/2004/02/skos/core#prefLabel> "test process improvement"@en .


###  http://purl.org/stc/ontology#test_progress_report
:test_progress_report rdf:type owl:Class ;
                      rdfs:subClassOf :test_report ;
                      :isInISTQBGlossary "true"^^xsd:boolean ;
                      rdfs:comment """A type of periodic test report that includes the progress of test activities against a baseline, risks, and alternatives requiring a decision. (ISTQB Glossary v4.5)

Report that provides information about the status of the testing that is being performed in a specified reporting period. (ISO/IEC/IEEE 29119-1:2022, defined as test status report)"""@en ;
                      rdfs:label "test progress report" ;
                      rdfs:seeAlso """ISO/IEC/IEEE 29119-1:2022 (Software and systems engineering — Software testing — Part 1: Concepts and definitions)

Foundation - v4.0
Advanced Test Automation Engineering - v2.0""" ;
                      <http://www.w3.org/2004/02/skos/core#altLabel> "test status report"@en ;
                      <http://www.w3.org/2004/02/skos/core#prefLabel> "test progress report"@en .


###  http://purl.org/stc/ontology#test_report
:test_report rdf:type owl:Class ;
             rdfs:subClassOf :Testware ;
             :isInISTQBGlossary "true"^^xsd:boolean ;
             rdfs:comment "Documentation summarizing testing and results. (ISTQB Glossary v4.5)"@en ;
             rdfs:label "test report" ;
             rdfs:seeAlso """Specialist - Mobile Application Testing - 2019
Specialist - Security Test Engineer - v1.0
Specialist - Test Automation Strategy - v1.0""" ;
             <http://www.w3.org/2004/02/skos/core#altLabel> "testreport"@en ;
             <http://www.w3.org/2004/02/skos/core#prefLabel> "test report"@en .


###  http://purl.org/stc/ontology#test_script
:test_script rdf:type owl:Class ;
             rdfs:subClassOf :Testware ;
             :isInISTQBGlossary "true"^^xsd:boolean ;
             rdfs:comment """A sequence of instructions for the execution of a test. (ISTQB Glossary v4.5)

Document specifying one or more test procedures. (ISO/IEC/IEEE 29119-1:2022)"""@en ;
             rdfs:label "test script" ;
             rdfs:seeAlso """ISO/IEC/IEEE 29119-1:2022 (Software and systems engineering — Software testing — Part 1: Concepts and definitions)

Advanced Test Manager - 2012
Advanced Test Analyst - v3.1
Advanced Test Analyst - v4.0
Advanced Test Automation Engineering - v2.0
Specialist - Test Automation Engineer - 2016""" ;
             <http://www.w3.org/2004/02/skos/core#altLabel> "test procedure specification"@en ;
             <http://www.w3.org/2004/02/skos/core#prefLabel> "test script"@en .


###  http://purl.org/stc/ontology#test_step
:test_step rdf:type owl:Class ;
           rdfs:subClassOf :Testware ;
           :isInISTQBGlossary "true"^^xsd:boolean ;
           rdfs:comment "A single interaction between an actor and a test object consisting of an input, an action, and an expected result. (ISTQB Glossary v4.5)"@en ,
                        "Advanced Test Automation Engineering - v2.0"@en ;
           rdfs:label "test step" ;
           <http://www.w3.org/2004/02/skos/core#altLabel> "teststep"@en ;
           <http://www.w3.org/2004/02/skos/core#prefLabel> "test step"@en .


###  http://purl.org/stc/ontology#test_suite
:test_suite rdf:type owl:Class ;
            rdfs:subClassOf :Testware ;
            :isInISTQBGlossary "true"^^xsd:boolean ;
            rdfs:comment """A set of test scripts or test procedures to be executed in a specific test run. (ISTQB Glossary v4.5)

Set of test cases or test procedures. (ISO/IEC/IEEE 29119-1:2022)"""@en ;
            rdfs:label "test suite" ;
            rdfs:seeAlso """Advanced Test Analyst - v3.1
Specialist - Test Automation Strategy - v1.0""" ;
            <http://www.w3.org/2004/02/skos/core#altLabel> """test set
test case suite
testsuite
testset
testcase suite"""@en ;
            <http://www.w3.org/2004/02/skos/core#prefLabel> "test suite"@en .


###  http://purl.org/stc/ontology#test_technique
:test_technique rdf:type owl:Class ;
                rdfs:subClassOf :software_testing_concepts ;
                :isInISTQBGlossary "true"^^xsd:boolean ;
                rdfs:comment "(ISTQB Glossary v4.5)"@en ,
                             """A procedure used to define test conditions, design test cases, and specify test data. (ISTQB Glossary v4.5)

Procedure used to create or select a test model, identify test coverage items, and derive
corresponding test cases. (ISO/IEC/IEEE 29119-1:2022, defined as test design technique)"""@en ;
                rdfs:label "test technique" ;
                rdfs:seeAlso """ISO/IEC/IEEE 29119-4 (Software and systems engineering — Software testing — Part 4: Test techniques)

Foundation - v4.0""" ;
                <http://www.w3.org/2004/02/skos/core#altLabel> "test design technique"@en ,
                                                               "test technique"@en .


###  http://purl.org/stc/ontology#test_type
:test_type rdf:type owl:Class ;
           rdfs:subClassOf :software_testing_concepts ;
           :isInISTQBGlossary "true"^^xsd:boolean ;
           rdfs:comment """A group of test activities based on specific test objectives aimed at specific characteristics of a component or system. (ISTQB Glossary v4.5)

Testing that is focused on specific quality characteristics. (ISO/IEC/IEEE 29119-1:2022)"""@en ;
           rdfs:label "test type" ;
           rdfs:seeAlso """ISO/IEC/IEEE 29119-1:2022 (Software and Systems Engineering — Software Testing — Part 1: Concepts and Definitions)

Foundation - v4.0
Advanced Test Manager - 2012
Advanced Test Management - v3.0
Advanced Test Analyst - v3.1
Advanced Test Analyst - v4.0
Advanced Technical Test Analyst - v4.0
Advanced Test Automation Engineering - v2.0
Specialist - Automotive Software Tester - 2018
Specialist - Automotive Software Tester - v1.1
Specialist - Gambling Industry Tester - 2018
Specialist - Game Testing - v1.0.1
Specialist - Mobile Application Testing - 2019
Specialist - Model-Based Testing - v1.1
Specialist - Test Automation Strategy - v1.0""" ;
           <http://www.w3.org/2004/02/skos/core#prefLabel> "test type"@en .


###  http://purl.org/stc/ontology#test_work_force
:test_work_force rdf:type owl:Class ;
                 rdfs:subClassOf :software_testing_concepts ;
                 :isInISTQBGlossary "false"^^xsd:boolean ;
                 rdfs:comment "Professions and roles in software testing"@en ;
                 rdfs:label "test work force" ;
                 rdfs:seeAlso "GTB: The Professional profile for testing. The reference scheme for people and organizations involved in the topics of quality and testing of software-based components and systems. 2018." ;
                 <http://www.w3.org/2004/02/skos/core#prefLabel> "test work force"@en .


###  http://purl.org/stc/ontology#tester
:tester rdf:type owl:Class ;
        rdfs:subClassOf :related_to_role ;
        :isInISTQBGlossary "true"^^xsd:boolean ;
        rdfs:comment """A person who performs testing. (ISTQB Glossary v4.5)

Develops the test deliverables and completes the processes associated with the
dynamic test process. (ISO/IEC/IEEE 29119-1:2022)"""@en ;
        rdfs:label "tester" ;
        rdfs:seeAlso "ISO/IEC/IEEE 29119-1:2022 (Software and systems engineering — Software testing — Part 1: Concepts and definitions)" ;
        <http://www.w3.org/2004/02/skos/core#prefLabel> "tester"@en .


###  http://purl.org/stc/ontology#tester_orientation_in_test_approach
:tester_orientation_in_test_approach rdf:type owl:Class ;
                                     rdfs:subClassOf :test_approach ;
                                     :isInISTQBGlossary "false"^^xsd:boolean ;
                                     rdfs:label "tester orientation" ;
                                     <http://www.w3.org/2004/02/skos/core#prefLabel> "tester orientation in test approach"@en .


###  http://purl.org/stc/ontology#testing
:testing rdf:type owl:Class ;
         rdfs:subClassOf :software_testing_concepts ;
         :isInISTQBGlossary "true"^^xsd:boolean ;
         rdfs:comment """Set of activities conducted to facilitate discovery and evaluation of properties of test items (ISO/IEC/IEEE 29119-1:2022, defined as test)

The process that consists of determining the degree to which a software product satisfies specified requirements (verification) and fulfills its intended purpose (validation). (ISO/IEC/IEEE 12207:2017)

The process of executing a system or component under specified conditions, observing or recording the results, and making an evaluation of some aspect of the system or component. (IEEE 610.12-1990)"""@en ;
         rdfs:seeAlso "Foundation - v4.0" ,
                      """IEEE Standard 610.12-1990 (IEEE Standard Glossary of Software Engineering Terminology)
ISO/IEC/IEEE 29119-1:2022 (Software and Systems Engineering — Software Testing — Part 1: Concepts and Definitions)
ISO/IEC/IEEE 12207:2017 (Software Life Cycle Processes)""" ;
         <http://www.w3.org/2004/02/skos/core#prefLabel> "testing"@en .


###  http://purl.org/stc/ontology#testing_in_production
:testing_in_production rdf:type owl:Class ;
                       rdfs:subClassOf :system_testing ;
                       :isInISTQBGlossary "true"^^xsd:boolean ;
                       rdfs:label "testing in production" ;
                       <http://www.w3.org/2004/02/skos/core#prefLabel> "testing in production"@en .


###  http://purl.org/stc/ontology#testing_quadrants
:testing_quadrants rdf:type owl:Class ;
                   rdfs:subClassOf :test_approach ;
                   :isInISTQBGlossary "true"^^xsd:boolean ;
                   rdfs:comment "A classification model of test types/test levels in four quadrants, relating them to two dimensions of test objectives: supporting the product team versus critiquing the product, and technology-facing versus business-facing. (ISTQB Glossary v4.5)"@en ;
                   rdfs:label "testing quadrants" ;
                   rdfs:seeAlso "Foundation - v4.0" ;
                   <http://www.w3.org/2004/02/skos/core#prefLabel> "testing quadrants"@en .


###  http://purl.org/stc/ontology#usability_testing
:usability_testing rdf:type owl:Class ;
                   rdfs:subClassOf :non-functional_testing ;
                   :isInISTQBGlossary "true"^^xsd:boolean ;
                   rdfs:comment "Testing to evaluate the degree to which the system can be used by specified users with effectiveness, efficiency and satisfaction in a specified context of use. (ISTQB Glossary v4.5)"@en ;
                   rdfs:label "usability testing" ;
                   rdfs:seeAlso """Specialist - Mobile Application Testing - 2019
Specialist - Usability Testing - 2018""" ;
                   <http://www.w3.org/2004/02/skos/core#prefLabel> "usability testing"@en .


###  http://purl.org/stc/ontology#user-agent_based_testing
:user-agent_based_testing rdf:type owl:Class ;
                          rdfs:subClassOf :mobile_app_testing ;
                          :isInISTQBGlossary "true"^^xsd:boolean ;
                          rdfs:label "user-agent based testing" ;
                          <http://www.w3.org/2004/02/skos/core#prefLabel> "user-agent based testing"@en .


###  http://purl.org/stc/ontology#user_acceptance_testing
:user_acceptance_testing rdf:type owl:Class ;
                         rdfs:subClassOf :acceptance_testing ;
                         :isInISTQBGlossary "true"^^xsd:boolean ;
                         rdfs:label "user acceptance testing" ;
                         <http://www.w3.org/2004/02/skos/core#prefLabel> "user acceptance testing"@en .


###  http://purl.org/stc/ontology#validation
:validation rdf:type owl:Class ;
            rdfs:subClassOf :basic_concepts .


###  http://purl.org/stc/ontology#verification
:verification rdf:type owl:Class ;
              rdfs:subClassOf :basic_concepts .


###  http://purl.org/stc/ontology#walkthrough
:walkthrough rdf:type owl:Class ;
             rdfs:subClassOf :informal_review ;
             :isInISTQBGlossary "true"^^xsd:boolean ;
             rdfs:comment "A type of review in which an author leads members of the review through a work product and the members ask questions and make comments about possible issues.  (ISTQB Glossary v4.5)"@en ;
             rdfs:label "walkthrough" ;
             rdfs:seeAlso """Foundation - v4.0
Advanced Test Manager - 2012""" ;
             <http://www.w3.org/2004/02/skos/core#altLabel> "structured walkthrough"@en ;
             <http://www.w3.org/2004/02/skos/core#prefLabel> "walkthrough"@en .


###  http://purl.org/stc/ontology#white_box_test_technique
:white_box_test_technique rdf:type owl:Class ;
                          rdfs:subClassOf :test_technique ;
                          :isInISTQBGlossary "true"^^xsd:boolean ;
                          rdfs:label "white box test technique" ;
                          <http://www.w3.org/2004/02/skos/core#altLabel> """white-box test technique
structure-based test design technique
structure based test design technique
structure-based test technique
structure based test technique
glass-box testing"""@en ;
                          <http://www.w3.org/2004/02/skos/core#prefLabel> "white box test technique"@en .


#################################################################
#    Individuals
#################################################################

###  http://purl.org/stc/terms#AI_testing
<http://purl.org/stc/terms#AI_testing> rdf:type owl:NamedIndividual ;
                                       <http://purl.org/stc/terms#hasParent> <http://purl.org/stc/terms#domain-specific_test_types> ;
                                       :isInISTQBGlossary "true"^^xsd:boolean ;
                                       rdfs:label "AI testing" ;
                                       <http://www.w3.org/2004/02/skos/core#prefLabel> "ai testing"@en .


###  http://purl.org/stc/terms#API_testing
<http://purl.org/stc/terms#API_testing> rdf:type owl:NamedIndividual ;
                                        <http://purl.org/stc/terms#hasParent> <http://purl.org/stc/terms#interface_testing> ;
                                        :isInISTQBGlossary "true"^^xsd:boolean ;
                                        rdfs:label "API testing" ;
                                        <http://www.w3.org/2004/02/skos/core#prefLabel> "api testing"@en .


###  http://purl.org/stc/terms#GUI_testing
<http://purl.org/stc/terms#GUI_testing> rdf:type owl:NamedIndividual ;
                                        <http://purl.org/stc/terms#hasParent> <http://purl.org/stc/terms#interface_testing> ;
                                        :isInISTQBGlossary "true"^^xsd:boolean ;
                                        rdfs:label "GUI testing" ;
                                        <http://www.w3.org/2004/02/skos/core#altLabel> "graphical user interface testing"@en ;
                                        <http://www.w3.org/2004/02/skos/core#prefLabel> "GUI testing"@en .


###  http://purl.org/stc/terms#LLM_structural_coverage
<http://purl.org/stc/terms#LLM_structural_coverage> rdf:type owl:NamedIndividual ;
                                                    <http://purl.org/stc/terms#hasParent> <http://purl.org/stc/terms#structural_coverage> ;
                                                    :isInISTQBGlossary "false"^^xsd:boolean ;
                                                    rdfs:comment "Coverage measures based on the internal structure of an LLM. (own))"@en ;
                                                    rdfs:label "LLM structural coverage" ;
                                                    <http://www.w3.org/2004/02/skos/core#prefLabel> "llm structural coverage"@en .


###  http://purl.org/stc/terms#MBT_modeller
<http://purl.org/stc/terms#MBT_modeller> rdf:type owl:NamedIndividual ;
                                         <http://purl.org/stc/terms#hasParent> <http://purl.org/stc/terms#related_to_role> ;
                                         :isInISTQBGlossary "false"^^xsd:boolean ;
                                         rdfs:comment "Develops formal test specifications in the form of models used to generate test cases as part of model-based testing. (ISO/IEC/IEEE 29119-1:2022)"@en ;
                                         rdfs:label "MBT modeller" ;
                                         rdfs:seeAlso "ISO/IEC/IEEE 29119-1:2022 (Software and systems engineering — Software testing — Part 1: Concepts and definitions)" ;
                                         <http://www.w3.org/2004/02/skos/core#prefLabel> "MBT modeller"@en .


###  http://purl.org/stc/terms#N-switch_coverage
<http://purl.org/stc/terms#N-switch_coverage> rdf:type owl:NamedIndividual ;
                                              <http://purl.org/stc/terms#hasParent> <http://purl.org/stc/terms#structural_coverage> ;
                                              :isInISTQBGlossary "true"^^xsd:boolean ;
                                              rdfs:comment "The coverage of sequences of N+1 transitions. (ISTQB Glossary v4.5)"@en ;
                                              rdfs:label "N-switch coverage" ;
                                              rdfs:seeAlso "" ;
                                              <http://www.w3.org/2004/02/skos/core#altLabel> "chow's coverage metric"@en ;
                                              <http://www.w3.org/2004/02/skos/core#prefLabel> """n-switch coverage
N-switch coverage"""@en .


###  http://purl.org/stc/terms#Testware
<http://purl.org/stc/terms#Testware> rdf:type owl:NamedIndividual ;
                                     <http://purl.org/stc/terms#hasParent> <http://purl.org/stc/terms#software> ,
                                                                           <http://purl.org/stc/terms#software_testing_concepts> ;
                                     :isInISTQBGlossary "true"^^xsd:boolean ;
                                     rdfs:comment """Work products produced during the test process for use in planning, designing, executing, evaluating and reporting on testing. (ISTQB Glossary v4.5)

Artefacts produced during the test process required to plan, design, and execute tests. (ISO/IEC/IEEE 29119-1:2022)"""@en ;
                                     rdfs:label "testware" ;
                                     rdfs:seeAlso """ISO/IEC/IEEE 29119-1 (2022) Software and systems engineering -- Software testing -- Part 1: Concepts and definitions

Foundation - v4.0
Advanced Test Manager - 2012
Advanced Test Management - v3.0
Advanced Test Analyst - v3.1
Advanced Test Analyst - v4.0
Advanced Test Automation Engineering - v2.0
Specialist - Automotive Software Tester - v1.1
Specialist - Game Testing - v1.0.1
Specialist - Model-Based Testing - v1.1
Specialist - Performance Testing - 2018
Specialist - Test Automation Engineer - 2016
Specialist - Test Automation Strategy - v1.0""" ;
                                     <http://www.w3.org/2004/02/skos/core#altLabel> """test artefact
test artifact""" ;
                                     <http://www.w3.org/2004/02/skos/core#prefLabel> "testware"@en .


###  http://purl.org/stc/terms#a_b_testing
<http://purl.org/stc/terms#a_b_testing> rdf:type owl:NamedIndividual ;
                                        <http://purl.org/stc/terms#hasParent> <http://purl.org/stc/terms#oracle_orientation_in_test_approach> ;
                                        :isInISTQBGlossary "true"^^xsd:boolean ;
                                        rdfs:comment """A test approach in which two components or systems are statistically evaluated to determine which performs better for specified criteria. (ISTQB Glossary v4.5) 

Statistical testing approach that allows testers to determine which of two systems or components performs better. (ISO/IEC/IEEE 29119-1:2022)"""@en ;
                                        rdfs:label "a/b testing" ;
                                        <http://www.w3.org/2004/02/skos/core#prefLabel> "a/b testing"@en .


###  http://purl.org/stc/terms#acceptance
<http://purl.org/stc/terms#acceptance> rdf:type owl:NamedIndividual ;
                                       <http://purl.org/stc/terms#hasParent> <http://purl.org/stc/terms#software_engineering_activity> .


###  http://purl.org/stc/terms#acceptance_criteria
<http://purl.org/stc/terms#acceptance_criteria> rdf:type owl:NamedIndividual ;
                                                <http://purl.org/stc/terms#hasParent> <http://purl.org/stc/terms#Testware> ;
                                                :isInISTQBGlossary "true"^^xsd:boolean ;
                                                rdfs:comment """The criteria that a work product must satisfy to be accepted by the stakeholders. (ISTQB Glossary v4.5, after IREB Glossary)

Criteria that a system or system component must satisfy to be accepted by a user, customer, or other authorized entity.(ISO/IEC/IEEE 29148:2018)"""@en ;
                                                rdfs:label "acceptance criteria" ;
                                                rdfs:seeAlso "ISO/IEC/IEEE 29148:2018 (Systems and software engineering — Life cycle processes — Requirements engineering)" ;
                                                <http://www.w3.org/2004/02/skos/core#prefLabel> "acceptance criteria"@en .


###  http://purl.org/stc/terms#acceptance_test-driven_development
<http://purl.org/stc/terms#acceptance_test-driven_development> rdf:type owl:NamedIndividual ;
                                                               <http://purl.org/stc/terms#hasParent> <http://purl.org/stc/terms#test_first_approach> ;
                                                               :isInISTQBGlossary "true"^^xsd:boolean ;
                                                               rdfs:label "acceptance test-driven development" ;
                                                               <http://www.w3.org/2004/02/skos/core#prefLabel> "acceptance test-driven development"@en .


###  http://purl.org/stc/terms#acceptance_testing
<http://purl.org/stc/terms#acceptance_testing> rdf:type owl:NamedIndividual ;
                                               <http://purl.org/stc/terms#hasParent> <http://purl.org/stc/terms#test_level> ;
                                               :isInISTQBGlossary "true"^^xsd:boolean ;
                                               rdfs:label "acceptance testing" ;
                                               <http://www.w3.org/2004/02/skos/core#prefLabel> "acceptance testing"@en .


###  http://purl.org/stc/terms#accessibility_testing
<http://purl.org/stc/terms#accessibility_testing> rdf:type owl:NamedIndividual ;
                                                  <http://purl.org/stc/terms#hasParent> <http://purl.org/stc/terms#system_testing> ;
                                                  :isInISTQBGlossary "false"^^xsd:boolean ;
                                                  rdfs:label "accessibility testing" ;
                                                  <http://www.w3.org/2004/02/skos/core#prefLabel> "accessibility testing"@en .


###  http://purl.org/stc/terms#ad_hoc_testing
<http://purl.org/stc/terms#ad_hoc_testing> rdf:type owl:NamedIndividual ;
                                           <http://purl.org/stc/terms#hasParent> <http://purl.org/stc/terms#method_orientation_in_test_approach> ;
                                           :isInISTQBGlossary "true"^^xsd:boolean ;
                                           rdfs:comment "Informal testing performed without test analysis and test design."@en ;
                                           rdfs:label "ad hoc testing" ;
                                           rdfs:seeAlso "Specialist - Game Testing - v1.0.1" ;
                                           <http://www.w3.org/2004/02/skos/core#altLabel> """adhoc testing
ad hoc-testing"""@en ;
                                           <http://www.w3.org/2004/02/skos/core#prefLabel> "ad hoc testing"@en .


###  http://purl.org/stc/terms#adversarial_testing
<http://purl.org/stc/terms#adversarial_testing> rdf:type owl:NamedIndividual ;
                                                <http://purl.org/stc/terms#hasParent> <http://purl.org/stc/terms#AI_testing> ;
                                                :isInISTQBGlossary "true"^^xsd:boolean ;
                                                rdfs:label "adversarial testing" ;
                                                <http://www.w3.org/2004/02/skos/core#prefLabel> "adversarial testing"@en .


###  http://purl.org/stc/terms#agile_software_development
<http://purl.org/stc/terms#agile_software_development> rdf:type owl:NamedIndividual ;
                                                       <http://purl.org/stc/terms#hasParent> <http://purl.org/stc/terms#process_orientation_in_software_development> ;
                                                       :isInISTQBGlossary "true"^^xsd:boolean ;
                                                       rdfs:label "agile" ;
                                                       <http://www.w3.org/2004/02/skos/core#prefLabel> "agile software development"@en .


###  http://purl.org/stc/terms#agile_test_leader
<http://purl.org/stc/terms#agile_test_leader> rdf:type owl:NamedIndividual ;
                                              <http://purl.org/stc/terms#hasParent> <http://purl.org/stc/terms#test_leader> ;
                                              :isInISTQBGlossary "true"^^xsd:boolean ;
                                              rdfs:comment "A leadership role that serves agile teams, championing testing and quality at the organizational level. (ISTQB Glossary v4.5)"@en ;
                                              rdfs:label "agile test leader" ;
                                              rdfs:seeAlso """Agile Test Leadership at Scale - v1.0
Specialist - Agile Test Leadership at Scale - v2.0""" ;
                                              <http://www.w3.org/2004/02/skos/core#altLabel> """quality coach
agile test manager
quality leader"""@en ;
                                              <http://www.w3.org/2004/02/skos/core#prefLabel> "agile test leader"@en .


###  http://purl.org/stc/terms#agile_test_team_leader
<http://purl.org/stc/terms#agile_test_team_leader> rdf:type owl:NamedIndividual ;
                                                   <http://purl.org/stc/terms#hasParent> <http://purl.org/stc/terms#test_manager> ;
                                                   :isInISTQBGlossary "true"^^xsd:boolean ;
                                                   rdfs:comment "A role that is responsible for maintaining solution quality within an agile delivery team. (ISTQB Glossary v4.5)"@en ;
                                                   rdfs:label "agile test team leader" ;
                                                   rdfs:seeAlso """Agile Test Leadership at Scale - v1.0
Specialist - Agile Test Leadership at Scale - v2.0""" ;
                                                   <http://www.w3.org/2004/02/skos/core#prefLabel> "agile test team leader"@en .


###  http://purl.org/stc/terms#alpha_testing
<http://purl.org/stc/terms#alpha_testing> rdf:type owl:NamedIndividual ;
                                          <http://purl.org/stc/terms#hasParent> <http://purl.org/stc/terms#acceptance_testing> ;
                                          :isInISTQBGlossary "true"^^xsd:boolean ;
                                          rdfs:label "alpha testing" ;
                                          <http://www.w3.org/2004/02/skos/core#prefLabel> "alpha testing"@en .


###  http://purl.org/stc/terms#architectural_design
<http://purl.org/stc/terms#architectural_design> rdf:type owl:NamedIndividual ;
                                                 <http://purl.org/stc/terms#hasParent> <http://purl.org/stc/terms#software_engineering_activity> .


###  http://purl.org/stc/terms#automated_testing
<http://purl.org/stc/terms#automated_testing> rdf:type owl:NamedIndividual ;
                                              <http://purl.org/stc/terms#hasParent> <http://purl.org/stc/terms#test_execution> ;
                                              :isInISTQBGlossary "false"^^xsd:boolean ;
                                              rdfs:label "automated testing" ;
                                              <http://www.w3.org/2004/02/skos/core#prefLabel> "automated testing"@en .


###  http://purl.org/stc/terms#back-to-back_testing
<http://purl.org/stc/terms#back-to-back_testing> rdf:type owl:NamedIndividual ;
                                                 <http://purl.org/stc/terms#hasParent> <http://purl.org/stc/terms#oracle_orientation_in_test_approach> ;
                                                 :isInISTQBGlossary "true"^^xsd:boolean ;
                                                 rdfs:label "back-to-back testing" ;
                                                 <http://www.w3.org/2004/02/skos/core#altLabel> "back to back testing"@en ;
                                                 <http://www.w3.org/2004/02/skos/core#prefLabel> "back-to-back testing"@en .


###  http://purl.org/stc/terms#base_choice_coverage
<http://purl.org/stc/terms#base_choice_coverage> rdf:type owl:NamedIndividual ;
                                                 <http://purl.org/stc/terms#hasParent> <http://purl.org/stc/terms#specification_coverage> ;
                                                 :isInISTQBGlossary "true"^^xsd:boolean ;
                                                 rdfs:comment """The coverage of parameter-value combinations in which each value of a parameter is combined with the base values of all other parameters, for a chosen base value per parameter. (ISTQB Glossary v4.5)

Coverage for base choice testing. (ISO/IEC/IEEE 29119-4)"""@en ;
                                                 rdfs:label "base choice coverage" ;
                                                 rdfs:seeAlso "ISO/IEC/IEEE 29119-4 (Software and systems engineering — Software testing — Part 4: Test techniques)" ;
                                                 <http://www.w3.org/2004/02/skos/core#altLabel> "p-v pair coverage"@en ;
                                                 <http://www.w3.org/2004/02/skos/core#prefLabel> "base choice coverage"@en .


###  http://purl.org/stc/terms#basic_concepts
<http://purl.org/stc/terms#basic_concepts> rdf:type owl:NamedIndividual ;
                                           <http://purl.org/stc/terms#hasParent> <http://purl.org/stc/terms#software_engineering_concepts> ;
                                           :isInISTQBGlossary "false"^^xsd:boolean ;
                                           rdfs:label "basic concepts" ;
                                           <http://www.w3.org/2004/02/skos/core#prefLabel> "basic concepts"@en .


###  http://purl.org/stc/terms#behavior-driven_development
<http://purl.org/stc/terms#behavior-driven_development> rdf:type owl:NamedIndividual ;
                                                        <http://purl.org/stc/terms#hasParent> <http://purl.org/stc/terms#target_orientation_in_software_development> ;
                                                        :isInISTQBGlossary "true"^^xsd:boolean ;
                                                        rdfs:label "behavior-driven" ;
                                                        <http://www.w3.org/2004/02/skos/core#altLabel> """behavior driven development
bdd
BDD"""@en ;
                                                        <http://www.w3.org/2004/02/skos/core#prefLabel> "behavior-driven development"@en .


###  http://purl.org/stc/terms#beta_testing
<http://purl.org/stc/terms#beta_testing> rdf:type owl:NamedIndividual ;
                                         <http://purl.org/stc/terms#hasParent> <http://purl.org/stc/terms#acceptance_testing> ;
                                         :isInISTQBGlossary "true"^^xsd:boolean ;
                                         rdfs:label "beta testing" ;
                                         <http://www.w3.org/2004/02/skos/core#prefLabel> "beta testing"@en .


###  http://purl.org/stc/terms#black_box_test_technique
<http://purl.org/stc/terms#black_box_test_technique> rdf:type owl:NamedIndividual ;
                                                     <http://purl.org/stc/terms#hasParent> <http://purl.org/stc/terms#test_technique> ;
                                                     :isInISTQBGlossary "true"^^xsd:boolean ;
                                                     rdfs:comment "(ISTQB Glossary v4.5)"@en ;
                                                     rdfs:label "black box test technique" ;
                                                     <http://www.w3.org/2004/02/skos/core#altLabel> """specification-based testing
specification based testing
closed box testing
black-box test technique"""@en ;
                                                     <http://www.w3.org/2004/02/skos/core#prefLabel> "black box test technique"@en .


###  http://purl.org/stc/terms#boundary_value_analysis
<http://purl.org/stc/terms#boundary_value_analysis> rdf:type owl:NamedIndividual ;
                                                    <http://purl.org/stc/terms#hasParent> <http://purl.org/stc/terms#black_box_test_technique> ;
                                                    :isInISTQBGlossary "true"^^xsd:boolean ;
                                                    rdfs:label "boundary value analysis" ;
                                                    <http://www.w3.org/2004/02/skos/core#prefLabel> "boundary value analysis"@en .


###  http://purl.org/stc/terms#branch_coverage
<http://purl.org/stc/terms#branch_coverage> rdf:type owl:NamedIndividual ;
                                            <http://purl.org/stc/terms#hasParent> <http://purl.org/stc/terms#structural_coverage> ;
                                            :isInISTQBGlossary "true"^^xsd:boolean ;
                                            rdfs:comment "The coverage of branches in a control flow graph.  (ISTQB Glossary v4.5)"@en ;
                                            rdfs:label "branch coverage" ;
                                            rdfs:seeAlso "Foundation - v4.0" ;
                                            <http://www.w3.org/2004/02/skos/core#prefLabel> "branch coverage"@en .


###  http://purl.org/stc/terms#branch_testing
<http://purl.org/stc/terms#branch_testing> rdf:type owl:NamedIndividual ;
                                           <http://purl.org/stc/terms#hasParent> <http://purl.org/stc/terms#white_box_test_technique> ;
                                           :isInISTQBGlossary "true"^^xsd:boolean ;
                                           rdfs:label "branch testing" ;
                                           <http://www.w3.org/2004/02/skos/core#prefLabel> "branch testing"@en .


###  http://purl.org/stc/terms#change_orientation_in_test_approach
<http://purl.org/stc/terms#change_orientation_in_test_approach> rdf:type owl:NamedIndividual ;
                                                                <http://purl.org/stc/terms#hasParent> <http://purl.org/stc/terms#test_approach> ;
                                                                :isInISTQBGlossary "false"^^xsd:boolean ;
                                                                rdfs:label "change orientation" ;
                                                                <http://www.w3.org/2004/02/skos/core#prefLabel> "change orientation in test approach"@en .


###  http://purl.org/stc/terms#checklist_based_testing
<http://purl.org/stc/terms#checklist_based_testing> rdf:type owl:NamedIndividual ;
                                                    <http://purl.org/stc/terms#hasParent> <http://purl.org/stc/terms#experience-based_testing> ;
                                                    :isInISTQBGlossary "true"^^xsd:boolean ;
                                                    rdfs:label "checklist based testing" ;
                                                    <http://www.w3.org/2004/02/skos/core#prefLabel> "checklist based testing"@en .


###  http://purl.org/stc/terms#code
<http://purl.org/stc/terms#code> rdf:type owl:NamedIndividual ;
                                 <http://purl.org/stc/terms#hasParent> <http://purl.org/stc/terms#basic_concepts> .


###  http://purl.org/stc/terms#coding
<http://purl.org/stc/terms#coding> rdf:type owl:NamedIndividual ;
                                   <http://purl.org/stc/terms#hasParent> <http://purl.org/stc/terms#software_engineering_activity> .


###  http://purl.org/stc/terms#compliance_testing
<http://purl.org/stc/terms#compliance_testing> rdf:type owl:NamedIndividual ;
                                               <http://purl.org/stc/terms#hasParent> <http://purl.org/stc/terms#functional_testing> ;
                                               :isInISTQBGlossary "true"^^xsd:boolean ;
                                               rdfs:comment "The term conformance testing (defined by ISTQB to be a synonym for compliance testing) is used differently in telecommunication/protocol testing - see also protocol testing."@en ;
                                               rdfs:label "compliance testing" ;
                                               rdfs:seeAlso "Specialist - Gambling Industry Tester - 2018" ;
                                               <http://www.w3.org/2004/02/skos/core#altLabel> """conformance testing
regulation testing
standards testing""" ;
                                               <http://www.w3.org/2004/02/skos/core#prefLabel> "compliance testing"@en .


###  http://purl.org/stc/terms#component_integration_testing
<http://purl.org/stc/terms#component_integration_testing> rdf:type owl:NamedIndividual ;
                                                          <http://purl.org/stc/terms#hasParent> <http://purl.org/stc/terms#integration_testing> ;
                                                          :isInISTQBGlossary "true"^^xsd:boolean ;
                                                          rdfs:comment "The integration testing of components. (ISTQB Glossary v4.5)"@en ;
                                                          rdfs:label "component integration testing" ;
                                                          rdfs:seeAlso "Foundation - v4.0" ;
                                                          <http://www.w3.org/2004/02/skos/core#altLabel> """module integration testing
unit integration testing"""@en ;
                                                          <http://www.w3.org/2004/02/skos/core#prefLabel> "component integration testing"@en .


###  http://purl.org/stc/terms#component_testing
<http://purl.org/stc/terms#component_testing> rdf:type owl:NamedIndividual ;
                                              <http://purl.org/stc/terms#hasParent> <http://purl.org/stc/terms#test_level> ;
                                              :isInISTQBGlossary "true"^^xsd:boolean ;
                                              rdfs:label "component testing" ;
                                              <http://www.w3.org/2004/02/skos/core#prefLabel> "component testing"@en .


###  http://purl.org/stc/terms#condition_coverage
<http://purl.org/stc/terms#condition_coverage> rdf:type owl:NamedIndividual ;
                                               <http://purl.org/stc/terms#hasParent> <http://purl.org/stc/terms#structural_coverage> ;
                                               :isInISTQBGlossary "true"^^xsd:boolean ;
                                               rdfs:comment """The coverage of condition outcomes. (ISTQB Glossary v4.5)

Coverage for branch condition testing. (ISO/IEC/IEEE 29119-4)"""@en ;
                                               rdfs:label "condition coverage" ;
                                               rdfs:seeAlso "ISO/IEC/IEEE 29119-4 (Software and systems engineering — Software testing — Part 4: Test techniques)" ;
                                               <http://www.w3.org/2004/02/skos/core#altLabel> "branch condition coverage"@en ;
                                               <http://www.w3.org/2004/02/skos/core#prefLabel> "condition coverage"@en .


###  http://purl.org/stc/terms#configuration_management
<http://purl.org/stc/terms#configuration_management> rdf:type owl:NamedIndividual ;
                                                     <http://purl.org/stc/terms#hasParent> <http://purl.org/stc/terms#support_processes> .


###  http://purl.org/stc/terms#confirmation_testing
<http://purl.org/stc/terms#confirmation_testing> rdf:type owl:NamedIndividual ;
                                                 <http://purl.org/stc/terms#hasParent> <http://purl.org/stc/terms#defect_orientation_in_test_approach> ;
                                                 :isInISTQBGlossary "true"^^xsd:boolean ;
                                                 rdfs:comment """A type of change-related testing performed after fixing a defect to confirm that a failure caused by that defect does not reoccur. (ISTQB Glossary v4.5)

Testing performed to check that modifications made to correct a fault have successfully removed the fault. (ISO/IEC/IEEE 29119-1:2022)"""@en ;
                                                 rdfs:label "confirmation testing" ;
                                                 rdfs:seeAlso """ISO/IEC/IEEE 29119-1:2022 (Software and systems engineering — Software testing — Part 1: Concepts and definitions)

Foundation - v4.0
Specialist - Test Automation Engineer - 2016
Specialist - Test Automation Strategy - v1.0""" ;
                                                 <http://www.w3.org/2004/02/skos/core#altLabel> "retesting"@en ;
                                                 <http://www.w3.org/2004/02/skos/core#prefLabel> "confirmation testing"@en .


###  http://purl.org/stc/terms#conformance_testing
<http://purl.org/stc/terms#conformance_testing> rdf:type owl:NamedIndividual ;
                                                <http://purl.org/stc/terms#hasParent> <http://purl.org/stc/terms#protocol_or_service_testing> ;
                                                :isInISTQBGlossary "false"^^xsd:boolean ;
                                                rdfs:comment "The process of verifying that a system or component meets the requirements of a specified standard. (ISO/IEC 9646-1:1994)"@en ;
                                                rdfs:label "conformance testing" ;
                                                rdfs:seeAlso "ISO/IEC 9646-1:1994 (Information technology — Open Systems Interconnection — Conformance testing methodology and framework. Part 1: General concepts)" ;
                                                <http://www.w3.org/2004/02/skos/core#prefLabel> "conformance testing"@en .


###  http://purl.org/stc/terms#continuous_testing
<http://purl.org/stc/terms#continuous_testing> rdf:type owl:NamedIndividual ;
                                               <http://purl.org/stc/terms#hasParent> <http://purl.org/stc/terms#process_orientation_in_test_approach> ;
                                               :isInISTQBGlossary "true"^^xsd:boolean ;
                                               rdfs:label "continuous testing" ;
                                               <http://www.w3.org/2004/02/skos/core#prefLabel> "continuous testing"@en .


###  http://purl.org/stc/terms#contract_testing
<http://purl.org/stc/terms#contract_testing> rdf:type owl:NamedIndividual ;
                                             <http://purl.org/stc/terms#hasParent> <http://purl.org/stc/terms#target_orientation_in_test_approach> ;
                                             :isInISTQBGlossary "true"^^xsd:boolean ;
                                             rdfs:label "contract testing" ;
                                             <http://www.w3.org/2004/02/skos/core#prefLabel> "contract testing"@en .


###  http://purl.org/stc/terms#coverage
<http://purl.org/stc/terms#coverage> rdf:type owl:NamedIndividual ;
                                     <http://purl.org/stc/terms#hasParent> <http://purl.org/stc/terms#test_metric> ;
                                     :isInISTQBGlossary "true"^^xsd:boolean ;
                                     rdfs:comment "The degree to which specified coverage items are exercised by a test suite, expressed as a percentage. (ISTQB Glossary v4.5)"@en ;
                                     rdfs:label "coverage" ;
                                     <http://www.w3.org/2004/02/skos/core#altLabel> """coverage metric
test coverage
coverage-oriented metric"""@en ;
                                     <http://www.w3.org/2004/02/skos/core#prefLabel> "coverage"@en .


###  http://purl.org/stc/terms#coverage_item
<http://purl.org/stc/terms#coverage_item> rdf:type owl:NamedIndividual ;
                                          <http://purl.org/stc/terms#hasParent> <http://purl.org/stc/terms#Testware> ;
                                          :isInISTQBGlossary "true"^^xsd:boolean ;
                                          rdfs:comment """An attribute or combination of attributes derived from one or more test conditions by using a test technique. (ISTQB Glossary v4.5)

Measurable attribute of a test item that is the focus of testing (ISO/IEC/IEEE 29119-1:2022, defined as test (coverage) item)"""@en ;
                                          rdfs:label "coverage item" ;
                                          rdfs:seeAlso """ISO/IEC/IEEE 29119-1:2022 (Software and systems engineering — Software testing — Part 1: Concepts and definitions)

Foundation - v4.0
Specialist - Model-Based Testing - v1.1""" ;
                                          <http://www.w3.org/2004/02/skos/core#altLabel> "test coverage item"@en ;
                                          <http://www.w3.org/2004/02/skos/core#prefLabel> "coverage item"@en .


###  http://purl.org/stc/terms#crowd_testing
<http://purl.org/stc/terms#crowd_testing> rdf:type owl:NamedIndividual ;
                                          <http://purl.org/stc/terms#hasParent> <http://purl.org/stc/terms#tester_orientation_in_test_approach> ;
                                          :isInISTQBGlossary "true"^^xsd:boolean ;
                                          rdfs:label "crowd testing" ;
                                          <http://www.w3.org/2004/02/skos/core#prefLabel> "crowd testing"@en .


###  http://purl.org/stc/terms#data
<http://purl.org/stc/terms#data> rdf:type owl:NamedIndividual ;
                                 <http://purl.org/stc/terms#hasParent> <http://purl.org/stc/terms#basic_concepts> .


###  http://purl.org/stc/terms#decision_coverage
<http://purl.org/stc/terms#decision_coverage> rdf:type owl:NamedIndividual ;
                                              <http://purl.org/stc/terms#hasParent> <http://purl.org/stc/terms#structural_coverage> ;
                                              :isInISTQBGlossary "true"^^xsd:boolean ;
                                              rdfs:comment """The coverage of decision outcomes. (ISTQB Glossary v4.5)

Coverage for decision testing. (ISO/IEC/IEEE 29119-4)"""@en ;
                                              rdfs:label "decision coverage" ;
                                              rdfs:seeAlso "ISO/IEC/IEEE 29119-4 (Software and systems engineering — Software testing — Part 4: Test techniques)" ;
                                              <http://www.w3.org/2004/02/skos/core#prefLabel> "decision coverage"@en .


###  http://purl.org/stc/terms#decision_table_testing
<http://purl.org/stc/terms#decision_table_testing> rdf:type owl:NamedIndividual ;
                                                   <http://purl.org/stc/terms#hasParent> <http://purl.org/stc/terms#black_box_test_technique> ;
                                                   :isInISTQBGlossary "true"^^xsd:boolean ;
                                                   rdfs:label "decision table testing" ;
                                                   <http://www.w3.org/2004/02/skos/core#prefLabel> "decision table testing"@en .


###  http://purl.org/stc/terms#defect
<http://purl.org/stc/terms#defect> rdf:type owl:NamedIndividual ;
                                   <http://purl.org/stc/terms#hasParent> <http://purl.org/stc/terms#basic_concepts> .


###  http://purl.org/stc/terms#defect_orientation_in_test_approach
<http://purl.org/stc/terms#defect_orientation_in_test_approach> rdf:type owl:NamedIndividual ;
                                                                <http://purl.org/stc/terms#hasParent> <http://purl.org/stc/terms#change_orientation_in_test_approach> ;
                                                                :isInISTQBGlossary "false"^^xsd:boolean ;
                                                                rdfs:label "defect orientation" ;
                                                                <http://www.w3.org/2004/02/skos/core#prefLabel> "defect orientation in test approach"@en .


###  http://purl.org/stc/terms#defect_oriented_metric
<http://purl.org/stc/terms#defect_oriented_metric> rdf:type owl:NamedIndividual ;
                                                   <http://purl.org/stc/terms#hasParent> <http://purl.org/stc/terms#test_metric> ;
                                                   :isInISTQBGlossary "false"^^xsd:boolean ;
                                                   rdfs:label "defect oriented metric" ;
                                                   <http://www.w3.org/2004/02/skos/core#altLabel> """defect-oriented metric
defect metric"""@en ;
                                                   <http://www.w3.org/2004/02/skos/core#prefLabel> "defect oriented metric"@en .


###  http://purl.org/stc/terms#destructive_testing
<http://purl.org/stc/terms#destructive_testing> rdf:type owl:NamedIndividual ;
                                                <http://purl.org/stc/terms#hasParent> <http://purl.org/stc/terms#security_testing> ;
                                                :isInISTQBGlossary "true"^^xsd:boolean ;
                                                rdfs:label "destructive testing" ;
                                                <http://www.w3.org/2004/02/skos/core#prefLabel> "destructive testing"@en .


###  http://purl.org/stc/terms#detailed_design
<http://purl.org/stc/terms#detailed_design> rdf:type owl:NamedIndividual ;
                                            <http://purl.org/stc/terms#hasParent> <http://purl.org/stc/terms#software_engineering_activity> .


###  http://purl.org/stc/terms#development
<http://purl.org/stc/terms#development> rdf:type owl:NamedIndividual ;
                                        <http://purl.org/stc/terms#hasParent> <http://purl.org/stc/terms#software_lifecycle> .


###  http://purl.org/stc/terms#device-based_testing
<http://purl.org/stc/terms#device-based_testing> rdf:type owl:NamedIndividual ;
                                                 <http://purl.org/stc/terms#hasParent> <http://purl.org/stc/terms#mobile_app_testing> ;
                                                 :isInISTQBGlossary "true"^^xsd:boolean ;
                                                 rdfs:label "device-based testing" ;
                                                 <http://www.w3.org/2004/02/skos/core#prefLabel> "device-based testing"@en .


###  http://purl.org/stc/terms#domain-specific_test_types
<http://purl.org/stc/terms#domain-specific_test_types> rdf:type owl:NamedIndividual ;
                                                       <http://purl.org/stc/terms#hasParent> <http://purl.org/stc/terms#test_type> ;
                                                       :isInISTQBGlossary "false"^^xsd:boolean ;
                                                       rdfs:label "domain-specific test types" ;
                                                       <http://www.w3.org/2004/02/skos/core#prefLabel> "domain-specific test types"@en .


###  http://purl.org/stc/terms#dynamic_application_security_testing
<http://purl.org/stc/terms#dynamic_application_security_testing> rdf:type owl:NamedIndividual ;
                                                                 <http://purl.org/stc/terms#hasParent> <http://purl.org/stc/terms#security_testing> ;
                                                                 :isInISTQBGlossary "true"^^xsd:boolean ;
                                                                 rdfs:label "dynamic application security testing" ;
                                                                 <http://www.w3.org/2004/02/skos/core#prefLabel> "dynamic application security testing"@en .


###  http://purl.org/stc/terms#dynamic_testing
<http://purl.org/stc/terms#dynamic_testing> rdf:type owl:NamedIndividual ;
                                            <http://purl.org/stc/terms#hasParent> <http://purl.org/stc/terms#testing> ;
                                            :isInISTQBGlossary "true"^^xsd:boolean ;
                                            rdfs:comment """Testing that involves the execution of the test item. (ISTQB Glossary v4.5)

Testing in which a test item is evaluated by executing it. (ISO/IEC/IEEE 29119-1)"""@en ;
                                            rdfs:label "dynamic testing" ;
                                            rdfs:seeAlso """ISO/IEC/IEEE 29119-1:2022 (Software and systems engineering — Software testing — Part 1: Concepts and definitions)

Foundation - v4.0""" ;
                                            <http://www.w3.org/2004/02/skos/core#prefLabel> "dynamic testing"@en .


###  http://purl.org/stc/terms#each_choice_coverage
<http://purl.org/stc/terms#each_choice_coverage> rdf:type owl:NamedIndividual ;
                                                 <http://purl.org/stc/terms#hasParent> <http://purl.org/stc/terms#specification_coverage> ;
                                                 :isInISTQBGlossary "true"^^xsd:boolean ;
                                                 rdfs:comment """The coverage of equivalence partitions in multiple sets of partitions. (ISTQB Glossary v4.5)

Coverage for each choice testing. (ISO/IEC/IEEE 29119-4:2015)"""@en ;
                                                 rdfs:label "each choice coverage" ;
                                                 rdfs:seeAlso "ISO/IEC/IEEE 29119-4 (Software and systems engineering — Software testing — Part 4: Test techniques)" ;
                                                 <http://www.w3.org/2004/02/skos/core#altLabel> """ecc
ECC"""@en ;
                                                 <http://www.w3.org/2004/02/skos/core#prefLabel> "each choice coverage"@en .


###  http://purl.org/stc/terms#end-to-end_testing
<http://purl.org/stc/terms#end-to-end_testing> rdf:type owl:NamedIndividual ;
                                               <http://purl.org/stc/terms#hasParent> <http://purl.org/stc/terms#system_testing> ;
                                               :isInISTQBGlossary "true"^^xsd:boolean ;
                                               rdfs:label "end-to-end testing" ;
                                               <http://www.w3.org/2004/02/skos/core#altLabel> """e2e testing
E2E testing"""@en ;
                                               <http://www.w3.org/2004/02/skos/core#prefLabel> "end-to-end testing"@en .


###  http://purl.org/stc/terms#entry_criteria
<http://purl.org/stc/terms#entry_criteria> rdf:type owl:NamedIndividual ;
                                           <http://purl.org/stc/terms#hasParent> <http://purl.org/stc/terms#Testware> ;
                                           :isInISTQBGlossary "true"^^xsd:boolean ;
                                           rdfs:comment "The set of conditions for officially completing a defined task. (ISTQB Glossary v4.5)"@en ;
                                           rdfs:label "entry criteria" ;
                                           rdfs:seeAlso "Foundation - v4.0" ;
                                           <http://www.w3.org/2004/02/skos/core#altLabel> """test completion criteria
completion criteria"""@en ;
                                           <http://www.w3.org/2004/02/skos/core#prefLabel> "entry criteria"@en .


###  http://purl.org/stc/terms#equivalence_partitioning
<http://purl.org/stc/terms#equivalence_partitioning> rdf:type owl:NamedIndividual ;
                                                     <http://purl.org/stc/terms#hasParent> <http://purl.org/stc/terms#black_box_test_technique> ;
                                                     :isInISTQBGlossary "true"^^xsd:boolean ;
                                                     rdfs:label "equivalence partitioning" ;
                                                     <http://www.w3.org/2004/02/skos/core#prefLabel> "equivalence partitioning"@en .


###  http://purl.org/stc/terms#error
<http://purl.org/stc/terms#error> rdf:type owl:NamedIndividual ;
                                  <http://purl.org/stc/terms#hasParent> <http://purl.org/stc/terms#basic_concepts> .


###  http://purl.org/stc/terms#error_guessing
<http://purl.org/stc/terms#error_guessing> rdf:type owl:NamedIndividual ;
                                           <http://purl.org/stc/terms#hasParent> <http://purl.org/stc/terms#experience-based_testing> ;
                                           :isInISTQBGlossary "true"^^xsd:boolean ;
                                           rdfs:label "error guessing" ;
                                           <http://www.w3.org/2004/02/skos/core#prefLabel> "error guessing"@en .


###  http://purl.org/stc/terms#exhaustive_testing
<http://purl.org/stc/terms#exhaustive_testing> rdf:type owl:NamedIndividual ;
                                               <http://purl.org/stc/terms#hasParent> <http://purl.org/stc/terms#method_orientation_in_test_approach> ;
                                               :isInISTQBGlossary "true"^^xsd:boolean ;
                                               rdfs:comment "A test approach in which the test suite comprises all combinations of input values and preconditions."@en ;
                                               rdfs:label "exhaustive testing" ;
                                               <http://www.w3.org/2004/02/skos/core#altLabel> "complete testing"@en ;
                                               <http://www.w3.org/2004/02/skos/core#prefLabel> "exhaustive testing"@en .


###  http://purl.org/stc/terms#exit_criteria
<http://purl.org/stc/terms#exit_criteria> rdf:type owl:NamedIndividual ;
                                          <http://purl.org/stc/terms#hasParent> <http://purl.org/stc/terms#Testware> ;
                                          :isInISTQBGlossary "true"^^xsd:boolean ;
                                          rdfs:comment "The set of conditions for officially starting a defined task. (ISTQB Glossary v4-5)"@en ;
                                          rdfs:label "exit criteria" ;
                                          rdfs:seeAlso """Foundation - v4.0
Advanced Test Manager - 2012
Advanced Test Analyst - v3.1""" ;
                                          <http://www.w3.org/2004/02/skos/core#altLabel> """test completion criteria
completion criteria""" ;
                                          <http://www.w3.org/2004/02/skos/core#prefLabel> "exit criteria"@en .


###  http://purl.org/stc/terms#experience-based_testing
<http://purl.org/stc/terms#experience-based_testing> rdf:type owl:NamedIndividual ;
                                                     <http://purl.org/stc/terms#hasParent> <http://purl.org/stc/terms#test_technique> ;
                                                     :isInISTQBGlossary "true"^^xsd:boolean ;
                                                     rdfs:label "experience-based testing" ;
                                                     <http://www.w3.org/2004/02/skos/core#altLabel> """experience based testing
experience-based test technique
experience based test technique"""@en ;
                                                     <http://www.w3.org/2004/02/skos/core#prefLabel> "experience-based testing"@en .


###  http://purl.org/stc/terms#experience_based_test_metric
<http://purl.org/stc/terms#experience_based_test_metric> rdf:type owl:NamedIndividual ;
                                                         <http://purl.org/stc/terms#hasParent> <http://purl.org/stc/terms#coverage> ;
                                                         :isInISTQBGlossary "false"^^xsd:boolean ;
                                                         rdfs:comment "There is currently no industry agreed approach to calculating experience-based coverage. (ISO/IEC/IEEE 29119-4)"@en ;
                                                         rdfs:label "experience coverage" ;
                                                         rdfs:seeAlso "ISO/IEC/IEEE 29119-4 (Software and systems engineering — Software testing — Part 4: Test techniques)" ;
                                                         <http://www.w3.org/2004/02/skos/core#altLabel> "experience based test metric"@en ,
                                                                                                        """experience based test metric
experience-based test metric"""@en ;
                                                         <http://www.w3.org/2004/02/skos/core#prefLabel> "experience coverage"@en .


###  http://purl.org/stc/terms#exploratory_testing
<http://purl.org/stc/terms#exploratory_testing> rdf:type owl:NamedIndividual ;
                                                <http://purl.org/stc/terms#hasParent> <http://purl.org/stc/terms#method_orientation_in_test_approach> ;
                                                :isInISTQBGlossary "true"^^xsd:boolean ;
                                                rdfs:comment "An approach to testing in which the testers dynamically design and execute tests based on their knowledge, exploration of the test item and the results of previous tests. (ISTQB Glossary v4.5)"@en ;
                                                rdfs:label "exploratory testing" ;
                                                rdfs:seeAlso """ISO/IEC/IEEE 29119-1:2022 (Software and systems engineering — Software testing — Part 1: Concepts and definitions)

Foundation - v4.0
Advanced Test Analyst - v3.1""" ;
                                                <http://www.w3.org/2004/02/skos/core#prefLabel> "exploratory testing"@en .


###  http://purl.org/stc/terms#failure
<http://purl.org/stc/terms#failure> rdf:type owl:NamedIndividual ;
                                    <http://purl.org/stc/terms#hasParent> <http://purl.org/stc/terms#basic_concepts> .


###  http://purl.org/stc/terms#feature-driven_development
<http://purl.org/stc/terms#feature-driven_development> rdf:type owl:NamedIndividual ;
                                                       <http://purl.org/stc/terms#hasParent> <http://purl.org/stc/terms#target_orientation_in_software_development> ;
                                                       :isInISTQBGlossary "true"^^xsd:boolean ;
                                                       rdfs:label "feature-driven development" ;
                                                       <http://www.w3.org/2004/02/skos/core#prefLabel> "feature-driven development"@en .


###  http://purl.org/stc/terms#formal_review
<http://purl.org/stc/terms#formal_review> rdf:type owl:NamedIndividual ;
                                          <http://purl.org/stc/terms#hasParent> <http://purl.org/stc/terms#review> ;
                                          rdfs:label "formal review" ;
                                          <http://www.w3.org/2004/02/skos/core#prefLabel> "formal review"@en .


###  http://purl.org/stc/terms#functional_testing
<http://purl.org/stc/terms#functional_testing> rdf:type owl:NamedIndividual ;
                                               <http://purl.org/stc/terms#hasParent> <http://purl.org/stc/terms#test_type> ;
                                               :isInISTQBGlossary "true"^^xsd:boolean ;
                                               rdfs:comment "Testing performed to evaluate if a component or system satisfies functional requirements. (ISTQB Glossary v4.5)"@en ;
                                               rdfs:label "functional testing" ;
                                               rdfs:seeAlso """Foundation - v4.0
Advanced Test Management - v3.0
Advanced Test Analyst - v4.0
Specialist - Game Testing - v1.0.1""" ;
                                               <http://www.w3.org/2004/02/skos/core#prefLabel> "functional testing"@en .


###  http://purl.org/stc/terms#fundamental_test_process
<http://purl.org/stc/terms#fundamental_test_process> rdf:type owl:NamedIndividual ;
                                                     <http://purl.org/stc/terms#hasParent> <http://purl.org/stc/terms#test_process> ;
                                                     :isInISTQBGlossary "false"^^xsd:boolean ;
                                                     rdfs:label "fundamental test process" ;
                                                     <http://www.w3.org/2004/02/skos/core#prefLabel> "fundamental test process"@en .


###  http://purl.org/stc/terms#gambling_testing
<http://purl.org/stc/terms#gambling_testing> rdf:type owl:NamedIndividual ;
                                             <http://purl.org/stc/terms#hasParent> <http://purl.org/stc/terms#domain-specific_test_types> ;
                                             :isInISTQBGlossary "false"^^xsd:boolean ;
                                             rdfs:label "gambling testing" ;
                                             <http://www.w3.org/2004/02/skos/core#prefLabel> "gambling testing"@en .


###  http://purl.org/stc/terms#grey_box_test_technique
<http://purl.org/stc/terms#grey_box_test_technique> rdf:type owl:NamedIndividual ;
                                                    <http://purl.org/stc/terms#hasParent> <http://purl.org/stc/terms#test_technique> ;
                                                    :isInISTQBGlossary "true"^^xsd:boolean ;
                                                    rdfs:label "grey-box testing" ;
                                                    <http://www.w3.org/2004/02/skos/core#altLabel> """grey box testing
gray-box testing
gray box testing"""@en ;
                                                    <http://www.w3.org/2004/02/skos/core#prefLabel> "grey-box testing"@en .


###  http://purl.org/stc/terms#high_level_test_case
<http://purl.org/stc/terms#high_level_test_case> rdf:type owl:NamedIndividual ;
                                                 <http://purl.org/stc/terms#hasParent> <http://purl.org/stc/terms#test_case> ;
                                                 :isInISTQBGlossary "true"^^xsd:boolean ;
                                                 rdfs:comment "A test case with abstract preconditions, input data, expected results, postconditions, and actions (where applicable). (ISTQB Glossary v4.5)"@en ;
                                                 rdfs:label "high-level test case" ;
                                                 rdfs:seeAlso """Advanced Test Manager - 2012
Advanced Test Analyst - v3.1
Advanced Test Analyst - v4.0""" ;
                                                 <http://www.w3.org/2004/02/skos/core#altLabel> """high level test case
logical test case
abstract test case
high level testcase
logical testcase
abstract testcase""" ;
                                                 <http://www.w3.org/2004/02/skos/core#prefLabel> "high-level test case"@en .


###  http://purl.org/stc/terms#incremental_software_development
<http://purl.org/stc/terms#incremental_software_development> rdf:type owl:NamedIndividual ;
                                                             <http://purl.org/stc/terms#hasParent> <http://purl.org/stc/terms#process_orientation_in_software_development> ;
                                                             :isInISTQBGlossary "false"^^xsd:boolean ;
                                                             rdfs:label "incremental" ;
                                                             <http://www.w3.org/2004/02/skos/core#prefLabel> "incremental software development"@en .


###  http://purl.org/stc/terms#informal_review
<http://purl.org/stc/terms#informal_review> rdf:type owl:NamedIndividual ;
                                            <http://purl.org/stc/terms#hasParent> <http://purl.org/stc/terms#review> ;
                                            rdfs:label "informal review" ;
                                            <http://www.w3.org/2004/02/skos/core#prefLabel> "informal review"@en .


###  http://purl.org/stc/terms#inspection
<http://purl.org/stc/terms#inspection> rdf:type owl:NamedIndividual ;
                                       <http://purl.org/stc/terms#hasParent> <http://purl.org/stc/terms#formal_review> ;
                                       :isInISTQBGlossary "true"^^xsd:boolean ;
                                       rdfs:comment "A type of formal review that uses defined team roles and measurement to identify defects in a work product, and improve the review process and the software development process. (ISTQB Glossary v4.5)"@en ;
                                       rdfs:label "inspection" ;
                                       rdfs:seeAlso """Foundation - v4.0
Advanced Test Manager - 2012""" ;
                                       <http://www.w3.org/2004/02/skos/core#prefLabel> "inspection"@en .


###  http://purl.org/stc/terms#integration
<http://purl.org/stc/terms#integration> rdf:type owl:NamedIndividual ;
                                        <http://purl.org/stc/terms#hasParent> <http://purl.org/stc/terms#software_engineering_activity> .


###  http://purl.org/stc/terms#integration_testing
<http://purl.org/stc/terms#integration_testing> rdf:type owl:NamedIndividual ;
                                                <http://purl.org/stc/terms#hasParent> <http://purl.org/stc/terms#test_level> ;
                                                :isInISTQBGlossary "true"^^xsd:boolean ;
                                                rdfs:label "integration testing" ;
                                                <http://www.w3.org/2004/02/skos/core#prefLabel> "integration testing"@en .


###  http://purl.org/stc/terms#interactive_application_security_testing
<http://purl.org/stc/terms#interactive_application_security_testing> rdf:type owl:NamedIndividual ;
                                                                     <http://purl.org/stc/terms#hasParent> <http://purl.org/stc/terms#security_testing> ;
                                                                     :isInISTQBGlossary "true"^^xsd:boolean ;
                                                                     rdfs:label "interactive application security testing" ;
                                                                     <http://www.w3.org/2004/02/skos/core#prefLabel> "interactive application security testing"@en .


###  http://purl.org/stc/terms#interface_testing
<http://purl.org/stc/terms#interface_testing> rdf:type owl:NamedIndividual ;
                                              <http://purl.org/stc/terms#hasParent> <http://purl.org/stc/terms#target_orientation_in_test_approach> ;
                                              :isInISTQBGlossary "true"^^xsd:boolean ;
                                              rdfs:label "interface testing" ;
                                              <http://www.w3.org/2004/02/skos/core#prefLabel> "interface testing"@en .


###  http://purl.org/stc/terms#interoperability_testing
<http://purl.org/stc/terms#interoperability_testing> rdf:type owl:NamedIndividual ;
                                                     <http://purl.org/stc/terms#hasParent> <http://purl.org/stc/terms#protocol_or_service_testing> ;
                                                     :isInISTQBGlossary "false"^^xsd:boolean ;
                                                     rdfs:comment "Testing conducted to ensure that a modified system retains the capability of exchanging information with systems of different types, and of using that information (ISO/IEC/IEEE 24765:2017)"@en ;
                                                     rdfs:label "interoperability testing" ;
                                                     rdfs:seeAlso """ISO/IEC/IEEE 24765:2017 (Systems and software engineering —
Vocabulary)""" ;
                                                     <http://www.w3.org/2004/02/skos/core#prefLabel> "interoperability testing"@en .


###  http://purl.org/stc/terms#iterative_software_development
<http://purl.org/stc/terms#iterative_software_development> rdf:type owl:NamedIndividual ;
                                                           <http://purl.org/stc/terms#hasParent> <http://purl.org/stc/terms#process_orientation_in_software_development> ;
                                                           :isInISTQBGlossary "true"^^xsd:boolean ;
                                                           rdfs:label "iterative" ;
                                                           <http://www.w3.org/2004/02/skos/core#prefLabel> "iterative software development"@en .


###  http://purl.org/stc/terms#level_test_plan
<http://purl.org/stc/terms#level_test_plan> rdf:type owl:NamedIndividual ;
                                            <http://purl.org/stc/terms#hasParent> <http://purl.org/stc/terms#test_plan> ;
                                            :isInISTQBGlossary "true"^^xsd:boolean ;
                                            rdfs:comment "A test plan that typically addresses one test level. (ISTQB Glossary v4.5)"@en ;
                                            rdfs:label "level test plan" ;
                                            rdfs:seeAlso "Advanced Test Manager - 2012" ;
                                            <http://www.w3.org/2004/02/skos/core#altLabel> "level testplan"@en ;
                                            <http://www.w3.org/2004/02/skos/core#prefLabel> "level test plan"@en .


###  http://purl.org/stc/terms#load_testing
<http://purl.org/stc/terms#load_testing> rdf:type owl:NamedIndividual ;
                                         <http://purl.org/stc/terms#hasParent> <http://purl.org/stc/terms#performance_testing> ;
                                         :isInISTQBGlossary "true"^^xsd:boolean ;
                                         rdfs:label "load testing" ;
                                         <http://www.w3.org/2004/02/skos/core#prefLabel> "load testing"@en .


###  http://purl.org/stc/terms#low_level_test_case
<http://purl.org/stc/terms#low_level_test_case> rdf:type owl:NamedIndividual ;
                                                <http://purl.org/stc/terms#hasParent> <http://purl.org/stc/terms#test_case> ;
                                                :isInISTQBGlossary "true"^^xsd:boolean ;
                                                rdfs:comment "A test case with concrete values for preconditions, input data, expected results, postconditions, and a detailed description of actions (where applicable). (ISTQB Glossary v4.5)"@en ;
                                                rdfs:label "low-level test case" ;
                                                rdfs:seeAlso """Advanced Test Analyst - v3.1
Advanced Test Analyst - v4.0""" ;
                                                <http://www.w3.org/2004/02/skos/core#altLabel> """low level test case
concrete test case
physical test case
low level testcase
concrete testcase
physical testcase"""@en ;
                                                <http://www.w3.org/2004/02/skos/core#prefLabel> "low-level test case"@en .


###  http://purl.org/stc/terms#maintenance
<http://purl.org/stc/terms#maintenance> rdf:type owl:NamedIndividual ;
                                        <http://purl.org/stc/terms#hasParent> <http://purl.org/stc/terms#software_lifecycle> .


###  http://purl.org/stc/terms#maintenance_testing
<http://purl.org/stc/terms#maintenance_testing> rdf:type owl:NamedIndividual ;
                                                <http://purl.org/stc/terms#hasParent> <http://purl.org/stc/terms#change_orientation_in_test_approach> ;
                                                :isInISTQBGlossary "true"^^xsd:boolean ;
                                                rdfs:comment "Testing the changes to an operational system or the impact of a changed environment to an operational system. (ISTQB Glossary v4.5)"@en ;
                                                rdfs:label "maintenance testing" ;
                                                rdfs:seeAlso "Foundation - v4.0" ;
                                                <http://www.w3.org/2004/02/skos/core#prefLabel> "maintenance testing"@en .


###  http://purl.org/stc/terms#manual_testing
<http://purl.org/stc/terms#manual_testing> rdf:type owl:NamedIndividual ;
                                           <http://purl.org/stc/terms#hasParent> <http://purl.org/stc/terms#test_execution> ;
                                           :isInISTQBGlossary "false"^^xsd:boolean ;
                                           rdfs:comment "Humans performing tests by entering information into a test item and verifying the results. (ISO/IEC/IEEE 29119-1:2022)"@en ,
                                                        "ISO/IEC/IEEE 29119-1:2022 (Software and systems engineering — Software testing — Part 1: Concepts and definitions)"@en ;
                                           rdfs:label "manual testing" ;
                                           <http://www.w3.org/2004/02/skos/core#altLabel> "unscripted testing" ;
                                           <http://www.w3.org/2004/02/skos/core#prefLabel> "manual testing"@en .


###  http://purl.org/stc/terms#master_test_plan
<http://purl.org/stc/terms#master_test_plan> rdf:type owl:NamedIndividual ;
                                             <http://purl.org/stc/terms#hasParent> <http://purl.org/stc/terms#test_plan> ;
                                             :isInISTQBGlossary "true"^^xsd:boolean ;
                                             rdfs:comment "A test plan that is used to coordinate multiple test levels or test types. (ISTQB Glossary v4.5)"@en ;
                                             rdfs:label "master test plan" ;
                                             rdfs:seeAlso "Advanced Test Manager - 2012" ;
                                             <http://www.w3.org/2004/02/skos/core#altLabel> "master testplan"@en ;
                                             <http://www.w3.org/2004/02/skos/core#prefLabel> "master test plan"@en .


###  http://purl.org/stc/terms#math_testing
<http://purl.org/stc/terms#math_testing> rdf:type owl:NamedIndividual ;
                                         <http://purl.org/stc/terms#hasParent> <http://purl.org/stc/terms#gambling_testing> ;
                                         :isInISTQBGlossary "true"^^xsd:boolean ;
                                         rdfs:label "math testing" ;
                                         <http://www.w3.org/2004/02/skos/core#prefLabel> "math testing"@en .


###  http://purl.org/stc/terms#method_orientation_in_test_approach
<http://purl.org/stc/terms#method_orientation_in_test_approach> rdf:type owl:NamedIndividual ;
                                                                <http://purl.org/stc/terms#hasParent> <http://purl.org/stc/terms#test_approach> ;
                                                                :isInISTQBGlossary "false"^^xsd:boolean ;
                                                                rdfs:label "method orientation" ;
                                                                <http://www.w3.org/2004/02/skos/core#prefLabel> "method orientation in test approach"@en .


###  http://purl.org/stc/terms#metric
<http://purl.org/stc/terms#metric> rdf:type owl:NamedIndividual ;
                                   <http://purl.org/stc/terms#hasParent> <http://purl.org/stc/terms#basic_concepts> ;
                                   :isInISTQBGlossary "true"^^xsd:boolean ;
                                   rdfs:comment """A measurement scale and the method used for measurement. (ISTQB Glossary v4.5) 

A quantitative measure of the degree to which a system, component, or process possesses a given attribute. (ISO/IEC/IEEE 24765:2017)"""@en ;
                                   rdfs:label "metric" ;
                                   rdfs:seeAlso """ISO/IEC/IEEE 24765:2017 (Systems and Software Engineering – Vocabulary)

Foundation - v4.0
Advanced Test Manager - 2012
Advanced Test Management - v3.0
Advanced Test Analyst - v3.1
Advanced Test Analyst - v4.0
Advanced Technical Test Analyst - v4.0
Advanced Test Automation Engineering - v2.0
Expert Improving the Test Process - 2011
Expert Test Management - 2011
Foundation Agile Tester - 2014
Advanced Agile Technical Tester - 2019
Agile Test Leadership at Scale - v1.0
Specialist - Acceptance Testing - 2019
Specialist - Agile Test Leadership at Scale - v2.0
Specialist - AI Testing - v1.0
Specialist - Automotive Software Tester - 2018
Specialist - Automotive Software Tester - v1.1
Specialist - Gambling Industry Tester - 2018
Specialist - Game Testing - v1.0.1
Specialist - Model-Based Tester - 2015
Specialist - Model-Based Testing - v1.1
Specialist - Performance Testing - 2018
Specialist - Security Tester - 2016
Specialist - Security Test Engineer - v1.0
Specialist - Test Automation Engineer - 2016
Specialist - Test Automation Strategy - v1.0""" ;
                                   <http://www.w3.org/2004/02/skos/core#prefLabel> "metric"@en .


###  http://purl.org/stc/terms#mobile_app_testing
<http://purl.org/stc/terms#mobile_app_testing> rdf:type owl:NamedIndividual ;
                                               <http://purl.org/stc/terms#hasParent> <http://purl.org/stc/terms#domain-specific_test_types> ;
                                               :isInISTQBGlossary "false"^^xsd:boolean ;
                                               rdfs:label "mobile app testing" ;
                                               <http://www.w3.org/2004/02/skos/core#altLabel> "mobile application testing"@en ;
                                               <http://www.w3.org/2004/02/skos/core#prefLabel> "mobile app testing"@en .


###  http://purl.org/stc/terms#model
<http://purl.org/stc/terms#model> rdf:type owl:NamedIndividual ;
                                  <http://purl.org/stc/terms#hasParent> <http://purl.org/stc/terms#basic_concepts> .


###  http://purl.org/stc/terms#model_based_testing
<http://purl.org/stc/terms#model_based_testing> rdf:type owl:NamedIndividual ;
                                                <http://purl.org/stc/terms#hasParent> <http://purl.org/stc/terms#black_box_test_technique> ;
                                                :isInISTQBGlossary "true"^^xsd:boolean ;
                                                rdfs:comment "Testing based on or involving models. (ISTQB Glossary v4.5)"@en ;
                                                rdfs:label "model-based testing" ;
                                                rdfs:seeAlso """Advanced Test Analyst - v4.0
Advanced Technical Test Analyst - v4.0
Advanced Test Automation Engineering - v2.0
Specialist - Acceptance Testing - 2019
Specialist - Model-Based Tester - 2015
Specialist - Model-Based Testing - v1.1
Specialist - Test Automation Engineer - 2016""" ;
                                                <http://www.w3.org/2004/02/skos/core#altLabel> """model based testing
mbt
MBT
model driven testing
model-driven testing
mdt
MDT"""@en ;
                                                <http://www.w3.org/2004/02/skos/core#prefLabel> "model-based testing"@en .


###  http://purl.org/stc/terms#model_coverage
<http://purl.org/stc/terms#model_coverage> rdf:type owl:NamedIndividual ;
                                           <http://purl.org/stc/terms#hasParent> <http://purl.org/stc/terms#specification_coverage> ;
                                           :isInISTQBGlossary "true"^^xsd:boolean ;
                                           rdfs:comment "The coverage of model elements. (ISTQB Glossary v4.5)"@en ;
                                           rdfs:label "model coverage" ;
                                           rdfs:seeAlso "Specialist - Model-Based Testing - v1.1" ;
                                           <http://www.w3.org/2004/02/skos/core#prefLabel> "model coverage"@en .


###  http://purl.org/stc/terms#model_verification
<http://purl.org/stc/terms#model_verification> rdf:type owl:NamedIndividual ;
                                               <http://purl.org/stc/terms#hasParent> <http://purl.org/stc/terms#static_testing> ;
                                               :isInISTQBGlossary "false"^^xsd:boolean ;
                                               rdfs:comment "The process of determining that a model accurately represents the required conceptual description and specifications. (own)"@en ;
                                               rdfs:label "model verification" ;
                                               <http://www.w3.org/2004/02/skos/core#prefLabel> "model verification"@en .


###  http://purl.org/stc/terms#modified_condition_decision_coverage
<http://purl.org/stc/terms#modified_condition_decision_coverage> rdf:type owl:NamedIndividual ;
                                                                 <http://purl.org/stc/terms#hasParent> <http://purl.org/stc/terms#structural_coverage> ;
                                                                 :isInISTQBGlossary "true"^^xsd:boolean ;
                                                                 rdfs:comment """The coverage of all outcomes of the atomic conditions that independently affect the overall decision outcome. (ISTQB Glossary v4.5)

Coverage for modified condition/decision coverage testing. (ISO/IEC/IEEE 29119-4)"""@en ;
                                                                 rdfs:label "modified condition/decision coverage" ;
                                                                 rdfs:seeAlso "ISO/IEC/IEEE 29119-4 (Software and systems engineering — Software testing — Part 4: Test techniques)" ;
                                                                 <http://www.w3.org/2004/02/skos/core#altLabel> """mc/dc
MC/DC
condition determination coverage
modified multiple condition coverage"""@en ;
                                                                 <http://www.w3.org/2004/02/skos/core#prefLabel> "modified condition/decision coverage"@en .


###  http://purl.org/stc/terms#multiple_condition_coverage
<http://purl.org/stc/terms#multiple_condition_coverage> rdf:type owl:NamedIndividual ;
                                                        <http://purl.org/stc/terms#hasParent> <http://purl.org/stc/terms#structural_coverage> ;
                                                        :isInISTQBGlossary "true"^^xsd:boolean ;
                                                        rdfs:comment """The coverage of all possible combinations of all single condition outcomes within one statement. (ISTQB Glossary v4.5)

Coverage for branch condition combination testing. (ISO/IEC/IEEE 29119-4 as branch condition combination coverage)"""@en ;
                                                        rdfs:label "multiple condition coverage" ;
                                                        rdfs:seeAlso "ISO/IEC/IEEE 29119-4 (Software and systems engineering — Software testing — Part 4: Test techniques)" ;
                                                        <http://www.w3.org/2004/02/skos/core#altLabel> """branch condition combination coverage
condition combination coverage""" ;
                                                        <http://www.w3.org/2004/02/skos/core#prefLabel> "multiple condition coverage"@en .


###  http://purl.org/stc/terms#neuron_coverage
<http://purl.org/stc/terms#neuron_coverage> rdf:type owl:NamedIndividual ;
                                            <http://purl.org/stc/terms#hasParent> <http://purl.org/stc/terms#LLM_structural_coverage> ;
                                            :isInISTQBGlossary "true"^^xsd:boolean ;
                                            rdfs:comment "The coverage of activated neurons in the neural network for a set of tests. (ISTQB Glossary v4.5)"@en ;
                                            rdfs:label "neuron coverage" ;
                                            rdfs:seeAlso "Specialist - AI Testing - v1.0" ;
                                            <http://www.w3.org/2004/02/skos/core#prefLabel> "neuron coverage"@en .


###  http://purl.org/stc/terms#non-functional_testing
<http://purl.org/stc/terms#non-functional_testing> rdf:type owl:NamedIndividual ;
                                                   <http://purl.org/stc/terms#hasParent> <http://purl.org/stc/terms#test_type> ;
                                                   :isInISTQBGlossary "true"^^xsd:boolean ;
                                                   rdfs:comment "Testing performed to evaluate that a component or system complies with non-functional requirements. (ISTQB Glossary v4.5)"@en ;
                                                   rdfs:label "non-functional testing" ;
                                                   rdfs:seeAlso """Foundation - v4.0
Advanced Test Management - v3.0""" ;
                                                   <http://www.w3.org/2004/02/skos/core#altLabel> "extra-functional testing"@en ;
                                                   <http://www.w3.org/2004/02/skos/core#prefLabel> "non-functional testing"@en .


###  http://purl.org/stc/terms#operation
<http://purl.org/stc/terms#operation> rdf:type owl:NamedIndividual ;
                                      <http://purl.org/stc/terms#hasParent> <http://purl.org/stc/terms#software_lifecycle> .


###  http://purl.org/stc/terms#oracle_orientation_in_test_approach
<http://purl.org/stc/terms#oracle_orientation_in_test_approach> rdf:type owl:NamedIndividual ;
                                                                <http://purl.org/stc/terms#hasParent> <http://purl.org/stc/terms#test_approach> ;
                                                                :isInISTQBGlossary "false"^^xsd:boolean ;
                                                                rdfs:label "oracle orientation" ;
                                                                <http://www.w3.org/2004/02/skos/core#prefLabel> "oracle orientation in test approach"@en .


###  http://purl.org/stc/terms#pair_testing
<http://purl.org/stc/terms#pair_testing> rdf:type owl:NamedIndividual ;
                                         <http://purl.org/stc/terms#hasParent> <http://purl.org/stc/terms#tester_orientation_in_test_approach> ;
                                         :isInISTQBGlossary "true"^^xsd:boolean ;
                                         rdfs:label "pair testing" ;
                                         <http://www.w3.org/2004/02/skos/core#prefLabel> "pair testing"@en .


###  http://purl.org/stc/terms#peer_review
<http://purl.org/stc/terms#peer_review> rdf:type owl:NamedIndividual ;
                                        <http://purl.org/stc/terms#hasParent> <http://purl.org/stc/terms#informal_review> ;
                                        :isInISTQBGlossary "true"^^xsd:boolean ;
                                        rdfs:comment "A type of review performed on a work product by persons that have the abilities required to create it.  (ISTQB Glossary v4.5)"@en ;
                                        rdfs:label "peer review" ;
                                        rdfs:seeAlso "" ;
                                        <http://www.w3.org/2004/02/skos/core#prefLabel> "peer review"@en .


###  http://purl.org/stc/terms#performance_testing
<http://purl.org/stc/terms#performance_testing> rdf:type owl:NamedIndividual ;
                                                <http://purl.org/stc/terms#hasParent> <http://purl.org/stc/terms#non-functional_testing> ;
                                                :isInISTQBGlossary "true"^^xsd:boolean ;
                                                rdfs:label "performance testing" ;
                                                <http://www.w3.org/2004/02/skos/core#prefLabel> "performance testing"@en .


###  http://purl.org/stc/terms#process_improvement
<http://purl.org/stc/terms#process_improvement> rdf:type owl:NamedIndividual ;
                                                <http://purl.org/stc/terms#hasParent> <http://purl.org/stc/terms#support_processes> .


###  http://purl.org/stc/terms#process_orientation_in_software_development
<http://purl.org/stc/terms#process_orientation_in_software_development> rdf:type owl:NamedIndividual ;
                                                                        <http://purl.org/stc/terms#hasParent> <http://purl.org/stc/terms#software_development_model> ;
                                                                        :isInISTQBGlossary "false"^^xsd:boolean ;
                                                                        rdfs:label "process orientation" ;
                                                                        <http://www.w3.org/2004/02/skos/core#prefLabel> "process orientation in software development"@en .


###  http://purl.org/stc/terms#process_orientation_in_test_approach
<http://purl.org/stc/terms#process_orientation_in_test_approach> rdf:type owl:NamedIndividual ;
                                                                 <http://purl.org/stc/terms#hasParent> <http://purl.org/stc/terms#test_approach> ;
                                                                 :isInISTQBGlossary "false"^^xsd:boolean ;
                                                                 rdfs:label "process orientation" ;
                                                                 <http://www.w3.org/2004/02/skos/core#prefLabel> "process orientation in test approach"@en .


###  http://purl.org/stc/terms#project_management
<http://purl.org/stc/terms#project_management> rdf:type owl:NamedIndividual ;
                                               <http://purl.org/stc/terms#hasParent> <http://purl.org/stc/terms#support_processes> .


###  http://purl.org/stc/terms#property-based_testing
<http://purl.org/stc/terms#property-based_testing> rdf:type owl:NamedIndividual ;
                                                   <http://purl.org/stc/terms#hasParent> <http://purl.org/stc/terms#target_orientation_in_test_approach> ;
                                                   :isInISTQBGlossary "true"^^xsd:boolean ;
                                                   rdfs:label "property-based testing" ;
                                                   <http://www.w3.org/2004/02/skos/core#prefLabel> "property-based testing"@en .


###  http://purl.org/stc/terms#protocol_or_service_testing
<http://purl.org/stc/terms#protocol_or_service_testing> rdf:type owl:NamedIndividual ;
                                                        <http://purl.org/stc/terms#hasParent> <http://purl.org/stc/terms#domain-specific_test_types> ;
                                                        :isInISTQBGlossary "false"^^xsd:boolean ;
                                                        rdfs:label "protocol or service testing" ;
                                                        <http://www.w3.org/2004/02/skos/core#prefLabel> "protocol or service testing"@en .


###  http://purl.org/stc/terms#quality_assurance
<http://purl.org/stc/terms#quality_assurance> rdf:type owl:NamedIndividual ;
                                              <http://purl.org/stc/terms#hasParent> <http://purl.org/stc/terms#support_processes> .


###  http://purl.org/stc/terms#reactive_testing
<http://purl.org/stc/terms#reactive_testing> rdf:type owl:NamedIndividual ;
                                             <http://purl.org/stc/terms#hasParent> <http://purl.org/stc/terms#dynamic_testing> ;
                                             :isInISTQBGlossary "true"^^xsd:boolean ;
                                             rdfs:label "reactive testing" ;
                                             <http://www.w3.org/2004/02/skos/core#prefLabel> "reactive testing"@en .


###  http://purl.org/stc/terms#regression_testing
<http://purl.org/stc/terms#regression_testing> rdf:type owl:NamedIndividual ;
                                               <http://purl.org/stc/terms#hasParent> <http://purl.org/stc/terms#change_orientation_in_test_approach> ;
                                               :isInISTQBGlossary "true"^^xsd:boolean ;
                                               rdfs:comment """A type of change-related testing to detect whether defects have been introduced or uncovered in unchanged areas of the software. (ISTQB Glossary v4.5)

Testingperformed following modifications to a test item or to its operational environment, to identify whether failures in unmodified parts of the test item occur. (ISO/IEC/IEEE 29119-1:2022)"""@en ;
                                               rdfs:label "regression testing" ;
                                               rdfs:seeAlso """ISO/IEC/IEEE 29119-1:2022 (Software and systems engineering — Software testing — Part 1: Concepts and definitions)

Foundation - v4.0
Advanced Test Analyst - v4.0
Specialist - Test Automation Engineer - 2016""" ;
                                               <http://www.w3.org/2004/02/skos/core#prefLabel> "regression testing"@en .


###  http://purl.org/stc/terms#regulatory_acceptance_testing
<http://purl.org/stc/terms#regulatory_acceptance_testing> rdf:type owl:NamedIndividual ;
                                                          <http://purl.org/stc/terms#hasParent> <http://purl.org/stc/terms#acceptance_testing> ;
                                                          :isInISTQBGlossary "true"^^xsd:boolean ;
                                                          rdfs:label "regulatory acceptance testing" ;
                                                          <http://www.w3.org/2004/02/skos/core#prefLabel> "regulatory acceptance testing"@en .


###  http://purl.org/stc/terms#related_to_role
<http://purl.org/stc/terms#related_to_role> rdf:type owl:NamedIndividual ;
                                            <http://purl.org/stc/terms#hasParent> <http://purl.org/stc/terms#test_work_force> ;
                                            :isInISTQBGlossary "false"^^xsd:boolean ;
                                            rdfs:label "related to role" ;
                                            <http://www.w3.org/2004/02/skos/core#prefLabel> "related to role"@en .


###  http://purl.org/stc/terms#related_to_team
<http://purl.org/stc/terms#related_to_team> rdf:type owl:NamedIndividual ;
                                            <http://purl.org/stc/terms#hasParent> <http://purl.org/stc/terms#test_work_force> ;
                                            :isInISTQBGlossary "false"^^xsd:boolean ;
                                            rdfs:label "related to team" ;
                                            <http://www.w3.org/2004/02/skos/core#prefLabel> "related to team"@en .


###  http://purl.org/stc/terms#release
<http://purl.org/stc/terms#release> rdf:type owl:NamedIndividual ;
                                    <http://purl.org/stc/terms#hasParent> <http://purl.org/stc/terms#software_lifecycle> .


###  http://purl.org/stc/terms#requirements-based_testing
<http://purl.org/stc/terms#requirements-based_testing> rdf:type owl:NamedIndividual ;
                                                       <http://purl.org/stc/terms#hasParent> <http://purl.org/stc/terms#black_box_test_technique> ;
                                                       :isInISTQBGlossary "true"^^xsd:boolean ;
                                                       rdfs:label "requirements-based testing" ;
                                                       <http://www.w3.org/2004/02/skos/core#prefLabel> "requirements-based testing"@en .


###  http://purl.org/stc/terms#requirements_coverage
<http://purl.org/stc/terms#requirements_coverage> rdf:type owl:NamedIndividual ;
                                                  <http://purl.org/stc/terms#hasParent> <http://purl.org/stc/terms#specification_coverage> ;
                                                  :isInISTQBGlossary "false"^^xsd:boolean ;
                                                  rdfs:comment "Number of requirements covered by executed tests (ISO/IEC/IEEE 29119-1:2022, defined as test coverage)"@en ;
                                                  rdfs:label "requirement coverage" ;
                                                  rdfs:seeAlso "ISO/IEC/IEEE 29119-1:2022 (Software and systems engineering — Software testing — Part 1: Concepts and definitions)" ;
                                                  <http://www.w3.org/2004/02/skos/core#altLabel> "requirements coverage"@en ;
                                                  <http://www.w3.org/2004/02/skos/core#prefLabel> "requirement coverage"@en .


###  http://purl.org/stc/terms#requirements_engineering
<http://purl.org/stc/terms#requirements_engineering> rdf:type owl:NamedIndividual ;
                                                     <http://purl.org/stc/terms#hasParent> <http://purl.org/stc/terms#software_engineering_activity> .


###  http://purl.org/stc/terms#review
<http://purl.org/stc/terms#review> rdf:type owl:NamedIndividual ;
                                   <http://purl.org/stc/terms#hasParent> <http://purl.org/stc/terms#static_testing> .


###  http://purl.org/stc/terms#risk-based_testing
<http://purl.org/stc/terms#risk-based_testing> rdf:type owl:NamedIndividual ;
                                               <http://purl.org/stc/terms#hasParent> <http://purl.org/stc/terms#target_orientation_in_test_approach> ;
                                               :isInISTQBGlossary "true"^^xsd:boolean ;
                                               rdfs:label "risk-based testing" ;
                                               <http://www.w3.org/2004/02/skos/core#prefLabel> "risk-based testing"@en .


###  http://purl.org/stc/terms#risk_oriented_metric
<http://purl.org/stc/terms#risk_oriented_metric> rdf:type owl:NamedIndividual ;
                                                 <http://purl.org/stc/terms#hasParent> <http://purl.org/stc/terms#test_metric> ;
                                                 :isInISTQBGlossary "false"^^xsd:boolean ;
                                                 rdfs:label "risk oriented metric" ;
                                                 <http://www.w3.org/2004/02/skos/core#altLabel> """risk-oriented metric
risk metric"""@en ;
                                                 <http://www.w3.org/2004/02/skos/core#prefLabel> "risk oriented metric"@en .


###  http://purl.org/stc/terms#safety_testing
<http://purl.org/stc/terms#safety_testing> rdf:type owl:NamedIndividual ;
                                           <http://purl.org/stc/terms#hasParent> <http://purl.org/stc/terms#non-functional_testing> ;
                                           :isInISTQBGlossary "false"^^xsd:boolean ;
                                           rdfs:label "safety testing" ;
                                           <http://www.w3.org/2004/02/skos/core#prefLabel> "safety testing"@en .


###  http://purl.org/stc/terms#scripted_testing
<http://purl.org/stc/terms#scripted_testing> rdf:type owl:NamedIndividual ;
                                             <http://purl.org/stc/terms#hasParent> <http://purl.org/stc/terms#manual_testing> ;
                                             :isInISTQBGlossary "true"^^xsd:boolean ;
                                             rdfs:comment "Testing performed based on a documented test script. (ISO/IEC/IEEE 29119-1:2022)"@en ;
                                             rdfs:label "scripted testing" ;
                                             rdfs:seeAlso "ISO/IEC/IEEE 29119-1:2022 (Software and systems engineering — Software testing — Part 1: Concepts and definitions)" ;
                                             <http://www.w3.org/2004/02/skos/core#prefLabel> "scripted testing"@en .


###  http://purl.org/stc/terms#security_testing
<http://purl.org/stc/terms#security_testing> rdf:type owl:NamedIndividual ;
                                             <http://purl.org/stc/terms#hasParent> <http://purl.org/stc/terms#non-functional_testing> ;
                                             :isInISTQBGlossary "true"^^xsd:boolean ;
                                             rdfs:comment """A test type to determine the security of a component or system. (ISTQB Glossary v4.5)

Test type conducted to evaluate the degree to which a test item, and associated data and information, are protected so that unauthorized persons or systems cannot use, read, or modify them, and authorized persons or systems are not denied access to them. (ISO/IEC/IEEE 29119-1:2022)"""@en ;
                                             rdfs:label "security testing" ;
                                             rdfs:seeAlso """ISO/IEC/IEEE 29119-1:2022 (Software and systems engineering — Software testing — Part 1: Concepts and definitions)

Specialist - Mobile Application Testing - 2019
Specialist - Security Tester - 2016
Specialist - Security Test Engineer - v1.0""" ;
                                             <http://www.w3.org/2004/02/skos/core#prefLabel> "security testing"@en .


###  http://purl.org/stc/terms#sequential_development_model
<http://purl.org/stc/terms#sequential_development_model> rdf:type owl:NamedIndividual ;
                                                         <http://purl.org/stc/terms#hasParent> <http://purl.org/stc/terms#process_orientation_in_software_development> ;
                                                         :isInISTQBGlossary "true"^^xsd:boolean ;
                                                         rdfs:label "sequential" ;
                                                         <http://www.w3.org/2004/02/skos/core#prefLabel> "sequential development model"@en .


###  http://purl.org/stc/terms#session-based_testing
<http://purl.org/stc/terms#session-based_testing> rdf:type owl:NamedIndividual ;
                                                  <http://purl.org/stc/terms#hasParent> <http://purl.org/stc/terms#process_orientation_in_test_approach> ;
                                                  :isInISTQBGlossary "true"^^xsd:boolean ;
                                                  rdfs:label "session-based testing" ;
                                                  <http://www.w3.org/2004/02/skos/core#altLabel> """session based testing
session-oriented testing
session oriented testing"""@en ;
                                                  <http://www.w3.org/2004/02/skos/core#prefLabel> "session-based testing"@en .


###  http://purl.org/stc/terms#software
<http://purl.org/stc/terms#software> rdf:type owl:NamedIndividual ;
                                     <http://purl.org/stc/terms#hasParent> <http://purl.org/stc/terms#software_engineering_concepts> .


###  http://purl.org/stc/terms#software_development_model
<http://purl.org/stc/terms#software_development_model> rdf:type owl:NamedIndividual ;
                                                       <http://purl.org/stc/terms#hasParent> <http://purl.org/stc/terms#software_engineering_concepts> ;
                                                       :isInISTQBGlossary "false"^^xsd:boolean ;
                                                       rdfs:label "software development model" ;
                                                       <http://www.w3.org/2004/02/skos/core#prefLabel> "software development model"@en .


###  http://purl.org/stc/terms#software_engineering
<http://purl.org/stc/terms#software_engineering> rdf:type owl:NamedIndividual ;
                                                 <http://purl.org/stc/terms#hasParent> <http://purl.org/stc/terms#basic_concepts> ;
                                                 :isInISTQBGlossary "false"^^xsd:boolean ;
                                                 rdfs:comment """The application of a systematic, disciplined, quantifiable approach to the development, operation, and maintenance of software; that is, the application of engineering to software. (IEEE 610.12-1990, ISO/IEC/IEEE 24765:2017)

A set of systematic processes for the acquisition, supply, development, operation, maintenance, and disposal of software products. (ISO/IEC 12207:2017)"""@en ;
                                                 rdfs:label "software engineering" ;
                                                 rdfs:seeAlso """ISO/IEC/IEEE 24765:2017 (Systems and Software Engineering – Vocabulary)
ISO/IEC 12207:2017 (Systems and software engineering — Software life cycle processes)
ISO/IEC 12207:2017 (Systems and software engineering — Software life cycle processes)""" ;
                                                 <http://www.w3.org/2004/02/skos/core#altLabel> """se
software development"""@en ;
                                                 <http://www.w3.org/2004/02/skos/core#prefLabel> "software engineering"@en .


###  http://purl.org/stc/terms#software_engineering_activity
<http://purl.org/stc/terms#software_engineering_activity> rdf:type owl:NamedIndividual ;
                                                          <http://purl.org/stc/terms#hasParent> <http://purl.org/stc/terms#software_engineering_concepts> .


###  http://purl.org/stc/terms#software_engineering_concepts
<http://purl.org/stc/terms#software_engineering_concepts> rdf:type owl:NamedIndividual ;
                                                          rdfs:comment "Selection of software engineering concepts that relate to software testing concepts."@en ;
                                                          rdfs:label "software engineering concepts" ;
                                                          <http://www.w3.org/2004/02/skos/core#prefLabel> "software engineering concepts"@en .


###  http://purl.org/stc/terms#software_lifecycle
<http://purl.org/stc/terms#software_lifecycle> rdf:type owl:NamedIndividual ;
                                               <http://purl.org/stc/terms#hasParent> <http://purl.org/stc/terms#software_engineering_concepts> .


###  http://purl.org/stc/terms#software_testing_concepts
<http://purl.org/stc/terms#software_testing_concepts> rdf:type owl:NamedIndividual ;
                                                      rdfs:comment "Rather exhaustive collection of software testing concepts"@en ;
                                                      rdfs:label "software testing concepts" ;
                                                      <http://www.w3.org/2004/02/skos/core#prefLabel> "software testing concepts"@en .


###  http://purl.org/stc/terms#specialist_tester
<http://purl.org/stc/terms#specialist_tester> rdf:type owl:NamedIndividual ;
                                              <http://purl.org/stc/terms#hasParent> <http://purl.org/stc/terms#related_to_role> ;
                                              :isInISTQBGlossary "false"^^xsd:boolean ;
                                              rdfs:comment """Performs testing for specific quality characteristics, such as usability, accessibility,
security, performance. (ISO/IEC/IEEE 29119-1:2022)"""@en ;
                                              rdfs:label "specialist tester" ;
                                              rdfs:seeAlso "ISO/IEC/IEEE 29119-1:2022 (Software and systems engineering — Software testing — Part 1: Concepts and definitions)" ;
                                              <http://www.w3.org/2004/02/skos/core#prefLabel> "specialist tester"@en .


###  http://purl.org/stc/terms#specification_coverage
<http://purl.org/stc/terms#specification_coverage> rdf:type owl:NamedIndividual ;
                                                   <http://purl.org/stc/terms#hasParent> <http://purl.org/stc/terms#coverage> ;
                                                   :isInISTQBGlossary "false"^^xsd:boolean ;
                                                   rdfs:comment "There is currently no industry agreed approach to calculating experience-based coverage. (ISO/IEC/IEEE 29119-4)"@en ;
                                                   rdfs:label "specification coverage" ;
                                                   rdfs:seeAlso "ISO/IEC/IEEE 29119-4 (Software and systems engineering — Software testing — Part 4: Test techniques)" ;
                                                   <http://www.w3.org/2004/02/skos/core#altLabel> """black-box test metric
black box test metric
specification-based test metric
specification based test metric"""@en ;
                                                   <http://www.w3.org/2004/02/skos/core#prefLabel> "specification coverage"@en .


###  http://purl.org/stc/terms#state_transition_testing
<http://purl.org/stc/terms#state_transition_testing> rdf:type owl:NamedIndividual ;
                                                     <http://purl.org/stc/terms#hasParent> <http://purl.org/stc/terms#black_box_test_technique> ;
                                                     :isInISTQBGlossary "true"^^xsd:boolean ;
                                                     rdfs:label "state transition testing" ;
                                                     <http://www.w3.org/2004/02/skos/core#prefLabel> "state transition testing"@en .


###  http://purl.org/stc/terms#statement_coverage
<http://purl.org/stc/terms#statement_coverage> rdf:type owl:NamedIndividual ;
                                               <http://purl.org/stc/terms#hasParent> <http://purl.org/stc/terms#structural_coverage> ;
                                               :isInISTQBGlossary "true"^^xsd:boolean ;
                                               rdfs:comment """The coverage of executable statements. (ISTQB Glossary v4.5)

Coverage for statement testing. (ISO/IEC/IEEE 29119-4)"""@en ;
                                               rdfs:label "statement coverage" ;
                                               rdfs:seeAlso """ISO/IEC/IEEE 29119-4 (Software and systems engineering — Software testing — Part 4: Test techniques)

Foundation - v4.0""" ;
                                               <http://www.w3.org/2004/02/skos/core#altLabel> "statement testing coverage"@en ;
                                               <http://www.w3.org/2004/02/skos/core#prefLabel> "statement coverage"@en .


###  http://purl.org/stc/terms#statement_testing
<http://purl.org/stc/terms#statement_testing> rdf:type owl:NamedIndividual ;
                                              <http://purl.org/stc/terms#hasParent> <http://purl.org/stc/terms#white_box_test_technique> ;
                                              :isInISTQBGlossary "true"^^xsd:boolean ;
                                              rdfs:label "statement testing" ;
                                              <http://www.w3.org/2004/02/skos/core#prefLabel> "statement testing"@en .


###  http://purl.org/stc/terms#static_analysis
<http://purl.org/stc/terms#static_analysis> rdf:type owl:NamedIndividual ;
                                            <http://purl.org/stc/terms#hasParent> <http://purl.org/stc/terms#static_testing> ;
                                            :isInISTQBGlossary "true"^^xsd:boolean ;
                                            rdfs:comment "The process of evaluating a component or system without executing it, based on its form, structure, content, or documentation. (ISTQB Glossary v4.5)"@en ;
                                            rdfs:label "static analysis" ;
                                            rdfs:seeAlso """Foundation - v4.0
Advanced Technical Test Analyst - v4.0
Advanced Test Automation Engineering - v2.0""" ;
                                            <http://www.w3.org/2004/02/skos/core#prefLabel> "static analysis"@en .


###  http://purl.org/stc/terms#static_application_security_testing
<http://purl.org/stc/terms#static_application_security_testing> rdf:type owl:NamedIndividual ;
                                                                <http://purl.org/stc/terms#hasParent> <http://purl.org/stc/terms#security_testing> ;
                                                                :isInISTQBGlossary "true"^^xsd:boolean ;
                                                                rdfs:label "static application security testing" ;
                                                                <http://www.w3.org/2004/02/skos/core#prefLabel> "static application security testing"@en .


###  http://purl.org/stc/terms#static_testing
<http://purl.org/stc/terms#static_testing> rdf:type owl:NamedIndividual ;
                                           <http://purl.org/stc/terms#hasParent> <http://purl.org/stc/terms#testing> ;
                                           :isInISTQBGlossary "true"^^xsd:boolean ;
                                           rdfs:comment """Testing that does not involve the execution of a test item. (ISTQB Glossary v4.5)

Testing in which a test item is examined against a set of quality or other criteria without the test item being executed. (ISO/IEC/IEEE 29119-1:2022)"""@en ;
                                           rdfs:label "static testing" ;
                                           rdfs:seeAlso """ISO/IEC/IEEE 29119-1:2022 (Software and systems engineering — Software testing — Part 1: Concepts and definitions)

Foundation - v4.0""" ;
                                           <http://www.w3.org/2004/02/skos/core#prefLabel> "static testing"@en .


###  http://purl.org/stc/terms#stress_testing
<http://purl.org/stc/terms#stress_testing> rdf:type owl:NamedIndividual ;
                                           <http://purl.org/stc/terms#hasParent> <http://purl.org/stc/terms#performance_testing> ;
                                           :isInISTQBGlossary "true"^^xsd:boolean ;
                                           rdfs:label "stress testing" ;
                                           <http://www.w3.org/2004/02/skos/core#prefLabel> "stress testing"@en .


###  http://purl.org/stc/terms#structural_coverage
<http://purl.org/stc/terms#structural_coverage> rdf:type owl:NamedIndividual ;
                                                <http://purl.org/stc/terms#hasParent> <http://purl.org/stc/terms#coverage> ;
                                                :isInISTQBGlossary "true"^^xsd:boolean ;
                                                rdfs:comment "Coverage measures based on the internal structure of a component or system. (ISTQB Glossary v4.5)"@en ;
                                                rdfs:label "structural coverage" ;
                                                rdfs:seeAlso "ISO/IEC/IEEE 29119-4 (Software and systems engineering — Software testing — Part 4: Test techniques)" ;
                                                <http://www.w3.org/2004/02/skos/core#altLabel> """white box test metric
white-box test metric
structure-based test metric
structure based test metric"""@en ;
                                                <http://www.w3.org/2004/02/skos/core#prefLabel> "structural coverage"@en .


###  http://purl.org/stc/terms#support_processes
<http://purl.org/stc/terms#support_processes> rdf:type owl:NamedIndividual ;
                                              <http://purl.org/stc/terms#hasParent> <http://purl.org/stc/terms#software_lifecycle> .


###  http://purl.org/stc/terms#system_integration_testing
<http://purl.org/stc/terms#system_integration_testing> rdf:type owl:NamedIndividual ;
                                                       <http://purl.org/stc/terms#hasParent> <http://purl.org/stc/terms#integration_testing> ;
                                                       :isInISTQBGlossary "true"^^xsd:boolean ;
                                                       rdfs:comment "The integration testing of systems. (ISTQB Glossary v4.5)"@en ;
                                                       rdfs:label "system integration testing" ;
                                                       rdfs:seeAlso "Foundation - v4.0" ;
                                                       <http://www.w3.org/2004/02/skos/core#prefLabel> "system integration testing"@en .


###  http://purl.org/stc/terms#system_testing
<http://purl.org/stc/terms#system_testing> rdf:type owl:NamedIndividual ;
                                           <http://purl.org/stc/terms#hasParent> <http://purl.org/stc/terms#test_level> ;
                                           :isInISTQBGlossary "true"^^xsd:boolean ;
                                           rdfs:label "system testing" ;
                                           <http://www.w3.org/2004/02/skos/core#prefLabel> "system testing"@en .


###  http://purl.org/stc/terms#target_orientation_in_software_development
<http://purl.org/stc/terms#target_orientation_in_software_development> rdf:type owl:NamedIndividual ;
                                                                       <http://purl.org/stc/terms#hasParent> <http://purl.org/stc/terms#software_development_model> ;
                                                                       :isInISTQBGlossary "false"^^xsd:boolean ;
                                                                       rdfs:label "target orientation" ;
                                                                       <http://www.w3.org/2004/02/skos/core#prefLabel> "target orientation in software development"@en .


###  http://purl.org/stc/terms#target_orientation_in_test_approach
<http://purl.org/stc/terms#target_orientation_in_test_approach> rdf:type owl:NamedIndividual ;
                                                                <http://purl.org/stc/terms#hasParent> <http://purl.org/stc/terms#test_approach> ;
                                                                :isInISTQBGlossary "false"^^xsd:boolean ;
                                                                rdfs:label "target orientation" ;
                                                                <http://www.w3.org/2004/02/skos/core#prefLabel> "target orientation in test approach"@en .


###  http://purl.org/stc/terms#technical_review
<http://purl.org/stc/terms#technical_review> rdf:type owl:NamedIndividual ;
                                             <http://purl.org/stc/terms#hasParent> <http://purl.org/stc/terms#formal_review> ;
                                             :isInISTQBGlossary "true"^^xsd:boolean ;
                                             rdfs:comment "A formal review by technical experts that examine the quality of a work product and identify discrepancies from specifications and standards. (ISTQB Glossary v4.5)"@en ;
                                             rdfs:label "technical review" ;
                                             rdfs:seeAlso """Foundation - v4.0
Advanced Test Manager - 2012
Advanced Technical Test Analyst - v4.0""" ;
                                             <http://www.w3.org/2004/02/skos/core#prefLabel> "technical review"@en .


###  http://purl.org/stc/terms#test_activity
<http://purl.org/stc/terms#test_activity> rdf:type owl:NamedIndividual ;
                                          <http://purl.org/stc/terms#hasParent> <http://purl.org/stc/terms#software_engineering_activity> ,
                                                                                <http://purl.org/stc/terms#software_testing_concepts> ;
                                          :isInISTQBGlossary "false"^^xsd:boolean ;
                                          rdfs:label "test activity" ;
                                          <http://www.w3.org/2004/02/skos/core#prefLabel> "test activity"@en .


###  http://purl.org/stc/terms#test_analysis
<http://purl.org/stc/terms#test_analysis> rdf:type owl:NamedIndividual ;
                                          <http://purl.org/stc/terms#hasParent> <http://purl.org/stc/terms#test_activity> ;
                                          :isInISTQBGlossary "true"^^xsd:boolean ;
                                          rdfs:comment "The activity that identifies test conditions by analyzing the test basis. (ISTQB Glossary v4.5)"@en ;
                                          rdfs:label "test analysis" ;
                                          rdfs:seeAlso """Foundation - v4.0
Advanced Test Analyst - v3.1
Advanced Test Analyst - v4.0""" ;
                                          <http://www.w3.org/2004/02/skos/core#prefLabel> "test analysis"@en .


###  http://purl.org/stc/terms#test_analyst
<http://purl.org/stc/terms#test_analyst> rdf:type owl:NamedIndividual ;
                                         <http://purl.org/stc/terms#hasParent> <http://purl.org/stc/terms#related_to_role> ;
                                         :isInISTQBGlossary "false"^^xsd:boolean ;
                                         rdfs:comment "Develops oracles and/or analyses test results for correctness and issues.  (ISO/IEC/IEEE 29119-1:2022)"@en ;
                                         rdfs:label "test analyst" ;
                                         rdfs:seeAlso "ISO/IEC/IEEE 29119-1:2022 (Software and systems engineering — Software testing — Part 1: Concepts and definitions)" ;
                                         <http://www.w3.org/2004/02/skos/core#altLabel> "TA"@en ;
                                         <http://www.w3.org/2004/02/skos/core#prefLabel> "test analyst"@en .


###  http://purl.org/stc/terms#test_approach
<http://purl.org/stc/terms#test_approach> rdf:type owl:NamedIndividual ;
                                          <http://purl.org/stc/terms#hasParent> <http://purl.org/stc/terms#software_testing_concepts> ;
                                          :isInISTQBGlossary "true"^^xsd:boolean ;
                                          rdfs:comment "The manner of implementing testing tasks. (ISTQB Glossary v4.5)"@en ;
                                          rdfs:label "test approach" ;
                                          rdfs:seeAlso """Foundation - v4.0
Advanced Test Manager - 2012""" ;
                                          <http://www.w3.org/2004/02/skos/core#prefLabel> "test approach"@en .


###  http://purl.org/stc/terms#test_architect
<http://purl.org/stc/terms#test_architect> rdf:type owl:NamedIndividual ;
                                           <http://purl.org/stc/terms#hasParent> <http://purl.org/stc/terms#related_to_role> ;
                                           :isInISTQBGlossary "false"^^xsd:boolean ;
                                           rdfs:comment "Defines the test strategy, test environment and test plan for programmes and projects. Specifies the organizational test requirements and helps ensure conformance to these requirements. (ISO/IEC/IEEE 29119-1:2022)"@en ;
                                           rdfs:label "test architect" ;
                                           rdfs:seeAlso "ISO/IEC/IEEE 29119-1:2022 (Software and systems engineering — Software testing — Part 1: Concepts and definitions)" ;
                                           <http://www.w3.org/2004/02/skos/core#prefLabel> "test architect"@en .


###  http://purl.org/stc/terms#test_automation
<http://purl.org/stc/terms#test_automation> rdf:type owl:NamedIndividual ;
                                            <http://purl.org/stc/terms#hasParent> <http://purl.org/stc/terms#test_activity> ;
                                            :isInISTQBGlossary "true"^^xsd:boolean ;
                                            rdfs:comment "The conversion of test activities to automatic operation. (ISTQB Glossary v4.5)"@en ;
                                            rdfs:label "test automation" ;
                                            rdfs:seeAlso """Advanced Test Automation Engineering - v2.0
Specialist - Test Automation Engineer - 2016""" ;
                                            <http://www.w3.org/2004/02/skos/core#prefLabel> "test automation"@en .


###  http://purl.org/stc/terms#test_automation_engineer
<http://purl.org/stc/terms#test_automation_engineer> rdf:type owl:NamedIndividual ;
                                                     <http://purl.org/stc/terms#hasParent> <http://purl.org/stc/terms#related_to_role> ;
                                                     :isInISTQBGlossary "false"^^xsd:boolean ;
                                                     rdfs:comment "Implements tests cases/scripts within a test automation framework. (ISO/IEC/IEEE 29119-1:2022)"@en ;
                                                     rdfs:label "test automation engineer" ;
                                                     rdfs:seeAlso "ISO/IEC/IEEE 29119-1:2022 (Software and systems engineering — Software testing — Part 1: Concepts and definitions)" ;
                                                     <http://www.w3.org/2004/02/skos/core#altLabel> """TAE
test automator"""@en ;
                                                     <http://www.w3.org/2004/02/skos/core#prefLabel> "test automation engineer"@en .


###  http://purl.org/stc/terms#test_basis
<http://purl.org/stc/terms#test_basis> rdf:type owl:NamedIndividual ;
                                       <http://purl.org/stc/terms#hasParent> <http://purl.org/stc/terms#Testware> ;
                                       :isInISTQBGlossary "true"^^xsd:boolean ;
                                       rdfs:comment """The body of knowledge used as the basis for test analysis and test design. (ISTQB Glossary v4.5)

Information used as the basis for designing and implementing test cases. (ISO/IEC/IEEE 29119-1:2022)"""@en ;
                                       rdfs:label "test basis" ;
                                       rdfs:seeAlso """ISO/IEC/IEEE 29119-1 (2022) Software and systems engineering -- Software testing -- Part 1: Concepts and definitions

Foundation - v4.0
Advanced Test Analyst - v3.1""" ;
                                       <http://www.w3.org/2004/02/skos/core#prefLabel> "test basis"@en .


###  http://purl.org/stc/terms#test_case
<http://purl.org/stc/terms#test_case> rdf:type owl:NamedIndividual ;
                                      <http://purl.org/stc/terms#hasParent> <http://purl.org/stc/terms#Testware> ;
                                      :isInISTQBGlossary "true"^^xsd:boolean ;
                                      rdfs:comment """A set of preconditions, inputs, actions (where applicable), expected results and postconditions, developed based on test conditions. (ISTQB Glossary v4.5)

Set of preconditions, inputs and expected results, developed to drive the execution of a test item to meet test objectives. (ISO/IEC/IEEE 29119-1:2022)"""@en ;
                                      rdfs:label "test case" ;
                                      rdfs:seeAlso """ISO/IEC/IEEE 29119-1 (2022) Software and systems engineering -- Software testing -- Part 1: Concepts and definitions

Foundation - v4.0
Advanced Test Manager - 2012
Advanced Test Management - v3.0
Advanced Test Analyst - v4.0
Specialist - Acceptance Testing - 2019""" ;
                                      <http://www.w3.org/2004/02/skos/core#altLabel> "testcase"@en ;
                                      <http://www.w3.org/2004/02/skos/core#prefLabel> "test case"@en .


###  http://purl.org/stc/terms#test_completion
<http://purl.org/stc/terms#test_completion> rdf:type owl:NamedIndividual ;
                                            <http://purl.org/stc/terms#hasParent> <http://purl.org/stc/terms#test_activity> ;
                                            :isInISTQBGlossary "true"^^xsd:boolean ;
                                            rdfs:comment "The activity that makes testware available for later use, leaves test environments in a satisfactory condition and communicates the results of testing to relevant stakeholders. (ISTQB Glossary v4.5)"@en ;
                                            rdfs:label "test completion" ;
                                            rdfs:seeAlso """Foundation - v4.0
Advanced Test Management - v3.0""" ;
                                            <http://www.w3.org/2004/02/skos/core#prefLabel> "test completion"@en .


###  http://purl.org/stc/terms#test_completion_report
<http://purl.org/stc/terms#test_completion_report> rdf:type owl:NamedIndividual ;
                                                   <http://purl.org/stc/terms#hasParent> <http://purl.org/stc/terms#test_report> ;
                                                   :isInISTQBGlossary "true"^^xsd:boolean ;
                                                   rdfs:comment """A type of test report produced at completion milestones that provides an evaluation of the corresponding test items against exit criteria. (ISTQB Glossary v4.5)

Report that provides a summary of the testing that was performed. (ISO/IEC/IEEE 29119-1:2022)"""@en ;
                                                   rdfs:label "test completion report" ;
                                                   rdfs:seeAlso """ISO/IEC/IEEE 29119-1:2022 (Software and systems engineering — Software testing — Part 1: Concepts and definitions)

Foundation - v4.0
Advanced Test Manager - 2012""" ;
                                                   <http://www.w3.org/2004/02/skos/core#altLabel> "test summary report"@en ;
                                                   <http://www.w3.org/2004/02/skos/core#prefLabel> "test completion report"@en .


###  http://purl.org/stc/terms#test_condition
<http://purl.org/stc/terms#test_condition> rdf:type owl:NamedIndividual ;
                                           <http://purl.org/stc/terms#hasParent> <http://purl.org/stc/terms#Testware> ;
                                           :isInISTQBGlossary "true"^^xsd:boolean ;
                                           rdfs:comment """A testable aspect of a component or system identified as a basis for testing. (ISTQB Glossary v4.5)

Testable aspect of a component or system, such as a function, transaction, feature, quality attribute, or structural element identified as a basis for testing. (ISO/IEC/IEEE 29119-1:2022)"""@en ;
                                           rdfs:label "test condition" ;
                                           rdfs:seeAlso """ISO/IEC/IEEE 29119-1:2022 (Software and systems engineering — Software testing — Part 1: Concepts and definitions)

Foundation - v4.0
Advanced Test Manager - 2012
Advanced Test Analyst - v3.1
Advanced Test Analyst - v4.0
Specialist - Test Automation Strategy - v1.0""" ;
                                           <http://www.w3.org/2004/02/skos/core#altLabel> """test situation
test requirement"""@en ;
                                           <http://www.w3.org/2004/02/skos/core#prefLabel> "test condition"@en .


###  http://purl.org/stc/terms#test_control
<http://purl.org/stc/terms#test_control> rdf:type owl:NamedIndividual ;
                                         <http://purl.org/stc/terms#hasParent> <http://purl.org/stc/terms#test_activity> ;
                                         :isInISTQBGlossary "true"^^xsd:boolean ;
                                         rdfs:comment "The activity that develops and applies corrective actions to get a test project on track when it deviates from what was planned. (ISTQB Glossary v4.5)"@en ;
                                         rdfs:label "test control" ;
                                         rdfs:seeAlso """Foundation - v4.0
Advanced Test Manager - 2012
Advanced Test Management - v3.0""" ;
                                         <http://www.w3.org/2004/02/skos/core#prefLabel> "test control"@en .


###  http://purl.org/stc/terms#test_data
<http://purl.org/stc/terms#test_data> rdf:type owl:NamedIndividual ;
                                      <http://purl.org/stc/terms#hasParent> <http://purl.org/stc/terms#Testware> ;
                                      :isInISTQBGlossary "true"^^xsd:boolean ;
                                      rdfs:comment """Data needed for test execution. (ISTQB Glossary v4.5)

Data created or selected to satisfy the input requirements for executing one or more test cases, which may be defined in the test plan, test case or test procedure. (ISO/IEC/IEEE 29119-1:2022)"""@en ;
                                      rdfs:label "test data" ;
                                      rdfs:seeAlso """ISO/IEC/IEEE 29119-1:2022 (Software and systems engineering — Software testing — Part 1: Concepts and definitions)

Foundation - v4.0
Advanced Test Analyst - v3.1
Advanced Test Analyst - v4.0""" ;
                                      <http://www.w3.org/2004/02/skos/core#altLabel> """testdata
test data set
testdata set"""@en ;
                                      <http://www.w3.org/2004/02/skos/core#prefLabel> "test data"@en .


###  http://purl.org/stc/terms#test_design
<http://purl.org/stc/terms#test_design> rdf:type owl:NamedIndividual ;
                                        <http://purl.org/stc/terms#hasParent> <http://purl.org/stc/terms#test_activity> ;
                                        :isInISTQBGlossary "true"^^xsd:boolean ;
                                        rdfs:comment "The activity that derives and specifies test cases from test conditions. (ISTQB Glossary v4.5)"@en ;
                                        rdfs:label "test design" ;
                                        rdfs:seeAlso """Foundation - v4.0
Advanced Test Manager - 2012
Advanced Test Analyst - v3.1
Advanced Test Analyst - v4.0""" ;
                                        <http://www.w3.org/2004/02/skos/core#prefLabel> "test design"@en .


###  http://purl.org/stc/terms#test_designer
<http://purl.org/stc/terms#test_designer> rdf:type owl:NamedIndividual ;
                                          <http://purl.org/stc/terms#hasParent> <http://purl.org/stc/terms#related_to_role> ;
                                          :isInISTQBGlossary "false"^^xsd:boolean ;
                                          rdfs:comment "Develops the test design artefacts. (ISO/IEC/IEEE 29119-1:2022)"@en ;
                                          rdfs:label "test designer" ;
                                          rdfs:seeAlso "ISO/IEC/IEEE 29119-1:2022 (Software and systems engineering — Software testing — Part 1: Concepts and definitions)" ;
                                          <http://www.w3.org/2004/02/skos/core#prefLabel> "test designer"@en .


###  http://purl.org/stc/terms#test_director
<http://purl.org/stc/terms#test_director> rdf:type owl:NamedIndividual ;
                                          <http://purl.org/stc/terms#hasParent> <http://purl.org/stc/terms#related_to_role> ;
                                          :isInISTQBGlossary "true"^^xsd:boolean ;
                                          rdfs:comment "A senior manager who manages test managers."@en ;
                                          rdfs:label "test director" ;
                                          rdfs:seeAlso "Advanced Test Manager - 2012" ;
                                          <http://www.w3.org/2004/02/skos/core#prefLabel> "test director"@en .


###  http://purl.org/stc/terms#test_driven_development
<http://purl.org/stc/terms#test_driven_development> rdf:type owl:NamedIndividual ;
                                                    <http://purl.org/stc/terms#hasParent> <http://purl.org/stc/terms#target_orientation_in_software_development> ;
                                                    :isInISTQBGlossary "true"^^xsd:boolean ;
                                                    rdfs:comment "A software development technique in which the test cases are developed, automated and then the software is developed incrementally to pass those test cases. (ISTQB Glossary v4.5)"@en ;
                                                    rdfs:label "test-driven" ;
                                                    rdfs:seeAlso """Foundation - v4.0
Advanced Test Manager - 2012
Advanced Test Management - v3.0
Advanced Test Automation Engineering - v2.0
Advanced Agile Technical Tester - 2019
Specialist - Agile Test Leadership at Scale - v2.0
Specialist - Test Automation Strategy - v1.0""" ;
                                                    <http://www.w3.org/2004/02/skos/core#altLabel> """test driven development
tdd
TDD"""@en ;
                                                    <http://www.w3.org/2004/02/skos/core#prefLabel> "test-driven development"@en .


###  http://purl.org/stc/terms#test_execution
<http://purl.org/stc/terms#test_execution> rdf:type owl:NamedIndividual ;
                                           <http://purl.org/stc/terms#hasParent> <http://purl.org/stc/terms#test_activity> ;
                                           :isInISTQBGlossary "true"^^xsd:boolean ;
                                           rdfs:comment "The activity that runs a test on a component or system producing actual results. (ISTQB Glossary v4.5)"@en ;
                                           rdfs:label "test execution" ;
                                           rdfs:seeAlso """Foundation - v4.0
Advanced Test Manager - 2012
Advanced Test Analyst - v3.1
Advanced Test Analyst - v4.0
Advanced Technical Test Analyst - v4.0""" ;
                                           <http://www.w3.org/2004/02/skos/core#prefLabel> "test execution"@en .


###  http://purl.org/stc/terms#test_first_approach
<http://purl.org/stc/terms#test_first_approach> rdf:type owl:NamedIndividual ;
                                                <http://purl.org/stc/terms#hasParent> <http://purl.org/stc/terms#test_driven_development> ;
                                                :isInISTQBGlossary "true"^^xsd:boolean ;
                                                rdfs:comment "An approach to software development in which the test cases are designed and implemented before the associated component or system is developed. (ISTQB Glossary v4.5)"@en ;
                                                rdfs:label "test-first approach" ;
                                                rdfs:seeAlso """Foundation - v4.0
Advanced Test Analyst - v3.1
Foundation Agile Tester - 2014
Specialist - Agile Test Leadership at Scale - v2.0""" ;
                                                <http://www.w3.org/2004/02/skos/core#altLabel> "test first approach"@en ;
                                                <http://www.w3.org/2004/02/skos/core#prefLabel> "test-first approach"@en .


###  http://purl.org/stc/terms#test_implementation
<http://purl.org/stc/terms#test_implementation> rdf:type owl:NamedIndividual ;
                                                <http://purl.org/stc/terms#hasParent> <http://purl.org/stc/terms#test_activity> ;
                                                :isInISTQBGlossary "true"^^xsd:boolean ;
                                                rdfs:comment "The activity that prepares the testware needed for test execution based on test analysis and design. (ISTQB Glossary v4.5)"@en ;
                                                rdfs:label "test implementation" ;
                                                rdfs:seeAlso """Foundation - v4.0
Advanced Test Manager - 2012
Advanced Test Analyst - v3.1
Advanced Test Analyst - v4.0""" ;
                                                <http://www.w3.org/2004/02/skos/core#prefLabel> "test implementation"@en .


###  http://purl.org/stc/terms#test_item
<http://purl.org/stc/terms#test_item> rdf:type owl:NamedIndividual ;
                                      <http://purl.org/stc/terms#hasParent> <http://purl.org/stc/terms#Testware> ;
                                      :isInISTQBGlossary "true"^^xsd:boolean ;
                                      rdfs:comment "A part of a test object used in the test process. (ISTQB Glossary v4.5)"@en ,
                                                   "ISO/IEC/IEEE 29119-1:2022 defines the term test item differently: as a synonym to test object."@en ;
                                      rdfs:label "test item" ;
                                      <http://www.w3.org/2004/02/skos/core#prefLabel> "test item"@en .


###  http://purl.org/stc/terms#test_leader
<http://purl.org/stc/terms#test_leader> rdf:type owl:NamedIndividual ;
                                        <http://purl.org/stc/terms#hasParent> <http://purl.org/stc/terms#related_to_role> ;
                                        :isInISTQBGlossary "true"^^xsd:boolean ;
                                        rdfs:comment "On large projects, the person who reports to the test manager and is responsible for project management of a particular test level or a particular set of testing activities. (ISTQB Glossary v4.5)"@en ;
                                        rdfs:label "test leader" ;
                                        rdfs:seeAlso "Advanced Test Manager - 2012" ;
                                        <http://www.w3.org/2004/02/skos/core#altLabel> "lead tester"@en ;
                                        <http://www.w3.org/2004/02/skos/core#prefLabel> "test leader"@en .


###  http://purl.org/stc/terms#test_level
<http://purl.org/stc/terms#test_level> rdf:type owl:NamedIndividual ;
                                       <http://purl.org/stc/terms#hasParent> <http://purl.org/stc/terms#software_testing_concepts> ;
                                       :isInISTQBGlossary "true"^^xsd:boolean ;
                                       rdfs:comment """A specific instantiation of a test process. (ISTQB Glossary v4.5)

One of a sequence of test stages each of which is typically associated with the achievement of particular
objectives and used to treat particular risks. (ISO/IEC/IEEE 29119-1:2022)"""@en ;
                                       rdfs:label "test level" ;
                                       rdfs:seeAlso """ISO/IEC/IEEE 29119-1:2022 (Software and systems engineering — Software testing — Part 1: Concepts and definitions)

Foundation - v4.0
Advanced Test Manager - 2012
Advanced Test Management - v3.0
Specialist - Mobile Application Testing - 2019
Specialist - Test Automation Strategy - v1.0""" ;
                                       <http://www.w3.org/2004/02/skos/core#altLabel> """test stage
test phase"""@en ;
                                       <http://www.w3.org/2004/02/skos/core#prefLabel> "test level"@en .


###  http://purl.org/stc/terms#test_management
<http://purl.org/stc/terms#test_management> rdf:type owl:NamedIndividual ;
                                            <http://purl.org/stc/terms#hasParent> <http://purl.org/stc/terms#software_testing_concepts> ,
                                                                                  <http://purl.org/stc/terms#test_activity> ;
                                            :isInISTQBGlossary "true"^^xsd:boolean ;
                                            rdfs:comment "The process of planning, scheduling, estimating, monitoring, reporting, controlling, and completing test activities. (ISTQB Glossary v4.5)"@en ;
                                            rdfs:label "test management" ;
                                            <http://www.w3.org/2004/02/skos/core#prefLabel> "test management"@en .


###  http://purl.org/stc/terms#test_manager
<http://purl.org/stc/terms#test_manager> rdf:type owl:NamedIndividual ;
                                         <http://purl.org/stc/terms#hasParent> <http://purl.org/stc/terms#related_to_role> ;
                                         :isInISTQBGlossary "true"^^xsd:boolean ;
                                         rdfs:comment """The person responsible for project management of testing activities, resources, and evaluation of a test object. (ISTQB Glossary v4.5)

Develops, manages, and helps to ensure conformance with the test management process. The test manager also plans and controls the dynamic test process. (ISO/IEC/IEEE 29119-1:2022)"""@en ;
                                         rdfs:label "test manager" ;
                                         rdfs:seeAlso """ISO/IEC/IEEE 29119-1:2022 (Software and systems engineering — Software testing — Part 1: Concepts and definitions)

Advanced Test Manager - 2012""" ;
                                         <http://www.w3.org/2004/02/skos/core#prefLabel> "test manager"@en .


###  http://purl.org/stc/terms#test_metric
<http://purl.org/stc/terms#test_metric> rdf:type owl:NamedIndividual ;
                                        <http://purl.org/stc/terms#hasParent> <http://purl.org/stc/terms#metric> ,
                                                                              <http://purl.org/stc/terms#software_testing_concepts> ;
                                        :isInISTQBGlossary "false"^^xsd:boolean ;
                                        rdfs:comment "A measurement of a characteristic of a test process, test activity, test object or testware. (own)"@en ;
                                        rdfs:label "test metric" ;
                                        rdfs:seeAlso "ISO/IEC/IEEE 29119-4 (Software and systems engineering — Software testing — Part 4: Test techniques)" ;
                                        <http://www.w3.org/2004/02/skos/core#altLabel> "testmetric"@en ;
                                        <http://www.w3.org/2004/02/skos/core#prefLabel> "test metric"@en .


###  http://purl.org/stc/terms#test_model
<http://purl.org/stc/terms#test_model> rdf:type owl:NamedIndividual ;
                                       <http://purl.org/stc/terms#hasParent> <http://purl.org/stc/terms#Testware> ;
                                       :isInISTQBGlossary "true"^^xsd:boolean ;
                                       rdfs:comment """A model describing testware that is used for testing a component or a system under test. (ISTQB Glossary v4.5)

Representation of the test item, which allows the testing to be focused on particular
characteristics or qualities. (ISO/IEC/IEEE 29119-1:2022)"""@en ;
                                       rdfs:label "test model" ;
                                       rdfs:seeAlso """ISO/IEC/IEEE 29119-1:2022 (Software and systems engineering — Software testing — Part 1: Concepts and definitions)

Specialist - Model-Based Tester - 2015
Specialist - Model-Based Testing - v1.1""" ;
                                       <http://www.w3.org/2004/02/skos/core#altLabel> "test specification" ;
                                       <http://www.w3.org/2004/02/skos/core#prefLabel> "test model"@en .


###  http://purl.org/stc/terms#test_monitoring
<http://purl.org/stc/terms#test_monitoring> rdf:type owl:NamedIndividual ;
                                            <http://purl.org/stc/terms#hasParent> <http://purl.org/stc/terms#test_activity> ;
                                            :isInISTQBGlossary "true"^^xsd:boolean ;
                                            rdfs:comment "The activity that checks the status of testing activities, identifies any variances from planned or expected, and reports status to stakeholders. (ISTQB Glossary v4.5)"@en ;
                                            rdfs:label "test monitoring" ;
                                            rdfs:seeAlso """Foundation - v4.0
Advanced Test Manager - 2012
Advanced Test Management - v3.0""" ;
                                            <http://www.w3.org/2004/02/skos/core#prefLabel> "test monitoring"@en .


###  http://purl.org/stc/terms#test_object
<http://purl.org/stc/terms#test_object> rdf:type owl:NamedIndividual ;
                                        <http://purl.org/stc/terms#hasParent> <http://purl.org/stc/terms#Testware> ;
                                        :isInISTQBGlossary "true"^^xsd:boolean ;
                                        rdfs:comment "The work product to be tested. (ISTQB Glossary v4.5)"@en ;
                                        rdfs:label "test object" ;
                                        rdfs:seeAlso "Foundation - v4.0" ;
                                        <http://www.w3.org/2004/02/skos/core#altLabel> """test target
system under test
sut
SUT
object under test"""@en ;
                                        <http://www.w3.org/2004/02/skos/core#prefLabel> "test object"@en .


###  http://purl.org/stc/terms#test_objective
<http://purl.org/stc/terms#test_objective> rdf:type owl:NamedIndividual ;
                                           <http://purl.org/stc/terms#hasParent> <http://purl.org/stc/terms#Testware> ;
                                           :isInISTQBGlossary "true"^^xsd:boolean ;
                                           rdfs:comment "The purpose for testing. (ISTQB Gloassary v4.5)"@en ,
                                                        "test objective"@en ;
                                           rdfs:seeAlso """Foundation - v4.0
Advanced Test Management - v3.0""" ;
                                           <http://www.w3.org/2004/02/skos/core#altLabel> "test goal"@en ;
                                           <http://www.w3.org/2004/02/skos/core#prefLabel> "test objective"@en .


###  http://purl.org/stc/terms#test_oracle
<http://purl.org/stc/terms#test_oracle> rdf:type owl:NamedIndividual ;
                                        <http://purl.org/stc/terms#hasParent> <http://purl.org/stc/terms#Testware> ;
                                        :isInISTQBGlossary "true"^^xsd:boolean ;
                                        rdfs:comment "A source to determine an expected result to compare with the actual result of the system under test.  (ISTQB Glossary v4.5)"@en ;
                                        rdfs:label "test oracle" ;
                                        rdfs:seeAlso "Advanced Test Analyst - v4.0" ;
                                        <http://www.w3.org/2004/02/skos/core#altLabel> "oracle"@en ;
                                        <http://www.w3.org/2004/02/skos/core#prefLabel> "test oracle"@en .


###  http://purl.org/stc/terms#test_plan
<http://purl.org/stc/terms#test_plan> rdf:type owl:NamedIndividual ;
                                      <http://purl.org/stc/terms#hasParent> <http://purl.org/stc/terms#Testware> ;
                                      :isInISTQBGlossary "true"^^xsd:boolean ;
                                      rdfs:comment """Documentation describing the test objectives to be achieved and the means and the schedule for achieving them, organized to coordinate testing activities. (ISTQB Glossary v4.5)

Detailed description of test objectives to be achieved and the means and schedule for achieving them, organized to coordinate testing activities for some test item or set of test items. (ISO/IEC/IEEE 29119-1:2022)"""@en ;
                                      rdfs:label "test plan" ;
                                      rdfs:seeAlso """ISO/IEC/IEEE 29119-1 (2022) Software and systems engineering -- Software testing -- Part 1: Concepts and definitions

Foundation - v4.0
Advanced Test Manager - 2012
Advanced Test Management - v3.0
Specialist - Performance Testing - 2018
Specialist - Security Test Engineer - v1.0""" ;
                                      <http://www.w3.org/2004/02/skos/core#altLabel> "testplan"@en ;
                                      <http://www.w3.org/2004/02/skos/core#prefLabel> "test plan"@en .


###  http://purl.org/stc/terms#test_planning
<http://purl.org/stc/terms#test_planning> rdf:type owl:NamedIndividual ;
                                          <http://purl.org/stc/terms#hasParent> <http://purl.org/stc/terms#test_activity> ;
                                          :isInISTQBGlossary "true"^^xsd:boolean ;
                                          rdfs:comment "The activity of establishing or updating a test plan. (ISTQB Glossary v4.5)"@en ;
                                          rdfs:label "test planning" ;
                                          rdfs:seeAlso """Foundation - v4.0
Advanced Test Manager - 2012
Advanced Test Management - v3.0""" ;
                                          <http://www.w3.org/2004/02/skos/core#prefLabel> "test planning"@en .


###  http://purl.org/stc/terms#test_process
<http://purl.org/stc/terms#test_process> rdf:type owl:NamedIndividual ;
                                         <http://purl.org/stc/terms#hasParent> <http://purl.org/stc/terms#software_testing_concepts> ;
                                         :isInISTQBGlossary "true"^^xsd:boolean ;
                                         rdfs:comment "The set of interrelated activities comprising of test planning, test monitoring, test control, test analysis, test design, test implementation, test execution, and test completion."@en ,
                                                      """The set of interrelated activities comprising of test planning, test monitoring, test control, test analysis, test design, test implementation, test execution, and test completion. (ISTQB Glossary v4.5)

Set of testing activities performed to achieve a test objective. (ISO/IEC/IEEE 29119-1:2022)"""@en ;
                                         rdfs:label "test process" ;
                                         rdfs:seeAlso """ISO/IEC/IEEE 29119-1:2022 (Software and Systems Engineering — Software Testing — Part 1: Concepts and Definitions)

Foundation - v4.0
Specialist - Mobile Application Testing - 2019
Specialist - Security Test Engineer - v1.0""" ;
                                         <http://www.w3.org/2004/02/skos/core#prefLabel> "test process"@en .


###  http://purl.org/stc/terms#test_process_group
<http://purl.org/stc/terms#test_process_group> rdf:type owl:NamedIndividual ;
                                               <http://purl.org/stc/terms#hasParent> <http://purl.org/stc/terms#related_to_team> ;
                                               :isInISTQBGlossary "true"^^xsd:boolean ;
                                               rdfs:comment "A collection of specialists who facilitate the definition, maintenance, and improvement of the test processes used by an organization. (ISTQB Glossary v4.5)"@en ;
                                               rdfs:label "test process group" ;
                                               rdfs:seeAlso "Expert Improving the Test Process - v1.0.1" ;
                                               <http://www.w3.org/2004/02/skos/core#altLabel> "TPG"@en ;
                                               <http://www.w3.org/2004/02/skos/core#prefLabel> "test process group"@en .


###  http://purl.org/stc/terms#test_process_improvement
<http://purl.org/stc/terms#test_process_improvement> rdf:type owl:NamedIndividual ;
                                                     <http://purl.org/stc/terms#hasParent> <http://purl.org/stc/terms#test_management> ;
                                                     :isInISTQBGlossary "true"^^xsd:boolean ;
                                                     rdfs:label "test process improvement" ;
                                                     <http://www.w3.org/2004/02/skos/core#prefLabel> "test process improvement"@en .


###  http://purl.org/stc/terms#test_progress_report
<http://purl.org/stc/terms#test_progress_report> rdf:type owl:NamedIndividual ;
                                                 <http://purl.org/stc/terms#hasParent> <http://purl.org/stc/terms#test_report> ;
                                                 :isInISTQBGlossary "true"^^xsd:boolean ;
                                                 rdfs:comment """A type of periodic test report that includes the progress of test activities against a baseline, risks, and alternatives requiring a decision. (ISTQB Glossary v4.5)

Report that provides information about the status of the testing that is being performed in a specified reporting period. (ISO/IEC/IEEE 29119-1:2022, defined as test status report)"""@en ;
                                                 rdfs:label "test progress report" ;
                                                 rdfs:seeAlso """ISO/IEC/IEEE 29119-1:2022 (Software and systems engineering — Software testing — Part 1: Concepts and definitions)

Foundation - v4.0
Advanced Test Automation Engineering - v2.0""" ;
                                                 <http://www.w3.org/2004/02/skos/core#altLabel> "test status report"@en ;
                                                 <http://www.w3.org/2004/02/skos/core#prefLabel> "test progress report"@en .


###  http://purl.org/stc/terms#test_report
<http://purl.org/stc/terms#test_report> rdf:type owl:NamedIndividual ;
                                        <http://purl.org/stc/terms#hasParent> <http://purl.org/stc/terms#Testware> ;
                                        :isInISTQBGlossary "true"^^xsd:boolean ;
                                        rdfs:comment "Documentation summarizing testing and results. (ISTQB Glossary v4.5)"@en ;
                                        rdfs:label "test report" ;
                                        rdfs:seeAlso """Specialist - Mobile Application Testing - 2019
Specialist - Security Test Engineer - v1.0
Specialist - Test Automation Strategy - v1.0""" ;
                                        <http://www.w3.org/2004/02/skos/core#altLabel> "testreport"@en ;
                                        <http://www.w3.org/2004/02/skos/core#prefLabel> "test report"@en .


###  http://purl.org/stc/terms#test_script
<http://purl.org/stc/terms#test_script> rdf:type owl:NamedIndividual ;
                                        <http://purl.org/stc/terms#hasParent> <http://purl.org/stc/terms#Testware> ;
                                        :isInISTQBGlossary "true"^^xsd:boolean ;
                                        rdfs:comment """A sequence of instructions for the execution of a test. (ISTQB Glossary v4.5)

Document specifying one or more test procedures. (ISO/IEC/IEEE 29119-1:2022)"""@en ;
                                        rdfs:label "test script" ;
                                        rdfs:seeAlso """ISO/IEC/IEEE 29119-1:2022 (Software and systems engineering — Software testing — Part 1: Concepts and definitions)

Advanced Test Manager - 2012
Advanced Test Analyst - v3.1
Advanced Test Analyst - v4.0
Advanced Test Automation Engineering - v2.0
Specialist - Test Automation Engineer - 2016""" ;
                                        <http://www.w3.org/2004/02/skos/core#altLabel> "test procedure specification"@en ;
                                        <http://www.w3.org/2004/02/skos/core#prefLabel> "test script"@en .


###  http://purl.org/stc/terms#test_step
<http://purl.org/stc/terms#test_step> rdf:type owl:NamedIndividual ;
                                      <http://purl.org/stc/terms#hasParent> <http://purl.org/stc/terms#Testware> ;
                                      :isInISTQBGlossary "true"^^xsd:boolean ;
                                      rdfs:comment "A single interaction between an actor and a test object consisting of an input, an action, and an expected result. (ISTQB Glossary v4.5)"@en ,
                                                   "Advanced Test Automation Engineering - v2.0"@en ;
                                      rdfs:label "test step" ;
                                      <http://www.w3.org/2004/02/skos/core#altLabel> "teststep"@en ;
                                      <http://www.w3.org/2004/02/skos/core#prefLabel> "test step"@en .


###  http://purl.org/stc/terms#test_suite
<http://purl.org/stc/terms#test_suite> rdf:type owl:NamedIndividual ;
                                       <http://purl.org/stc/terms#hasParent> <http://purl.org/stc/terms#Testware> ;
                                       :isInISTQBGlossary "true"^^xsd:boolean ;
                                       rdfs:comment """A set of test scripts or test procedures to be executed in a specific test run. (ISTQB Glossary v4.5)

Set of test cases or test procedures. (ISO/IEC/IEEE 29119-1:2022)"""@en ;
                                       rdfs:label "test suite" ;
                                       rdfs:seeAlso """Advanced Test Analyst - v3.1
Specialist - Test Automation Strategy - v1.0""" ;
                                       <http://www.w3.org/2004/02/skos/core#altLabel> """test set
test case suite
testsuite
testset
testcase suite"""@en ;
                                       <http://www.w3.org/2004/02/skos/core#prefLabel> "test suite"@en .


###  http://purl.org/stc/terms#test_technique
<http://purl.org/stc/terms#test_technique> rdf:type owl:NamedIndividual ;
                                           <http://purl.org/stc/terms#hasParent> <http://purl.org/stc/terms#software_testing_concepts> ;
                                           :isInISTQBGlossary "true"^^xsd:boolean ;
                                           rdfs:comment "(ISTQB Glossary v4.5)"@en ,
                                                        """A procedure used to define test conditions, design test cases, and specify test data. (ISTQB Glossary v4.5)

Procedure used to create or select a test model, identify test coverage items, and derive
corresponding test cases. (ISO/IEC/IEEE 29119-1:2022, defined as test design technique)"""@en ;
                                           rdfs:label "test technique" ;
                                           rdfs:seeAlso """ISO/IEC/IEEE 29119-4 (Software and systems engineering — Software testing — Part 4: Test techniques)

Foundation - v4.0""" ;
                                           <http://www.w3.org/2004/02/skos/core#altLabel> "test design technique"@en ,
                                                                                          "test technique"@en .


###  http://purl.org/stc/terms#test_type
<http://purl.org/stc/terms#test_type> rdf:type owl:NamedIndividual ;
                                      <http://purl.org/stc/terms#hasParent> <http://purl.org/stc/terms#software_testing_concepts> ;
                                      :isInISTQBGlossary "true"^^xsd:boolean ;
                                      rdfs:comment """A group of test activities based on specific test objectives aimed at specific characteristics of a component or system. (ISTQB Glossary v4.5)

Testing that is focused on specific quality characteristics. (ISO/IEC/IEEE 29119-1:2022)"""@en ;
                                      rdfs:label "test type" ;
                                      rdfs:seeAlso """ISO/IEC/IEEE 29119-1:2022 (Software and Systems Engineering — Software Testing — Part 1: Concepts and Definitions)

Foundation - v4.0
Advanced Test Manager - 2012
Advanced Test Management - v3.0
Advanced Test Analyst - v3.1
Advanced Test Analyst - v4.0
Advanced Technical Test Analyst - v4.0
Advanced Test Automation Engineering - v2.0
Specialist - Automotive Software Tester - 2018
Specialist - Automotive Software Tester - v1.1
Specialist - Gambling Industry Tester - 2018
Specialist - Game Testing - v1.0.1
Specialist - Mobile Application Testing - 2019
Specialist - Model-Based Testing - v1.1
Specialist - Test Automation Strategy - v1.0""" ;
                                      <http://www.w3.org/2004/02/skos/core#prefLabel> "test type"@en .


###  http://purl.org/stc/terms#test_work_force
<http://purl.org/stc/terms#test_work_force> rdf:type owl:NamedIndividual ;
                                            <http://purl.org/stc/terms#hasParent> <http://purl.org/stc/terms#software_testing_concepts> ;
                                            :isInISTQBGlossary "false"^^xsd:boolean ;
                                            rdfs:comment "Professions and roles in software testing"@en ;
                                            rdfs:label "test work force" ;
                                            rdfs:seeAlso "GTB: The Professional profile for testing. The reference scheme for people and organizations involved in the topics of quality and testing of software-based components and systems. 2018." ;
                                            <http://www.w3.org/2004/02/skos/core#prefLabel> "test work force"@en .


###  http://purl.org/stc/terms#tester
<http://purl.org/stc/terms#tester> rdf:type owl:NamedIndividual ;
                                   <http://purl.org/stc/terms#hasParent> <http://purl.org/stc/terms#related_to_role> ;
                                   :isInISTQBGlossary "true"^^xsd:boolean ;
                                   rdfs:comment """A person who performs testing. (ISTQB Glossary v4.5)

Develops the test deliverables and completes the processes associated with the
dynamic test process. (ISO/IEC/IEEE 29119-1:2022)"""@en ;
                                   rdfs:label "tester" ;
                                   rdfs:seeAlso "ISO/IEC/IEEE 29119-1:2022 (Software and systems engineering — Software testing — Part 1: Concepts and definitions)" ;
                                   <http://www.w3.org/2004/02/skos/core#prefLabel> "tester"@en .


###  http://purl.org/stc/terms#tester_orientation_in_test_approach
<http://purl.org/stc/terms#tester_orientation_in_test_approach> rdf:type owl:NamedIndividual ;
                                                                <http://purl.org/stc/terms#hasParent> <http://purl.org/stc/terms#test_approach> ;
                                                                :isInISTQBGlossary "false"^^xsd:boolean ;
                                                                rdfs:label "tester orientation" ;
                                                                <http://www.w3.org/2004/02/skos/core#prefLabel> "tester orientation in test approach"@en .


###  http://purl.org/stc/terms#testing
<http://purl.org/stc/terms#testing> rdf:type owl:NamedIndividual ;
                                    <http://purl.org/stc/terms#hasParent> <http://purl.org/stc/terms#software_testing_concepts> ;
                                    :isInISTQBGlossary "true"^^xsd:boolean ;
                                    rdfs:comment """Set of activities conducted to facilitate discovery and evaluation of properties of test items (ISO/IEC/IEEE 29119-1:2022, defined as test)

The process that consists of determining the degree to which a software product satisfies specified requirements (verification) and fulfills its intended purpose (validation). (ISO/IEC/IEEE 12207:2017)

The process of executing a system or component under specified conditions, observing or recording the results, and making an evaluation of some aspect of the system or component. (IEEE 610.12-1990)"""@en ;
                                    rdfs:seeAlso "Foundation - v4.0" ,
                                                 """IEEE Standard 610.12-1990 (IEEE Standard Glossary of Software Engineering Terminology)
ISO/IEC/IEEE 29119-1:2022 (Software and Systems Engineering — Software Testing — Part 1: Concepts and Definitions)
ISO/IEC/IEEE 12207:2017 (Software Life Cycle Processes)""" ;
                                    <http://www.w3.org/2004/02/skos/core#prefLabel> "testing"@en .


###  http://purl.org/stc/terms#testing_in_production
<http://purl.org/stc/terms#testing_in_production> rdf:type owl:NamedIndividual ;
                                                  <http://purl.org/stc/terms#hasParent> <http://purl.org/stc/terms#system_testing> ;
                                                  :isInISTQBGlossary "true"^^xsd:boolean ;
                                                  rdfs:label "testing in production" ;
                                                  <http://www.w3.org/2004/02/skos/core#prefLabel> "testing in production"@en .


###  http://purl.org/stc/terms#testing_quadrants
<http://purl.org/stc/terms#testing_quadrants> rdf:type owl:NamedIndividual ;
                                              <http://purl.org/stc/terms#hasParent> <http://purl.org/stc/terms#test_approach> ;
                                              :isInISTQBGlossary "true"^^xsd:boolean ;
                                              rdfs:comment "A classification model of test types/test levels in four quadrants, relating them to two dimensions of test objectives: supporting the product team versus critiquing the product, and technology-facing versus business-facing. (ISTQB Glossary v4.5)"@en ;
                                              rdfs:label "testing quadrants" ;
                                              rdfs:seeAlso "Foundation - v4.0" ;
                                              <http://www.w3.org/2004/02/skos/core#prefLabel> "testing quadrants"@en .


###  http://purl.org/stc/terms#usability_testing
<http://purl.org/stc/terms#usability_testing> rdf:type owl:NamedIndividual ;
                                              <http://purl.org/stc/terms#hasParent> <http://purl.org/stc/terms#non-functional_testing> ;
                                              :isInISTQBGlossary "true"^^xsd:boolean ;
                                              rdfs:comment "Testing to evaluate the degree to which the system can be used by specified users with effectiveness, efficiency and satisfaction in a specified context of use. (ISTQB Glossary v4.5)"@en ;
                                              rdfs:label "usability testing" ;
                                              rdfs:seeAlso """Specialist - Mobile Application Testing - 2019
Specialist - Usability Testing - 2018""" ;
                                              <http://www.w3.org/2004/02/skos/core#prefLabel> "usability testing"@en .


###  http://purl.org/stc/terms#user-agent_based_testing
<http://purl.org/stc/terms#user-agent_based_testing> rdf:type owl:NamedIndividual ;
                                                     <http://purl.org/stc/terms#hasParent> <http://purl.org/stc/terms#mobile_app_testing> ;
                                                     :isInISTQBGlossary "true"^^xsd:boolean ;
                                                     rdfs:label "user-agent based testing" ;
                                                     <http://www.w3.org/2004/02/skos/core#prefLabel> "user-agent based testing"@en .


###  http://purl.org/stc/terms#user_acceptance_testing
<http://purl.org/stc/terms#user_acceptance_testing> rdf:type owl:NamedIndividual ;
                                                    <http://purl.org/stc/terms#hasParent> <http://purl.org/stc/terms#acceptance_testing> ;
                                                    :isInISTQBGlossary "true"^^xsd:boolean ;
                                                    rdfs:label "user acceptance testing" ;
                                                    <http://www.w3.org/2004/02/skos/core#prefLabel> "user acceptance testing"@en .


###  http://purl.org/stc/terms#validation
<http://purl.org/stc/terms#validation> rdf:type owl:NamedIndividual ;
                                       <http://purl.org/stc/terms#hasParent> <http://purl.org/stc/terms#basic_concepts> .


###  http://purl.org/stc/terms#verification
<http://purl.org/stc/terms#verification> rdf:type owl:NamedIndividual ;
                                         <http://purl.org/stc/terms#hasParent> <http://purl.org/stc/terms#basic_concepts> .


###  http://purl.org/stc/terms#walkthrough
<http://purl.org/stc/terms#walkthrough> rdf:type owl:NamedIndividual ;
                                        <http://purl.org/stc/terms#hasParent> <http://purl.org/stc/terms#informal_review> ;
                                        :isInISTQBGlossary "true"^^xsd:boolean ;
                                        rdfs:comment "A type of review in which an author leads members of the review through a work product and the members ask questions and make comments about possible issues.  (ISTQB Glossary v4.5)"@en ;
                                        rdfs:label "walkthrough" ;
                                        rdfs:seeAlso """Foundation - v4.0
Advanced Test Manager - 2012""" ;
                                        <http://www.w3.org/2004/02/skos/core#altLabel> "structured walkthrough"@en ;
                                        <http://www.w3.org/2004/02/skos/core#prefLabel> "walkthrough"@en .


###  http://purl.org/stc/terms#white_box_test_technique
<http://purl.org/stc/terms#white_box_test_technique> rdf:type owl:NamedIndividual ;
                                                     <http://purl.org/stc/terms#hasParent> <http://purl.org/stc/terms#test_technique> ;
                                                     :isInISTQBGlossary "true"^^xsd:boolean ;
                                                     rdfs:label "white box test technique" ;
                                                     <http://www.w3.org/2004/02/skos/core#altLabel> """white-box test technique
structure-based test design technique
structure based test design technique
structure-based test technique
structure based test technique
glass-box testing"""@en ;
                                                     <http://www.w3.org/2004/02/skos/core#prefLabel> "white box test technique"@en .


###  Generated by the OWL API (version 5.1.18) https://github.com/owlcs/owlapi/
